{
    "@context": {
        "rdf": "http://www.w3.org/1999/02/22-rdf-syntax-ns#",
        "owl": "http://www.w3.org/2002/07/owl#",
        "rdfs": "http://www.w3.org/2000/01/rdf-schema#",
        "schema": "https://schema.org/",
        "ConformityCredential": "https://test.uncefact.org/vocabulary/untp/cc/"
    },
    "@graph": [
        {
            "rdfs:label": "AssuranceClass",
            "@type": "rdfs:Class",
            "@id": "ConformityCredential:AssuranceClass",
            "rdfs:comment": ""
        },
        {
            "@id": "ConformityCredential:AssuranceClass#1A",
            "@type": "ConformityCredential:AssuranceClass",
            "ConformityCredential:Name": "1A",
            "rdf:value": "National government approval based on independent accreditation"
        },
        {
            "@id": "ConformityCredential:AssuranceClass#2A",
            "@type": "ConformityCredential:AssuranceClass",
            "ConformityCredential:Name": "2A",
            "rdf:value": "Accredited by IAF MLA or ILAC MRA signatory body"
        },
        {
            "@id": "ConformityCredential:AssuranceClass#3A",
            "@type": "ConformityCredential:AssuranceClass",
            "ConformityCredential:Name": "3A",
            "rdf:value": "Accredited by body independent from the accredited activity"
        },
        {
            "@id": "ConformityCredential:AssuranceClass#4A",
            "@type": "ConformityCredential:AssuranceClass",
            "ConformityCredential:Name": "4A",
            "rdf:value": "No independent accreditation"
        },
        {
            "rdfs:label": "AttestationType",
            "@type": "rdfs:Class",
            "@id": "ConformityCredential:AttestationType",
            "rdfs:comment": "A code for the type of the attestation credential"
        },
        {
            "@id": "ConformityCredential:AttestationType#test-report",
            "@type": "ConformityCredential:AttestationType",
            "ConformityCredential:Code": "test-report",
            "rdfs:comment": "Test report"
        },
        {
            "@id": "ConformityCredential:AttestationType#inspect-report",
            "@type": "ConformityCredential:AttestationType",
            "ConformityCredential:Code": "inspect-report",
            "rdfs:comment": "Inspection report"
        },
        {
            "@id": "ConformityCredential:AttestationType#product-cert",
            "@type": "ConformityCredential:AttestationType",
            "ConformityCredential:Code": "product-cert",
            "rdfs:comment": "Product certification"
        },
        {
            "@id": "ConformityCredential:AttestationType#service-cert",
            "@type": "ConformityCredential:AttestationType",
            "ConformityCredential:Code": "service-cert",
            "rdfs:comment": "Service certification"
        },
        {
            "@id": "ConformityCredential:AttestationType#process-cert",
            "@type": "ConformityCredential:AttestationType",
            "ConformityCredential:Code": "process-cert",
            "rdfs:comment": "Process certification"
        },
        {
            "@id": "ConformityCredential:AttestationType#management-cert",
            "@type": "ConformityCredential:AttestationType",
            "ConformityCredential:Code": "management-cert",
            "rdfs:comment": "Management system certification"
        },
        {
            "@id": "ConformityCredential:AttestationType#verification-report",
            "@type": "ConformityCredential:AttestationType",
            "ConformityCredential:Code": "verification-report",
            "rdfs:comment": "Verification report"
        },
        {
            "@id": "ConformityCredential:AttestationType#validation-report",
            "@type": "ConformityCredential:AttestationType",
            "ConformityCredential:Code": "validation-report",
            "rdfs:comment": "Validation report"
        },
        {
            "@id": "ConformityCredential:AttestationType#declaration",
            "@type": "ConformityCredential:AttestationType",
            "ConformityCredential:Code": "declaration",
            "rdfs:comment": "Declaration"
        },
        {
            "rdfs:label": "EncryptionMethod",
            "@type": "rdfs:Class",
            "@id": "ConformityCredential:EncryptionMethod",
            "rdfs:comment": ""
        },
        {
            "@id": "ConformityCredential:EncryptionMethod#none",
            "@type": "ConformityCredential:EncryptionMethod",
            "ConformityCredential:Name": "none",
            "rdf:value": "",
            "rdfs:comment": "no encryption"
        },
        {
            "@id": "ConformityCredential:EncryptionMethod#AES",
            "@type": "ConformityCredential:EncryptionMethod",
            "ConformityCredential:Name": "AES",
            "rdf:value": null,
            "rdfs:comment": "AES standard"
        },
        {
            "rdfs:label": "EvidenceType",
            "@type": "rdfs:Class",
            "@id": "ConformityCredential:EvidenceType",
            "rdfs:comment": ""
        },
        {
            "@id": "ConformityCredential:EvidenceType#VC",
            "@type": "ConformityCredential:EvidenceType",
            "ConformityCredential:Name": "VC",
            "rdf:value": "",
            "rdfs:comment": "A W3C Verifiable Credential "
        },
        {
            "@id": "ConformityCredential:EvidenceType#web",
            "@type": "ConformityCredential:EvidenceType",
            "ConformityCredential:Name": "web",
            "rdf:value": null,
            "rdfs:comment": "A public web page "
        },
        {
            "@id": "ConformityCredential:EvidenceType#seal",
            "@type": "ConformityCredential:EvidenceType",
            "ConformityCredential:Name": "seal",
            "rdf:value": null,
            "rdfs:comment": "A DAKKS digital seal"
        },
        {
            "rdfs:label": "RuleType",
            "@type": "rdfs:Class",
            "@id": "ConformityCredential:RuleType",
            "rdfs:comment": ""
        },
        {
            "@id": "ConformityCredential:RuleType#Regulation",
            "@type": "ConformityCredential:RuleType",
            "ConformityCredential:Name": "Regulation",
            "rdf:value": "",
            "rdfs:comment": ""
        },
        {
            "@id": "ConformityCredential:RuleType#NormativeStandard",
            "@type": "ConformityCredential:RuleType",
            "ConformityCredential:Name": "NormativeStandard",
            "rdf:value": null,
            "rdfs:comment": null
        },
        {
            "@id": "ConformityCredential:RuleType#IndustryStandard",
            "@type": "ConformityCredential:RuleType",
            "ConformityCredential:Name": "IndustryStandard",
            "rdf:value": null,
            "rdfs:comment": null
        },
        {
            "@id": "ConformityCredential:RuleType#Specification",
            "@type": "ConformityCredential:RuleType",
            "ConformityCredential:Name": "Specification",
            "rdf:value": null,
            "rdfs:comment": null
        },
        {
            "@id": "ConformityCredential:ConformityAttestation",
            "@type": "rdfs:Class",
            "rdfs:label": "ConformityAttestation",
            "schema:source": {
                "@id": "ConformityAttestation"
            },
            "rdfs:comment": "A conformity attestation issued by a competent body that defines one or more assessments (eg carbon intensity) about a product (eg batttery) against a specification (eg LCA method) defined in a standard or regulation."
        },
        {
            "@id": "ConformityCredential:SchemeOrProgram",
            "@type": "rdfs:Class",
            "rdfs:label": "SchemeOrProgram",
            "schema:source": {
                "@id": "SchemeOrProgram"
            },
            "rdfs:comment": "A formal governance scheme under which this attestation is issued (eg ACRS structural steel certification)"
        },
        {
            "@id": "ConformityCredential:Facility",
            "@type": "rdfs:Class",
            "rdfs:label": "Facility",
            "schema:source": {
                "@id": "Facility"
            },
            "rdfs:comment": ""
        },
        {
            "@id": "ConformityCredential:Product",
            "@type": "rdfs:Class",
            "rdfs:label": "Product",
            "schema:source": {
                "@id": "Product"
            },
            "rdfs:comment": "The facility (fatctory, farm, etc) or product or produciton batch that this conformity attestation is about."
        },
        {
            "@id": "ConformityCredential:Location",
            "@type": "rdfs:Class",
            "rdfs:label": "Location",
            "schema:source": {
                "@id": "Location"
            },
            "rdfs:comment": "A physical facility at a specified geolocation."
        },
        {
            "@id": "ConformityCredential:ConformityAssessment",
            "@type": "rdfs:Class",
            "rdfs:label": "ConformityAssessment",
            "schema:source": {
                "@id": "ConformityAssessment"
            },
            "rdfs:comment": "A specific assessment about the product or facility against a specific specification.  Eg the carbon intensity of a given product or batch."
        },
        {
            "@id": "ConformityCredential:Metric",
            "@type": "rdfs:Class",
            "rdfs:label": "Metric",
            "schema:source": {
                "@id": "Metric"
            },
            "rdfs:comment": "A numric value of the conformity claim - eg this product scope 1 emissions intensity is 5 KgCo2e/Kg"
        },
        {
            "@id": "ConformityCredential:ConformityEvidence",
            "@type": "rdfs:Class",
            "rdfs:label": "ConformityEvidence",
            "schema:source": {
                "@id": "ConformityEvidence"
            },
            "rdfs:comment": "The specific collection of evidence that was used to inform the conformity claim. Eg satellite images and supporting declarations in support of a deforestation claim."
        },
        {
            "@id": "ConformityCredential:File",
            "@type": "rdfs:Class",
            "rdfs:label": "File",
            "schema:source": {
                "@id": "File"
            },
            "rdfs:comment": "A file representing a data snapshot that is used to infomr the conformity assessment."
        },
        {
            "@id": "ConformityCredential:Authority",
            "@type": "rdfs:Class",
            "rdfs:label": "Authority",
            "schema:source": {
                "@id": "Authority"
            },
            "rdfs:comment": "The authority under which a conformity claim is issued.  For example a national accrediation authority may accredit a test lab to issue test certificates about a product against a standard. "
        },
        {
            "@id": "ConformityCredential:StandardOrRegulation",
            "@type": "rdfs:Class",
            "rdfs:label": "StandardOrRegulation",
            "schema:source": {
                "@id": "StandardOrRegulation"
            },
            "rdfs:comment": "A standard (eg ISO 14000) or regulation (eg EU deforestation regulation) that specifies the criteria for conformance."
        },
        {
            "@id": "ConformityCredential:Criteria",
            "@type": "rdfs:Class",
            "rdfs:label": "Criteria",
            "schema:source": {
                "@id": "Criteria"
            },
            "rdfs:comment": "A specific rule or criterion within a standard or regulation. eg a carbon intensity calculation rule within an emissions standard."
        },
        {
            "@id": "ConformityCredential:Party",
            "@type": "rdfs:Class",
            "rdfs:label": "Party",
            "schema:source": {
                "@id": "Party"
            },
            "rdfs:comment": "A party in the conformity domain such as the manufacturer, assessment body, standards authority, accreditation authority, etc"
        },
        {
            "@id": "ConformityCredential:id",
            "@type": [
                "rdf:Property",
                "owl:DatatypeProperty"
            ],
            "rdfs:label": "id",
            "schema:rangeIncludes": {
                "@id": "xsd:string"
            },
            "schema:domainIncludes": [
                {
                    "@id": "ConformityCredential:ConformityAttestation"
                },
                {
                    "@id": "ConformityCredential:SchemeOrProgram"
                },
                {
                    "@id": "ConformityCredential:StandardOrRegulation"
                },
                {
                    "@id": "ConformityCredential:Criteria"
                },
                {
                    "@id": "ConformityCredential:Party"
                }
            ],
            "rdfs:comment": "The unique identifier of this conformity attestation"
        },
        {
            "@id": "ConformityCredential:class",
            "@type": [
                "rdf:Property",
                "owl:ObjectProperty"
            ],
            "rdfs:label": "class",
            "schema:rangeIncludes": {
                "@id": "ConformityCredential:AssuranceClass"
            },
            "schema:domainIncludes": {
                "@id": "ConformityCredential:ConformityAttestation"
            },
            "rdfs:comment": "The type of attestation (formal conformity, industry or communituy, self assessed)"
        },
        {
            "@id": "ConformityCredential:type",
            "@type": [
                "rdf:Property",
                "owl:ObjectProperty"
            ],
            "rdfs:label": "type",
            "schema:rangeIncludes": {
                "@id": "ConformityCredential:AttestationType"
            },
            "schema:domainIncludes": [
                {
                    "@id": "ConformityCredential:ConformityAttestation"
                },
                {
                    "@id": "ConformityCredential:StandardOrRegulation"
                }
            ],
            "rdfs:comment": "The type of criterion (optional or mandatory)."
        },
        {
            "@id": "ConformityCredential:description",
            "@type": [
                "rdf:Property",
                "owl:DatatypeProperty"
            ],
            "rdfs:label": "description",
            "schema:rangeIncludes": {
                "@id": "xsd:string"
            },
            "schema:domainIncludes": [
                {
                    "@id": "ConformityCredential:ConformityAttestation"
                },
                {
                    "@id": "ConformityCredential:ConformityEvidence"
                },
                {
                    "@id": "ConformityCredential:Criteria"
                }
            ],
            "rdfs:comment": "A textual description of the scope or purpose of this confomrity attestation"
        },
        {
            "@id": "ConformityCredential:scope",
            "@type": [
                "rdf:Property",
                "owl:ObjectProperty"
            ],
            "rdfs:label": "scope",
            "schema:rangeIncludes": {
                "@id": "ConformityCredential:SchemeOrProgram"
            },
            "schema:domainIncludes": {
                "@id": "ConformityCredential:ConformityAttestation"
            },
            "rdfs:comment": "A list of relevant standards and/or regulations against which apply to this attestation (eg AS1163:2016)."
        },
        {
            "@id": "ConformityCredential:issuedBy",
            "@type": [
                "rdf:Property",
                "owl:ObjectProperty"
            ],
            "rdfs:label": "issuedBy",
            "schema:rangeIncludes": {
                "@id": "ConformityCredential:Party"
            },
            "schema:domainIncludes": {
                "@id": "ConformityCredential:ConformityAttestation"
            },
            "rdfs:comment": "The party that issued the conformity attestation."
        },
        {
            "@id": "ConformityCredential:issuedTo",
            "@type": [
                "rdf:Property",
                "owl:ObjectProperty"
            ],
            "rdfs:label": "issuedTo",
            "schema:rangeIncludes": {
                "@id": "ConformityCredential:Party"
            },
            "schema:domainIncludes": {
                "@id": "ConformityCredential:ConformityAttestation"
            },
            "rdfs:comment": "The party to whom the conformity attestation was issued."
        },
        {
            "@id": "ConformityCredential:validFrom",
            "@type": [
                "rdf:Property",
                "owl:DatatypeProperty"
            ],
            "rdfs:label": "validFrom",
            "schema:rangeIncludes": {
                "@id": "xsd:string"
            },
            "schema:domainIncludes": {
                "@id": "ConformityCredential:ConformityAttestation"
            },
            "rdfs:comment": "The date from which the conformity attestation is valid."
        },
        {
            "@id": "ConformityCredential:validTo",
            "@type": [
                "rdf:Property",
                "owl:DatatypeProperty"
            ],
            "rdfs:label": "validTo",
            "schema:rangeIncludes": {
                "@id": "xsd:string"
            },
            "schema:domainIncludes": {
                "@id": "ConformityCredential:ConformityAttestation"
            },
            "rdfs:comment": "The date until which the conformity attestation is valid."
        },
        {
            "@id": "ConformityCredential:status",
            "@type": [
                "rdf:Property",
                "owl:ObjectProperty"
            ],
            "rdfs:label": "status",
            "schema:rangeIncludes": {
                "@id": "ConformityCredential:Status"
            },
            "schema:domainIncludes": {
                "@id": "ConformityCredential:ConformityAttestation"
            },
            "rdfs:comment": "The status of this conformity attestation (eg pending, valid, expired, revoked)"
        },
        {
            "@id": "ConformityCredential:assessments",
            "@type": [
                "rdf:Property",
                "owl:ObjectProperty"
            ],
            "rdfs:label": "assessments",
            "schema:rangeIncludes": {
                "@id": "ConformityCredential:ConformityAssessment"
            },
            "schema:domainIncludes": {
                "@id": "ConformityCredential:ConformityAttestation"
            },
            "rdfs:comment": "The list of specific assessments made within this conformity attestation."
        },
        {
            "@id": "ConformityCredential:evidence",
            "@type": [
                "rdf:Property",
                "owl:ObjectProperty"
            ],
            "rdfs:label": "evidence",
            "schema:rangeIncludes": {
                "@id": "ConformityCredential:ConformityEvidence"
            },
            "schema:domainIncludes": {
                "@id": "ConformityCredential:ConformityAttestation"
            },
            "rdfs:comment": "Evidence supporting the assessment"
        },
        {
            "@id": "ConformityCredential:accreditation",
            "@type": [
                "rdf:Property",
                "owl:ObjectProperty"
            ],
            "rdfs:label": "accreditation",
            "schema:rangeIncludes": {
                "@id": "ConformityCredential:Authority"
            },
            "schema:domainIncludes": {
                "@id": "ConformityCredential:ConformityAttestation"
            },
            "rdfs:comment": "The accreditation that from a competent authority (ag NATA) that confirms the issuers authorised scope of assessments. "
        },
        {
            "@id": "ConformityCredential:regulatoryApproval",
            "@type": [
                "rdf:Property",
                "owl:ObjectProperty"
            ],
            "rdfs:label": "regulatoryApproval",
            "schema:rangeIncludes": {
                "@id": "ConformityCredential:Authority"
            },
            "schema:domainIncludes": {
                "@id": "ConformityCredential:ConformityAttestation"
            },
            "rdfs:comment": "The regulatory approval under which this conformity attestation is issued. "
        },
        {
            "@id": "ConformityCredential:certificate",
            "@type": [
                "rdf:Property",
                "owl:ObjectProperty"
            ],
            "rdfs:label": "certificate",
            "schema:rangeIncludes": {
                "@id": "ConformityCredential:File"
            },
            "schema:domainIncludes": {
                "@id": "ConformityCredential:ConformityAttestation"
            },
            "rdfs:comment": ""
        },
        {
            "@id": "ConformityCredential:name",
            "@type": [
                "rdf:Property",
                "owl:DatatypeProperty"
            ],
            "rdfs:label": "name",
            "schema:rangeIncludes": {
                "@id": "xsd:string"
            },
            "schema:domainIncludes": [
                {
                    "@id": "ConformityCredential:SchemeOrProgram"
                },
                {
                    "@id": "ConformityCredential:Facility"
                },
                {
                    "@id": "ConformityCredential:Product"
                },
                {
                    "@id": "ConformityCredential:StandardOrRegulation"
                },
                {
                    "@id": "ConformityCredential:Party"
                }
            ],
            "rdfs:comment": "The name of the conformity scheme (eg ACRS structural steel certification)"
        },
        {
            "@id": "ConformityCredential:trustmark",
            "@type": [
                "rdf:Property",
                "owl:DatatypeProperty"
            ],
            "rdfs:label": "trustmark",
            "schema:rangeIncludes": {
                "@id": "xsd:string"
            },
            "schema:domainIncludes": [
                {
                    "@id": "ConformityCredential:SchemeOrProgram"
                },
                {
                    "@id": "ConformityCredential:Authority"
                }
            ],
            "rdfs:comment": "The trust mark that represents the conformity assessment scheme."
        },
        {
            "@id": "ConformityCredential:issuingBody",
            "@type": [
                "rdf:Property",
                "owl:ObjectProperty"
            ],
            "rdfs:label": "issuingBody",
            "schema:rangeIncludes": {
                "@id": "ConformityCredential:Party"
            },
            "schema:domainIncludes": [
                {
                    "@id": "ConformityCredential:SchemeOrProgram"
                },
                {
                    "@id": "ConformityCredential:StandardOrRegulation"
                }
            ],
            "rdfs:comment": "The issuing body of the conformity scheme."
        },
        {
            "@id": "ConformityCredential:dateOfIssue",
            "@type": [
                "rdf:Property",
                "owl:DatatypeProperty"
            ],
            "rdfs:label": "dateOfIssue",
            "schema:rangeIncludes": {
                "@id": "xsd:string"
            },
            "schema:domainIncludes": [
                {
                    "@id": "ConformityCredential:SchemeOrProgram"
                },
                {
                    "@id": "ConformityCredential:StandardOrRegulation"
                }
            ],
            "rdfs:comment": "The date of issue of the scheme."
        },
        {
            "@id": "ConformityCredential:facilityId",
            "@type": [
                "rdf:Property",
                "owl:DatatypeProperty"
            ],
            "rdfs:label": "facilityId",
            "schema:rangeIncludes": {
                "@id": "xsd:string"
            },
            "schema:domainIncludes": {
                "@id": "ConformityCredential:Facility"
            },
            "rdfs:comment": "A unique, resolvable, and verifiable identifier for the facility (eg https://maps.app.goo.gl/ULJFeVuA75M8cuQc8) "
        },
        {
            "@id": "ConformityCredential:classification",
            "@type": [
                "rdf:Property",
                "owl:ObjectProperty"
            ],
            "rdfs:label": "classification",
            "schema:rangeIncludes": {
                "@id": "ConformityCredential:UNCPC"
            },
            "schema:domainIncludes": [
                {
                    "@id": "ConformityCredential:Facility"
                },
                {
                    "@id": "ConformityCredential:Product"
                }
            ],
            "rdfs:comment": "The UN CPC service calssificaiton for the activities undertaken at this facility."
        },
        {
            "@id": "ConformityCredential:location",
            "@type": [
                "rdf:Property",
                "owl:ObjectProperty"
            ],
            "rdfs:label": "location",
            "schema:rangeIncludes": {
                "@id": "ConformityCredential:Location"
            },
            "schema:domainIncludes": {
                "@id": "ConformityCredential:Facility"
            },
            "rdfs:comment": "The physical location of this facility."
        },
        {
            "@id": "ConformityCredential:verfifiedByCAB",
            "@type": [
                "rdf:Property",
                "owl:DatatypeProperty"
            ],
            "rdfs:label": "verfifiedByCAB",
            "schema:rangeIncludes": {
                "@id": "xsd:boolean"
            },
            "schema:domainIncludes": [
                {
                    "@id": "ConformityCredential:Facility"
                },
                {
                    "@id": "ConformityCredential:Product"
                }
            ],
            "rdfs:comment": "Indicates whether the conformity assessment body has verified the identity of the subject of the assement (a facility or product / batch)."
        },
        {
            "@id": "ConformityCredential:productId",
            "@type": [
                "rdf:Property",
                "owl:DatatypeProperty"
            ],
            "rdfs:label": "productId",
            "schema:rangeIncludes": {
                "@id": "xsd:string"
            },
            "schema:domainIncludes": {
                "@id": "ConformityCredential:Product"
            },
            "rdfs:comment": "A unique, resolvable, and verifiable identifier for the product (eg id.gs1.org/gtin/5000127163096)"
        },
        {
            "@id": "ConformityCredential:marking",
            "@type": [
                "rdf:Property",
                "owl:DatatypeProperty"
            ],
            "rdfs:label": "marking",
            "schema:rangeIncludes": {
                "@id": "xsd:string"
            },
            "schema:domainIncludes": {
                "@id": "ConformityCredential:Product"
            },
            "rdfs:comment": "Markings or codes on the product that can be used to match the physical product to this confomity assessment. if not provided then the productID MUST be marked on the product."
        },
        {
            "@id": "ConformityCredential:testedBatchId",
            "@type": [
                "rdf:Property",
                "owl:DatatypeProperty"
            ],
            "rdfs:label": "testedBatchId",
            "schema:rangeIncludes": {
                "@id": "xsd:string"
            },
            "schema:domainIncludes": {
                "@id": "ConformityCredential:Product"
            },
            "rdfs:comment": "A unique, resolvable, and verifiable identifier for the product serial number or batch (eg id.gs1.org/gtin/614141123452/lot/ABC1/ser/12345?exp=180426)"
        },
        {
            "@id": "ConformityCredential:locationId",
            "@type": [
                "rdf:Property",
                "owl:DatatypeProperty"
            ],
            "rdfs:label": "locationId",
            "schema:rangeIncludes": {
                "@id": "xsd:string"
            },
            "schema:domainIncludes": {
                "@id": "ConformityCredential:Location"
            },
            "rdfs:comment": "Identfier of the facility at which the assessment was undertaken. Eg A GLN."
        },
        {
            "@id": "ConformityCredential:Geolocation",
            "@type": [
                "rdf:Property",
                "owl:DatatypeProperty"
            ],
            "rdfs:label": "Geolocation",
            "schema:rangeIncludes": {
                "@id": "xsd:string"
            },
            "schema:domainIncludes": {
                "@id": "ConformityCredential:Location"
            },
            "rdfs:comment": "The geolocated point or area that can be used to place the location on a map. Should be a PlusCode - eg https://plus.codes/4RQGGVGP+"
        },
        {
            "@id": "ConformityCredential:requirementReference",
            "@type": [
                "rdf:Property",
                "owl:ObjectProperty"
            ],
            "rdfs:label": "requirementReference",
            "schema:rangeIncludes": {
                "@id": "ConformityCredential:StandardOrRegulation"
            },
            "schema:domainIncludes": {
                "@id": "ConformityCredential:ConformityAssessment"
            },
            "rdfs:comment": "The reference to the standard or regulation that defines the specification / criteria"
        },
        {
            "@id": "ConformityCredential:assessmentCriterion",
            "@type": [
                "rdf:Property",
                "owl:ObjectProperty"
            ],
            "rdfs:label": "assessmentCriterion",
            "schema:rangeIncludes": {
                "@id": "ConformityCredential:Criteria"
            },
            "schema:domainIncludes": {
                "@id": "ConformityCredential:ConformityAssessment"
            },
            "rdfs:comment": "The specification against which the assessment is made."
        },
        {
            "@id": "ConformityCredential:subjectProducts",
            "@type": [
                "rdf:Property",
                "owl:ObjectProperty"
            ],
            "rdfs:label": "subjectProducts",
            "schema:rangeIncludes": {
                "@id": "ConformityCredential:Product"
            },
            "schema:domainIncludes": {
                "@id": "ConformityCredential:ConformityAssessment"
            },
            "rdfs:comment": "The list of products that are the subject of this conformity assessment"
        },
        {
            "@id": "ConformityCredential:subjectFacilities",
            "@type": [
                "rdf:Property",
                "owl:ObjectProperty"
            ],
            "rdfs:label": "subjectFacilities",
            "schema:rangeIncludes": {
                "@id": "ConformityCredential:Facility"
            },
            "schema:domainIncludes": {
                "@id": "ConformityCredential:ConformityAssessment"
            },
            "rdfs:comment": "The list of facilities that are the subject of this conformity assessment."
        },
        {
            "@id": "ConformityCredential:measuredResults",
            "@type": [
                "rdf:Property",
                "owl:ObjectProperty"
            ],
            "rdfs:label": "measuredResults",
            "schema:rangeIncludes": {
                "@id": "ConformityCredential:Metric"
            },
            "schema:domainIncludes": {
                "@id": "ConformityCredential:ConformityAssessment"
            },
            "rdfs:comment": "The list of specific values measured as part of this assessment (eg tensile strength)"
        },
        {
            "@id": "ConformityCredential:compliance",
            "@type": [
                "rdf:Property",
                "owl:DatatypeProperty"
            ],
            "rdfs:label": "compliance",
            "schema:rangeIncludes": {
                "@id": "xsd:boolean"
            },
            "schema:domainIncludes": {
                "@id": "ConformityCredential:ConformityAssessment"
            },
            "rdfs:comment": "An indicator of whether or not the assessment meets the specification."
        },
        {
            "@id": "ConformityCredential:ESGtopic",
            "@type": [
                "rdf:Property",
                "owl:ObjectProperty"
            ],
            "rdfs:label": "ESGtopic",
            "schema:rangeIncludes": {
                "@id": "ConformityCredential:Topic"
            },
            "schema:domainIncludes": {
                "@id": "ConformityCredential:ConformityAssessment"
            },
            "rdfs:comment": "The UN ESG topic category for this assessment (eg vocabulary.uncefact.org/sustainability/emissions)"
        },
        {
            "@id": "ConformityCredential:metric",
            "@type": [
                "rdf:Property",
                "owl:DatatypeProperty"
            ],
            "rdfs:label": "metric",
            "schema:rangeIncludes": {
                "@id": "xsd:string"
            },
            "schema:domainIncludes": {
                "@id": "ConformityCredential:Metric"
            },
            "rdfs:comment": "A pointer to the definition of the metric - should be a vocabulary item URI mantained by the standards authority or regulator."
        },
        {
            "@id": "ConformityCredential:unit",
            "@type": [
                "rdf:Property",
                "owl:ObjectProperty"
            ],
            "rdfs:label": "unit",
            "schema:rangeIncludes": {
                "@id": "ConformityCredential:UOM"
            },
            "schema:domainIncludes": {
                "@id": "ConformityCredential:Metric"
            },
            "rdfs:comment": "The unit of measurement for the metric from UNECE Rec 20 UoM code list."
        },
        {
            "@id": "ConformityCredential:value",
            "@type": [
                "rdf:Property",
                "owl:DatatypeProperty"
            ],
            "rdfs:label": "value",
            "schema:rangeIncludes": {
                "@id": "xsd:decimal"
            },
            "schema:domainIncludes": {
                "@id": "ConformityCredential:Metric"
            },
            "rdfs:comment": "The measured value.  "
        },
        {
            "@id": "ConformityCredential:evidenceRootHash",
            "@type": [
                "rdf:Property",
                "owl:DatatypeProperty"
            ],
            "rdfs:label": "evidenceRootHash",
            "schema:rangeIncludes": {
                "@id": "xsd:string"
            },
            "schema:domainIncludes": {
                "@id": "ConformityCredential:ConformityEvidence"
            },
            "rdfs:comment": "An MD5 hash representing the root of the evidence."
        },
        {
            "@id": "ConformityCredential:evidenceData",
            "@type": [
                "rdf:Property",
                "owl:ObjectProperty"
            ],
            "rdfs:label": "evidenceData",
            "schema:rangeIncludes": {
                "@id": "ConformityCredential:File"
            },
            "schema:domainIncludes": {
                "@id": "ConformityCredential:ConformityEvidence"
            },
            "rdfs:comment": "Files that constitute the evidence."
        },
        {
            "@id": "ConformityCredential:decryptionKeyRequest",
            "@type": [
                "rdf:Property",
                "owl:DatatypeProperty"
            ],
            "rdfs:label": "decryptionKeyRequest",
            "schema:rangeIncludes": {
                "@id": "xsd:string"
            },
            "schema:domainIncludes": {
                "@id": "ConformityCredential:ConformityEvidence"
            },
            "rdfs:comment": "A URI to request the decryption key for the evidence."
        },
        {
            "@id": "ConformityCredential:fileHash",
            "@type": [
                "rdf:Property",
                "owl:DatatypeProperty"
            ],
            "rdfs:label": "fileHash",
            "schema:rangeIncludes": {
                "@id": "xsd:string"
            },
            "schema:domainIncludes": {
                "@id": "ConformityCredential:File"
            },
            "rdfs:comment": "The MD5 hash of the file."
        },
        {
            "@id": "ConformityCredential:fileLocation",
            "@type": [
                "rdf:Property",
                "owl:DatatypeProperty"
            ],
            "rdfs:label": "fileLocation",
            "schema:rangeIncludes": {
                "@id": "xsd:string"
            },
            "schema:domainIncludes": {
                "@id": "ConformityCredential:File"
            },
            "rdfs:comment": "The location of the evidence file."
        },
        {
            "@id": "ConformityCredential:fileType",
            "@type": [
                "rdf:Property",
                "owl:ObjectProperty"
            ],
            "rdfs:label": "fileType",
            "schema:rangeIncludes": {
                "@id": "ConformityCredential:mimeType"
            },
            "schema:domainIncludes": {
                "@id": "ConformityCredential:File"
            },
            "rdfs:comment": "The type of file, represented as a MIME type."
        },
        {
            "@id": "ConformityCredential:EncryptionMethod",
            "@type": [
                "rdf:Property",
                "owl:ObjectProperty"
            ],
            "rdfs:label": "EncryptionMethod",
            "schema:rangeIncludes": {
                "@id": "ConformityCredential:EncryptionMethod"
            },
            "schema:domainIncludes": {
                "@id": "ConformityCredential:File"
            },
            "rdfs:comment": "A code indicating the encryption method applied to the file."
        },
        {
            "@id": "ConformityCredential:number",
            "@type": [
                "rdf:Property",
                "owl:DatatypeProperty"
            ],
            "rdfs:label": "number",
            "schema:rangeIncludes": {
                "@id": "xsd:string"
            },
            "schema:domainIncludes": {
                "@id": "ConformityCredential:Authority"
            },
            "rdfs:comment": "The reference number for the accreditation - issued by the accreditation body (AB) to the confomrity assessment body (CAB)"
        },
        {
            "@id": "ConformityCredential:credential",
            "@type": [
                "rdf:Property",
                "owl:DatatypeProperty"
            ],
            "rdfs:label": "credential",
            "schema:rangeIncludes": {
                "@id": "xsd:string"
            },
            "schema:domainIncludes": {
                "@id": "ConformityCredential:Authority"
            },
            "rdfs:comment": "The pointer to the credential issued by a trust anchor that accredits the party making the assessment."
        },
        {
            "@id": "ConformityCredential:credentialType",
            "@type": [
                "rdf:Property",
                "owl:ObjectProperty"
            ],
            "rdfs:label": "credentialType",
            "schema:rangeIncludes": {
                "@id": "ConformityCredential:EvidenceType"
            },
            "schema:domainIncludes": {
                "@id": "ConformityCredential:Authority"
            },
            "rdfs:comment": "A code specifying the accreditaiotn evidence type (eg VC, web page, DAKKS seal)"
        },
        {
            "@id": "ConformityCredential:authority",
            "@type": [
                "rdf:Property",
                "owl:ObjectProperty"
            ],
            "rdfs:label": "authority",
            "schema:rangeIncludes": {
                "@id": "ConformityCredential:Party"
            },
            "schema:domainIncludes": {
                "@id": "ConformityCredential:Authority"
            },
            "rdfs:comment": "The competent authority that issued the accreditation."
        },
        {
            "@id": "ConformityCredential:criteria",
            "@type": [
                "rdf:Property",
                "owl:ObjectProperty"
            ],
            "rdfs:label": "criteria",
            "schema:rangeIncludes": {
                "@id": "ConformityCredential:Criteria"
            },
            "schema:domainIncludes": {
                "@id": "ConformityCredential:StandardOrRegulation"
            },
            "rdfs:comment": "The criteria associated with the standard or regulation."
        },
        {
            "@id": "ConformityCredential:thresholdValue",
            "@type": [
                "rdf:Property",
                "owl:ObjectProperty"
            ],
            "rdfs:label": "thresholdValue",
            "schema:rangeIncludes": {
                "@id": "ConformityCredential:Metric"
            },
            "schema:domainIncludes": {
                "@id": "ConformityCredential:Criteria"
            },
            "rdfs:comment": "A conformity threshold defined by the specification (eg minimum compressive strength)"
        }
    ]
}