{"@context":{"rdf":"http://www.w3.org/1999/02/22-rdf-syntax-ns#","owl":"http://www.w3.org/2002/07/owl#","rdfs":"http://www.w3.org/2000/01/rdf-schema#","schema":"https://schema.org/","untp-dpp":"https://jargon.sh/user/unece/untp-dpp/v/working/artefacts/jsonld/render.jsonld#"},"@graph":[{"rdfs:label":"epcisType","@type":"rdfs:Class","@id":"untp-dpp:epcisType","rdfs:comment":""},{"@id":"untp-dpp:epcisType#aggregation","@type":"untp-dpp:epcisType","untp-dpp:Name":"aggregation","rdf:value":"","rdfs:comment":""},{"@id":"untp-dpp:epcisType#transformation","@type":"untp-dpp:epcisType","untp-dpp:Name":"transformation","rdf:value":"","rdfs:comment":""},{"@id":"untp-dpp:epcisType#object","@type":"untp-dpp:epcisType","untp-dpp:Name":"object","rdf:value":"","rdfs:comment":""},{"@id":"untp-dpp:epcisType#transaction","@type":"untp-dpp:epcisType","untp-dpp:Name":"transaction","rdf:value":"","rdfs:comment":""},{"rdfs:label":"topic","@type":"rdfs:Class","@id":"untp-dpp:topic","rdfs:comment":""},{"@id":"untp-dpp:topic#environment.emissions","@type":"untp-dpp:topic","untp-dpp:Name":"environment.emissions","rdf:value":"","rdfs:comment":""},{"@id":"untp-dpp:topic#environment.water","@type":"untp-dpp:topic","untp-dpp:Name":"environment.water","rdf:value":"","rdfs:comment":""},{"@id":"untp-dpp:topic#environment.waste","@type":"untp-dpp:topic","untp-dpp:Name":"environment.waste","rdf:value":"","rdfs:comment":""},{"@id":"untp-dpp:topic#environment.deforestation","@type":"untp-dpp:topic","untp-dpp:Name":"environment.deforestation","rdf:value":"","rdfs:comment":""},{"@id":"untp-dpp:topic#environment.emissions","@type":"untp-dpp:topic","untp-dpp:Name":"environment.emissions","rdf:value":"","rdfs:comment":""},{"@id":"untp-dpp:topic#social.employment","@type":"untp-dpp:topic","untp-dpp:Name":"social.employment","rdf:value":"","rdfs:comment":""},{"@id":"untp-dpp:topic#social.safety","@type":"untp-dpp:topic","untp-dpp:Name":"social.safety","rdf:value":"","rdfs:comment":""},{"@id":"untp-dpp:topic#social.biosecurity","@type":"untp-dpp:topic","untp-dpp:Name":"social.biosecurity","rdf:value":"","rdfs:comment":""},{"@id":"untp-dpp:topic#governance.ethics","@type":"untp-dpp:topic","untp-dpp:Name":"governance.ethics","rdf:value":"","rdfs:comment":""},{"@id":"untp-dpp:VerifiableCredential","@type":"rdfs:Class","rdfs:label":"VerifiableCredential","schema:source":{"@id":"VerifiableCredential"},"rdfs:comment":"A cryptographically verifiable set of claims about a product."},{"@id":"untp-dpp:ProductPassport","@type":"rdfs:Class","rdfs:label":"ProductPassport","schema:source":{"@id":"ProductPassport"},"rdfs:comment":"The ProductPassport is a comprehensive data structure that encapsulates various details pertaining to a product, including its identification details, who issued it, batch information, and different scores relating to sustainability and trustworthiness."},{"@id":"untp-dpp:Party","@type":"rdfs:Class","rdfs:label":"Party","schema:source":{"@id":"Party"},"rdfs:comment":"The Party class represents an entity such as an organization, or a company that manufactured the product."},{"@id":"untp-dpp:Facility","@type":"rdfs:Class","rdfs:label":"Facility","schema:source":{"@id":"Facility"},"rdfs:comment":"The Facility class embodies information about a specific facility, which manufactured the product."},{"@id":"untp-dpp:ProductInformation","@type":"rdfs:Class","rdfs:label":"ProductInformation","schema:source":{"@id":"ProductInformation"},"rdfs:comment":"The ProductInformation class encapsulates detailed information regarding a specific product, including its identification details, manufacturer, and other pertinent details."},{"@id":"untp-dpp:ProductBatch","@type":"rdfs:Class","rdfs:label":"ProductBatch","schema:source":{"@id":"ProductBatch"},"rdfs:comment":"The ProductBatch class holds information related to a specific batch of products, including manufacturing details, sustainability claims and provenance information."},{"@id":"untp-dpp:SustainabilityClaim","@type":"rdfs:Class","rdfs:label":"SustainabilityClaim","schema:source":{"@id":"SustainabilityClaim"},"rdfs:comment":"The SustainabilityClaim class represents specific claims regarding the sustainability of a product, providing details about the metrics, thresholds, and evidences supporting the claim."},{"@id":"untp-dpp:SustainabilityMetric","@type":"rdfs:Class","rdfs:label":"SustainabilityMetric","schema:source":{"@id":"SustainabilityMetric"},"rdfs:comment":"A specific measure of performance against the criteria that governs the claim.  Expressed as an array of metric (ie unit of emasure) / value (ie the actual numeric value) pairs.  "},{"@id":"untp-dpp:TraceabilityEvent","@type":"rdfs:Class","rdfs:label":"TraceabilityEvent","schema:source":{"@id":"TraceabilityEvent"},"rdfs:comment":"The TraceabilityEvent class represents a specific EPCIS event in the traceability chain of a product, including details about the event type and reference."},{"@id":"untp-dpp:Provenance","@type":"rdfs:Class","rdfs:label":"Provenance","schema:source":{"@id":"Provenance"},"rdfs:comment":"The Provenance class encapsulates details about the origin or source of components or ingredients in a product, including the country of origin and the percentage composition."},{"@id":"untp-dpp:id","@type":["rdf:Property","owl:DatatypeProperty"],"rdfs:label":"id","schema:rangeIncludes":{"@id":"xsd:string"},"schema:domainIncludes":[{"@id":"untp-dpp:VerifiableCredential"},{"@id":"untp-dpp:ProductPassport"},{"@id":"untp-dpp:Party"},{"@id":"untp-dpp:Facility"}],"rdfs:comment":"A unique identifier assigned to the credential, typically formatted as a URI of the stored credential."},{"@id":"untp-dpp:issuer","@type":["rdf:Property","owl:DatatypeProperty"],"rdfs:label":"issuer","schema:rangeIncludes":{"@id":"xsd:string"},"schema:domainIncludes":{"@id":"untp-dpp:VerifiableCredential"},"rdfs:comment":"A unique identifier of the entity that issued the credential. Typically expessed as a DID."},{"@id":"untp-dpp:validFrom","@type":["rdf:Property","owl:DatatypeProperty"],"rdfs:label":"validFrom","schema:rangeIncludes":{"@id":"xsd:string"},"schema:domainIncludes":{"@id":"untp-dpp:VerifiableCredential"},"rdfs:comment":"The ISO-8601 date time from which the credential is valid."},{"@id":"untp-dpp:status","@type":["rdf:Property","owl:DatatypeProperty"],"rdfs:label":"status","schema:rangeIncludes":{"@id":"xsd:string"},"schema:domainIncludes":{"@id":"untp-dpp:VerifiableCredential"},"rdfs:comment":"The current status of the credential, represented by a specific code."},{"@id":"untp-dpp:subject","@type":["rdf:Property","owl:ObjectProperty"],"rdfs:label":"subject","schema:rangeIncludes":{"@id":"untp-dpp:ProductPassport"},"schema:domainIncludes":{"@id":"untp-dpp:VerifiableCredential"},"rdfs:comment":"The ProductPassport object that the credential pertains to."},{"@id":"untp-dpp:issuedBy","@type":["rdf:Property","owl:ObjectProperty"],"rdfs:label":"issuedBy","schema:rangeIncludes":{"@id":"untp-dpp:Party"},"schema:domainIncludes":{"@id":"untp-dpp:ProductPassport"},"rdfs:comment":"The Party entity that issued the product passport."},{"@id":"untp-dpp:product","@type":["rdf:Property","owl:ObjectProperty"],"rdfs:label":"product","schema:rangeIncludes":{"@id":"untp-dpp:ProductInformation"},"schema:domainIncludes":{"@id":"untp-dpp:ProductPassport"},"rdfs:comment":"Detailed information about the product encapsulated in a ProductInformation object."},{"@id":"untp-dpp:batch","@type":["rdf:Property","owl:ObjectProperty"],"rdfs:label":"batch","schema:rangeIncludes":{"@id":"untp-dpp:ProductBatch"},"schema:domainIncludes":{"@id":"untp-dpp:ProductPassport"},"rdfs:comment":"Information regarding the specific batch the product belongs to, encapsulated in a ProductBatch object."},{"@id":"untp-dpp:sustainabilityScore","@type":["rdf:Property","owl:DatatypeProperty"],"rdfs:label":"sustainabilityScore","schema:rangeIncludes":{"@id":"xsd:decimal"},"schema:domainIncludes":{"@id":"untp-dpp:ProductPassport"},"rdfs:comment":"An aggregate numeric metric calculated based on the various sustainability claims associated with the product. It amalgamates scores assigned to individual sustainability claims, which are validated by various issuing bodies. The score provides a comprehensive view of the product's overall sustainability performance, giving users a quantifiable measure of the product's environmental and social impacts."},{"@id":"untp-dpp:trustScore","@type":["rdf:Property","owl:DatatypeProperty"],"rdfs:label":"trustScore","schema:rangeIncludes":{"@id":"xsd:decimal"},"schema:domainIncludes":{"@id":"untp-dpp:ProductPassport"},"rdfs:comment":"An aggregate numeric metric that represents the level of trustworthiness associated with the product. This score is derived based on the credibility and reliability of the issuing bodies that substantiate the claims being made about the product. The trustworthiness of each issuing body is assessed to compute an overall trust score, giving users a quantifiable measure of the trust they can place in the product's claims."},{"@id":"untp-dpp:name","@type":["rdf:Property","owl:DatatypeProperty"],"rdfs:label":"name","schema:rangeIncludes":{"@id":"xsd:string"},"schema:domainIncludes":[{"@id":"untp-dpp:Party"},{"@id":"untp-dpp:Facility"}],"rdfs:comment":"The name of the organization or company, represented as a text string."},{"@id":"untp-dpp:operatedBy","@type":["rdf:Property","owl:ObjectProperty"],"rdfs:label":"operatedBy","schema:rangeIncludes":{"@id":"untp-dpp:Party"},"schema:domainIncludes":{"@id":"untp-dpp:Facility"},"rdfs:comment":"The Party entity responsible for operating the facility."},{"@id":"untp-dpp:productId","@type":["rdf:Property","owl:DatatypeProperty"],"rdfs:label":"productId","schema:rangeIncludes":{"@id":"xsd:string"},"schema:domainIncludes":{"@id":"untp-dpp:ProductInformation"},"rdfs:comment":"A unique identifier (URI) assigned to the product. (Link Resolver - GS1 GTIN?)"},{"@id":"untp-dpp:model","@type":["rdf:Property","owl:DatatypeProperty"],"rdfs:label":"model","schema:rangeIncludes":{"@id":"xsd:string"},"schema:domainIncludes":{"@id":"untp-dpp:ProductInformation"},"rdfs:comment":"The model name or number of the product, represented as text."},{"@id":"untp-dpp:productClass","@type":["rdf:Property","owl:DatatypeProperty"],"rdfs:label":"productClass","schema:rangeIncludes":{"@id":"xsd:string"},"schema:domainIncludes":{"@id":"untp-dpp:ProductInformation"},"rdfs:comment":"A code representing the product's class, typically using the UNSPSC (United Nations Standard Products and Services Code) classification."},{"@id":"untp-dpp:image","@type":["rdf:Property","owl:DatatypeProperty"],"rdfs:label":"image","schema:rangeIncludes":{"@id":"xsd:string"},"schema:domainIncludes":{"@id":"untp-dpp:ProductInformation"},"rdfs:comment":"A unique identifier (URI) pointing to an image of the product."},{"@id":"untp-dpp:description","@type":["rdf:Property","owl:DatatypeProperty"],"rdfs:label":"description","schema:rangeIncludes":{"@id":"xsd:string"},"schema:domainIncludes":{"@id":"untp-dpp:ProductInformation"},"rdfs:comment":"A textual description providing details about the product."},{"@id":"untp-dpp:recyclingInfo","@type":["rdf:Property","owl:DatatypeProperty"],"rdfs:label":"recyclingInfo","schema:rangeIncludes":{"@id":"xsd:string"},"schema:domainIncludes":{"@id":"untp-dpp:ProductInformation"},"rdfs:comment":"A URI pointing to information regarding the recycling aspects of the product."},{"@id":"untp-dpp:manufacturer","@type":["rdf:Property","owl:ObjectProperty"],"rdfs:label":"manufacturer","schema:rangeIncludes":{"@id":"untp-dpp:Party"},"schema:domainIncludes":{"@id":"untp-dpp:ProductInformation"},"rdfs:comment":"The Party entity that manufactured the product."},{"@id":"untp-dpp:batchId","@type":["rdf:Property","owl:DatatypeProperty"],"rdfs:label":"batchId","schema:rangeIncludes":{"@id":"xsd:string"},"schema:domainIncludes":{"@id":"untp-dpp:ProductBatch"},"rdfs:comment":"A unique identifier (URI) assigned to the product batch. (Link Resolver - GS1-128?)"},{"@id":"untp-dpp:serialNumber","@type":["rdf:Property","owl:DatatypeProperty"],"rdfs:label":"serialNumber","schema:rangeIncludes":{"@id":"xsd:string"},"schema:domainIncludes":{"@id":"untp-dpp:ProductBatch"},"rdfs:comment":"The serial number(s) of the product or products in the batch, represented as text."},{"@id":"untp-dpp:manufacturedAt","@type":["rdf:Property","owl:ObjectProperty"],"rdfs:label":"manufacturedAt","schema:rangeIncludes":{"@id":"untp-dpp:Facility"},"schema:domainIncludes":{"@id":"untp-dpp:ProductBatch"},"rdfs:comment":"The Facility where the product batch was manufactured."},{"@id":"untp-dpp:manufacturedDate","@type":["rdf:Property","owl:DatatypeProperty"],"rdfs:label":"manufacturedDate","schema:rangeIncludes":{"@id":"xsd:string"},"schema:domainIncludes":{"@id":"untp-dpp:ProductBatch"},"rdfs:comment":"The ISO 8601 date on which the product batch was manufactured."},{"@id":"untp-dpp:provenance","@type":["rdf:Property","owl:ObjectProperty"],"rdfs:label":"provenance","schema:rangeIncludes":{"@id":"untp-dpp:Provenance"},"schema:domainIncludes":{"@id":"untp-dpp:ProductBatch"},"rdfs:comment":"An array of Provenance objects providing details on the origin of components or ingredients of the product batch."},{"@id":"untp-dpp:sustainabilityInfo","@type":["rdf:Property","owl:ObjectProperty"],"rdfs:label":"sustainabilityInfo","schema:rangeIncludes":{"@id":"untp-dpp:SustainabilityClaim"},"schema:domainIncludes":{"@id":"untp-dpp:ProductBatch"},"rdfs:comment":"An array of SustainabilityClaim objects representing various sustainability claims about the product batch."},{"@id":"untp-dpp:traceabilityInfo","@type":["rdf:Property","owl:ObjectProperty"],"rdfs:label":"traceabilityInfo","schema:rangeIncludes":{"@id":"untp-dpp:TraceabilityEvent"},"schema:domainIncludes":{"@id":"untp-dpp:ProductBatch"},"rdfs:comment":"An array of TraceabilityEvent objects detailing EPCIS events related to the traceability of the product batch."},{"@id":"untp-dpp:topic","@type":["rdf:Property","owl:ObjectProperty"],"rdfs:label":"topic","schema:rangeIncludes":{"@id":"untp-dpp:topic"},"schema:domainIncludes":{"@id":"untp-dpp:SustainabilityClaim"},"rdfs:comment":"A code representing the topic of the sustainability claim. E.g. environment.deforestation, environment.ghg-emission-intensity, etc..  Drawn from a standard code list.  "},{"@id":"untp-dpp:criteria","@type":["rdf:Property","owl:DatatypeProperty"],"rdfs:label":"criteria","schema:rangeIncludes":{"@id":"xsd:string"},"schema:domainIncludes":{"@id":"untp-dpp:SustainabilityClaim"},"rdfs:comment":"A URI pointing to the regulation or standard governing the claim."},{"@id":"untp-dpp:sustainabilityCredential","@type":["rdf:Property","owl:DatatypeProperty"],"rdfs:label":"sustainabilityCredential","schema:rangeIncludes":{"@id":"xsd:string"},"schema:domainIncludes":{"@id":"untp-dpp:SustainabilityClaim"},"rdfs:comment":"A URI pointing to the evidence supporting the claim. Most likely in the form of a verifiable credential."},{"@id":"untp-dpp:metric","@type":["rdf:Property","owl:ObjectProperty"],"rdfs:label":"metric","schema:rangeIncludes":{"@id":"untp-dpp:SustainabilityMetric"},"schema:domainIncludes":[{"@id":"untp-dpp:SustainabilityClaim"},{"@id":"untp-dpp:SustainabilityMetric"}],"rdfs:comment":"One or more actual measures supporting the claim. For example for GHG emissions there may be a metric for total emissions intensity and also a metric for amount of offsets included."},{"@id":"untp-dpp:compliance","@type":["rdf:Property","owl:DatatypeProperty"],"rdfs:label":"compliance","schema:rangeIncludes":{"@id":"xsd:boolean"},"schema:domainIncludes":{"@id":"untp-dpp:SustainabilityClaim"},"rdfs:comment":"and indicator (boolean) that expresses whether or not this product has acehived compliance against the rule.  for example, if the topic is environment.deforstation and the rule is EU.2023.1115 then the product is complianct if it has not touched any facility throughout it's lifecycle that is not deforestation free since dec 2020."},{"@id":"untp-dpp:unit","@type":["rdf:Property","owl:DatatypeProperty"],"rdfs:label":"unit","schema:rangeIncludes":{"@id":"xsd:string"},"schema:domainIncludes":{"@id":"untp-dpp:SustainabilityMetric"},"rdfs:comment":"The unit of measure. for example, energy generaiton intensity in Kg Co2e per kWh produced. Or Kg Co2e per Kg of livestock gross weight.  "},{"@id":"untp-dpp:value","@type":["rdf:Property","owl:DatatypeProperty"],"rdfs:label":"value","schema:rangeIncludes":{"@id":"xsd:decimal"},"schema:domainIncludes":{"@id":"untp-dpp:SustainabilityMetric"},"rdfs:comment":"A numeric value representing the measurement or evaluation outcome for the claim."},{"@id":"untp-dpp:eventReference","@type":["rdf:Property","owl:DatatypeProperty"],"rdfs:label":"eventReference","schema:rangeIncludes":{"@id":"xsd:string"},"schema:domainIncludes":{"@id":"untp-dpp:TraceabilityEvent"},"rdfs:comment":"A URI pointing to the detailed information about the EPCIS event. Most likely in the form of a verifiable credential."},{"@id":"untp-dpp:eventType","@type":["rdf:Property","owl:ObjectProperty"],"rdfs:label":"eventType","schema:rangeIncludes":{"@id":"untp-dpp:epcisType"},"schema:domainIncludes":{"@id":"untp-dpp:TraceabilityEvent"},"rdfs:comment":"A code representing the type of EPCIS event. ObjectEvent, AggregationEvent, TransactionEvent, TransformationEvent, ObjectEvent."},{"@id":"untp-dpp:country","@type":["rdf:Property","owl:ObjectProperty"],"rdfs:label":"country","schema:rangeIncludes":{"@id":"untp-dpp:country"},"schema:domainIncludes":{"@id":"untp-dpp:Provenance"},"rdfs:comment":"A ISO 3166-1 code representing the country of origin of the component or ingredient."},{"@id":"untp-dpp:percentage","@type":["rdf:Property","owl:DatatypeProperty"],"rdfs:label":"percentage","schema:rangeIncludes":{"@id":"xsd:decimal"},"schema:domainIncludes":{"@id":"untp-dpp:Provenance"},"rdfs:comment":"A numeric value representing the percentage composition of the component or ingredient in the product."},{"@id":"untp-dpp:guaranteeOfOriginCredential","@type":["rdf:Property","owl:DatatypeProperty"],"rdfs:label":"guaranteeOfOriginCredential","schema:rangeIncludes":{"@id":"xsd:string"},"schema:domainIncludes":{"@id":"untp-dpp:Provenance"},"rdfs:comment":""}]}