{"@context":{"rdf":"http://www.w3.org/1999/02/22-rdf-syntax-ns#","owl":"http://www.w3.org/2002/07/owl#","rdfs":"http://www.w3.org/2000/01/rdf-schema#","schema":"https://schema.org/","sustainability":"https://vocabulary.uncefact.org/sustainability/"},"@graph":[{"rdfs:label":"DegreeOfObligation","@type":"rdfs:Class","@id":"sustainability:DegreeOfObligation","rdfs:comment":""},{"@id":"sustainability:DegreeOfObligation#Requirementsforimmediateaction","@type":"sustainability:DegreeOfObligation","rdf:value":"Requirements for immediate action","rdfs:comment":"Requirements for immediate action indicate that compliance must be met immediately; otherwise applicants are excluded from the certification/verification process"},{"@id":"sustainability:DegreeOfObligation#Requirementstobemetwithin1year","@type":"sustainability:DegreeOfObligation","rdf:value":"Requirements to be met within 1 year","rdfs:comment":"Requirements to be met within one year (Short-term) requirements: indicate that compliance must be met in less than 12 months"},{"@id":"sustainability:DegreeOfObligation#Requirementstobemetwithin3years","@type":"sustainability:DegreeOfObligation","rdf:value":"Requirements to be met within 3 years","rdfs:comment":"Requirements to be met within three year (Mid-term) requirements: indicate that compliance must be met in less than 36 months"},{"@id":"sustainability:DegreeOfObligation#Requirementstobemetwithin5years","@type":"sustainability:DegreeOfObligation","rdf:value":"Requirements to be met within 5 years","rdfs:comment":"Requirements to be met within 5 year (Long-term) requirements: indicate that compliance must be met in a period of time that is defined as more than 36 months"},{"@id":"sustainability:DegreeOfObligation#Recommendations","@type":"sustainability:DegreeOfObligation","rdf:value":"Recommendations","rdfs:comment":"Recommendations are those requirements that “should” be met but for which non-compliance is not a matter of exclusion or sanction"},{"rdfs:label":"DegreeOfCriticality","@type":"rdfs:Class","@id":"sustainability:DegreeOfCriticality","rdfs:comment":""},{"@id":"sustainability:DegreeOfCriticality#Deal-breaker-definitionandpolicy","@type":"sustainability:DegreeOfCriticality","rdf:value":"Deal-breaker - definition and policy","rdfs:comment":"A deal-breaker is a requirement that if not met by the certified operation will lead to automatic de-certification with no chance for implementation of correction action plan"},{"@id":"sustainability:DegreeOfCriticality#Majornon-compliance-definitionandcorrectiveactionspolicy","@type":"sustainability:DegreeOfCriticality","rdf:value":"Major non-compliance - definition and corrective actions policy","rdfs:comment":"A major non-compliance is a requirement that if not met has to be addressed as priority in a corrective actions plan and will be checked in a more restricted timeframe than usual surveillance audit."},{"@id":"sustainability:DegreeOfCriticality#Minornon-compliance-definitionandcorrectiveactionspolicy","@type":"sustainability:DegreeOfCriticality","rdf:value":"Minor non-compliance - definition and corrective actions policy","rdfs:comment":"Minor non-compliance refers to requirements that if they are not met need to lead to improvements as part of normal corrective actions plan and surveillance audits"},{"@id":"sustainability:DegreeOfCriticality#Optionalcompliance-definitionandactionplan","@type":"sustainability:DegreeOfCriticality","rdf:value":"Optional compliance - definition and action plan","rdfs:comment":"The scheme’s audit policy on optional compliance could apply to requirements labelled as recommendations or those suggested in a continuous improvement plan"},{"rdfs:label":"VerificationOfCompliance","@type":"rdfs:Class","@id":"sustainability:VerificationOfCompliance","rdfs:comment":""},{"@id":"sustainability:VerificationOfCompliance#Pass/fail","@type":"sustainability:VerificationOfCompliance","rdf:value":"Pass/fail","rdfs:comment":"The auditors take their decision using a Pass or Fail method: this is commonly used when assessing compliance to critical requirements, either the assessee complies with the requirement, or not."},{"@id":"sustainability:VerificationOfCompliance#Scoring","@type":"sustainability:VerificationOfCompliance","rdf:value":"Scoring","rdfs:comment":"Scoring systems are used to assess compliance, which may include totals / percentages / averages or other types of calculations."},{"@id":"sustainability:VerificationOfCompliance#Risk-based","@type":"sustainability:VerificationOfCompliance","rdf:value":"Risk-based","rdfs:comment":"A risk-based approach to compliance involves identifying the areas of high risk within the company's compliance and building and prioritizing its compliance monitoring program around these risks."},{"@id":"sustainability:VerificationOfCompliance#Trafficlight","@type":"sustainability:VerificationOfCompliance","rdf:value":"Traffic light","rdfs:comment":"The traffic light system is primarily a tool that can be used during compliance assessments to highlight the good practices, practices that need to get improved, and the bad practices that are unacceptable."},{"@id":"sustainability:VerificationOfCompliance#Correctiveactions:planningandauditprocess","@type":"sustainability:VerificationOfCompliance","rdf:value":"Corrective actions: planning and audit process","rdfs:comment":"When non-compliances are identified, standard systems may require sanctions and corrective actions to be taken."},{"@id":"sustainability:VerificationOfCompliance#Majornon-compliance:allowedtimeframebeforere-audit","@type":"sustainability:VerificationOfCompliance","rdf:value":"Major non-compliance: allowed timeframe before re-audit","rdfs:comment":"Major non-compliances are those non-compliances that shall be fully corrected with the implementation of corrective actions within a certain period of time set by the scheme policies. In the majority of the cases, major non-conformities shall lead to suspension of the certificate if not corrected within the allowed timeframe."},{"@id":"sustainability:VerificationOfCompliance#Minornon-compliance:allowedtimeframebeforere-audit","@type":"sustainability:VerificationOfCompliance","rdf:value":"Minor non-compliance: allowed timeframe before re-audit","rdfs:comment":"Minor non-compliances are those non-compliances that shall be fully corrected with the implementation of a normal corrective action within a certain period of time set by the scheme policies. For some schemes, if the action taken is not considered adequate, minor non-conformities shall become 'major' non-conformities."},{"@id":"sustainability:VerificationOfCompliance#Progressiverequirementsandcontinuousimprovement","@type":"sustainability:VerificationOfCompliance","rdf:value":"Progressive requirements and continuous improvement","rdfs:comment":"Standards systems may have developed policies to promote continuous improvement: these incentives may be in terms of scope of the audit being reduced in the case of good audit results (risk-based approach)."},{"rdfs:label":"SoilCompaction","@type":"rdfs:Class","@id":"sustainability:SoilCompaction","rdfs:comment":""},{"@id":"sustainability:SoilCompaction#1","@type":"sustainability:SoilCompaction","rdf:value":"1","rdfs:comment":"Measure compaction"},{"@id":"sustainability:SoilCompaction#2","@type":"sustainability:SoilCompaction","rdf:value":"2","rdfs:comment":"Monitor compaction over time"},{"@id":"sustainability:SoilCompaction#3","@type":"sustainability:SoilCompaction","rdf:value":"3","rdfs:comment":"Prevent compaction"},{"rdfs:label":"SoilErosion","@type":"rdfs:Class","@id":"sustainability:SoilErosion","rdfs:comment":""},{"@id":"sustainability:SoilErosion#1","@type":"sustainability:SoilErosion","rdf:value":"1","rdfs:comment":"Measure erosion"},{"@id":"sustainability:SoilErosion#2","@type":"sustainability:SoilErosion","rdf:value":"2","rdfs:comment":"Monitor erosion over time"},{"@id":"sustainability:SoilErosion#3","@type":"sustainability:SoilErosion","rdf:value":"3","rdfs:comment":"Prevent erosion"},{"rdfs:label":"SoilFertility","@type":"rdfs:Class","@id":"sustainability:SoilFertility","rdfs:comment":""},{"@id":"sustainability:SoilFertility#1","@type":"sustainability:SoilFertility","rdf:value":"1","rdfs:comment":"Measure soil fertility"},{"@id":"sustainability:SoilFertility#2","@type":"sustainability:SoilFertility","rdf:value":"2","rdfs:comment":"Monitor soil fertility over time"},{"@id":"sustainability:SoilFertility#3","@type":"sustainability:SoilFertility","rdf:value":"3","rdfs:comment":"Maintain soil fertility"},{"rdfs:label":"SoilContamination","@type":"rdfs:Class","@id":"sustainability:SoilContamination","rdfs:comment":""},{"@id":"sustainability:SoilContamination#1","@type":"sustainability:SoilContamination","rdf:value":"1","rdfs:comment":"Measure contamination"},{"@id":"sustainability:SoilContamination#2","@type":"sustainability:SoilContamination","rdf:value":"2","rdfs:comment":"Monitor contamination over time"},{"@id":"sustainability:SoilContamination#3","@type":"sustainability:SoilContamination","rdf:value":"3","rdfs:comment":"Prevent contamination"},{"rdfs:label":"TheConversionOfForestsIntoProductionLands","@type":"rdfs:Class","@id":"sustainability:TheConversionOfForestsIntoProductionLands","rdfs:comment":""},{"@id":"sustainability:TheConversionOfForestsIntoProductionLands#1","@type":"sustainability:TheConversionOfForestsIntoProductionLands","rdf:value":"1","rdfs:comment":"Conversion is prohibited with exemption"},{"@id":"sustainability:TheConversionOfForestsIntoProductionLands#2","@type":"sustainability:TheConversionOfForestsIntoProductionLands","rdf:value":"2","rdfs:comment":"Conversion is prohibited w/out exemption"},{"@id":"sustainability:TheConversionOfForestsIntoProductionLands#3","@type":"sustainability:TheConversionOfForestsIntoProductionLands","rdf:value":"3","rdfs:comment":"Conversion is prohibited w/out exemption and cut-off dates are defined"},{"rdfs:label":"ChemicalsUseAndApplicationRecords","@type":"rdfs:Class","@id":"sustainability:ChemicalsUseAndApplicationRecords","rdfs:comment":""},{"@id":"sustainability:ChemicalsUseAndApplicationRecords#1","@type":"sustainability:ChemicalsUseAndApplicationRecords","rdf:value":"1","rdfs:comment":"Document use of all chemicals"},{"@id":"sustainability:ChemicalsUseAndApplicationRecords#2","@type":"sustainability:ChemicalsUseAndApplicationRecords","rdf:value":"2","rdfs:comment":"Increase efficiency/reduce chemical use"},{"rdfs:label":"UseOfOrganicFertilizer","@type":"rdfs:Class","@id":"sustainability:UseOfOrganicFertilizer","rdfs:comment":""},{"@id":"sustainability:UseOfOrganicFertilizer#1","@type":"sustainability:UseOfOrganicFertilizer","rdf:value":"1","rdfs:comment":"Use organic fertilizer (instead of synthetic fertilizer)"},{"@id":"sustainability:UseOfOrganicFertilizer#2","@type":"sustainability:UseOfOrganicFertilizer","rdf:value":"2","rdfs:comment":"A maximum amount of organic fertilizer per ha is defined"},{"rdfs:label":"ProhibitionOfUseOfHazardousChemicalsAsDefinedByWho1aAndB2AndTheStockholmAndRotterdamConventions","@type":"rdfs:Class","@id":"sustainability:ProhibitionOfUseOfHazardousChemicalsAsDefinedByWho1aAndB2AndTheStockholmAndRotterdamConventions","rdfs:comment":""},{"rdfs:label":"UseAndManagementOfGmos","@type":"rdfs:Class","@id":"sustainability:UseAndManagementOfGmos","rdfs:comment":""},{"@id":"sustainability:UseAndManagementOfGmos#1","@type":"sustainability:UseAndManagementOfGmos","rdf:value":"1","rdfs:comment":"Allow use with adequate controls to prohibit contamination"},{"@id":"sustainability:UseAndManagementOfGmos#2","@type":"sustainability:UseAndManagementOfGmos","rdf:value":"2","rdfs:comment":"Prohibit use"},{"rdfs:label":"RiskPreventionWithRegardsToUseOfGmos","@type":"rdfs:Class","@id":"sustainability:RiskPreventionWithRegardsToUseOfGmos","rdfs:comment":""},{"@id":"sustainability:RiskPreventionWithRegardsToUseOfGmos#1","@type":"sustainability:RiskPreventionWithRegardsToUseOfGmos","rdf:value":"1","rdfs:comment":"Allow use with adequate controls to prohibit contamination"},{"@id":"sustainability:RiskPreventionWithRegardsToUseOfGmos#2","@type":"sustainability:RiskPreventionWithRegardsToUseOfGmos","rdf:value":"2","rdfs:comment":"Prohibit use"},{"rdfs:label":"ProhibitionOfUseOfHazardousChemicalsAsDefinedByThePanInternationalListOfHighlyHazardousPesticides","@type":"rdfs:Class","@id":"sustainability:ProhibitionOfUseOfHazardousChemicalsAsDefinedByThePanInternationalListOfHighlyHazardousPesticides","rdfs:comment":""},{"@id":"sustainability:ProhibitionOfUseOfHazardousChemicalsAsDefinedByThePanInternationalListOfHighlyHazardousPesticides#1","@type":"sustainability:ProhibitionOfUseOfHazardousChemicalsAsDefinedByThePanInternationalListOfHighlyHazardousPesticides","rdf:value":"1","rdfs:comment":"Restrict use"},{"@id":"sustainability:ProhibitionOfUseOfHazardousChemicalsAsDefinedByThePanInternationalListOfHighlyHazardousPesticides#2","@type":"sustainability:ProhibitionOfUseOfHazardousChemicalsAsDefinedByThePanInternationalListOfHighlyHazardousPesticides","rdf:value":"2","rdfs:comment":"Prohibit use"},{"rdfs:label":"RespectListOfProhibitedChemicalsAsHarmfulToHumanHealthHStatementsH340H350H360","@type":"rdfs:Class","@id":"sustainability:RespectListOfProhibitedChemicalsAsHarmfulToHumanHealthHStatementsH340H350H360","rdfs:comment":""},{"@id":"sustainability:RespectListOfProhibitedChemicalsAsHarmfulToHumanHealthHStatementsH340H350H360#1","@type":"sustainability:RespectListOfProhibitedChemicalsAsHarmfulToHumanHealthHStatementsH340H350H360","rdf:value":"1","rdfs:comment":"Prohibit use for some applications"},{"@id":"sustainability:RespectListOfProhibitedChemicalsAsHarmfulToHumanHealthHStatementsH340H350H360#2","@type":"sustainability:RespectListOfProhibitedChemicalsAsHarmfulToHumanHealthHStatementsH340H350H360","rdf:value":"2","rdfs:comment":"Prohibit use for all applications"},{"@id":"sustainability:RespectListOfProhibitedChemicalsAsHarmfulToHumanHealthHStatementsH340H350H360#3","@type":"sustainability:RespectListOfProhibitedChemicalsAsHarmfulToHumanHealthHStatementsH340H350H360","rdf:value":"3","rdfs:comment":"Prohibit use of additional H statements for all applications"},{"rdfs:label":"RegulatedAndSustainableAccessToResourcesAndUseOfWildlifeSpecies","@type":"rdfs:Class","@id":"sustainability:RegulatedAndSustainableAccessToResourcesAndUseOfWildlifeSpecies","rdfs:comment":""},{"@id":"sustainability:RegulatedAndSustainableAccessToResourcesAndUseOfWildlifeSpecies#1","@type":"sustainability:RegulatedAndSustainableAccessToResourcesAndUseOfWildlifeSpecies","rdf:value":"1","rdfs:comment":"Monitor activities"},{"@id":"sustainability:RegulatedAndSustainableAccessToResourcesAndUseOfWildlifeSpecies#2","@type":"sustainability:RegulatedAndSustainableAccessToResourcesAndUseOfWildlifeSpecies","rdf:value":"2","rdfs:comment":"Control and regulate activities"},{"rdfs:label":"SpecificRareThreatenedOrEndangeredWildlifeSpecies","@type":"rdfs:Class","@id":"sustainability:SpecificRareThreatenedOrEndangeredWildlifeSpecies","rdfs:comment":""},{"@id":"sustainability:SpecificRareThreatenedOrEndangeredWildlifeSpecies#1","@type":"sustainability:SpecificRareThreatenedOrEndangeredWildlifeSpecies","rdf:value":"1","rdfs:comment":"Protect species - species list below IUCN red-list"},{"@id":"sustainability:SpecificRareThreatenedOrEndangeredWildlifeSpecies#2","@type":"sustainability:SpecificRareThreatenedOrEndangeredWildlifeSpecies","rdf:value":"2","rdfs:comment":"Protect species - based on IUCN red list"},{"@id":"sustainability:SpecificRareThreatenedOrEndangeredWildlifeSpecies#3","@type":"sustainability:SpecificRareThreatenedOrEndangeredWildlifeSpecies","rdf:value":"3","rdfs:comment":"Protect species - species list goes beyond IUCN red-list"},{"rdfs:label":"TheProtectionOfEcosystemsAgainstInvasiveSpecies","@type":"rdfs:Class","@id":"sustainability:TheProtectionOfEcosystemsAgainstInvasiveSpecies","rdfs:comment":""},{"@id":"sustainability:TheProtectionOfEcosystemsAgainstInvasiveSpecies#1","@type":"sustainability:TheProtectionOfEcosystemsAgainstInvasiveSpecies","rdf:value":"1","rdfs:comment":"Restrict introduction of invasive species"},{"@id":"sustainability:TheProtectionOfEcosystemsAgainstInvasiveSpecies#2","@type":"sustainability:TheProtectionOfEcosystemsAgainstInvasiveSpecies","rdf:value":"2","rdfs:comment":"Prohibit introduction of invasive species"},{"rdfs:label":"CriteriaAndPracticesRelatingToTheClearingOfLandWithFireOrExplosives","@type":"rdfs:Class","@id":"sustainability:CriteriaAndPracticesRelatingToTheClearingOfLandWithFireOrExplosives","rdfs:comment":""},{"@id":"sustainability:CriteriaAndPracticesRelatingToTheClearingOfLandWithFireOrExplosives#1","@type":"sustainability:CriteriaAndPracticesRelatingToTheClearingOfLandWithFireOrExplosives","rdf:value":"1","rdfs:comment":"Control application of fire or explosives"},{"@id":"sustainability:CriteriaAndPracticesRelatingToTheClearingOfLandWithFireOrExplosives#2","@type":"sustainability:CriteriaAndPracticesRelatingToTheClearingOfLandWithFireOrExplosives","rdf:value":"2","rdfs:comment":"Prohibit application of fire or explosives"},{"rdfs:label":"NaturalWetlandsAndOrWatercoursesAffectedByProduction","@type":"rdfs:Class","@id":"sustainability:NaturalWetlandsAndOrWatercoursesAffectedByProduction","rdfs:comment":""},{"@id":"sustainability:NaturalWetlandsAndOrWatercoursesAffectedByProduction#1","@type":"sustainability:NaturalWetlandsAndOrWatercoursesAffectedByProduction","rdf:value":"1","rdfs:comment":"Identify wetlands and/or watercourses"},{"@id":"sustainability:NaturalWetlandsAndOrWatercoursesAffectedByProduction#2","@type":"sustainability:NaturalWetlandsAndOrWatercoursesAffectedByProduction","rdf:value":"2","rdfs:comment":"Monitor wetlands and/or watercourses over time"},{"@id":"sustainability:NaturalWetlandsAndOrWatercoursesAffectedByProduction#3","@type":"sustainability:NaturalWetlandsAndOrWatercoursesAffectedByProduction","rdf:value":"3","rdfs:comment":"Maintain wetlands and/or watercourses"},{"rdfs:label":"TransportOfAnimals","@type":"rdfs:Class","@id":"sustainability:TransportOfAnimals","rdfs:comment":""},{"@id":"sustainability:TransportOfAnimals#1","@type":"sustainability:TransportOfAnimals","rdf:value":"1","rdfs:comment":"Unspecific transportation procedures OR time/distance"},{"@id":"sustainability:TransportOfAnimals#2","@type":"sustainability:TransportOfAnimals","rdf:value":"2","rdfs:comment":"Specific transportation procedures OR time/distance"},{"@id":"sustainability:TransportOfAnimals#3","@type":"sustainability:TransportOfAnimals","rdf:value":"3","rdfs:comment":"Specific transportation procedures AND time/distance"},{"rdfs:label":"TheUseOfElectricProdsWithLivestock","@type":"rdfs:Class","@id":"sustainability:TheUseOfElectricProdsWithLivestock","rdfs:comment":""},{"@id":"sustainability:TheUseOfElectricProdsWithLivestock#1","@type":"sustainability:TheUseOfElectricProdsWithLivestock","rdf:value":"1","rdfs:comment":"Use of electric prods is restricted"},{"@id":"sustainability:TheUseOfElectricProdsWithLivestock#2","@type":"sustainability:TheUseOfElectricProdsWithLivestock","rdf:value":"2","rdfs:comment":"Use of electric prods is prohibited"},{"rdfs:label":"TechniquesToBeUsedForAnimalIdentificationAndOrCastration","@type":"rdfs:Class","@id":"sustainability:TechniquesToBeUsedForAnimalIdentificationAndOrCastration","rdfs:comment":""},{"@id":"sustainability:TechniquesToBeUsedForAnimalIdentificationAndOrCastration#1","@type":"sustainability:TechniquesToBeUsedForAnimalIdentificationAndOrCastration","rdf:value":"1","rdfs:comment":"Techniques are restricted"},{"@id":"sustainability:TechniquesToBeUsedForAnimalIdentificationAndOrCastration#2","@type":"sustainability:TechniquesToBeUsedForAnimalIdentificationAndOrCastration","rdf:value":"2","rdfs:comment":"Techniques are prohibited"},{"rdfs:label":"AnimalPhysicalIntegrityEgRemovingOfTailsEarsNoseWingsHornsOrOtherBodyParts","@type":"rdfs:Class","@id":"sustainability:AnimalPhysicalIntegrityEgRemovingOfTailsEarsNoseWingsHornsOrOtherBodyParts","rdfs:comment":""},{"@id":"sustainability:AnimalPhysicalIntegrityEgRemovingOfTailsEarsNoseWingsHornsOrOtherBodyParts#1","@type":"sustainability:AnimalPhysicalIntegrityEgRemovingOfTailsEarsNoseWingsHornsOrOtherBodyParts","rdf:value":"1","rdfs:comment":"Removing of body parts is restricted"},{"@id":"sustainability:AnimalPhysicalIntegrityEgRemovingOfTailsEarsNoseWingsHornsOrOtherBodyParts#2","@type":"sustainability:AnimalPhysicalIntegrityEgRemovingOfTailsEarsNoseWingsHornsOrOtherBodyParts","rdf:value":"2","rdfs:comment":"Removing of body parts is prohibited"},{"rdfs:label":"LivestockDensityFollowingAtLeastOfficialRegulationsEGEcRegulation8892008","@type":"rdfs:Class","@id":"sustainability:LivestockDensityFollowingAtLeastOfficialRegulationsEGEcRegulation8892008","rdfs:comment":""},{"@id":"sustainability:LivestockDensityFollowingAtLeastOfficialRegulationsEGEcRegulation8892008#1","@type":"sustainability:LivestockDensityFollowingAtLeastOfficialRegulationsEGEcRegulation8892008","rdf:value":"1","rdfs:comment":"The allowed stock density is higher than defined in the EU Organic Farming Regulations"},{"@id":"sustainability:LivestockDensityFollowingAtLeastOfficialRegulationsEGEcRegulation8892008#2","@type":"sustainability:LivestockDensityFollowingAtLeastOfficialRegulationsEGEcRegulation8892008","rdf:value":"2","rdfs:comment":"The allowed stock density is as defined in the EU Organic Farming Regulations"},{"@id":"sustainability:LivestockDensityFollowingAtLeastOfficialRegulationsEGEcRegulation8892008#3","@type":"sustainability:LivestockDensityFollowingAtLeastOfficialRegulationsEGEcRegulation8892008","rdf:value":"3","rdfs:comment":"The allowed stock density is lower than defined in the EU Organic Farming Regulations"},{"rdfs:label":"OutdoorAccessLivestock","@type":"rdfs:Class","@id":"sustainability:OutdoorAccessLivestock","rdfs:comment":""},{"@id":"sustainability:OutdoorAccessLivestock#1","@type":"sustainability:OutdoorAccessLivestock","rdf:value":"1","rdfs:comment":"Outdoor access under some constraints"},{"@id":"sustainability:OutdoorAccessLivestock#2","@type":"sustainability:OutdoorAccessLivestock","rdf:value":"2","rdfs:comment":"Outdoor access without any constraints except animal welfare consideration"},{"@id":"sustainability:OutdoorAccessLivestock#3","@type":"sustainability:OutdoorAccessLivestock","rdf:value":"3","rdfs:comment":"Outdoor access is supported by specific measures"},{"rdfs:label":"AnimalHousing","@type":"rdfs:Class","@id":"sustainability:AnimalHousing","rdfs:comment":""},{"@id":"sustainability:AnimalHousing#1","@type":"sustainability:AnimalHousing","rdf:value":"1","rdfs:comment":"Animals need clean and sufficient space"},{"@id":"sustainability:AnimalHousing#2","@type":"sustainability:AnimalHousing","rdf:value":"2","rdfs:comment":"Animals need clean and sufficient space defined by specific stock density values"},{"rdfs:label":"SpecificOriginOfAnimalFeed","@type":"rdfs:Class","@id":"sustainability:SpecificOriginOfAnimalFeed","rdfs:comment":""},{"@id":"sustainability:SpecificOriginOfAnimalFeed#1","@type":"sustainability:SpecificOriginOfAnimalFeed","rdf:value":"1","rdfs:comment":"Less than 50% of the feed must be produced by the farm itself "},{"@id":"sustainability:SpecificOriginOfAnimalFeed#2","@type":"sustainability:SpecificOriginOfAnimalFeed","rdf:value":"2","rdfs:comment":"More than 50% of the feed must be produced by the farm itself"},{"rdfs:label":"SpecialQualityOfAnimalFeed","@type":"rdfs:Class","@id":"sustainability:SpecialQualityOfAnimalFeed","rdfs:comment":""},{"@id":"sustainability:SpecialQualityOfAnimalFeed#1","@type":"sustainability:SpecialQualityOfAnimalFeed","rdf:value":"1","rdfs:comment":"Quality of the feed is described"},{"@id":"sustainability:SpecialQualityOfAnimalFeed#2","@type":"sustainability:SpecialQualityOfAnimalFeed","rdf:value":"2","rdfs:comment":"Quality of the feed is defined species and age appropriate"},{"rdfs:label":"SpecialRequirementsForOrganicAnimalFeed","@type":"rdfs:Class","@id":"sustainability:SpecialRequirementsForOrganicAnimalFeed","rdfs:comment":""},{"@id":"sustainability:SpecialRequirementsForOrganicAnimalFeed#1","@type":"sustainability:SpecialRequirementsForOrganicAnimalFeed","rdf:value":"1","rdfs:comment":"A certain amount of the use of organic feed is required"},{"@id":"sustainability:SpecialRequirementsForOrganicAnimalFeed#2","@type":"sustainability:SpecialRequirementsForOrganicAnimalFeed","rdf:value":"2","rdfs:comment":"100% organic feed is required"},{"rdfs:label":"AnimalsMedication","@type":"rdfs:Class","@id":"sustainability:AnimalsMedication","rdfs:comment":""},{"@id":"sustainability:AnimalsMedication#1","@type":"sustainability:AnimalsMedication","rdf:value":"1","rdfs:comment":"Medication application is restricted"},{"@id":"sustainability:AnimalsMedication#2","@type":"sustainability:AnimalsMedication","rdf:value":"2","rdfs:comment":"Preventative application of antibiotics is prohibited"},{"rdfs:label":"AirQualityPollutionMonitoring","@type":"rdfs:Class","@id":"sustainability:AirQualityPollutionMonitoring","rdfs:comment":""},{"@id":"sustainability:AirQualityPollutionMonitoring#1","@type":"sustainability:AirQualityPollutionMonitoring","rdf:value":"1","rdfs:comment":"Measure emissions (inventory of main point source emissions to air)"},{"@id":"sustainability:AirQualityPollutionMonitoring#2","@type":"sustainability:AirQualityPollutionMonitoring","rdf:value":"2","rdfs:comment":"Monitor emissions over time"},{"@id":"sustainability:AirQualityPollutionMonitoring#3","@type":"sustainability:AirQualityPollutionMonitoring","rdf:value":"3","rdfs:comment":"Reduce emissions (through end-of-pipe technology)"},{"@id":"sustainability:AirQualityPollutionMonitoring#4","@type":"sustainability:AirQualityPollutionMonitoring","rdf:value":"4","rdfs:comment":"Increase emission efficiency (reduce emissions at source"},{"rdfs:label":"AirPollutionAlongTheTextilesProductionProcessSsct","@type":"rdfs:Class","@id":"sustainability:AirPollutionAlongTheTextilesProductionProcessSsct","rdfs:comment":""},{"@id":"sustainability:AirPollutionAlongTheTextilesProductionProcessSsct#1","@type":"sustainability:AirPollutionAlongTheTextilesProductionProcessSsct","rdf:value":"1","rdfs:comment":"For some production steps"},{"@id":"sustainability:AirPollutionAlongTheTextilesProductionProcessSsct#2","@type":"sustainability:AirPollutionAlongTheTextilesProductionProcessSsct","rdf:value":"2","rdfs:comment":"For all production steps"},{"rdfs:label":"SpecificRequirementsForHandlingDisposalOfWasteByThirdParties","@type":"rdfs:Class","@id":"sustainability:SpecificRequirementsForHandlingDisposalOfWasteByThirdParties","rdfs:comment":""},{"@id":"sustainability:SpecificRequirementsForHandlingDisposalOfWasteByThirdParties#1","@type":"sustainability:SpecificRequirementsForHandlingDisposalOfWasteByThirdParties","rdf:value":"1","rdfs:comment":"Keep records on third party contractors"},{"@id":"sustainability:SpecificRequirementsForHandlingDisposalOfWasteByThirdParties#2","@type":"sustainability:SpecificRequirementsForHandlingDisposalOfWasteByThirdParties","rdf:value":"2","rdfs:comment":"Evaluate third party contractors (in terms of suitability and disposal/treatment methods"},{"rdfs:label":"PracticesRelatedToTheUseOfFireToEliminateWaste","@type":"rdfs:Class","@id":"sustainability:PracticesRelatedToTheUseOfFireToEliminateWaste","rdfs:comment":""},{"@id":"sustainability:PracticesRelatedToTheUseOfFireToEliminateWaste#1","@type":"sustainability:PracticesRelatedToTheUseOfFireToEliminateWaste","rdf:value":"1","rdfs:comment":"Restrict waste burning"},{"@id":"sustainability:PracticesRelatedToTheUseOfFireToEliminateWaste#2","@type":"sustainability:PracticesRelatedToTheUseOfFireToEliminateWaste","rdf:value":"2","rdfs:comment":"Prohibit waste burning"},{"rdfs:label":"PrinciplesAndPracticesRelatedToAvoidanceOfUncontrolledWasteLandfilling","@type":"rdfs:Class","@id":"sustainability:PrinciplesAndPracticesRelatedToAvoidanceOfUncontrolledWasteLandfilling","rdfs:comment":""},{"@id":"sustainability:PrinciplesAndPracticesRelatedToAvoidanceOfUncontrolledWasteLandfilling#1","@type":"sustainability:PrinciplesAndPracticesRelatedToAvoidanceOfUncontrolledWasteLandfilling","rdf:value":"1","rdfs:comment":"Restrict waste landfilling"},{"@id":"sustainability:PrinciplesAndPracticesRelatedToAvoidanceOfUncontrolledWasteLandfilling#2","@type":"sustainability:PrinciplesAndPracticesRelatedToAvoidanceOfUncontrolledWasteLandfilling","rdf:value":"2","rdfs:comment":"Prohibit waste landfilling"},{"rdfs:label":"MonitoringAndMeasuringSolidWasteVolumes","@type":"rdfs:Class","@id":"sustainability:MonitoringAndMeasuringSolidWasteVolumes","rdfs:comment":""},{"@id":"sustainability:MonitoringAndMeasuringSolidWasteVolumes#1","@type":"sustainability:MonitoringAndMeasuringSolidWasteVolumes","rdf:value":"1","rdfs:comment":"Measure volumes of waste"},{"@id":"sustainability:MonitoringAndMeasuringSolidWasteVolumes#2","@type":"sustainability:MonitoringAndMeasuringSolidWasteVolumes","rdf:value":"2","rdfs:comment":"Monitor volumes of waste over time"},{"rdfs:label":"MonitoringAndMeasuringWasteToxicity","@type":"rdfs:Class","@id":"sustainability:MonitoringAndMeasuringWasteToxicity","rdfs:comment":""},{"@id":"sustainability:MonitoringAndMeasuringWasteToxicity#1","@type":"sustainability:MonitoringAndMeasuringWasteToxicity","rdf:value":"1","rdfs:comment":"Document toxic waste"},{"@id":"sustainability:MonitoringAndMeasuringWasteToxicity#2","@type":"sustainability:MonitoringAndMeasuringWasteToxicity","rdf:value":"2","rdfs:comment":"Reduce and/or treat toxic waste"},{"rdfs:label":"WaterResourcesMonitoringUseAndConsumption","@type":"rdfs:Class","@id":"sustainability:WaterResourcesMonitoringUseAndConsumption","rdfs:comment":""},{"@id":"sustainability:WaterResourcesMonitoringUseAndConsumption#1","@type":"sustainability:WaterResourcesMonitoringUseAndConsumption","rdf:value":"1","rdfs:comment":"Measure volumes of water consumption"},{"@id":"sustainability:WaterResourcesMonitoringUseAndConsumption#2","@type":"sustainability:WaterResourcesMonitoringUseAndConsumption","rdf:value":"2","rdfs:comment":"Monitor volumes of water consumption over time"},{"@id":"sustainability:WaterResourcesMonitoringUseAndConsumption#3","@type":"sustainability:WaterResourcesMonitoringUseAndConsumption","rdf:value":"3","rdfs:comment":"Increase efficiency/reduce water consumption (up to a defined threshold"},{"rdfs:label":"QualityOfWaterUsedInProductionAgricultureForestry","@type":"rdfs:Class","@id":"sustainability:QualityOfWaterUsedInProductionAgricultureForestry","rdfs:comment":""},{"@id":"sustainability:QualityOfWaterUsedInProductionAgricultureForestry#1","@type":"sustainability:QualityOfWaterUsedInProductionAgricultureForestry","rdf:value":"1","rdfs:comment":"Measure quality of input water"},{"@id":"sustainability:QualityOfWaterUsedInProductionAgricultureForestry#2","@type":"sustainability:QualityOfWaterUsedInProductionAgricultureForestry","rdf:value":"2","rdfs:comment":"Monitor quality of input water over time"},{"@id":"sustainability:QualityOfWaterUsedInProductionAgricultureForestry#3","@type":"sustainability:QualityOfWaterUsedInProductionAgricultureForestry","rdf:value":"3","rdfs:comment":"Ensure appropriate quality of input water"},{"rdfs:label":"WastewaterQualityManagementAndTreatment","@type":"rdfs:Class","@id":"sustainability:WastewaterQualityManagementAndTreatment","rdfs:comment":""},{"@id":"sustainability:WastewaterQualityManagementAndTreatment#1","@type":"sustainability:WastewaterQualityManagementAndTreatment","rdf:value":"1","rdfs:comment":"Measure wastewater quality"},{"@id":"sustainability:WastewaterQualityManagementAndTreatment#2","@type":"sustainability:WastewaterQualityManagementAndTreatment","rdf:value":"2","rdfs:comment":"Monitor wastewater quality over time"},{"@id":"sustainability:WastewaterQualityManagementAndTreatment#3","@type":"sustainability:WastewaterQualityManagementAndTreatment","rdf:value":"3","rdfs:comment":"Treat wastewater"},{"@id":"sustainability:WastewaterQualityManagementAndTreatment#4","@type":"sustainability:WastewaterQualityManagementAndTreatment","rdf:value":"4","rdfs:comment":"Treat wastewater with parameters defined to ensure appropriate quality of wastewater"},{"rdfs:label":"LimitationsOfWastewaterVolume","@type":"rdfs:Class","@id":"sustainability:LimitationsOfWastewaterVolume","rdfs:comment":""},{"@id":"sustainability:LimitationsOfWastewaterVolume#1","@type":"sustainability:LimitationsOfWastewaterVolume","rdf:value":"1","rdfs:comment":"Measure wastewater volumes"},{"@id":"sustainability:LimitationsOfWastewaterVolume#2","@type":"sustainability:LimitationsOfWastewaterVolume","rdf:value":"2","rdfs:comment":"Monitor wastewater volumes over time"},{"@id":"sustainability:LimitationsOfWastewaterVolume#3","@type":"sustainability:LimitationsOfWastewaterVolume","rdf:value":"3","rdfs:comment":"Limit wastewater volumes"},{"rdfs:label":"WastewaterBasicParametersForTextileIndustry","@type":"rdfs:Class","@id":"sustainability:WastewaterBasicParametersForTextileIndustry","rdfs:comment":""},{"@id":"sustainability:WastewaterBasicParametersForTextileIndustry#1","@type":"sustainability:WastewaterBasicParametersForTextileIndustry","rdf:value":"1","rdfs:comment":"Only for one production step"},{"@id":"sustainability:WastewaterBasicParametersForTextileIndustry#2","@type":"sustainability:WastewaterBasicParametersForTextileIndustry","rdf:value":"2","rdfs:comment":"For different production steps"},{"rdfs:label":"WastewaterAdvancedParametersForTextileIndustry","@type":"rdfs:Class","@id":"sustainability:WastewaterAdvancedParametersForTextileIndustry","rdfs:comment":""},{"@id":"sustainability:WastewaterAdvancedParametersForTextileIndustry#1","@type":"sustainability:WastewaterAdvancedParametersForTextileIndustry","rdf:value":"1","rdfs:comment":"Not all of these parameters are covered"},{"@id":"sustainability:WastewaterAdvancedParametersForTextileIndustry#2","@type":"sustainability:WastewaterAdvancedParametersForTextileIndustry","rdf:value":"2","rdfs:comment":"All of these parameters are covered"},{"rdfs:label":"WastewaterParametersForPaperIndustry","@type":"rdfs:Class","@id":"sustainability:WastewaterParametersForPaperIndustry","rdfs:comment":""},{"@id":"sustainability:WastewaterParametersForPaperIndustry#1","@type":"sustainability:WastewaterParametersForPaperIndustry","rdf:value":"1","rdfs:comment":"Not all of these parameters are covered"},{"@id":"sustainability:WastewaterParametersForPaperIndustry#2","@type":"sustainability:WastewaterParametersForPaperIndustry","rdf:value":"2","rdfs:comment":"All of these parameters are covered"},{"rdfs:label":"EnergyConsumptionMonitoringRecording","@type":"rdfs:Class","@id":"sustainability:EnergyConsumptionMonitoringRecording","rdfs:comment":""},{"@id":"sustainability:EnergyConsumptionMonitoringRecording#1","@type":"sustainability:EnergyConsumptionMonitoringRecording","rdf:value":"1","rdfs:comment":"Measure energy consumption"},{"@id":"sustainability:EnergyConsumptionMonitoringRecording#2","@type":"sustainability:EnergyConsumptionMonitoringRecording","rdf:value":"2","rdfs:comment":"Monitor energy consumption over time"},{"@id":"sustainability:EnergyConsumptionMonitoringRecording#3","@type":"sustainability:EnergyConsumptionMonitoringRecording","rdf:value":"3","rdfs:comment":"Increase efficiency/reduce energy consumption OR increase use of renewables"},{"@id":"sustainability:EnergyConsumptionMonitoringRecording#4","@type":"sustainability:EnergyConsumptionMonitoringRecording","rdf:value":"4","rdfs:comment":"Increase efficiency/reduce energy consumption AND increase use of renewables"},{"rdfs:label":"TheProtectionOfHighCarbonLandscapesLandWithHighCarbonStockHcs","@type":"rdfs:Class","@id":"sustainability:TheProtectionOfHighCarbonLandscapesLandWithHighCarbonStockHcs","rdfs:comment":""},{"@id":"sustainability:TheProtectionOfHighCarbonLandscapesLandWithHighCarbonStockHcs#1","@type":"sustainability:TheProtectionOfHighCarbonLandscapesLandWithHighCarbonStockHcs","rdf:value":"1","rdfs:comment":"Calculate carbon stocks"},{"@id":"sustainability:TheProtectionOfHighCarbonLandscapesLandWithHighCarbonStockHcs#2","@type":"sustainability:TheProtectionOfHighCarbonLandscapesLandWithHighCarbonStockHcs","rdf:value":"2","rdfs:comment":"Monitor carbon stocks over time"},{"@id":"sustainability:TheProtectionOfHighCarbonLandscapesLandWithHighCarbonStockHcs#3","@type":"sustainability:TheProtectionOfHighCarbonLandscapesLandWithHighCarbonStockHcs","rdf:value":"3","rdfs:comment":"Protect high carbon landscape"},{"rdfs:label":"MonitoringGhgCarbonEmissions","@type":"rdfs:Class","@id":"sustainability:MonitoringGhgCarbonEmissions","rdfs:comment":""},{"@id":"sustainability:MonitoringGhgCarbonEmissions#1","@type":"sustainability:MonitoringGhgCarbonEmissions","rdf:value":"1","rdfs:comment":"Measure/calculate GHG emissions"},{"@id":"sustainability:MonitoringGhgCarbonEmissions#2","@type":"sustainability:MonitoringGhgCarbonEmissions","rdf:value":"2","rdfs:comment":"Monitor GHG emissions over time"},{"@id":"sustainability:MonitoringGhgCarbonEmissions#3","@type":"sustainability:MonitoringGhgCarbonEmissions","rdf:value":"3","rdfs:comment":"Reduce GHG net emissions/GHG intensity"},{"rdfs:label":"TheUseOfSyntheticPesticides","@type":"rdfs:Class","@id":"sustainability:TheUseOfSyntheticPesticides","rdfs:comment":""},{"@id":"sustainability:TheUseOfSyntheticPesticides#1","@type":"sustainability:TheUseOfSyntheticPesticides","rdf:value":"1","rdfs:comment":"Restrict use of synthetic pesticides"},{"@id":"sustainability:TheUseOfSyntheticPesticides#2","@type":"sustainability:TheUseOfSyntheticPesticides","rdf:value":"2","rdfs:comment":"Prohibit use of synthetic pesticides"},{"rdfs:label":"TheUseOfChlorineGasAsBleachingAgent","@type":"rdfs:Class","@id":"sustainability:TheUseOfChlorineGasAsBleachingAgent","rdfs:comment":""},{"@id":"sustainability:TheUseOfChlorineGasAsBleachingAgent#1","@type":"sustainability:TheUseOfChlorineGasAsBleachingAgent","rdf:value":"1","rdfs:comment":"Restrict use"},{"@id":"sustainability:TheUseOfChlorineGasAsBleachingAgent#2","@type":"sustainability:TheUseOfChlorineGasAsBleachingAgent","rdf:value":"2","rdfs:comment":"Prohibit use"},{"rdfs:label":"ChemicalsDescribedAsARiskToTheEnvironment","@type":"rdfs:Class","@id":"sustainability:ChemicalsDescribedAsARiskToTheEnvironment","rdfs:comment":""},{"@id":"sustainability:ChemicalsDescribedAsARiskToTheEnvironment#1","@type":"sustainability:ChemicalsDescribedAsARiskToTheEnvironment","rdf:value":"1","rdfs:comment":"Prohibit use for some applications"},{"@id":"sustainability:ChemicalsDescribedAsARiskToTheEnvironment#2","@type":"sustainability:ChemicalsDescribedAsARiskToTheEnvironment","rdf:value":"2","rdfs:comment":"Prohibit use for all applications"},{"@id":"sustainability:ChemicalsDescribedAsARiskToTheEnvironment#3","@type":"sustainability:ChemicalsDescribedAsARiskToTheEnvironment","rdf:value":"3","rdfs:comment":"Prohibit use of additional H statements for all applications"},{"rdfs:label":"ChemicalsDescribedAsARiskToHumanHealth","@type":"rdfs:Class","@id":"sustainability:ChemicalsDescribedAsARiskToHumanHealth","rdfs:comment":""},{"@id":"sustainability:ChemicalsDescribedAsARiskToHumanHealth#1","@type":"sustainability:ChemicalsDescribedAsARiskToHumanHealth","rdf:value":"1","rdfs:comment":"Prohibit use for some applications"},{"@id":"sustainability:ChemicalsDescribedAsARiskToHumanHealth#2","@type":"sustainability:ChemicalsDescribedAsARiskToHumanHealth","rdf:value":"2","rdfs:comment":"Prohibit use for all applications"},{"@id":"sustainability:ChemicalsDescribedAsARiskToHumanHealth#3","@type":"sustainability:ChemicalsDescribedAsARiskToHumanHealth","rdf:value":"3","rdfs:comment":"Prohibit use of additional H statements for all applications"},{"rdfs:label":"TestingTheFinalProductRegardingAccumulationOfChemicalResidues","@type":"rdfs:Class","@id":"sustainability:TestingTheFinalProductRegardingAccumulationOfChemicalResidues","rdfs:comment":""},{"@id":"sustainability:TestingTheFinalProductRegardingAccumulationOfChemicalResidues#1","@type":"sustainability:TestingTheFinalProductRegardingAccumulationOfChemicalResidues","rdf:value":"1","rdfs:comment":"Limit values for less or equal than 10 residues are defined"},{"@id":"sustainability:TestingTheFinalProductRegardingAccumulationOfChemicalResidues#2","@type":"sustainability:TestingTheFinalProductRegardingAccumulationOfChemicalResidues","rdf:value":"2","rdfs:comment":"Limit values for more than 10 residues are defined"},{"rdfs:label":"TheProductionOfNaturalFibres","@type":"rdfs:Class","@id":"sustainability:TheProductionOfNaturalFibres","rdfs:comment":""},{"@id":"sustainability:TheProductionOfNaturalFibres#1","@type":"sustainability:TheProductionOfNaturalFibres","rdf:value":"1","rdfs:comment":"Fibres are extensively tested for agrochemical residues"},{"@id":"sustainability:TheProductionOfNaturalFibres#2","@type":"sustainability:TheProductionOfNaturalFibres","rdf:value":"2","rdfs:comment":"Fibres are extensively tested for agrochemical residues AND production follows IPM"},{"@id":"sustainability:TheProductionOfNaturalFibres#3","@type":"sustainability:TheProductionOfNaturalFibres","rdf:value":"3","rdfs:comment":"Less than 50% of fibres is organic (non-organic fibres has to be tested for agrochemical residues)"},{"@id":"sustainability:TheProductionOfNaturalFibres#4","@type":"sustainability:TheProductionOfNaturalFibres","rdf:value":"4","rdfs:comment":"51% - 90% of fibres is organic (non-organic fibres has to be tested for agrochemical residues)"},{"@id":"sustainability:TheProductionOfNaturalFibres#5","@type":"sustainability:TheProductionOfNaturalFibres","rdf:value":"5","rdfs:comment":"More than 90% of fibres is organic"},{"rdfs:label":"TheProductionOfSyntheticFibers","@type":"rdfs:Class","@id":"sustainability:TheProductionOfSyntheticFibers","rdfs:comment":""},{"@id":"sustainability:TheProductionOfSyntheticFibers#1","@type":"sustainability:TheProductionOfSyntheticFibers","rdf:value":"1","rdfs:comment":"General criteria"},{"@id":"sustainability:TheProductionOfSyntheticFibers#2","@type":"sustainability:TheProductionOfSyntheticFibers","rdf:value":"2","rdfs:comment":"Specific criteria depending on different types of synthetic fibers"},{"rdfs:label":"TheUsageOfRecycledFibres","@type":"rdfs:Class","@id":"sustainability:TheUsageOfRecycledFibres","rdfs:comment":""},{"@id":"sustainability:TheUsageOfRecycledFibres#1","@type":"sustainability:TheUsageOfRecycledFibres","rdf:value":"1","rdfs:comment":"Use of recycled material in packaging"},{"@id":"sustainability:TheUsageOfRecycledFibres#2","@type":"sustainability:TheUsageOfRecycledFibres","rdf:value":"2","rdfs:comment":"Use of recycled material in product"},{"@id":"sustainability:TheUsageOfRecycledFibres#3","@type":"sustainability:TheUsageOfRecycledFibres","rdf:value":"3","rdfs:comment":"Use of recycled material in packaging and produce"},{"rdfs:label":"OnSyntheticFertilizers","@type":"rdfs:Class","@id":"sustainability:OnSyntheticFertilizers","rdfs:comment":""},{"@id":"sustainability:OnSyntheticFertilizers#1","@type":"sustainability:OnSyntheticFertilizers","rdf:value":"1","rdfs:comment":"Restrict use of synthetic fertilizers"},{"@id":"sustainability:OnSyntheticFertilizers#2","@type":"sustainability:OnSyntheticFertilizers","rdf:value":"2","rdfs:comment":"Prohibit use of synthetic fertilizers"},{"rdfs:label":"TheUseOfWoodenFibres","@type":"rdfs:Class","@id":"sustainability:TheUseOfWoodenFibres","rdfs:comment":""},{"@id":"sustainability:TheUseOfWoodenFibres#1","@type":"sustainability:TheUseOfWoodenFibres","rdf:value":"1","rdfs:comment":"50% - 69% of certified fibres from sustainable forestry"},{"@id":"sustainability:TheUseOfWoodenFibres#2","@type":"sustainability:TheUseOfWoodenFibres","rdf:value":"2","rdfs:comment":"50% - 69% of recycled fibres or 70% - 94% of certified fibres from sustainable forestry"},{"@id":"sustainability:TheUseOfWoodenFibres#3","@type":"sustainability:TheUseOfWoodenFibres","rdf:value":"3","rdfs:comment":"70% - 94% of recycled fibres or min. 95% of certified fibres from sustainable forestry"},{"@id":"sustainability:TheUseOfWoodenFibres#4","@type":"sustainability:TheUseOfWoodenFibres","rdf:value":"4","rdfs:comment":"Min. 95% of recycled fibre"},{"rdfs:label":"EnergyConsumptionInTheProductionPhase","@type":"rdfs:Class","@id":"sustainability:EnergyConsumptionInTheProductionPhase","rdfs:comment":""},{"@id":"sustainability:EnergyConsumptionInTheProductionPhase#1","@type":"sustainability:EnergyConsumptionInTheProductionPhase","rdf:value":"1","rdfs:comment":"Measure energy consumption of the main nine suppliers (details see guidance)"},{"@id":"sustainability:EnergyConsumptionInTheProductionPhase#2","@type":"sustainability:EnergyConsumptionInTheProductionPhase","rdf:value":"2","rdfs:comment":"Reduce energy consumption of the main nine suppliers (details see guidance)"},{"rdfs:label":"TheUsageOfRenewableEnergyInTheProductionPhaseOfTheHardware","@type":"rdfs:Class","@id":"sustainability:TheUsageOfRenewableEnergyInTheProductionPhaseOfTheHardware","rdfs:comment":""},{"@id":"sustainability:TheUsageOfRenewableEnergyInTheProductionPhaseOfTheHardware#1","@type":"sustainability:TheUsageOfRenewableEnergyInTheProductionPhaseOfTheHardware","rdf:value":"1","rdfs:comment":"Balance sheet of electricity usage or comparable evidence for selected major suppliers of hardware components that purchased electricity leads to additional environmental benefits"},{"@id":"sustainability:TheUsageOfRenewableEnergyInTheProductionPhaseOfTheHardware#2","@type":"sustainability:TheUsageOfRenewableEnergyInTheProductionPhaseOfTheHardware","rdf:value":"2","rdfs:comment":"Balance sheet of electricity usage or comparable evidence for selected major suppliers of hardware components and certified by external, third-party institution that purchased electricity leads to additional environmental benefits"},{"rdfs:label":"FGhgEmissions","@type":"rdfs:Class","@id":"sustainability:FGhgEmissions","rdfs:comment":""},{"@id":"sustainability:FGhgEmissions#1","@type":"sustainability:FGhgEmissions","rdf:value":"1","rdfs:comment":"Require information on F-GHG emissions from suppliers"},{"@id":"sustainability:FGhgEmissions#2","@type":"sustainability:FGhgEmissions","rdf:value":"2","rdfs:comment":"Require an installed abatement system or a certain reduction of F-GHG emissions from supplies"},{"rdfs:label":"PowerConsumptionAndPowerManagementDuringTheUsePhase","@type":"rdfs:Class","@id":"sustainability:PowerConsumptionAndPowerManagementDuringTheUsePhase","rdfs:comment":""},{"@id":"sustainability:PowerConsumptionAndPowerManagementDuringTheUsePhase#1","@type":"sustainability:PowerConsumptionAndPowerManagementDuringTheUsePhase","rdf:value":"1","rdfs:comment":"Energy efficiency criteria equivalent to current version of energy star OR criteria meet EU Regulation including requirements effecting on 1 January 2016"},{"@id":"sustainability:PowerConsumptionAndPowerManagementDuringTheUsePhase#2","@type":"sustainability:PowerConsumptionAndPowerManagementDuringTheUsePhase","rdf:value":"2","rdfs:comment":"Energy efficiency criteria stricter than current version of energy star OR criteria are stricter than EU Regulation including requirements effecting on 1 January 2016"},{"rdfs:label":"HStatementsH340H341H350H351H360H361","@type":"rdfs:Class","@id":"sustainability:HStatementsH340H341H350H351H360H361","rdfs:comment":""},{"@id":"sustainability:HStatementsH340H341H350H351H360H361#1","@type":"sustainability:HStatementsH340H341H350H351H360H361","rdf:value":"1","rdfs:comment":"Prohibit use for some applications"},{"@id":"sustainability:HStatementsH340H341H350H351H360H361#2","@type":"sustainability:HStatementsH340H341H350H351H360H361","rdf:value":"2","rdfs:comment":"Prohibit use for all applications"},{"@id":"sustainability:HStatementsH340H341H350H351H360H361#3","@type":"sustainability:HStatementsH340H341H350H351H360H361","rdf:value":"3","rdfs:comment":"Prohibit use of additional H statements for all applications"},{"rdfs:label":"TheUseOfMercuryCadmiumLeadChromiumVi","@type":"rdfs:Class","@id":"sustainability:TheUseOfMercuryCadmiumLeadChromiumVi","rdfs:comment":""},{"@id":"sustainability:TheUseOfMercuryCadmiumLeadChromiumVi#1","@type":"sustainability:TheUseOfMercuryCadmiumLeadChromiumVi","rdf:value":"1","rdfs:comment":"Comply with RoHS directive"},{"@id":"sustainability:TheUseOfMercuryCadmiumLeadChromiumVi#2","@type":"sustainability:TheUseOfMercuryCadmiumLeadChromiumVi","rdf:value":"2","rdfs:comment":"Goes beyond RoHS directive for some heavy metals"},{"@id":"sustainability:TheUseOfMercuryCadmiumLeadChromiumVi#3","@type":"sustainability:TheUseOfMercuryCadmiumLeadChromiumVi","rdf:value":"3","rdfs:comment":"Goes beyond RoHS directive for all heavy metals"},{"rdfs:label":"TheUseOfFlameRetardants","@type":"rdfs:Class","@id":"sustainability:TheUseOfFlameRetardants","rdfs:comment":""},{"@id":"sustainability:TheUseOfFlameRetardants#1","@type":"sustainability:TheUseOfFlameRetardants","rdf:value":"1","rdfs:comment":"Prohibit use of some halogenated flame retardants"},{"@id":"sustainability:TheUseOfFlameRetardants#2","@type":"sustainability:TheUseOfFlameRetardants","rdf:value":"2","rdfs:comment":"Prohibit use of halogenated flame retardants"},{"@id":"sustainability:TheUseOfFlameRetardants#3","@type":"sustainability:TheUseOfFlameRetardants","rdf:value":"3","rdfs:comment":"Prohibit use of halogenated and other problematic flame retardants"},{"@id":"sustainability:TheUseOfFlameRetardants#1","@type":"sustainability:TheUseOfFlameRetardants","rdf:value":"1","rdfs:comment":"Prohibit use of halogenated flame retardants"},{"@id":"sustainability:TheUseOfFlameRetardants#2","@type":"sustainability:TheUseOfFlameRetardants","rdf:value":"2","rdfs:comment":"Prohibit use of halogenated and other flame retardants"},{"rdfs:label":"TheUseOfFlameRetardants","@type":"rdfs:Class","@id":"sustainability:TheUseOfFlameRetardants","rdfs:comment":""},{"@id":"sustainability:TheUseOfFlameRetardants#1","@type":"sustainability:TheUseOfFlameRetardants","rdf:value":"1","rdfs:comment":"Prohibit use of some halogenated flame retardants"},{"@id":"sustainability:TheUseOfFlameRetardants#2","@type":"sustainability:TheUseOfFlameRetardants","rdf:value":"2","rdfs:comment":"Prohibit use of halogenated flame retardants"},{"@id":"sustainability:TheUseOfFlameRetardants#3","@type":"sustainability:TheUseOfFlameRetardants","rdf:value":"3","rdfs:comment":"Prohibit use of halogenated and other problematic flame retardants"},{"@id":"sustainability:TheUseOfFlameRetardants#1","@type":"sustainability:TheUseOfFlameRetardants","rdf:value":"1","rdfs:comment":"Prohibit use of halogenated flame retardants"},{"@id":"sustainability:TheUseOfFlameRetardants#2","@type":"sustainability:TheUseOfFlameRetardants","rdf:value":"2","rdfs:comment":"Prohibit use of halogenated and other flame retardants"},{"rdfs:label":"TheUseOfPlasticizersWithAdverseEnvironmentalAndHealthImpact","@type":"rdfs:Class","@id":"sustainability:TheUseOfPlasticizersWithAdverseEnvironmentalAndHealthImpact","rdfs:comment":""},{"@id":"sustainability:TheUseOfPlasticizersWithAdverseEnvironmentalAndHealthImpact#1","@type":"sustainability:TheUseOfPlasticizersWithAdverseEnvironmentalAndHealthImpact","rdf:value":"1","rdfs:comment":"Restrict use of problematic phthalates"},{"@id":"sustainability:TheUseOfPlasticizersWithAdverseEnvironmentalAndHealthImpact#2","@type":"sustainability:TheUseOfPlasticizersWithAdverseEnvironmentalAndHealthImpact","rdf:value":"2","rdfs:comment":"Restrict use of phthalates and other problematic plasticizers (e.g. halogenated plasticizers"},{"rdfs:label":"TheUseOfBiocidesInTheFinishingProcess","@type":"rdfs:Class","@id":"sustainability:TheUseOfBiocidesInTheFinishingProcess","rdfs:comment":""},{"@id":"sustainability:TheUseOfBiocidesInTheFinishingProcess#1","@type":"sustainability:TheUseOfBiocidesInTheFinishingProcess","rdf:value":"1","rdfs:comment":"Restrict use"},{"@id":"sustainability:TheUseOfBiocidesInTheFinishingProcess#2","@type":"sustainability:TheUseOfBiocidesInTheFinishingProcess","rdf:value":"2","rdfs:comment":"Prohibit use"},{"rdfs:label":"TheUseOfPolymersContainingHalogens","@type":"rdfs:Class","@id":"sustainability:TheUseOfPolymersContainingHalogens","rdfs:comment":""},{"@id":"sustainability:TheUseOfPolymersContainingHalogens#1","@type":"sustainability:TheUseOfPolymersContainingHalogens","rdf:value":"1","rdfs:comment":"Restrict use"},{"@id":"sustainability:TheUseOfPolymersContainingHalogens#2","@type":"sustainability:TheUseOfPolymersContainingHalogens","rdf:value":"2","rdfs:comment":"Prohibit use"},{"rdfs:label":"TheRecyclabilityOfPlasticsUsed","@type":"rdfs:Class","@id":"sustainability:TheRecyclabilityOfPlasticsUsed","rdfs:comment":""},{"@id":"sustainability:TheRecyclabilityOfPlasticsUsed#1","@type":"sustainability:TheRecyclabilityOfPlasticsUsed","rdf:value":"1","rdfs:comment":"One of the listed aspects are covered"},{"@id":"sustainability:TheRecyclabilityOfPlasticsUsed#2","@type":"sustainability:TheRecyclabilityOfPlasticsUsed","rdf:value":"2","rdfs:comment":"At least two of the listed aspects are covered"},{"rdfs:label":"EnvironmentalResponsibleMiningPractices","@type":"rdfs:Class","@id":"sustainability:EnvironmentalResponsibleMiningPractices","rdfs:comment":""},{"@id":"sustainability:EnvironmentalResponsibleMiningPractices#1","@type":"sustainability:EnvironmentalResponsibleMiningPractices","rdf:value":"1","rdfs:comment":"Implement risk assessments"},{"@id":"sustainability:EnvironmentalResponsibleMiningPractices#2","@type":"sustainability:EnvironmentalResponsibleMiningPractices","rdf:value":"2","rdfs:comment":"Implement risk assessments and identified improvement measures OR implement a credible mining certification scheme"},{"rdfs:label":"TheUseOfRecycledMaterialInThePackaging","@type":"rdfs:Class","@id":"sustainability:TheUseOfRecycledMaterialInThePackaging","rdfs:comment":""},{"@id":"sustainability:TheUseOfRecycledMaterialInThePackaging#1","@type":"sustainability:TheUseOfRecycledMaterialInThePackaging","rdf:value":"1","rdfs:comment":"Information on recycled material content in packaging"},{"@id":"sustainability:TheUseOfRecycledMaterialInThePackaging#2","@type":"sustainability:TheUseOfRecycledMaterialInThePackaging","rdf:value":"2","rdfs:comment":"Recycled material content of card boxes in packaging ≥ 50% and < 70%"},{"@id":"sustainability:TheUseOfRecycledMaterialInThePackaging#3","@type":"sustainability:TheUseOfRecycledMaterialInThePackaging","rdf:value":"3","rdfs:comment":"Recycled material content of card boxes in packaging ≥ 70%"},{"rdfs:label":"TheUseOfPostconsumerRecycledContentInTheProduct","@type":"rdfs:Class","@id":"sustainability:TheUseOfPostconsumerRecycledContentInTheProduct","rdfs:comment":""},{"@id":"sustainability:TheUseOfPostconsumerRecycledContentInTheProduct#1","@type":"sustainability:TheUseOfPostconsumerRecycledContentInTheProduct","rdf:value":"1","rdfs:comment":"Information on postconsumer recycled content in product"},{"@id":"sustainability:TheUseOfPostconsumerRecycledContentInTheProduct#2","@type":"sustainability:TheUseOfPostconsumerRecycledContentInTheProduct","rdf:value":"2","rdfs:comment":"Postconsumer recycled content in product ≥ 5% and < 10%"},{"@id":"sustainability:TheUseOfPostconsumerRecycledContentInTheProduct#3","@type":"sustainability:TheUseOfPostconsumerRecycledContentInTheProduct","rdf:value":"3","rdfs:comment":"Postconsumer recycled content in product ≥ 10%"},{"rdfs:label":"EnvironmentalManagementInstrumentsLikeEmasOrIso14001","@type":"rdfs:Class","@id":"sustainability:EnvironmentalManagementInstrumentsLikeEmasOrIso14001","rdfs:comment":""},{"@id":"sustainability:EnvironmentalManagementInstrumentsLikeEmasOrIso14001#1","@type":"sustainability:EnvironmentalManagementInstrumentsLikeEmasOrIso14001","rdf:value":"1","rdfs:comment":"Verification (self-declaration) of final manufacturing plant"},{"@id":"sustainability:EnvironmentalManagementInstrumentsLikeEmasOrIso14001#2","@type":"sustainability:EnvironmentalManagementInstrumentsLikeEmasOrIso14001","rdf:value":"2","rdfs:comment":"Certification (third party) of final manufacturing plant"},{"@id":"sustainability:EnvironmentalManagementInstrumentsLikeEmasOrIso14001#3","@type":"sustainability:EnvironmentalManagementInstrumentsLikeEmasOrIso14001","rdf:value":"3","rdfs:comment":"Certification (third party) of final manufacturing plant and suppliers"},{"rdfs:label":"TheUseOfFormaldehyde","@type":"rdfs:Class","@id":"sustainability:TheUseOfFormaldehyde","rdfs:comment":""},{"@id":"sustainability:TheUseOfFormaldehyde#1","@type":"sustainability:TheUseOfFormaldehyde","rdf:value":"1","rdfs:comment":"Restrict use"},{"@id":"sustainability:TheUseOfFormaldehyde#2","@type":"sustainability:TheUseOfFormaldehyde","rdf:value":"2","rdfs:comment":"Prohibit use"},{"rdfs:label":"AnAdditionalLifetimeGuaranteeForTheProductBeyondTheLegalObligations","@type":"rdfs:Class","@id":"sustainability:AnAdditionalLifetimeGuaranteeForTheProductBeyondTheLegalObligations","rdfs:comment":""},{"@id":"sustainability:AnAdditionalLifetimeGuaranteeForTheProductBeyondTheLegalObligations#1","@type":"sustainability:AnAdditionalLifetimeGuaranteeForTheProductBeyondTheLegalObligations","rdf:value":"1","rdfs:comment":"Period of guarantee ≥ 1 year and ≤ 2 years"},{"@id":"sustainability:AnAdditionalLifetimeGuaranteeForTheProductBeyondTheLegalObligations#2","@type":"sustainability:AnAdditionalLifetimeGuaranteeForTheProductBeyondTheLegalObligations","rdf:value":"2","rdfs:comment":"Period of guarantee > 2 years"},{"rdfs:label":"TheAvailabilityOfSparePartsForTheProduct","@type":"rdfs:Class","@id":"sustainability:TheAvailabilityOfSparePartsForTheProduct","rdfs:comment":""},{"@id":"sustainability:TheAvailabilityOfSparePartsForTheProduct#1","@type":"sustainability:TheAvailabilityOfSparePartsForTheProduct","rdf:value":"1","rdfs:comment":"Availability for 3 years after end of production"},{"@id":"sustainability:TheAvailabilityOfSparePartsForTheProduct#2","@type":"sustainability:TheAvailabilityOfSparePartsForTheProduct","rdf:value":"2","rdfs:comment":"Availability for 5 years after end of production"},{"rdfs:label":"TheUseOfNanomaterials","@type":"rdfs:Class","@id":"sustainability:TheUseOfNanomaterials","rdfs:comment":""},{"@id":"sustainability:TheUseOfNanomaterials#1","@type":"sustainability:TheUseOfNanomaterials","rdf:value":"1","rdfs:comment":"Restrict use"},{"@id":"sustainability:TheUseOfNanomaterials#2","@type":"sustainability:TheUseOfNanomaterials","rdf:value":"2","rdfs:comment":"Prohibit use"},{"rdfs:label":"TheUseOfDyesOrPigmentsBasedOnLeadCopperChromiumNickelAndAluminum","@type":"rdfs:Class","@id":"sustainability:TheUseOfDyesOrPigmentsBasedOnLeadCopperChromiumNickelAndAluminum","rdfs:comment":""},{"@id":"sustainability:TheUseOfDyesOrPigmentsBasedOnLeadCopperChromiumNickelAndAluminum#1","@type":"sustainability:TheUseOfDyesOrPigmentsBasedOnLeadCopperChromiumNickelAndAluminum","rdf:value":"1","rdfs:comment":"Prohibit use of some substances"},{"@id":"sustainability:TheUseOfDyesOrPigmentsBasedOnLeadCopperChromiumNickelAndAluminum#2","@type":"sustainability:TheUseOfDyesOrPigmentsBasedOnLeadCopperChromiumNickelAndAluminum","rdf:value":"2","rdfs:comment":"Prohibit use of all substances"},{"rdfs:label":"TheUseOfAzoDyesThatMayCleaveAromaticAminesWhichAreHarmfulToHumanHealth","@type":"rdfs:Class","@id":"sustainability:TheUseOfAzoDyesThatMayCleaveAromaticAminesWhichAreHarmfulToHumanHealth","rdfs:comment":""},{"@id":"sustainability:TheUseOfAzoDyesThatMayCleaveAromaticAminesWhichAreHarmfulToHumanHealth#1","@type":"sustainability:TheUseOfAzoDyesThatMayCleaveAromaticAminesWhichAreHarmfulToHumanHealth","rdf:value":"1","rdfs:comment":"Restrict use"},{"@id":"sustainability:TheUseOfAzoDyesThatMayCleaveAromaticAminesWhichAreHarmfulToHumanHealth#2","@type":"sustainability:TheUseOfAzoDyesThatMayCleaveAromaticAminesWhichAreHarmfulToHumanHealth","rdf:value":"2","rdfs:comment":"Prohibit use"},{"rdfs:label":"SocioCulturalSites","@type":"rdfs:Class","@id":"sustainability:SocioCulturalSites","rdfs:comment":""},{"@id":"sustainability:SocioCulturalSites#1","@type":"sustainability:SocioCulturalSites","rdf:value":"1","rdfs:comment":"protect"},{"@id":"sustainability:SocioCulturalSites#2","@type":"sustainability:SocioCulturalSites","rdf:value":"2","rdfs:comment":"protect + do not impede access"},{"rdfs:label":"CompensationForUseOfLocalCommunitiesFacilities","@type":"rdfs:Class","@id":"sustainability:CompensationForUseOfLocalCommunitiesFacilities","rdfs:comment":""},{"@id":"sustainability:CompensationForUseOfLocalCommunitiesFacilities#1","@type":"sustainability:CompensationForUseOfLocalCommunitiesFacilities","rdf:value":"1","rdfs:comment":"Compensation mechanisms in place prior to commencement of forest operations"},{"@id":"sustainability:CompensationForUseOfLocalCommunitiesFacilities#2","@type":"sustainability:CompensationForUseOfLocalCommunitiesFacilities","rdf:value":"2","rdfs:comment":"Written/formal agreements with local and indigenous communities on the terms of compensation"},{"rdfs:label":"GrievanceMechanismsForAffectedCommunities","@type":"rdfs:Class","@id":"sustainability:GrievanceMechanismsForAffectedCommunities","rdfs:comment":""},{"@id":"sustainability:GrievanceMechanismsForAffectedCommunities#1","@type":"sustainability:GrievanceMechanismsForAffectedCommunities","rdf:value":"1","rdfs:comment":"grievance mechanism ; "},{"@id":"sustainability:GrievanceMechanismsForAffectedCommunities#2","@type":"sustainability:GrievanceMechanismsForAffectedCommunities","rdf:value":"2","rdfs:comment":"+ compensation mechanism"},{"rdfs:label":"OccupationalHealthAndSafetyAsDefinedInIlo155","@type":"rdfs:Class","@id":"sustainability:OccupationalHealthAndSafetyAsDefinedInIlo155","rdfs:comment":""},{"@id":"sustainability:OccupationalHealthAndSafetyAsDefinedInIlo155#1","@type":"sustainability:OccupationalHealthAndSafetyAsDefinedInIlo155","rdf:value":"1","rdfs:comment":"partial compliance with ILO 155"},{"@id":"sustainability:OccupationalHealthAndSafetyAsDefinedInIlo155#2","@type":"sustainability:OccupationalHealthAndSafetyAsDefinedInIlo155","rdf:value":"2","rdfs:comment":"full compliance with ILO 155"},{"rdfs:label":"WorkplaceConditionsAirQualityLightingNoise","@type":"rdfs:Class","@id":"sustainability:WorkplaceConditionsAirQualityLightingNoise","rdfs:comment":""},{"@id":"sustainability:WorkplaceConditionsAirQualityLightingNoise#1","@type":"sustainability:WorkplaceConditionsAirQualityLightingNoise","rdf:value":"1","rdfs:comment":"yes, some"},{"@id":"sustainability:WorkplaceConditionsAirQualityLightingNoise#2","@type":"sustainability:WorkplaceConditionsAirQualityLightingNoise","rdf:value":"2","rdfs:comment":"yes, all"},{"rdfs:label":"WorkersAccessToBasicMedicalServices","@type":"rdfs:Class","@id":"sustainability:WorkersAccessToBasicMedicalServices","rdfs:comment":""},{"@id":"sustainability:WorkersAccessToBasicMedicalServices#1","@type":"sustainability:WorkersAccessToBasicMedicalServices","rdf:value":"1","rdfs:comment":"only treatment of acute work-related accidents/ illness"},{"@id":"sustainability:WorkersAccessToBasicMedicalServices#2","@type":"sustainability:WorkersAccessToBasicMedicalServices","rdf:value":"2","rdfs:comment":"work-related accidents plus preventative care"},{"rdfs:label":"SafetyAtWorkIlo184","@type":"rdfs:Class","@id":"sustainability:SafetyAtWorkIlo184","rdfs:comment":""},{"@id":"sustainability:SafetyAtWorkIlo184#1","@type":"sustainability:SafetyAtWorkIlo184","rdf:value":"1","rdfs:comment":"partial compliance w/ 184"},{"@id":"sustainability:SafetyAtWorkIlo184#2","@type":"sustainability:SafetyAtWorkIlo184","rdf:value":"2","rdfs:comment":"full compliance w/ 184"},{"rdfs:label":"PaidLeaveGeneralPolicyPublicHolidaysAnnualLeaveSickLeaveCasualLeave","@type":"rdfs:Class","@id":"sustainability:PaidLeaveGeneralPolicyPublicHolidaysAnnualLeaveSickLeaveCasualLeave","rdfs:comment":""},{"@id":"sustainability:PaidLeaveGeneralPolicyPublicHolidaysAnnualLeaveSickLeaveCasualLeave#1","@type":"sustainability:PaidLeaveGeneralPolicyPublicHolidaysAnnualLeaveSickLeaveCasualLeave","rdf:value":"1","rdfs:comment":"one out of three (casual/ sick/ annual)"},{"@id":"sustainability:PaidLeaveGeneralPolicyPublicHolidaysAnnualLeaveSickLeaveCasualLeave#2","@type":"sustainability:PaidLeaveGeneralPolicyPublicHolidaysAnnualLeaveSickLeaveCasualLeave","rdf:value":"2","rdfs:comment":"two out of three"},{"@id":"sustainability:PaidLeaveGeneralPolicyPublicHolidaysAnnualLeaveSickLeaveCasualLeave#3","@type":"sustainability:PaidLeaveGeneralPolicyPublicHolidaysAnnualLeaveSickLeaveCasualLeave","rdf:value":"3","rdfs:comment":"all"},{"rdfs:label":"SpecificMaternityPaternityLeaveDays","@type":"rdfs:Class","@id":"sustainability:SpecificMaternityPaternityLeaveDays","rdfs:comment":""},{"@id":"sustainability:SpecificMaternityPaternityLeaveDays#1","@type":"sustainability:SpecificMaternityPaternityLeaveDays","rdf:value":"1","rdfs:comment":"partial compliance"},{"@id":"sustainability:SpecificMaternityPaternityLeaveDays#2","@type":"sustainability:SpecificMaternityPaternityLeaveDays","rdf:value":"2","rdfs:comment":"full compliance"},{"@id":"sustainability:SpecificMaternityPaternityLeaveDays#3","@type":"sustainability:SpecificMaternityPaternityLeaveDays","rdf:value":"3","rdfs:comment":"beyond 18"},{"rdfs:label":"FairAndTimelyPaymentOfWages","@type":"rdfs:Class","@id":"sustainability:FairAndTimelyPaymentOfWages","rdfs:comment":""},{"@id":"sustainability:FairAndTimelyPaymentOfWages#1","@type":"sustainability:FairAndTimelyPaymentOfWages","rdf:value":"1","rdfs:comment":"yes, some"},{"@id":"sustainability:FairAndTimelyPaymentOfWages#2","@type":"sustainability:FairAndTimelyPaymentOfWages","rdf:value":"2","rdfs:comment":"yes, all"},{"rdfs:label":"WorkersCompensationForMedicalCostsInCaseOfWorkRelatedAccidents","@type":"rdfs:Class","@id":"sustainability:WorkersCompensationForMedicalCostsInCaseOfWorkRelatedAccidents","rdfs:comment":""},{"@id":"sustainability:WorkersCompensationForMedicalCostsInCaseOfWorkRelatedAccidents#1","@type":"sustainability:WorkersCompensationForMedicalCostsInCaseOfWorkRelatedAccidents","rdf:value":"1","rdfs:comment":"partial coverage of costs"},{"@id":"sustainability:WorkersCompensationForMedicalCostsInCaseOfWorkRelatedAccidents#2","@type":"sustainability:WorkersCompensationForMedicalCostsInCaseOfWorkRelatedAccidents","rdf:value":"2","rdfs:comment":"full coverage of costs"},{"@id":"sustainability:WorkersCompensationForMedicalCostsInCaseOfWorkRelatedAccidents#3","@type":"sustainability:WorkersCompensationForMedicalCostsInCaseOfWorkRelatedAccidents","rdf:value":"3","rdfs:comment":"compensation"},{"rdfs:label":"FormationOfWorkersRepresentationInCountriesWhereFreedomOfAssociationAndCollectiveBargainingIsNotSupportedByLegislation","@type":"rdfs:Class","@id":"sustainability:FormationOfWorkersRepresentationInCountriesWhereFreedomOfAssociationAndCollectiveBargainingIsNotSupportedByLegislation","rdfs:comment":""},{"@id":"sustainability:FormationOfWorkersRepresentationInCountriesWhereFreedomOfAssociationAndCollectiveBargainingIsNotSupportedByLegislation#1","@type":"sustainability:FormationOfWorkersRepresentationInCountriesWhereFreedomOfAssociationAndCollectiveBargainingIsNotSupportedByLegislation","rdf:value":"1","rdfs:comment":"allow"},{"@id":"sustainability:FormationOfWorkersRepresentationInCountriesWhereFreedomOfAssociationAndCollectiveBargainingIsNotSupportedByLegislation#2","@type":"sustainability:FormationOfWorkersRepresentationInCountriesWhereFreedomOfAssociationAndCollectiveBargainingIsNotSupportedByLegislation","rdf:value":"2","rdfs:comment":"promote"},{"rdfs:label":"RisksAndImpactsOnWaterLevelsOfWaterResourcesUsedSurfaceAndOrGroundWater","@type":"rdfs:Class","@id":"sustainability:RisksAndImpactsOnWaterLevelsOfWaterResourcesUsedSurfaceAndOrGroundWater","rdfs:comment":""},{"@id":"sustainability:RisksAndImpactsOnWaterLevelsOfWaterResourcesUsedSurfaceAndOrGroundWater#1","@type":"sustainability:RisksAndImpactsOnWaterLevelsOfWaterResourcesUsedSurfaceAndOrGroundWater","rdf:value":"1","rdfs:comment":"Measure water levels of surface and/or ground water"},{"@id":"sustainability:RisksAndImpactsOnWaterLevelsOfWaterResourcesUsedSurfaceAndOrGroundWater#2","@type":"sustainability:RisksAndImpactsOnWaterLevelsOfWaterResourcesUsedSurfaceAndOrGroundWater","rdf:value":"2","rdfs:comment":"Monitor water levels of surface and/or ground water over time"},{"@id":"sustainability:RisksAndImpactsOnWaterLevelsOfWaterResourcesUsedSurfaceAndOrGroundWater#3","@type":"sustainability:RisksAndImpactsOnWaterLevelsOfWaterResourcesUsedSurfaceAndOrGroundWater","rdf:value":"3","rdfs:comment":"Avoid negative impacts on water levels of surface and/or ground water"},{"rdfs:label":"RisksAndImpactsOnWaterQualityOfWaterResourcesUsedSurfaceAndOrGroundWater","@type":"rdfs:Class","@id":"sustainability:RisksAndImpactsOnWaterQualityOfWaterResourcesUsedSurfaceAndOrGroundWater","rdfs:comment":""},{"@id":"sustainability:RisksAndImpactsOnWaterQualityOfWaterResourcesUsedSurfaceAndOrGroundWater#1","@type":"sustainability:RisksAndImpactsOnWaterQualityOfWaterResourcesUsedSurfaceAndOrGroundWater","rdf:value":"1","rdfs:comment":"Measure quality of surface and/or ground water"},{"@id":"sustainability:RisksAndImpactsOnWaterQualityOfWaterResourcesUsedSurfaceAndOrGroundWater#2","@type":"sustainability:RisksAndImpactsOnWaterQualityOfWaterResourcesUsedSurfaceAndOrGroundWater","rdf:value":"2","rdfs:comment":"Monitor quality of surface and/or ground water over time"},{"@id":"sustainability:RisksAndImpactsOnWaterQualityOfWaterResourcesUsedSurfaceAndOrGroundWater#3","@type":"sustainability:RisksAndImpactsOnWaterQualityOfWaterResourcesUsedSurfaceAndOrGroundWater","rdf:value":"3","rdfs:comment":"Avoid negative impacts on quality of surface and/or ground water"},{"rdfs:label":"EnvironmentalRisksAndImpacts","@type":"rdfs:Class","@id":"sustainability:EnvironmentalRisksAndImpacts","rdfs:comment":""},{"@id":"sustainability:EnvironmentalRisksAndImpacts#1","@type":"sustainability:EnvironmentalRisksAndImpacts","rdf:value":"1","rdfs:comment":"Require Environmental Impact Assessment according to national law"},{"@id":"sustainability:EnvironmentalRisksAndImpacts#2","@type":"sustainability:EnvironmentalRisksAndImpacts","rdf:value":"2","rdfs:comment":"Require Environmental Impact Assessment that go beyond national law"},{"rdfs:label":"SupplyChainResponsibilityBeyondPrimaryProduction","@type":"rdfs:Class","@id":"sustainability:SupplyChainResponsibilityBeyondPrimaryProduction","rdfs:comment":""},{"@id":"sustainability:SupplyChainResponsibilityBeyondPrimaryProduction#1","@type":"sustainability:SupplyChainResponsibilityBeyondPrimaryProduction","rdf:value":"1","rdfs:comment":"only next phase"},{"@id":"sustainability:SupplyChainResponsibilityBeyondPrimaryProduction#2","@type":"sustainability:SupplyChainResponsibilityBeyondPrimaryProduction","rdf:value":"2","rdfs:comment":"entire chain"},{"rdfs:label":"DoesTheStandardCoverTheQualityOfTextiles","@type":"rdfs:Class","@id":"sustainability:DoesTheStandardCoverTheQualityOfTextiles","rdfs:comment":""},{"@id":"sustainability:DoesTheStandardCoverTheQualityOfTextiles#1","@type":"sustainability:DoesTheStandardCoverTheQualityOfTextiles","rdf:value":"1","rdfs:comment":"Less than four aspects are tested"},{"@id":"sustainability:DoesTheStandardCoverTheQualityOfTextiles#2","@type":"sustainability:DoesTheStandardCoverTheQualityOfTextiles","rdf:value":"2","rdfs:comment":"All four aspects (fastness of rubbing/ perspiration/ light/ washing) are tested"},{"rdfs:label":"ComplianceToNationalAndRegionalEnvironmentalLawsAndRegulations","@type":"rdfs:Class","@id":"sustainability:ComplianceToNationalAndRegionalEnvironmentalLawsAndRegulations","rdfs:comment":""},{"@id":"sustainability:ComplianceToNationalAndRegionalEnvironmentalLawsAndRegulations#1","@type":"sustainability:ComplianceToNationalAndRegionalEnvironmentalLawsAndRegulations","rdf:value":"1","rdfs:comment":"Demonstrate awareness of all relevant laws and regulations"},{"@id":"sustainability:ComplianceToNationalAndRegionalEnvironmentalLawsAndRegulations#2","@type":"sustainability:ComplianceToNationalAndRegionalEnvironmentalLawsAndRegulations","rdf:value":"2","rdfs:comment":"Ensure compliance with all relevant laws and regulations"},{"@id":"sustainability:ITC_Criteria","@type":"rdfs:Class","rdfs:label":"ITC_Criteria","schema:source":{"@id":"http://vocab.unece.org/sustainabilityITC_Criteria"},"rdfs:comment":""},{"@id":"sustainability:Environment","@type":"rdfs:Class","rdfs:label":"Environment","schema:source":{"@id":"http://vocab.unece.org/sustainabilityEnvironment"},"rdfs:comment":""},{"@id":"sustainability:Social","@type":"rdfs:Class","rdfs:label":"Social","schema:source":{"@id":"http://vocab.unece.org/sustainabilitySocial"},"rdfs:comment":""},{"@id":"sustainability:Management","@type":"rdfs:Class","rdfs:label":"Management","schema:source":{"@id":"http://vocab.unece.org/sustainabilityManagement"},"rdfs:comment":""},{"@id":"sustainability:Quality","@type":"rdfs:Class","rdfs:label":"Quality","schema:source":{"@id":"http://vocab.unece.org/sustainabilityQuality"},"rdfs:comment":""},{"@id":"sustainability:NonFoodProducts","@type":"rdfs:Class","rdfs:label":"NonFoodProducts","schema:source":{"@id":"http://vocab.unece.org/sustainabilityNonFoodProducts"},"rdfs:comment":""},{"@id":"sustainability:FoodProducts","@type":"rdfs:Class","rdfs:label":"FoodProducts","schema:source":{"@id":"http://vocab.unece.org/sustainabilityFoodProducts"},"rdfs:comment":""},{"@id":"sustainability:FeedManagement","@type":"rdfs:Class","rdfs:label":"FeedManagement","schema:source":{"@id":"http://vocab.unece.org/sustainabilityFeedManagement"},"rdfs:comment":""},{"@id":"sustainability:Ethics","@type":"rdfs:Class","rdfs:label":"Ethics","schema:source":{"@id":"http://vocab.unece.org/sustainabilityEthics"},"rdfs:comment":""},{"@id":"sustainability:CompliancePolicies","@type":"rdfs:Class","rdfs:label":"CompliancePolicies","schema:source":{"@id":"http://vocab.unece.org/sustainabilityCompliancePolicies"},"rdfs:comment":""},{"@id":"sustainability:Soil","@type":"rdfs:Class","rdfs:label":"Soil","schema:source":{"@id":"http://vocab.unece.org/sustainabilitySoil"},"rdfs:comment":""},{"@id":"sustainability:Forests","@type":"rdfs:Class","rdfs:label":"Forests","schema:source":{"@id":"http://vocab.unece.org/sustainabilityForests"},"rdfs:comment":""},{"@id":"sustainability:ChemicalInputs","@type":"rdfs:Class","rdfs:label":"ChemicalInputs","schema:source":{"@id":"http://vocab.unece.org/sustainabilityChemicalInputs"},"rdfs:comment":""},{"@id":"sustainability:Biodiversity","@type":"rdfs:Class","rdfs:label":"Biodiversity","schema:source":{"@id":"http://vocab.unece.org/sustainabilityBiodiversity"},"rdfs:comment":""},{"@id":"sustainability:Livestock","@type":"rdfs:Class","rdfs:label":"Livestock","schema:source":{"@id":"http://vocab.unece.org/sustainabilityLivestock"},"rdfs:comment":""},{"@id":"sustainability:Waste","@type":"rdfs:Class","rdfs:label":"Waste","schema:source":{"@id":"http://vocab.unece.org/sustainabilityWaste"},"rdfs:comment":""},{"@id":"sustainability:Water","@type":"rdfs:Class","rdfs:label":"Water","schema:source":{"@id":"http://vocab.unece.org/sustainabilityWater"},"rdfs:comment":""},{"@id":"sustainability:Energy","@type":"rdfs:Class","rdfs:label":"Energy","schema:source":{"@id":"http://vocab.unece.org/sustainabilityEnergy"},"rdfs:comment":""},{"@id":"sustainability:ClimateCarbon","@type":"rdfs:Class","rdfs:label":"ClimateCarbon","schema:source":{"@id":"http://vocab.unece.org/sustainabilityClimateCarbon"},"rdfs:comment":""},{"@id":"sustainability:SsctAndOther","@type":"rdfs:Class","rdfs:label":"SsctAndOther","schema:source":{"@id":"http://vocab.unece.org/sustainabilitySsctAndOther"},"rdfs:comment":""},{"@id":"sustainability:HumanRights","@type":"rdfs:Class","rdfs:label":"HumanRights","schema:source":{"@id":"http://vocab.unece.org/sustainabilityHumanRights"},"rdfs:comment":""},{"@id":"sustainability:ConditionsOfWork","@type":"rdfs:Class","rdfs:label":"ConditionsOfWork","schema:source":{"@id":"http://vocab.unece.org/sustainabilityConditionsOfWork"},"rdfs:comment":""},{"@id":"sustainability:Employment","@type":"rdfs:Class","rdfs:label":"Employment","schema:source":{"@id":"http://vocab.unece.org/sustainabilityEmployment"},"rdfs:comment":""},{"@id":"sustainability:HumanDevelopment","@type":"rdfs:Class","rdfs:label":"HumanDevelopment","schema:source":{"@id":"http://vocab.unece.org/sustainabilityHumanDevelopment"},"rdfs:comment":""},{"@id":"sustainability:EconomicViability","@type":"rdfs:Class","rdfs:label":"EconomicViability","schema:source":{"@id":"http://vocab.unece.org/sustainabilityEconomicViability"},"rdfs:comment":""},{"@id":"sustainability:SustainabilityManagement","@type":"rdfs:Class","rdfs:label":"SustainabilityManagement","schema:source":{"@id":"http://vocab.unece.org/sustainabilitySustainabilityManagement"},"rdfs:comment":""},{"@id":"sustainability:SupplyChain","@type":"rdfs:Class","rdfs:label":"SupplyChain","schema:source":{"@id":"http://vocab.unece.org/sustainabilitySupplyChain"},"rdfs:comment":""},{"@id":"sustainability:QualityManagement","@type":"rdfs:Class","rdfs:label":"QualityManagement","schema:source":{"@id":"http://vocab.unece.org/sustainabilityQualityManagement"},"rdfs:comment":""},{"@id":"sustainability:TechnicalSpecifications","@type":"rdfs:Class","rdfs:label":"TechnicalSpecifications","schema:source":{"@id":"http://vocab.unece.org/sustainabilityTechnicalSpecifications"},"rdfs:comment":""},{"@id":"sustainability:TraceabilityAndRecall","@type":"rdfs:Class","rdfs:label":"TraceabilityAndRecall","schema:source":{"@id":"http://vocab.unece.org/sustainabilityTraceabilityAndRecall"},"rdfs:comment":""},{"@id":"sustainability:StaffRequirements","@type":"rdfs:Class","rdfs:label":"StaffRequirements","schema:source":{"@id":"http://vocab.unece.org/sustainabilityStaffRequirements"},"rdfs:comment":""},{"@id":"sustainability:SafetyHaccpSystem","@type":"rdfs:Class","rdfs:label":"SafetyHaccpSystem","schema:source":{"@id":"http://vocab.unece.org/sustainabilitySafetyHaccpSystem"},"rdfs:comment":""},{"@id":"sustainability:ProductionSite","@type":"rdfs:Class","rdfs:label":"ProductionSite","schema:source":{"@id":"http://vocab.unece.org/sustainabilityProductionSite"},"rdfs:comment":""},{"@id":"sustainability:TracebilityRecallAndAllergens","@type":"rdfs:Class","rdfs:label":"TracebilityRecallAndAllergens","schema:source":{"@id":"http://vocab.unece.org/sustainabilityTracebilityRecallAndAllergens"},"rdfs:comment":""},{"@id":"sustainability:ForeignBodiesAndContamination","@type":"rdfs:Class","rdfs:label":"ForeignBodiesAndContamination","schema:source":{"@id":"http://vocab.unece.org/sustainabilityForeignBodiesAndContamination"},"rdfs:comment":""},{"@id":"sustainability:ProcessAndProductControl","@type":"rdfs:Class","rdfs:label":"ProcessAndProductControl","schema:source":{"@id":"http://vocab.unece.org/sustainabilityProcessAndProductControl"},"rdfs:comment":""},{"@id":"sustainability:WorkersRequirements","@type":"rdfs:Class","rdfs:label":"WorkersRequirements","schema:source":{"@id":"http://vocab.unece.org/sustainabilityWorkersRequirements"},"rdfs:comment":""},{"@id":"sustainability:ManagementSystem","@type":"rdfs:Class","rdfs:label":"ManagementSystem","schema:source":{"@id":"http://vocab.unece.org/sustainabilityManagementSystem"},"rdfs:comment":""},{"@id":"sustainability:Specifications","@type":"rdfs:Class","rdfs:label":"Specifications","schema:source":{"@id":"http://vocab.unece.org/sustainabilitySpecifications"},"rdfs:comment":""},{"@id":"sustainability:Documentation","@type":"rdfs:Class","rdfs:label":"Documentation","schema:source":{"@id":"http://vocab.unece.org/sustainabilityDocumentation"},"rdfs:comment":""},{"@id":"sustainability:ManagementResponsibility","@type":"rdfs:Class","rdfs:label":"ManagementResponsibility","schema:source":{"@id":"http://vocab.unece.org/sustainabilityManagementResponsibility"},"rdfs:comment":""},{"@id":"sustainability:VerificationAndImprovement","@type":"rdfs:Class","rdfs:label":"VerificationAndImprovement","schema:source":{"@id":"http://vocab.unece.org/sustainabilityVerificationAndImprovement"},"rdfs:comment":""},{"@id":"sustainability:PrerequisiteProgrammes","@type":"rdfs:Class","rdfs:label":"PrerequisiteProgrammes","schema:source":{"@id":"http://vocab.unece.org/sustainabilityPrerequisiteProgrammes"},"rdfs:comment":""},{"@id":"sustainability:Purchase","@type":"rdfs:Class","rdfs:label":"Purchase","schema:source":{"@id":"http://vocab.unece.org/sustainabilityPurchase"},"rdfs:comment":""},{"@id":"sustainability:Production","@type":"rdfs:Class","rdfs:label":"Production","schema:source":{"@id":"http://vocab.unece.org/sustainabilityProduction"},"rdfs:comment":""},{"@id":"sustainability:OutsourcedActivities","@type":"rdfs:Class","rdfs:label":"OutsourcedActivities","schema:source":{"@id":"http://vocab.unece.org/sustainabilityOutsourcedActivities"},"rdfs:comment":""},{"@id":"sustainability:Formulation","@type":"rdfs:Class","rdfs:label":"Formulation","schema:source":{"@id":"http://vocab.unece.org/sustainabilityFormulation"},"rdfs:comment":""},{"@id":"sustainability:Labeling","@type":"rdfs:Class","rdfs:label":"Labeling","schema:source":{"@id":"http://vocab.unece.org/sustainabilityLabeling"},"rdfs:comment":""},{"@id":"sustainability:ControlOfNonConformity","@type":"rdfs:Class","rdfs:label":"ControlOfNonConformity","schema:source":{"@id":"http://vocab.unece.org/sustainabilityControlOfNonConformity"},"rdfs:comment":""},{"@id":"sustainability:Haccp","@type":"rdfs:Class","rdfs:label":"Haccp","schema:source":{"@id":"http://vocab.unece.org/sustainabilityHaccp"},"rdfs:comment":""},{"@id":"sustainability:MonitoringAndVerification","@type":"rdfs:Class","rdfs:label":"MonitoringAndVerification","schema:source":{"@id":"http://vocab.unece.org/sustainabilityMonitoringAndVerification"},"rdfs:comment":""},{"@id":"sustainability:AntiCorruption","@type":"rdfs:Class","rdfs:label":"AntiCorruption","schema:source":{"@id":"http://vocab.unece.org/sustainabilityAntiCorruption"},"rdfs:comment":""},{"@id":"sustainability:ComplianceToLegislation","@type":"rdfs:Class","rdfs:label":"ComplianceToLegislation","schema:source":{"@id":"http://vocab.unece.org/sustainabilityComplianceToLegislation"},"rdfs:comment":""},{"@id":"sustainability:compliancePolicies","@type":["rdf:Property","owl:ObjectProperty"],"rdfs:label":"compliancePolicies","schema:rangeIncludes":{"@id":"sustainability:CompliancePolicies"},"schema:domainIncludes":{"@id":"sustainability:ITC_Criteria"},"rdfs:comment":""},{"@id":"sustainability:environment","@type":["rdf:Property","owl:ObjectProperty"],"rdfs:label":"environment","schema:rangeIncludes":{"@id":"sustainability:Environment"},"schema:domainIncludes":{"@id":"sustainability:ITC_Criteria"},"rdfs:comment":""},{"@id":"sustainability:social","@type":["rdf:Property","owl:ObjectProperty"],"rdfs:label":"social","schema:rangeIncludes":{"@id":"sustainability:Social"},"schema:domainIncludes":{"@id":"sustainability:ITC_Criteria"},"rdfs:comment":""},{"@id":"sustainability:management","@type":["rdf:Property","owl:ObjectProperty"],"rdfs:label":"management","schema:rangeIncludes":{"@id":"sustainability:Management"},"schema:domainIncludes":{"@id":"sustainability:ITC_Criteria"},"rdfs:comment":""},{"@id":"sustainability:quality","@type":["rdf:Property","owl:ObjectProperty"],"rdfs:label":"quality","schema:rangeIncludes":{"@id":"sustainability:Quality"},"schema:domainIncludes":{"@id":"sustainability:ITC_Criteria"},"rdfs:comment":""},{"@id":"sustainability:ethics","@type":["rdf:Property","owl:ObjectProperty"],"rdfs:label":"ethics","schema:rangeIncludes":{"@id":"sustainability:Ethics"},"schema:domainIncludes":{"@id":"sustainability:ITC_Criteria"},"rdfs:comment":""},{"@id":"sustainability:soil","@type":["rdf:Property","owl:ObjectProperty"],"rdfs:label":"soil","schema:rangeIncludes":{"@id":"sustainability:Soil"},"schema:domainIncludes":{"@id":"sustainability:Environment"},"rdfs:comment":""},{"@id":"sustainability:forests","@type":["rdf:Property","owl:ObjectProperty"],"rdfs:label":"forests","schema:rangeIncludes":{"@id":"sustainability:Forests"},"schema:domainIncludes":{"@id":"sustainability:Environment"},"rdfs:comment":""},{"@id":"sustainability:chemicalInputs","@type":["rdf:Property","owl:ObjectProperty"],"rdfs:label":"chemicalInputs","schema:rangeIncludes":{"@id":"sustainability:ChemicalInputs"},"schema:domainIncludes":{"@id":"sustainability:Environment"},"rdfs:comment":""},{"@id":"sustainability:biodiversity","@type":["rdf:Property","owl:ObjectProperty"],"rdfs:label":"biodiversity","schema:rangeIncludes":{"@id":"sustainability:Biodiversity"},"schema:domainIncludes":{"@id":"sustainability:Environment"},"rdfs:comment":""},{"@id":"sustainability:livestock","@type":["rdf:Property","owl:ObjectProperty"],"rdfs:label":"livestock","schema:rangeIncludes":{"@id":"sustainability:Livestock"},"schema:domainIncludes":{"@id":"sustainability:Environment"},"rdfs:comment":""},{"@id":"sustainability:waste","@type":["rdf:Property","owl:ObjectProperty"],"rdfs:label":"waste","schema:rangeIncludes":{"@id":"sustainability:Waste"},"schema:domainIncludes":{"@id":"sustainability:Environment"},"rdfs:comment":""},{"@id":"sustainability:water","@type":["rdf:Property","owl:ObjectProperty"],"rdfs:label":"water","schema:rangeIncludes":{"@id":"sustainability:Water"},"schema:domainIncludes":{"@id":"sustainability:Environment"},"rdfs:comment":""},{"@id":"sustainability:energy","@type":["rdf:Property","owl:ObjectProperty"],"rdfs:label":"energy","schema:rangeIncludes":{"@id":"sustainability:Energy"},"schema:domainIncludes":{"@id":"sustainability:Environment"},"rdfs:comment":""},{"@id":"sustainability:climateCarbon","@type":["rdf:Property","owl:ObjectProperty"],"rdfs:label":"climateCarbon","schema:rangeIncludes":{"@id":"sustainability:ClimateCarbon"},"schema:domainIncludes":{"@id":"sustainability:Environment"},"rdfs:comment":""},{"@id":"sustainability:ssctAndOther","@type":["rdf:Property","owl:ObjectProperty"],"rdfs:label":"ssctAndOther","schema:rangeIncludes":{"@id":"sustainability:SsctAndOther"},"schema:domainIncludes":{"@id":"sustainability:Environment"},"rdfs:comment":""},{"@id":"sustainability:humanRights","@type":["rdf:Property","owl:ObjectProperty"],"rdfs:label":"humanRights","schema:rangeIncludes":{"@id":"sustainability:HumanRights"},"schema:domainIncludes":{"@id":"sustainability:Social"},"rdfs:comment":""},{"@id":"sustainability:conditionsOfWork","@type":["rdf:Property","owl:ObjectProperty"],"rdfs:label":"conditionsOfWork","schema:rangeIncludes":{"@id":"sustainability:ConditionsOfWork"},"schema:domainIncludes":{"@id":"sustainability:Social"},"rdfs:comment":""},{"@id":"sustainability:employment","@type":["rdf:Property","owl:ObjectProperty"],"rdfs:label":"employment","schema:rangeIncludes":{"@id":"sustainability:Employment"},"schema:domainIncludes":{"@id":"sustainability:Social"},"rdfs:comment":""},{"@id":"sustainability:humanDevelopment","@type":["rdf:Property","owl:ObjectProperty"],"rdfs:label":"humanDevelopment","schema:rangeIncludes":{"@id":"sustainability:HumanDevelopment"},"schema:domainIncludes":{"@id":"sustainability:Social"},"rdfs:comment":""},{"@id":"sustainability:economicViability","@type":["rdf:Property","owl:ObjectProperty"],"rdfs:label":"economicViability","schema:rangeIncludes":{"@id":"sustainability:EconomicViability"},"schema:domainIncludes":{"@id":"sustainability:Management"},"rdfs:comment":""},{"@id":"sustainability:sustainabilityManagement","@type":["rdf:Property","owl:ObjectProperty"],"rdfs:label":"sustainabilityManagement","schema:rangeIncludes":{"@id":"sustainability:SustainabilityManagement"},"schema:domainIncludes":{"@id":"sustainability:Management"},"rdfs:comment":""},{"@id":"sustainability:supplyChain","@type":["rdf:Property","owl:ObjectProperty"],"rdfs:label":"supplyChain","schema:rangeIncludes":{"@id":"sustainability:SupplyChain"},"schema:domainIncludes":{"@id":"sustainability:Management"},"rdfs:comment":""},{"@id":"sustainability:qualityManagement","@type":["rdf:Property","owl:ObjectProperty"],"rdfs:label":"qualityManagement","schema:rangeIncludes":{"@id":"sustainability:QualityManagement"},"schema:domainIncludes":{"@id":"sustainability:Quality"},"rdfs:comment":""},{"@id":"sustainability:nonFoodProducts","@type":["rdf:Property","owl:ObjectProperty"],"rdfs:label":"nonFoodProducts","schema:rangeIncludes":{"@id":"sustainability:NonFoodProducts"},"schema:domainIncludes":{"@id":"sustainability:Quality"},"rdfs:comment":""},{"@id":"sustainability:foodProducts","@type":["rdf:Property","owl:ObjectProperty"],"rdfs:label":"foodProducts","schema:rangeIncludes":{"@id":"sustainability:FoodProducts"},"schema:domainIncludes":{"@id":"sustainability:Quality"},"rdfs:comment":""},{"@id":"sustainability:feedManagement","@type":["rdf:Property","owl:ObjectProperty"],"rdfs:label":"feedManagement","schema:rangeIncludes":{"@id":"sustainability:FeedManagement"},"schema:domainIncludes":{"@id":"sustainability:Quality"},"rdfs:comment":""},{"@id":"sustainability:technicalSpecifications","@type":["rdf:Property","owl:ObjectProperty"],"rdfs:label":"technicalSpecifications","schema:rangeIncludes":{"@id":"sustainability:TechnicalSpecifications"},"schema:domainIncludes":{"@id":"sustainability:NonFoodProducts"},"rdfs:comment":""},{"@id":"sustainability:traceabilityAndRecall","@type":["rdf:Property","owl:ObjectProperty"],"rdfs:label":"traceabilityAndRecall","schema:rangeIncludes":{"@id":"sustainability:TraceabilityAndRecall"},"schema:domainIncludes":{"@id":"sustainability:NonFoodProducts"},"rdfs:comment":""},{"@id":"sustainability:staffRequirements","@type":["rdf:Property","owl:ObjectProperty"],"rdfs:label":"staffRequirements","schema:rangeIncludes":{"@id":"sustainability:StaffRequirements"},"schema:domainIncludes":{"@id":"sustainability:NonFoodProducts"},"rdfs:comment":""},{"@id":"sustainability:workersRequirements","@type":["rdf:Property","owl:ObjectProperty"],"rdfs:label":"workersRequirements","schema:rangeIncludes":{"@id":"sustainability:WorkersRequirements"},"schema:domainIncludes":{"@id":"sustainability:NonFoodProducts"},"rdfs:comment":""},{"@id":"sustainability:safetyHaccpSystem","@type":["rdf:Property","owl:ObjectProperty"],"rdfs:label":"safetyHaccpSystem","schema:rangeIncludes":{"@id":"sustainability:SafetyHaccpSystem"},"schema:domainIncludes":{"@id":"sustainability:FoodProducts"},"rdfs:comment":""},{"@id":"sustainability:productionSite","@type":["rdf:Property","owl:ObjectProperty"],"rdfs:label":"productionSite","schema:rangeIncludes":{"@id":"sustainability:ProductionSite"},"schema:domainIncludes":{"@id":"sustainability:FoodProducts"},"rdfs:comment":""},{"@id":"sustainability:tracebilityRecallAndAllergens","@type":["rdf:Property","owl:ObjectProperty"],"rdfs:label":"tracebilityRecallAndAllergens","schema:rangeIncludes":{"@id":"sustainability:TracebilityRecallAndAllergens"},"schema:domainIncludes":{"@id":"sustainability:FoodProducts"},"rdfs:comment":""},{"@id":"sustainability:foreignBodiesAndContamination","@type":["rdf:Property","owl:ObjectProperty"],"rdfs:label":"foreignBodiesAndContamination","schema:rangeIncludes":{"@id":"sustainability:ForeignBodiesAndContamination"},"schema:domainIncludes":{"@id":"sustainability:FoodProducts"},"rdfs:comment":""},{"@id":"sustainability:processAndProductControl","@type":["rdf:Property","owl:ObjectProperty"],"rdfs:label":"processAndProductControl","schema:rangeIncludes":{"@id":"sustainability:ProcessAndProductControl"},"schema:domainIncludes":{"@id":"sustainability:FoodProducts"},"rdfs:comment":""},{"@id":"sustainability:managementSystem","@type":["rdf:Property","owl:ObjectProperty"],"rdfs:label":"managementSystem","schema:rangeIncludes":{"@id":"sustainability:ManagementSystem"},"schema:domainIncludes":{"@id":"sustainability:FeedManagement"},"rdfs:comment":""},{"@id":"sustainability:specifications","@type":["rdf:Property","owl:ObjectProperty"],"rdfs:label":"specifications","schema:rangeIncludes":{"@id":"sustainability:Specifications"},"schema:domainIncludes":{"@id":"sustainability:FeedManagement"},"rdfs:comment":""},{"@id":"sustainability:documentation","@type":["rdf:Property","owl:ObjectProperty"],"rdfs:label":"documentation","schema:rangeIncludes":{"@id":"sustainability:Documentation"},"schema:domainIncludes":{"@id":"sustainability:FeedManagement"},"rdfs:comment":""},{"@id":"sustainability:managementResponsibility","@type":["rdf:Property","owl:ObjectProperty"],"rdfs:label":"managementResponsibility","schema:rangeIncludes":{"@id":"sustainability:ManagementResponsibility"},"schema:domainIncludes":{"@id":"sustainability:FeedManagement"},"rdfs:comment":""},{"@id":"sustainability:verificationAndImprovement","@type":["rdf:Property","owl:ObjectProperty"],"rdfs:label":"verificationAndImprovement","schema:rangeIncludes":{"@id":"sustainability:VerificationAndImprovement"},"schema:domainIncludes":{"@id":"sustainability:FeedManagement"},"rdfs:comment":""},{"@id":"sustainability:prerequisiteProgrammes","@type":["rdf:Property","owl:ObjectProperty"],"rdfs:label":"prerequisiteProgrammes","schema:rangeIncludes":{"@id":"sustainability:PrerequisiteProgrammes"},"schema:domainIncludes":{"@id":"sustainability:FeedManagement"},"rdfs:comment":""},{"@id":"sustainability:purchase","@type":["rdf:Property","owl:ObjectProperty"],"rdfs:label":"purchase","schema:rangeIncludes":{"@id":"sustainability:Purchase"},"schema:domainIncludes":{"@id":"sustainability:FeedManagement"},"rdfs:comment":""},{"@id":"sustainability:production","@type":["rdf:Property","owl:ObjectProperty"],"rdfs:label":"production","schema:rangeIncludes":{"@id":"sustainability:Production"},"schema:domainIncludes":{"@id":"sustainability:FeedManagement"},"rdfs:comment":""},{"@id":"sustainability:outsourcedActivities","@type":["rdf:Property","owl:ObjectProperty"],"rdfs:label":"outsourcedActivities","schema:rangeIncludes":{"@id":"sustainability:OutsourcedActivities"},"schema:domainIncludes":{"@id":"sustainability:FeedManagement"},"rdfs:comment":""},{"@id":"sustainability:formulation","@type":["rdf:Property","owl:ObjectProperty"],"rdfs:label":"formulation","schema:rangeIncludes":{"@id":"sustainability:Formulation"},"schema:domainIncludes":{"@id":"sustainability:FeedManagement"},"rdfs:comment":""},{"@id":"sustainability:labeling","@type":["rdf:Property","owl:ObjectProperty"],"rdfs:label":"labeling","schema:rangeIncludes":{"@id":"sustainability:Labeling"},"schema:domainIncludes":{"@id":"sustainability:FeedManagement"},"rdfs:comment":""},{"@id":"sustainability:controlOfNonConformity","@type":["rdf:Property","owl:ObjectProperty"],"rdfs:label":"controlOfNonConformity","schema:rangeIncludes":{"@id":"sustainability:ControlOfNonConformity"},"schema:domainIncludes":{"@id":"sustainability:FeedManagement"},"rdfs:comment":""},{"@id":"sustainability:haccp","@type":["rdf:Property","owl:ObjectProperty"],"rdfs:label":"haccp","schema:rangeIncludes":{"@id":"sustainability:Haccp"},"schema:domainIncludes":{"@id":"sustainability:FeedManagement"},"rdfs:comment":""},{"@id":"sustainability:monitoringAndVerification","@type":["rdf:Property","owl:ObjectProperty"],"rdfs:label":"monitoringAndVerification","schema:rangeIncludes":{"@id":"sustainability:MonitoringAndVerification"},"schema:domainIncludes":{"@id":"sustainability:FeedManagement"},"rdfs:comment":""},{"@id":"sustainability:antiCorruption","@type":["rdf:Property","owl:ObjectProperty"],"rdfs:label":"antiCorruption","schema:rangeIncludes":{"@id":"sustainability:AntiCorruption"},"schema:domainIncludes":{"@id":"sustainability:Ethics"},"rdfs:comment":""},{"@id":"sustainability:complianceToLegislation","@type":["rdf:Property","owl:ObjectProperty"],"rdfs:label":"complianceToLegislation","schema:rangeIncludes":{"@id":"sustainability:ComplianceToLegislation"},"schema:domainIncludes":{"@id":"sustainability:Ethics"},"rdfs:comment":""},{"@id":"sustainability:degree_of_obligation","@type":["rdf:Property","owl:DatatypeProperty"],"rdfs:label":"degree_of_obligation","schema:rangeIncludes":{"@id":"sustainability:DegreeOfObligation"},"schema:domainIncludes":{"@id":"sustainability:CompliancePolicies"},"rdfs:comment":"The degree of obligation refers to the timeframe of implementation of a given requirement."},{"@id":"sustainability:degree_of_criticality","@type":["rdf:Property","owl:DatatypeProperty"],"rdfs:label":"degree_of_criticality","schema:rangeIncludes":{"@id":"sustainability:DegreeOfCriticality"},"schema:domainIncludes":{"@id":"sustainability:CompliancePolicies"},"rdfs:comment":"It provides the criticality framework regarding the compliance of the requirements of the standard."},{"@id":"sustainability:verification_of_compliance","@type":["rdf:Property","owl:DatatypeProperty"],"rdfs:label":"verification_of_compliance","schema:rangeIncludes":{"@id":"sustainability:VerificationOfCompliance"},"schema:domainIncludes":{"@id":"sustainability:CompliancePolicies"},"rdfs:comment":"This section presents the assessment method(s) that are used by auditors / certification bodies when verifying compliance to the standard's content requirements."},{"@id":"sustainability:soil_general_principle","@type":["rdf:Property","owl:DatatypeProperty"],"rdfs:label":"soil_general_principle","schema:rangeIncludes":{"@id":"xsd:string"},"schema:domainIncludes":{"@id":"sustainability:Soil"},"rdfs:comment":"General principle on soil management, as described in the standard"},{"@id":"sustainability:soil_preparation_for_specific_crops_plant_spacing","@type":["rdf:Property","owl:DatatypeProperty"],"rdfs:label":"soil_preparation_for_specific_crops_plant_spacing","schema:rangeIncludes":{"@id":"xsd:boolean"},"schema:domainIncludes":{"@id":"sustainability:Soil"},"rdfs:comment":"Processes in place for sustainable soil preparation for specific crops and adequate plant spacing.Does the standard include criteria on soil preparation and plant spacing?"},{"@id":"sustainability:soil_enhancement_by_crop_rotation_or_intercropping","@type":["rdf:Property","owl:DatatypeProperty"],"rdfs:label":"soil_enhancement_by_crop_rotation_or_intercropping","schema:rangeIncludes":{"@id":"xsd:boolean"},"schema:domainIncludes":{"@id":"sustainability:Soil"},"rdfs:comment":"Processes and practices in place for alternating the species or families of crops grown to maintain or improve soil fertility and organic matter content.Does the standard include criteria on crop rotation or intercropping?"},{"@id":"sustainability:soil_enhancement_by_use_of_cover_crops","@type":["rdf:Property","owl:DatatypeProperty"],"rdfs:label":"soil_enhancement_by_use_of_cover_crops","schema:rangeIncludes":{"@id":"xsd:boolean"},"schema:domainIncludes":{"@id":"sustainability:Soil"},"rdfs:comment":"Processes in place to grow cover crops in order to prevent soil erosion and maintain soil organic matter and soil nutrients, increase nitrogen availability, suppress weed growth and attract beneficial insects.Does the standard include criteria on including cover crop in the crop rotation?"},{"@id":"sustainability:soil_compaction","@type":["rdf:Property","owl:DatatypeProperty"],"rdfs:label":"soil_compaction","schema:rangeIncludes":{"@id":"sustainability:SoilCompaction"},"schema:domainIncludes":{"@id":"sustainability:Soil"},"rdfs:comment":"Management strategies in place to measure, monitor and prevent soil compactionDoes the standard include criteria on soil compaction?"},{"@id":"sustainability:other_soil","@type":["rdf:Property","owl:DatatypeProperty"],"rdfs:label":"other_soil","schema:rangeIncludes":{"@id":"xsd:string"},"schema:domainIncludes":{"@id":"sustainability:Soil"},"rdfs:comment":"Does the standard include other criteria relating to soil"},{"@id":"sustainability:soil_erosion","@type":["rdf:Property","owl:DatatypeProperty"],"rdfs:label":"soil_erosion","schema:rangeIncludes":{"@id":"sustainability:SoilErosion"},"schema:domainIncludes":{"@id":"sustainability:Soil"},"rdfs:comment":"Management strategies in place for the prevention of soils being eroded from the earth’s surface or becoming chemically altered by overuse, salinization, acidification, or other chemical soil contamination.Does the standard include criteria on soil erosion?"},{"@id":"sustainability:soil_conservation","@type":["rdf:Property","owl:DatatypeProperty"],"rdfs:label":"soil_conservation","schema:rangeIncludes":{"@id":"xsd:boolean"},"schema:domainIncludes":{"@id":"sustainability:Soil"},"rdfs:comment":"Managements strategies in place to prevent the decline of soil fertility, development of acidity, salinization, alkalization, deterioration of soil structure, accelerated wind and water erosion, loss of organic matter and diversity.Does the standard include criteria on soil conservation?"},{"@id":"sustainability:soil_quality","@type":["rdf:Property","owl:DatatypeProperty"],"rdfs:label":"soil_quality","schema:rangeIncludes":{"@id":"xsd:boolean"},"schema:domainIncludes":{"@id":"sustainability:Soil"},"rdfs:comment":"Processes in place to determine how well a soil performs the functions of maintaining biodiversity and productivity, partitioning water and solute flow, filtering and buffering, nutrient cycling, and providing support for plants and other structures.Does the standard include criteria on soil quality?"},{"@id":"sustainability:soil_nutrients","@type":["rdf:Property","owl:DatatypeProperty"],"rdfs:label":"soil_nutrients","schema:rangeIncludes":{"@id":"xsd:boolean"},"schema:domainIncludes":{"@id":"sustainability:Soil"},"rdfs:comment":"Processes in place to determine the level of soil nutrients, minerals and organic matter to maintain plant production.Does the standard include criteria on soil nutrients?"},{"@id":"sustainability:soil_fertility","@type":["rdf:Property","owl:DatatypeProperty"],"rdfs:label":"soil_fertility","schema:rangeIncludes":{"@id":"sustainability:SoilFertility"},"schema:domainIncludes":{"@id":"sustainability:Soil"},"rdfs:comment":"Processes in place to determine the ability of the soil to supply essential plant nutrients and water adequately for plant growth and production.Does the standard include criteria on soil fertility?"},{"@id":"sustainability:soil_productivity","@type":["rdf:Property","owl:DatatypeProperty"],"rdfs:label":"soil_productivity","schema:rangeIncludes":{"@id":"xsd:boolean"},"schema:domainIncludes":{"@id":"sustainability:Soil"},"rdfs:comment":"Processes in place to determine the ability of the soil to provide water and nutrients to allow for deep rooting of agricultural plants.Does the standard include criteria on soil productivity?"},{"@id":"sustainability:soil_biodiversity","@type":["rdf:Property","owl:DatatypeProperty"],"rdfs:label":"soil_biodiversity","schema:rangeIncludes":{"@id":"xsd:boolean"},"schema:domainIncludes":{"@id":"sustainability:Soil"},"rdfs:comment":"Processes in place to determine the variability among living organisms in soil.Does the standard include criteria on soil biodiversity?"},{"@id":"sustainability:soil_contamination","@type":["rdf:Property","owl:DatatypeProperty"],"rdfs:label":"soil_contamination","schema:rangeIncludes":{"@id":"sustainability:SoilContamination"},"schema:domainIncludes":{"@id":"sustainability:Soil"},"rdfs:comment":"Processes in place to measure, monitor and prevent soil contamination and pollution.Does the standard include criteria on soil contamination?"},{"@id":"sustainability:forestry_issues_general_principle","@type":["rdf:Property","owl:DatatypeProperty"],"rdfs:label":"forestry_issues_general_principle","schema:rangeIncludes":{"@id":"xsd:string"},"schema:domainIncludes":{"@id":"sustainability:Forests"},"rdfs:comment":"The standard includes a general principle on forests.Does the standard include a general principle on forests?"},{"@id":"sustainability:inclusion_of_all_forest_resources_in_at_least_long_term_objectives_of_forest_management_plan_fmp","@type":["rdf:Property","owl:DatatypeProperty"],"rdfs:label":"inclusion_of_all_forest_resources_in_at_least_long_term_objectives_of_forest_management_plan_fmp","schema:rangeIncludes":{"@id":"xsd:boolean"},"schema:domainIncludes":{"@id":"sustainability:Forests"},"rdfs:comment":"The forest management plan lays out long-term objectives.Does the standard require that the forest management plan lays out long-term objectives?"},{"@id":"sustainability:use_of_verifiable_targets_in_fmp_by_which_progress_can_be_assessed","@type":["rdf:Property","owl:DatatypeProperty"],"rdfs:label":"use_of_verifiable_targets_in_fmp_by_which_progress_can_be_assessed","schema:rangeIncludes":{"@id":"xsd:boolean"},"schema:domainIncludes":{"@id":"sustainability:Forests"},"rdfs:comment":"The forest management plan includes verifiable targets for assessing progress.Does the standard require the forest management plan to include verifiable targets by which progress can be assessed?"},{"@id":"sustainability:fmp_annual_allowable_cut","@type":["rdf:Property","owl:DatatypeProperty"],"rdfs:label":"fmp_annual_allowable_cut","schema:rangeIncludes":{"@id":"xsd:boolean"},"schema:domainIncludes":{"@id":"sustainability:Forests"},"rdfs:comment":"The forest management plan defines the annual allowable cut.Does the standard require that the forest management plan defines the annual allowable cut?"},{"@id":"sustainability:fmp_annual_allowable_exploitation_of_non_timber_forest_products","@type":["rdf:Property","owl:DatatypeProperty"],"rdfs:label":"fmp_annual_allowable_exploitation_of_non_timber_forest_products","schema:rangeIncludes":{"@id":"xsd:boolean"},"schema:domainIncludes":{"@id":"sustainability:Forests"},"rdfs:comment":"The forest management plan defines the annual allowable exploitation of NTFP's (non-timber forest products).Does the standard require that the forest management plan defines the annual allowable exploitation of NTFP's (non-timber forest products)?"},{"@id":"sustainability:fmp_results_be_incorporated_in_a_consistent_and_replicable_monitoring_system","@type":["rdf:Property","owl:DatatypeProperty"],"rdfs:label":"fmp_results_be_incorporated_in_a_consistent_and_replicable_monitoring_system","schema:rangeIncludes":{"@id":"xsd:boolean"},"schema:domainIncludes":{"@id":"sustainability:Forests"},"rdfs:comment":"The standard requires that the forest management plan incorporates results of a consistent and reliable monitoring system.Does the standard require incorporating results of a consistent and replicable monitoring system into forest management planning?"},{"@id":"sustainability:monitoring_of_forests_resources_and_management_practices_that_reflect_natural_disturbance","@type":["rdf:Property","owl:DatatypeProperty"],"rdfs:label":"monitoring_of_forests_resources_and_management_practices_that_reflect_natural_disturbance","schema:rangeIncludes":{"@id":"xsd:boolean"},"schema:domainIncludes":{"@id":"sustainability:Forests"},"rdfs:comment":"Processes in place for the monitoring of forest resources apart from regularity.Does the standard specify minimum requirements for the monitoring of forest resources apart from regularity?"},{"@id":"sustainability:making_publicly_available_fmp_monitoring_results","@type":["rdf:Property","owl:DatatypeProperty"],"rdfs:label":"making_publicly_available_fmp_monitoring_results","schema:rangeIncludes":{"@id":"xsd:boolean"},"schema:domainIncludes":{"@id":"sustainability:Forests"},"rdfs:comment":"A summary of the monitoring results of forest resources and management practices is made publicly available. Does the standard require a publicly available summary of the monitoring results?"},{"@id":"sustainability:legal_compliance_harvest_rights","@type":["rdf:Property","owl:DatatypeProperty"],"rdfs:label":"legal_compliance_harvest_rights","schema:rangeIncludes":{"@id":"xsd:boolean"},"schema:domainIncludes":{"@id":"sustainability:Forests"},"rdfs:comment":"Systems in place to ensure that the timber is from legal origin.Does the standard include criteria on rights to harvest timber within legally gazetted boundaries?"},{"@id":"sustainability:legal_compliance_payments_for_harvest_rights","@type":["rdf:Property","owl:DatatypeProperty"],"rdfs:label":"legal_compliance_payments_for_harvest_rights","schema:rangeIncludes":{"@id":"xsd:boolean"},"schema:domainIncludes":{"@id":"sustainability:Forests"},"rdfs:comment":"There are systems in place to ensure payments for harvest rights and timber including all timber harvesting related duties.Does the standard include payments for harvest rights and timber including duties related to timber harvesting?"},{"@id":"sustainability:other_forestry_conservation_e_g_prohibition_of_genetically_modified_trees_natural_semi_natural_forests_reflecting_natural_disturbance_scenic_landscapes","@type":["rdf:Property","owl:DatatypeProperty"],"rdfs:label":"other_forestry_conservation_e_g_prohibition_of_genetically_modified_trees_natural_semi_natural_forests_reflecting_natural_disturbance_scenic_landscapes","schema:rangeIncludes":{"@id":"xsd:string"},"schema:domainIncludes":{"@id":"sustainability:Forests"},"rdfs:comment":"Standard addresses other criteria related to forestry conversion.Does the standard address other forestry related criteria not covered above"},{"@id":"sustainability:regeneration_of_tree_cover_after_logging_e_g_to_pre_harvesting_situation","@type":["rdf:Property","owl:DatatypeProperty"],"rdfs:label":"regeneration_of_tree_cover_after_logging_e_g_to_pre_harvesting_situation","schema:rangeIncludes":{"@id":"xsd:boolean"},"schema:domainIncludes":{"@id":"sustainability:Forests"},"rdfs:comment":"Procedures in place for the restocking of existing forests and woodlands which have been depleted.Does the standard include criteria on remedy issues after logging operations?"},{"@id":"sustainability:prevent_and_or_remediate_deforestation_e_g_use_tree_species_for_regeneration_that_are_well_adapted_to_site_conditions","@type":["rdf:Property","owl:DatatypeProperty"],"rdfs:label":"prevent_and_or_remediate_deforestation_e_g_use_tree_species_for_regeneration_that_are_well_adapted_to_site_conditions","schema:rangeIncludes":{"@id":"xsd:boolean"},"schema:domainIncludes":{"@id":"sustainability:Forests"},"rdfs:comment":"Procedures in place to prevent and/or remediate deforestation.Does the standard include requirements for the prevention and/or remediation of deforestation?"},{"@id":"sustainability:enhance_conservation_of_forests","@type":["rdf:Property","owl:DatatypeProperty"],"rdfs:label":"enhance_conservation_of_forests","schema:rangeIncludes":{"@id":"xsd:boolean"},"schema:domainIncludes":{"@id":"sustainability:Forests"},"rdfs:comment":"Resource management practices in place for maintaining ecosystem health and the resource base for continual use.Does the standard include criteria to enhance conservation of forests?"},{"@id":"sustainability:the_conversion_of_forests_into_production_lands","@type":["rdf:Property","owl:DatatypeProperty"],"rdfs:label":"the_conversion_of_forests_into_production_lands","schema:rangeIncludes":{"@id":"sustainability:TheConversionOfForestsIntoProductionLands"},"schema:domainIncludes":{"@id":"sustainability:Forests"},"rdfs:comment":"Does the standard include criteria on safeguards for the conversion of land or forests / the destruction of ecosystems for production?"},{"@id":"sustainability:the_conversion_of_agriculture_land_to_non_agriculture_purposes","@type":["rdf:Property","owl:DatatypeProperty"],"rdfs:label":"the_conversion_of_agriculture_land_to_non_agriculture_purposes","schema:rangeIncludes":{"@id":"xsd:boolean"},"schema:domainIncludes":{"@id":"sustainability:Forests"},"rdfs:comment":"Practices in place for impact assessment of the conversion of existing agricultural land to non-agricultural use.Does the standard include criteria on assessing impacts of agricultural land conversion?"},{"@id":"sustainability:maintenance_of_records_of_forests_at_least5_years_period","@type":["rdf:Property","owl:DatatypeProperty"],"rdfs:label":"maintenance_of_records_of_forests_at_least5_years_period","schema:rangeIncludes":{"@id":"xsd:boolean"},"schema:domainIncludes":{"@id":"sustainability:Forests"},"rdfs:comment":"Records on forests are maintained for a minimum of five years.Does the standard require maintenance of records on forests for a minimum of five years?"},{"@id":"sustainability:forest_management_plan_fmp_baseline_objectives_and_assessment_of_current_conditions_stockings_species_age_classes_of_trees_etc","@type":["rdf:Property","owl:DatatypeProperty"],"rdfs:label":"forest_management_plan_fmp_baseline_objectives_and_assessment_of_current_conditions_stockings_species_age_classes_of_trees_etc","schema:rangeIncludes":{"@id":"xsd:boolean"},"schema:domainIncludes":{"@id":"sustainability:Forests"},"rdfs:comment":"The forest management plan considers the current conditions of the Forest Management Unit as a baseline for long term objectives.Does the standard require that the forest management plan considers the current condition of the Forest Management Unit (e.g. through baseline studies)?"},{"@id":"sustainability:preparation_of_public_summary_of_the_forest_management_plan_fmp","@type":["rdf:Property","owl:DatatypeProperty"],"rdfs:label":"preparation_of_public_summary_of_the_forest_management_plan_fmp","schema:rangeIncludes":{"@id":"xsd:boolean"},"schema:domainIncludes":{"@id":"sustainability:Forests"},"rdfs:comment":"A summary of the forest management plan is made publicly available.Does the standard require a publicly available summary of the forest management plan?"},{"@id":"sustainability:chemicals_natural_organic_inputs_general_principle","@type":["rdf:Property","owl:DatatypeProperty"],"rdfs:label":"chemicals_natural_organic_inputs_general_principle","schema:rangeIncludes":{"@id":"xsd:string"},"schema:domainIncludes":{"@id":"sustainability:ChemicalInputs"},"rdfs:comment":"The standard includes a general principle on the use of chemicals.Does the standard include a general principle on the use of chemicals?"},{"@id":"sustainability:implementation_of_an_integrated_pest_management_ipm","@type":["rdf:Property","owl:DatatypeProperty"],"rdfs:label":"implementation_of_an_integrated_pest_management_ipm","schema:rangeIncludes":{"@id":"xsd:boolean"},"schema:domainIncludes":{"@id":"sustainability:ChemicalInputs"},"rdfs:comment":"Procedures in place for the use of Integrated Pest Management (IPM) approaches in order to reduce the need for chemical use.Does the standard require the use of Integrated Pest Management (IPM) practices?"},{"@id":"sustainability:training_on_integrated_pest_management_ipm","@type":["rdf:Property","owl:DatatypeProperty"],"rdfs:label":"training_on_integrated_pest_management_ipm","schema:rangeIncludes":{"@id":"xsd:boolean"},"schema:domainIncludes":{"@id":"sustainability:ChemicalInputs"},"rdfs:comment":"Requirements in place for the provision of education and training on the practices of Integrated Pest Management (IPM).Does the standard include criteria on the provision of training on Integrated Pest Management (IPM)?"},{"@id":"sustainability:chemicals_and_related_materials_general_principle","@type":["rdf:Property","owl:DatatypeProperty"],"rdfs:label":"chemicals_and_related_materials_general_principle","schema:rangeIncludes":{"@id":"xsd:boolean"},"schema:domainIncludes":{"@id":"sustainability:ChemicalInputs"},"rdfs:comment":"The standard includes a general principle on the use of synthetic inputs.Does the standard include a general principle on the use of chemicals and related materials?"},{"@id":"sustainability:chemicals_use_and_application_records","@type":["rdf:Property","owl:DatatypeProperty"],"rdfs:label":"chemicals_use_and_application_records","schema:rangeIncludes":{"@id":"sustainability:ChemicalsUseAndApplicationRecords"},"schema:domainIncludes":{"@id":"sustainability:ChemicalInputs"},"rdfs:comment":"Processes in place to document and reduce the use of chemicals. Does the standard require documentation and monitoring of chemical use?"},{"@id":"sustainability:chemicals_storage_and_labeling","@type":["rdf:Property","owl:DatatypeProperty"],"rdfs:label":"chemicals_storage_and_labeling","schema:rangeIncludes":{"@id":"xsd:boolean"},"schema:domainIncludes":{"@id":"sustainability:ChemicalInputs"},"rdfs:comment":"Procedures in place for chemical storage and labeling.Does the standard require safe storage and appropriate labeling of chemicals?"},{"@id":"sustainability:chemicals_equipment_and_containers_storage_cleaning","@type":["rdf:Property","owl:DatatypeProperty"],"rdfs:label":"chemicals_equipment_and_containers_storage_cleaning","schema:rangeIncludes":{"@id":"xsd:boolean"},"schema:domainIncludes":{"@id":"sustainability:ChemicalInputs"},"rdfs:comment":"Processes in place for appropriate documentation, application, handling, storage and disposal of chemicals.Does the standard require documentation, handling, storage and disposal of agrochemicals in line with good practices and/or manufacturer recommendations?"},{"@id":"sustainability:protection_of_non_target_areas_from_agro_chemical_use","@type":["rdf:Property","owl:DatatypeProperty"],"rdfs:label":"protection_of_non_target_areas_from_agro_chemical_use","schema:rangeIncludes":{"@id":"xsd:boolean"},"schema:domainIncludes":{"@id":"sustainability:ChemicalInputs"},"rdfs:comment":"Processes in place for the protection of non-target areas from agro-chemical use.Does the standard require non-target areas to be protected from agro-chemical use?"},{"@id":"sustainability:regular_re_calibration_of_agro_chemicals_application_equipment","@type":["rdf:Property","owl:DatatypeProperty"],"rdfs:label":"regular_re_calibration_of_agro_chemicals_application_equipment","schema:rangeIncludes":{"@id":"xsd:boolean"},"schema:domainIncludes":{"@id":"sustainability:ChemicalInputs"},"rdfs:comment":"Procedures in place for regular re-calibration of agro-chemical application equipment.Does the standard require regularly scheduled re-calibration of agro-chemical application equipment?"},{"@id":"sustainability:production_process_chemicals_extractive_industries_cleaning_food_non_food_manufacturing","@type":["rdf:Property","owl:DatatypeProperty"],"rdfs:label":"production_process_chemicals_extractive_industries_cleaning_food_non_food_manufacturing","schema:rangeIncludes":{"@id":"xsd:boolean"},"schema:domainIncludes":{"@id":"sustainability:ChemicalInputs"},"rdfs:comment":"Does the standard include criteria on the management of process chemicals and cleaning agents used in the production phase?"},{"@id":"sustainability:organic_natural_inputs_general_principles_practices","@type":["rdf:Property","owl:DatatypeProperty"],"rdfs:label":"organic_natural_inputs_general_principles_practices","schema:rangeIncludes":{"@id":"xsd:boolean"},"schema:domainIncludes":{"@id":"sustainability:ChemicalInputs"},"rdfs:comment":"Does the standard include a general principle on the use of natural inputs?"},{"@id":"sustainability:prohibition_of_use_of_any_pesticides_biological_control_of_pests_and_other_related_chemical_substances","@type":["rdf:Property","owl:DatatypeProperty"],"rdfs:label":"prohibition_of_use_of_any_pesticides_biological_control_of_pests_and_other_related_chemical_substances","schema:rangeIncludes":{"@id":"xsd:boolean"},"schema:domainIncludes":{"@id":"sustainability:ChemicalInputs"},"rdfs:comment":"Standard prohibits the use of all chemicals.Does the standard prohibit the use of pesticides, biological control of pests and other related chemical substances?"},{"@id":"sustainability:use_of_organic_fertilizer","@type":["rdf:Property","owl:DatatypeProperty"],"rdfs:label":"use_of_organic_fertilizer","schema:rangeIncludes":{"@id":"sustainability:UseOfOrganicFertilizer"},"schema:domainIncludes":{"@id":"sustainability:ChemicalInputs"},"rdfs:comment":"Procedures in place for the use of organic fertilizers (or biofertilizer).Does the standard include criteria on organic fertilizer, incl. manure?"},{"@id":"sustainability:equipment_maintenance_cleaning_and_warehousing_procedures","@type":["rdf:Property","owl:DatatypeProperty"],"rdfs:label":"equipment_maintenance_cleaning_and_warehousing_procedures","schema:rangeIncludes":{"@id":"xsd:boolean"},"schema:domainIncludes":{"@id":"sustainability:ChemicalInputs"},"rdfs:comment":"Does the standard include criteria on equipment maintenance, cleaning and warehouse procedures?"},{"@id":"sustainability:chemicals_selective_targeted_application","@type":["rdf:Property","owl:DatatypeProperty"],"rdfs:label":"chemicals_selective_targeted_application","schema:rangeIncludes":{"@id":"xsd:boolean"},"schema:domainIncludes":{"@id":"sustainability:ChemicalInputs"},"rdfs:comment":"Procedures in place to ensure selective and targeted application of chemicals.Does the standard include criteria on selective and targeted application of chemicals?"},{"@id":"sustainability:training_on_chemicals_handling_and_exposure","@type":["rdf:Property","owl:DatatypeProperty"],"rdfs:label":"training_on_chemicals_handling_and_exposure","schema:rangeIncludes":{"@id":"xsd:boolean"},"schema:domainIncludes":{"@id":"sustainability:ChemicalInputs"},"rdfs:comment":"Instruction and training procedures in place for handling of and exposure to chemicals.Does the standard require instruction and training on chemicals handling and exposure?"},{"@id":"sustainability:chemicals_variation_to_prevent_pest_resistance","@type":["rdf:Property","owl:DatatypeProperty"],"rdfs:label":"chemicals_variation_to_prevent_pest_resistance","schema:rangeIncludes":{"@id":"xsd:boolean"},"schema:domainIncludes":{"@id":"sustainability:ChemicalInputs"},"rdfs:comment":"Procedures in place for chemical variation for pest resistance management.Does the standard include criteria on pest resistance management (e.g. chemical variation)?"},{"@id":"sustainability:chemical_substances_storage_disposal_waste_labeling","@type":["rdf:Property","owl:DatatypeProperty"],"rdfs:label":"chemical_substances_storage_disposal_waste_labeling","schema:rangeIncludes":{"@id":"xsd:boolean"},"schema:domainIncludes":{"@id":"sustainability:ChemicalInputs"},"rdfs:comment":"Processes in place for proper management of chemical storage, disposal, labeling and/or waste.Does the standard include requirements for management of storage, disposal and labeling of chemicals and/or waste?"},{"@id":"sustainability:treatment_of_waste_of_chemical_substances_and_related_materials","@type":["rdf:Property","owl:DatatypeProperty"],"rdfs:label":"treatment_of_waste_of_chemical_substances_and_related_materials","schema:rangeIncludes":{"@id":"xsd:boolean"},"schema:domainIncludes":{"@id":"sustainability:ChemicalInputs"},"rdfs:comment":"Processes in place for proper treatment of different agrochemical wastes.Does the standard require proper treatment of waste from chemical substances and related materials?"},{"@id":"sustainability:use_and_management_of_hazardous_chemicals","@type":["rdf:Property","owl:DatatypeProperty"],"rdfs:label":"use_and_management_of_hazardous_chemicals","schema:rangeIncludes":{"@id":"xsd:boolean"},"schema:domainIncludes":{"@id":"sustainability:ChemicalInputs"},"rdfs:comment":"Processes in place for proper management of hazardous chemicals.Does the standard require proper identification, assessment and control procedures on the use and storage of hazardous chemicals?"},{"@id":"sustainability:biodegradability_of_chemicals","@type":["rdf:Property","owl:DatatypeProperty"],"rdfs:label":"biodegradability_of_chemicals","schema:rangeIncludes":{"@id":"xsd:boolean"},"schema:domainIncludes":{"@id":"sustainability:ChemicalInputs"},"rdfs:comment":"Procedures in place for the biodegradation of chemicals.Does the standard require procedures to be in place for the biodegradation of chemicals?"},{"@id":"sustainability:general_prohibition_of_use_of_gmos","@type":["rdf:Property","owl:DatatypeProperty"],"rdfs:label":"general_prohibition_of_use_of_gmos","schema:rangeIncludes":{"@id":"xsd:boolean"},"schema:domainIncludes":{"@id":"sustainability:ChemicalInputs"},"rdfs:comment":"General prohibition in place for the use of GMOs / genetically modified varieties Does the standard prohibit the use of GMO species?"},{"@id":"sustainability:prohibition_of_use_of_hazardous_chemicals_as_defined_by_who1a_and_b2_and_the_stockholm_and_rotterdam_conventions","@type":["rdf:Property","owl:DatatypeProperty"],"rdfs:label":"prohibition_of_use_of_hazardous_chemicals_as_defined_by_who1a_and_b2_and_the_stockholm_and_rotterdam_conventions","schema:rangeIncludes":{"@id":"sustainability:ProhibitionOfUseOfHazardousChemicalsAsDefinedByWho1aAndB2AndTheStockholmAndRotterdamConventions"},"schema:domainIncludes":{"@id":"sustainability:ChemicalInputs"},"rdfs:comment":"The standard specifies a list of prohibited substances.Does the standard include criteria on hazardous chemicals, as referenced by (1) Stockholm convention, (2) WHO class 1A and B or (3) Rotterdam convention?"},{"@id":"sustainability:use_and_management_of_gmos","@type":["rdf:Property","owl:DatatypeProperty"],"rdfs:label":"use_and_management_of_gmos","schema:rangeIncludes":{"@id":"sustainability:UseAndManagementOfGmos"},"schema:domainIncludes":{"@id":"sustainability:ChemicalInputs"},"rdfs:comment":"Procedures in place for the use and management of genetically modified organisms (GMOs) within production process.Does the standard include criteria on the use and management of genetically modified organisms (GMOs)?"},{"@id":"sustainability:risk_prevention_with_regards_to_use_of_gmos","@type":["rdf:Property","owl:DatatypeProperty"],"rdfs:label":"risk_prevention_with_regards_to_use_of_gmos","schema:rangeIncludes":{"@id":"sustainability:RiskPreventionWithRegardsToUseOfGmos"},"schema:domainIncludes":{"@id":"sustainability:ChemicalInputs"},"rdfs:comment":"Procedures in place to prevent risk from genetically modified varieties / GMOs by producer or surrounding community (e.g. invasion, contamination, or cross-pollination)Does the standard include requirements for risk prevention from GMOs?"},{"@id":"sustainability:traceability_and_labeling_of_genetically_modified_crops_and_products","@type":["rdf:Property","owl:DatatypeProperty"],"rdfs:label":"traceability_and_labeling_of_genetically_modified_crops_and_products","schema:rangeIncludes":{"@id":"xsd:boolean"},"schema:domainIncludes":{"@id":"sustainability:ChemicalInputs"},"rdfs:comment":"Procedures in place for the traceability and labeling of genetically modified crops and products.Does the standard have a separated supply-chain for non-GMO crops and products?"},{"@id":"sustainability:other","@type":["rdf:Property","owl:DatatypeProperty"],"rdfs:label":"other","schema:rangeIncludes":{"@id":"xsd:string"},"schema:domainIncludes":{"@id":"sustainability:ChemicalInputs"},"rdfs:comment":"Does the standard contain other criteria related to chemicals not addressed above"},{"@id":"sustainability:prohibition_of_use_of_hazardous_chemicals_as_defined_by_the_pan_international_list_of_highly_hazardous_pesticides","@type":["rdf:Property","owl:DatatypeProperty"],"rdfs:label":"prohibition_of_use_of_hazardous_chemicals_as_defined_by_the_pan_international_list_of_highly_hazardous_pesticides","schema:rangeIncludes":{"@id":"sustainability:ProhibitionOfUseOfHazardousChemicalsAsDefinedByThePanInternationalListOfHighlyHazardousPesticides"},"schema:domainIncludes":{"@id":"sustainability:ChemicalInputs"},"rdfs:comment":"Restrictions or prohibitions in place on the use of hazardous chemicals (as defined by the PAN International List of Highly Hazardous Pesticides)Does the standard restrict or prohibit the use of hazardous chemicals as defined by the PAN International List of Highly Hazardous Pesticides?"},{"@id":"sustainability:respect_of_list_of_permitted_chemicals_of_low_concern_for_the_intended_use_of_product","@type":["rdf:Property","owl:DatatypeProperty"],"rdfs:label":"respect_of_list_of_permitted_chemicals_of_low_concern_for_the_intended_use_of_product","schema:rangeIncludes":{"@id":"xsd:boolean"},"schema:domainIncludes":{"@id":"sustainability:ChemicalInputs"},"rdfs:comment":"The standard includes a list of chemical substances which are of low concern for the intended use of the product. Does the standard include a list of substances which are of low concern for the intended use?"},{"@id":"sustainability:respect_list_of_prohibited_chemicals_as_harmful_to_human_health_h_statements_h340_h350_h360","@type":["rdf:Property","owl:DatatypeProperty"],"rdfs:label":"respect_list_of_prohibited_chemicals_as_harmful_to_human_health_h_statements_h340_h350_h360","schema:rangeIncludes":{"@id":"sustainability:RespectListOfProhibitedChemicalsAsHarmfulToHumanHealthHStatementsH340H350H360"},"schema:domainIncludes":{"@id":"sustainability:ChemicalInputs"},"rdfs:comment":"The standard includes a list of prohibited chemicals as harmful to human health (as defined in hazard statements (H statements) H340, H350, H360).Does the standard include criteria on H statements H340, H350, H360?"},{"@id":"sustainability:the_restrictions_on_surfactants_cleaning_agents_and_foam_inhibitors","@type":["rdf:Property","owl:DatatypeProperty"],"rdfs:label":"the_restrictions_on_surfactants_cleaning_agents_and_foam_inhibitors","schema:rangeIncludes":{"@id":"xsd:boolean"},"schema:domainIncludes":{"@id":"sustainability:ChemicalInputs"},"rdfs:comment":"Restrictions in place on the use of surfactants, cleaning agents and foam inhibitors.Does the standard restrict the use of surfactants, cleaning agents and foam inhibitors?"},{"@id":"sustainability:appropriate_tests_of_toxicity","@type":["rdf:Property","owl:DatatypeProperty"],"rdfs:label":"appropriate_tests_of_toxicity","schema:rangeIncludes":{"@id":"xsd:boolean"},"schema:domainIncludes":{"@id":"sustainability:ChemicalInputs"},"rdfs:comment":"Procedures in place to test for toxicity (e.g. soil, plant, water, manure).Does the standard require appropriate testing for toxicity of agriculture chemicals to be performed?"},{"@id":"sustainability:use_of_biological_control_agents_must_comply_with_internationally_recognized_standards_e_g_authorized_list_of_substances","@type":["rdf:Property","owl:DatatypeProperty"],"rdfs:label":"use_of_biological_control_agents_must_comply_with_internationally_recognized_standards_e_g_authorized_list_of_substances","schema:rangeIncludes":{"@id":"xsd:boolean"},"schema:domainIncludes":{"@id":"sustainability:ChemicalInputs"},"rdfs:comment":"Requirements in place to ensure that any use of biological control agents comply with internationally recognized standards and/or protocols.Does the standard require that the use of biological control agents comply with internationally recognized standards and/or protocols?"},{"@id":"sustainability:overarching_policy_or_set_of_principles_on_biodiversity","@type":["rdf:Property","owl:DatatypeProperty"],"rdfs:label":"overarching_policy_or_set_of_principles_on_biodiversity","schema:rangeIncludes":{"@id":"xsd:string"},"schema:domainIncludes":{"@id":"sustainability:Biodiversity"},"rdfs:comment":"Does the standard include an overarching policy or set of principles on biodiversity?"},{"@id":"sustainability:wildlife_general_principle","@type":["rdf:Property","owl:DatatypeProperty"],"rdfs:label":"wildlife_general_principle","schema:rangeIncludes":{"@id":"xsd:boolean"},"schema:domainIncludes":{"@id":"sustainability:Biodiversity"},"rdfs:comment":"Does the standard include a general principle on wildlife?"},{"@id":"sustainability:regulated_and_sustainable_access_to_resources_and_use_of_wildlife_species","@type":["rdf:Property","owl:DatatypeProperty"],"rdfs:label":"regulated_and_sustainable_access_to_resources_and_use_of_wildlife_species","schema:rangeIncludes":{"@id":"sustainability:RegulatedAndSustainableAccessToResourcesAndUseOfWildlifeSpecies"},"schema:domainIncludes":{"@id":"sustainability:Biodiversity"},"rdfs:comment":"Procedures in place to regulate access to resources and use of wildlife species.Does the standard include criteria on illegal activities such as hunting, fishing, trapping, collection of NTFP's (non-timber forest products) etc.?"},{"@id":"sustainability:specific_rare_threatened_or_endangered_wildlife_species","@type":["rdf:Property","owl:DatatypeProperty"],"rdfs:label":"specific_rare_threatened_or_endangered_wildlife_species","schema:rangeIncludes":{"@id":"sustainability:SpecificRareThreatenedOrEndangeredWildlifeSpecies"},"schema:domainIncludes":{"@id":"sustainability:Biodiversity"},"rdfs:comment":"Processes in place for the protection of rare, threatened or endangered species within the unit of operations.Does the standard include criteria on rare, threatened or endangered species?"},{"@id":"sustainability:regulated_and_suitable_housing_of_wildlife_living_specimens","@type":["rdf:Property","owl:DatatypeProperty"],"rdfs:label":"regulated_and_suitable_housing_of_wildlife_living_specimens","schema:rangeIncludes":{"@id":"xsd:boolean"},"schema:domainIncludes":{"@id":"sustainability:Biodiversity"},"rdfs:comment":"Systems in place for the provision of regulated and suitable housing for wildlife living specimens.Does the standard require regulated and suitable housing of wildlife living specimens?"},{"@id":"sustainability:minimized_impacts_on_wildlife_populations","@type":["rdf:Property","owl:DatatypeProperty"],"rdfs:label":"minimized_impacts_on_wildlife_populations","schema:rangeIncludes":{"@id":"xsd:boolean"},"schema:domainIncludes":{"@id":"sustainability:Biodiversity"},"rdfs:comment":"Processes in place for minimal impacts on wildlife populations.Does the standard include criteria for minimized impacts on wildlife populations (e.g. UEBT)?"},{"@id":"sustainability:spatial_management_criteria","@type":["rdf:Property","owl:DatatypeProperty"],"rdfs:label":"spatial_management_criteria","schema:rangeIncludes":{"@id":"xsd:boolean"},"schema:domainIncludes":{"@id":"sustainability:Biodiversity"},"rdfs:comment":"Procedures in place for the integration of buffer zones.Does the standard include criteria on ecosystem protection through spatial management (conservation areas, 'set aside' or buffer zones)?"},{"@id":"sustainability:safeguards_against_fragmentation_of_ecosystems","@type":["rdf:Property","owl:DatatypeProperty"],"rdfs:label":"safeguards_against_fragmentation_of_ecosystems","schema:rangeIncludes":{"@id":"xsd:boolean"},"schema:domainIncludes":{"@id":"sustainability:Biodiversity"},"rdfs:comment":"Processes in place for the creation and or conservation of ecological niches.Does the standard include criteria on safeguards against fragmentation of good quality ecosystems/habitats?"},{"@id":"sustainability:maintaining_or_protecting_rare_threatened_or_endangered_ecosystems","@type":["rdf:Property","owl:DatatypeProperty"],"rdfs:label":"maintaining_or_protecting_rare_threatened_or_endangered_ecosystems","schema:rangeIncludes":{"@id":"xsd:boolean"},"schema:domainIncludes":{"@id":"sustainability:Biodiversity"},"rdfs:comment":"Does the standard include criteria on maintaining or protecting rare, threatened or endangered ecosystems?"},{"@id":"sustainability:criteria_to_avoid_crop_disease_cross_contamination","@type":["rdf:Property","owl:DatatypeProperty"],"rdfs:label":"criteria_to_avoid_crop_disease_cross_contamination","schema:rangeIncludes":{"@id":"xsd:boolean"},"schema:domainIncludes":{"@id":"sustainability:Biodiversity"},"rdfs:comment":"Does the standard require processes in place to avoid crop disease cross -contamination?"},{"@id":"sustainability:monitoring_and_preserving_aquaculture_diversity","@type":["rdf:Property","owl:DatatypeProperty"],"rdfs:label":"monitoring_and_preserving_aquaculture_diversity","schema:rangeIncludes":{"@id":"xsd:boolean"},"schema:domainIncludes":{"@id":"sustainability:Biodiversity"},"rdfs:comment":"Does the standard include criteria on fish density and diversity?"},{"@id":"sustainability:conventions_on_biodiversity_cites_cbd_cms_ccd","@type":["rdf:Property","owl:DatatypeProperty"],"rdfs:label":"conventions_on_biodiversity_cites_cbd_cms_ccd","schema:rangeIncludes":{"@id":"xsd:boolean"},"schema:domainIncludes":{"@id":"sustainability:Biodiversity"},"rdfs:comment":"Systems in place to ensure adherence to international conventions on biodiversity and best practices (CITES, CBD, CMS, CCD, among others).Is the standard consistent with relevant international conventions on biodiversity, ecosystems and conservation?"},{"@id":"sustainability:diversity_of_planting_materials_seeds_and_crops_genotypes","@type":["rdf:Property","owl:DatatypeProperty"],"rdfs:label":"diversity_of_planting_materials_seeds_and_crops_genotypes","schema:rangeIncludes":{"@id":"xsd:boolean"},"schema:domainIncludes":{"@id":"sustainability:Biodiversity"},"rdfs:comment":"Procedures in place for the cultivation of mixed genotypes of each main crop.Does the standard include requirements to cultivate a mix of genotypes of each main crop?"},{"@id":"sustainability:maintaining_restoring_prioritizing_native_species","@type":["rdf:Property","owl:DatatypeProperty"],"rdfs:label":"maintaining_restoring_prioritizing_native_species","schema:rangeIncludes":{"@id":"xsd:boolean"},"schema:domainIncludes":{"@id":"sustainability:Biodiversity"},"rdfs:comment":"Procedures in place for priority in use of native species over foreign species.Does the standard include criteria on the priority of native species?"},{"@id":"sustainability:the_protection_of_ecosystems_against_invasive_species","@type":["rdf:Property","owl:DatatypeProperty"],"rdfs:label":"the_protection_of_ecosystems_against_invasive_species","schema:rangeIncludes":{"@id":"sustainability:TheProtectionOfEcosystemsAgainstInvasiveSpecies"},"schema:domainIncludes":{"@id":"sustainability:Biodiversity"},"rdfs:comment":"Processes in place for the management or prohibition of introduction of alien invasive species.Does the standard include criteria on the use of alien invasive species?"},{"@id":"sustainability:monitoring_and_protection_of_high_conservation_value_areas","@type":["rdf:Property","owl:DatatypeProperty"],"rdfs:label":"monitoring_and_protection_of_high_conservation_value_areas","schema:rangeIncludes":{"@id":"xsd:boolean"},"schema:domainIncludes":{"@id":"sustainability:Biodiversity"},"rdfs:comment":"Procedures in place to address land-use planning and identification of conservation priorities.Does the standard include criteria for the monitoring and protection of High Conservation Value Areas?"},{"@id":"sustainability:prohibition_of_production_on_land_with_high_conservation_value","@type":["rdf:Property","owl:DatatypeProperty"],"rdfs:label":"prohibition_of_production_on_land_with_high_conservation_value","schema:rangeIncludes":{"@id":"xsd:boolean"},"schema:domainIncludes":{"@id":"sustainability:Biodiversity"},"rdfs:comment":"Prohibition of production on land with High Conservation Value (HCV) with conversion cut-off date no later than 2009 or at least five years history.Does the standard prohibit production on land with High Conservation Value (HCV)?"},{"@id":"sustainability:hcv_as_intended_in_the_hcv_resource_network","@type":["rdf:Property","owl:DatatypeProperty"],"rdfs:label":"hcv_as_intended_in_the_hcv_resource_network","schema:rangeIncludes":{"@id":"xsd:boolean"},"schema:domainIncludes":{"@id":"sustainability:Biodiversity"},"rdfs:comment":"Systems in place for identifying and managing environmental and social values based on the commonly used six HCV categories.Does the standard use the HCV terminology as intended by the HCV Resource Network?"},{"@id":"sustainability:prohibition_of_production_on_land_with_high_conservation_area_recognized_by_independent_expertise","@type":["rdf:Property","owl:DatatypeProperty"],"rdfs:label":"prohibition_of_production_on_land_with_high_conservation_area_recognized_by_independent_expertise","schema:rangeIncludes":{"@id":"xsd:boolean"},"schema:domainIncludes":{"@id":"sustainability:Biodiversity"},"rdfs:comment":"Procedures in place for the use of independent expertise in assessing HCVs prior to expansion of cultivation or plantation.Does the standard require independent expertise to be used as a resource in determining HCVs prior to expansion of operations?"},{"@id":"sustainability:legally_protected_and_internationally_recognized_areas_for_their_biodiversity","@type":["rdf:Property","owl:DatatypeProperty"],"rdfs:label":"legally_protected_and_internationally_recognized_areas_for_their_biodiversity","schema:rangeIncludes":{"@id":"xsd:boolean"},"schema:domainIncludes":{"@id":"sustainability:Biodiversity"},"rdfs:comment":"Procedures in place to maintain legally and internationally recognized protected areas for the achievement of long term conservation of nature.Does the standard have requirements to respect legally protected and internationally recognized protected areas?"},{"@id":"sustainability:identifying_risks_and_impacts_on_ecosystem_services","@type":["rdf:Property","owl:DatatypeProperty"],"rdfs:label":"identifying_risks_and_impacts_on_ecosystem_services","schema:rangeIncludes":{"@id":"xsd:boolean"},"schema:domainIncludes":{"@id":"sustainability:Biodiversity"},"rdfs:comment":"Does the standard include requirements to identify risks and regularly monitor production activity impacts on ecosystem function?"},{"@id":"sustainability:use_of_biotechnologies","@type":["rdf:Property","owl:DatatypeProperty"],"rdfs:label":"use_of_biotechnologies","schema:rangeIncludes":{"@id":"xsd:boolean"},"schema:domainIncludes":{"@id":"sustainability:Biodiversity"},"rdfs:comment":"Does the standard include requirements on biotechnologies (e.g. their use and management in production processes)?"},{"@id":"sustainability:sustainable_management_and_use_of_natural_resources","@type":["rdf:Property","owl:DatatypeProperty"],"rdfs:label":"sustainable_management_and_use_of_natural_resources","schema:rangeIncludes":{"@id":"xsd:boolean"},"schema:domainIncludes":{"@id":"sustainability:Biodiversity"},"rdfs:comment":"Processes in place to ensure that products are not harvested at levels above sustainable yields.Does the standard explicitly require that products are harvested at levels that ensure sustainable management and use of natural resources?"},{"@id":"sustainability:practices_and_open_pit_underground_extractive_metals_practices","@type":["rdf:Property","owl:DatatypeProperty"],"rdfs:label":"practices_and_open_pit_underground_extractive_metals_practices","schema:rangeIncludes":{"@id":"xsd:boolean"},"schema:domainIncludes":{"@id":"sustainability:Biodiversity"},"rdfs:comment":"Does the standard include criteria relating to open pit/underground extractive practices (e.g. mining sector)?"},{"@id":"sustainability:criteria_and_practices_relating_to_the_clearing_of_land_with_fire_or_explosives","@type":["rdf:Property","owl:DatatypeProperty"],"rdfs:label":"criteria_and_practices_relating_to_the_clearing_of_land_with_fire_or_explosives","schema:rangeIncludes":{"@id":"sustainability:CriteriaAndPracticesRelatingToTheClearingOfLandWithFireOrExplosives"},"schema:domainIncludes":{"@id":"sustainability:Biodiversity"},"rdfs:comment":"Procedures in place that control or prohibit using fire or explosives in production and / or for clearing land areas.Does the standard include criteria on the application of fire or explosives for the clearing of land (e.g. slash & burn)?"},{"@id":"sustainability:post_production_practices_impact_assessment_rotation_of_crops","@type":["rdf:Property","owl:DatatypeProperty"],"rdfs:label":"post_production_practices_impact_assessment_rotation_of_crops","schema:rangeIncludes":{"@id":"xsd:boolean"},"schema:domainIncludes":{"@id":"sustainability:Biodiversity"},"rdfs:comment":"Does the standard explicitly require implementation of post-production / post-harvesting practices that aim to protect and preserve biodiversity?"},{"@id":"sustainability:human_settlements_in_or_close_to_production_areas","@type":["rdf:Property","owl:DatatypeProperty"],"rdfs:label":"human_settlements_in_or_close_to_production_areas","schema:rangeIncludes":{"@id":"xsd:boolean"},"schema:domainIncludes":{"@id":"sustainability:Biodiversity"},"rdfs:comment":"Infrastructure in place to properly access agricultural inputs and services, as well as national and local markets, to reduce food losses.Does the standard include criteria related to infrastructure, storage buildings and proximity to human settlements?"},{"@id":"sustainability:other_biodiversity_e_g_offsets_compensation_policies","@type":["rdf:Property","owl:DatatypeProperty"],"rdfs:label":"other_biodiversity_e_g_offsets_compensation_policies","schema:rangeIncludes":{"@id":"xsd:boolean"},"schema:domainIncludes":{"@id":"sustainability:Biodiversity"},"rdfs:comment":"Other criteria related to biodiversity not covered above.Does the standard include additional criteria related to biodiversity not covered above?"},{"@id":"sustainability:natural_wetlands_and_or_watercourses_affected_by_production","@type":["rdf:Property","owl:DatatypeProperty"],"rdfs:label":"natural_wetlands_and_or_watercourses_affected_by_production","schema:rangeIncludes":{"@id":"sustainability:NaturalWetlandsAndOrWatercoursesAffectedByProduction"},"schema:domainIncludes":{"@id":"sustainability:Biodiversity"},"rdfs:comment":"Does the standard require the identification, monitoring and maintenance of natural wetlands and/or watercourses impacted by production?"},{"@id":"sustainability:sustainable_harvesting","@type":["rdf:Property","owl:DatatypeProperty"],"rdfs:label":"sustainable_harvesting","schema:rangeIncludes":{"@id":"xsd:boolean"},"schema:domainIncludes":{"@id":"sustainability:Biodiversity"},"rdfs:comment":"Does the standard require sustainable timber harvesting to conserve the forest stand?"},{"@id":"sustainability:wild_catch_fisheries_procedures_regarding_management_and_reduction_of_discards","@type":["rdf:Property","owl:DatatypeProperty"],"rdfs:label":"wild_catch_fisheries_procedures_regarding_management_and_reduction_of_discards","schema:rangeIncludes":{"@id":"xsd:boolean"},"schema:domainIncludes":{"@id":"sustainability:Biodiversity"},"rdfs:comment":"Does the standard include requirements on bycatch management and reduction of discards?"},{"@id":"sustainability:wild_catch_fisheries_prohibition_of_of_destructive_fishing_methods_such_as_dynamite_and_poison","@type":["rdf:Property","owl:DatatypeProperty"],"rdfs:label":"wild_catch_fisheries_prohibition_of_of_destructive_fishing_methods_such_as_dynamite_and_poison","schema:rangeIncludes":{"@id":"xsd:boolean"},"schema:domainIncludes":{"@id":"sustainability:Biodiversity"},"rdfs:comment":"Does the standard prohibit the use of destructive fishing methods such as dynamite and poison?"},{"@id":"sustainability:wild_catch_fisheries_sustainable_exploitation_of_marine_resources_including_restoration","@type":["rdf:Property","owl:DatatypeProperty"],"rdfs:label":"wild_catch_fisheries_sustainable_exploitation_of_marine_resources_including_restoration","schema:rangeIncludes":{"@id":"xsd:boolean"},"schema:domainIncludes":{"@id":"sustainability:Biodiversity"},"rdfs:comment":"Does the standard promote the sustainable exploitation of marine resources including restoration of overfished and depleted stocks?"},{"@id":"sustainability:habitat_eco_system_restoration_rehabilitation","@type":["rdf:Property","owl:DatatypeProperty"],"rdfs:label":"habitat_eco_system_restoration_rehabilitation","schema:rangeIncludes":{"@id":"xsd:boolean"},"schema:domainIncludes":{"@id":"sustainability:Biodiversity"},"rdfs:comment":"Systems in place to identify, restore and rehabilitate natural habitats and/or ecosystems.Does the standard include biodiversity requirements specific to the restoration or rehabilitation of natural habitats and/or ecosystems?"},{"@id":"sustainability:impact_assessment_policy_for_new_production","@type":["rdf:Property","owl:DatatypeProperty"],"rdfs:label":"impact_assessment_policy_for_new_production","schema:rangeIncludes":{"@id":"xsd:boolean"},"schema:domainIncludes":{"@id":"sustainability:Biodiversity"},"rdfs:comment":"Procedures in place to assess potential impacts on biodiversity values prior to any significant intensification or expansion of cultivation or infrastructure. Does the standard require an impact assessment policy in place to assess potential impacts of new production (production land, processes, new crops…)?"},{"@id":"sustainability:requirements_for_net_positive_gain_in_biodiversity","@type":["rdf:Property","owl:DatatypeProperty"],"rdfs:label":"requirements_for_net_positive_gain_in_biodiversity","schema:rangeIncludes":{"@id":"xsd:boolean"},"schema:domainIncludes":{"@id":"sustainability:Biodiversity"},"rdfs:comment":"Does the standard include requirements for net positive gain in biodiversity?"},{"@id":"sustainability:protection_of_rare_and_threatened_species_and_their_habitats","@type":["rdf:Property","owl:DatatypeProperty"],"rdfs:label":"protection_of_rare_and_threatened_species_and_their_habitats","schema:rangeIncludes":{"@id":"xsd:boolean"},"schema:domainIncludes":{"@id":"sustainability:Biodiversity"},"rdfs:comment":"Does the standard include requirements for the protection of rare and threatened species and their habitats within the unit of operations?"},{"@id":"sustainability:requirements_for_no_net_loss_in_biodiversity","@type":["rdf:Property","owl:DatatypeProperty"],"rdfs:label":"requirements_for_no_net_loss_in_biodiversity","schema:rangeIncludes":{"@id":"xsd:boolean"},"schema:domainIncludes":{"@id":"sustainability:Biodiversity"},"rdfs:comment":"Does the standard require processes in place to ensure that production activities avoid net loss in biodiversity?"},{"@id":"sustainability:impact_mitigation_prior_to_production_harvesting_operations","@type":["rdf:Property","owl:DatatypeProperty"],"rdfs:label":"impact_mitigation_prior_to_production_harvesting_operations","schema:rangeIncludes":{"@id":"xsd:boolean"},"schema:domainIncludes":{"@id":"sustainability:Biodiversity"},"rdfs:comment":"Systems in place to mitigate negative environmental impacts prior to production and harvesting operations.Does the standard include criteria on mitigating negative environmental impacts prior to production/operation?"},{"@id":"sustainability:animals_livestock_general_principles","@type":["rdf:Property","owl:DatatypeProperty"],"rdfs:label":"animals_livestock_general_principles","schema:rangeIncludes":{"@id":"xsd:string"},"schema:domainIncludes":{"@id":"sustainability:Livestock"},"rdfs:comment":"General principle on livestock.Does the standard include a general principle on livestock?"},{"@id":"sustainability:general_animals_welfare","@type":["rdf:Property","owl:DatatypeProperty"],"rdfs:label":"general_animals_welfare","schema:rangeIncludes":{"@id":"xsd:boolean"},"schema:domainIncludes":{"@id":"sustainability:Livestock"},"rdfs:comment":"Does the standard include general criteria on animal welfare?"},{"@id":"sustainability:animal_testing","@type":["rdf:Property","owl:DatatypeProperty"],"rdfs:label":"animal_testing","schema:rangeIncludes":{"@id":"xsd:boolean"},"schema:domainIncludes":{"@id":"sustainability:Livestock"},"rdfs:comment":"Does the standard require processes to be in place to ensure animal testing is necessary and humane?"},{"@id":"sustainability:transport_of_animals","@type":["rdf:Property","owl:DatatypeProperty"],"rdfs:label":"transport_of_animals","schema:rangeIncludes":{"@id":"sustainability:TransportOfAnimals"},"schema:domainIncludes":{"@id":"sustainability:Livestock"},"rdfs:comment":"Does the standard include criteria on the welfare of animals during transport?"},{"@id":"sustainability:slaughter_slaughtering_process_minimum_age","@type":["rdf:Property","owl:DatatypeProperty"],"rdfs:label":"slaughter_slaughtering_process_minimum_age","schema:rangeIncludes":{"@id":"xsd:boolean"},"schema:domainIncludes":{"@id":"sustainability:Livestock"},"rdfs:comment":"Does the standard require procedures to be in place to ensure the consideration of animal welfare during slaughter?"},{"@id":"sustainability:the_use_of_electric_prods_with_livestock","@type":["rdf:Property","owl:DatatypeProperty"],"rdfs:label":"the_use_of_electric_prods_with_livestock","schema:rangeIncludes":{"@id":"sustainability:TheUseOfElectricProdsWithLivestock"},"schema:domainIncludes":{"@id":"sustainability:Livestock"},"rdfs:comment":"Does the standard require restrictions on, or the prohibition of, the use of electric prods when handling live animals?"},{"@id":"sustainability:techniques_to_be_used_for_animal_identification_and_or_castration","@type":["rdf:Property","owl:DatatypeProperty"],"rdfs:label":"techniques_to_be_used_for_animal_identification_and_or_castration","schema:rangeIncludes":{"@id":"sustainability:TechniquesToBeUsedForAnimalIdentificationAndOrCastration"},"schema:domainIncludes":{"@id":"sustainability:Livestock"},"rdfs:comment":"Does the standard include requirements on minimizing suffering during castration of live animals and/or live animal identification techniques?"},{"@id":"sustainability:animal_physical_integrity_eg_removing_of_tails_ears_nose_wings_horns_or_other_body_parts","@type":["rdf:Property","owl:DatatypeProperty"],"rdfs:label":"animal_physical_integrity_eg_removing_of_tails_ears_nose_wings_horns_or_other_body_parts","schema:rangeIncludes":{"@id":"sustainability:AnimalPhysicalIntegrityEgRemovingOfTailsEarsNoseWingsHornsOrOtherBodyParts"},"schema:domainIncludes":{"@id":"sustainability:Livestock"},"rdfs:comment":"Does the standard require restrictions or prohibitions on the removal of animal body parts?"},{"@id":"sustainability:litter_manure","@type":["rdf:Property","owl:DatatypeProperty"],"rdfs:label":"litter_manure","schema:rangeIncludes":{"@id":"xsd:boolean"},"schema:domainIncludes":{"@id":"sustainability:Livestock"},"rdfs:comment":"Does the standard include requirements related to the use of litter and manure?"},{"@id":"sustainability:livestock_density_following_at_least_official_regulations_e_g_ec_regulation8892008","@type":["rdf:Property","owl:DatatypeProperty"],"rdfs:label":"livestock_density_following_at_least_official_regulations_e_g_ec_regulation8892008","schema:rangeIncludes":{"@id":"sustainability:LivestockDensityFollowingAtLeastOfficialRegulationsEGEcRegulation8892008"},"schema:domainIncludes":{"@id":"sustainability:Livestock"},"rdfs:comment":"Does the standard include criteria on livestock density limits as defined in the EU Organic Farming Regulations?"},{"@id":"sustainability:outdoor_access_livestock","@type":["rdf:Property","owl:DatatypeProperty"],"rdfs:label":"outdoor_access_livestock","schema:rangeIncludes":{"@id":"sustainability:OutdoorAccessLivestock"},"schema:domainIncludes":{"@id":"sustainability:Livestock"},"rdfs:comment":"Does the standard require measures to support adequate outdoor access of livestock?"},{"@id":"sustainability:breeding","@type":["rdf:Property","owl:DatatypeProperty"],"rdfs:label":"breeding","schema:rangeIncludes":{"@id":"xsd:boolean"},"schema:domainIncludes":{"@id":"sustainability:Livestock"},"rdfs:comment":"Does the standard include criteria on animal breeding?"},{"@id":"sustainability:animal_housing","@type":["rdf:Property","owl:DatatypeProperty"],"rdfs:label":"animal_housing","schema:rangeIncludes":{"@id":"sustainability:AnimalHousing"},"schema:domainIncludes":{"@id":"sustainability:Livestock"},"rdfs:comment":"Does the standard include requirements on animal housing?"},{"@id":"sustainability:specific_beekeeping_interior_exterior_housing","@type":["rdf:Property","owl:DatatypeProperty"],"rdfs:label":"specific_beekeeping_interior_exterior_housing","schema:rangeIncludes":{"@id":"xsd:boolean"},"schema:domainIncludes":{"@id":"sustainability:Livestock"},"rdfs:comment":"Does the standard include requirements on interior and exterior housing for beekeeping?"},{"@id":"sustainability:specific_beekeeping_honey_extraction_process","@type":["rdf:Property","owl:DatatypeProperty"],"rdfs:label":"specific_beekeeping_honey_extraction_process","schema:rangeIncludes":{"@id":"xsd:boolean"},"schema:domainIncludes":{"@id":"sustainability:Livestock"},"rdfs:comment":"Does the standard include requirements on the honey extraction process?"},{"@id":"sustainability:specific_aquaculture_polyculture","@type":["rdf:Property","owl:DatatypeProperty"],"rdfs:label":"specific_aquaculture_polyculture","schema:rangeIncludes":{"@id":"xsd:boolean"},"schema:domainIncludes":{"@id":"sustainability:Livestock"},"rdfs:comment":"Does the standard promote polyculture on fish farms?"},{"@id":"sustainability:specific_aquaculture_analysis_of_water_quality","@type":["rdf:Property","owl:DatatypeProperty"],"rdfs:label":"specific_aquaculture_analysis_of_water_quality","schema:rangeIncludes":{"@id":"xsd:boolean"},"schema:domainIncludes":{"@id":"sustainability:Livestock"},"rdfs:comment":"Does the standard include requirements on the analysis of water quality in aquaculture?"},{"@id":"sustainability:specific_aquaculture_systems_in_place_to_minimize_the_unintentional_release_or_escape_of_farmed_species","@type":["rdf:Property","owl:DatatypeProperty"],"rdfs:label":"specific_aquaculture_systems_in_place_to_minimize_the_unintentional_release_or_escape_of_farmed_species","schema:rangeIncludes":{"@id":"xsd:boolean"},"schema:domainIncludes":{"@id":"sustainability:Livestock"},"rdfs:comment":"Does the standard include requirements on minimizing the unintentional release or escape of farmed species?"},{"@id":"sustainability:specific_aquaculture_use_of_hatchery_raised_seed","@type":["rdf:Property","owl:DatatypeProperty"],"rdfs:label":"specific_aquaculture_use_of_hatchery_raised_seed","schema:rangeIncludes":{"@id":"xsd:boolean"},"schema:domainIncludes":{"@id":"sustainability:Livestock"},"rdfs:comment":"Does the standard include criteria promoting the use of hatchery raised seed for fish farming?"},{"@id":"sustainability:specific_aquaculture_prohibition_of_prophylactic_use_of_antimicrobials","@type":["rdf:Property","owl:DatatypeProperty"],"rdfs:label":"specific_aquaculture_prohibition_of_prophylactic_use_of_antimicrobials","schema:rangeIncludes":{"@id":"xsd:boolean"},"schema:domainIncludes":{"@id":"sustainability:Livestock"},"rdfs:comment":"Prophylactic use of antimicrobials are prohibited and used only in response to diagnosed disease.Does the standard prohibit the prophylactic use of antimicrobials?"},{"@id":"sustainability:other_animals_treatment","@type":["rdf:Property","owl:DatatypeProperty"],"rdfs:label":"other_animals_treatment","schema:rangeIncludes":{"@id":"xsd:string"},"schema:domainIncludes":{"@id":"sustainability:Livestock"},"rdfs:comment":"Does the standard include other criteria related to live animals not addressed above"},{"@id":"sustainability:general_animals_feeding","@type":["rdf:Property","owl:DatatypeProperty"],"rdfs:label":"general_animals_feeding","schema:rangeIncludes":{"@id":"xsd:boolean"},"schema:domainIncludes":{"@id":"sustainability:Livestock"},"rdfs:comment":"Does the standard include requirements for appropriate animal feeding?"},{"@id":"sustainability:animal_feed_responsible_sourcing_policy","@type":["rdf:Property","owl:DatatypeProperty"],"rdfs:label":"animal_feed_responsible_sourcing_policy","schema:rangeIncludes":{"@id":"xsd:boolean"},"schema:domainIncludes":{"@id":"sustainability:Livestock"},"rdfs:comment":"Does the standard include a policy for responsible sourcing of animal feed?"},{"@id":"sustainability:specific_origin_of_animal_feed","@type":["rdf:Property","owl:DatatypeProperty"],"rdfs:label":"specific_origin_of_animal_feed","schema:rangeIncludes":{"@id":"sustainability:SpecificOriginOfAnimalFeed"},"schema:domainIncludes":{"@id":"sustainability:Livestock"},"rdfs:comment":"Does the standard include criteria on self-produced feed?"},{"@id":"sustainability:special_quality_of_animal_feed","@type":["rdf:Property","owl:DatatypeProperty"],"rdfs:label":"special_quality_of_animal_feed","schema:rangeIncludes":{"@id":"sustainability:SpecialQualityOfAnimalFeed"},"schema:domainIncludes":{"@id":"sustainability:Livestock"},"rdfs:comment":"Processes in place to ensure that the quality of animal feed meets the nutrients required for proper animal maintenance and production.Does the standard include criteria on quality of animal feed?"},{"@id":"sustainability:special_requirements_for_organic_animal_feed","@type":["rdf:Property","owl:DatatypeProperty"],"rdfs:label":"special_requirements_for_organic_animal_feed","schema:rangeIncludes":{"@id":"sustainability:SpecialRequirementsForOrganicAnimalFeed"},"schema:domainIncludes":{"@id":"sustainability:Livestock"},"rdfs:comment":"Does the standard include criteria on the use of organic feed?"},{"@id":"sustainability:animals_medication","@type":["rdf:Property","owl:DatatypeProperty"],"rdfs:label":"animals_medication","schema:rangeIncludes":{"@id":"sustainability:AnimalsMedication"},"schema:domainIncludes":{"@id":"sustainability:Livestock"},"rdfs:comment":"Processes and document procedures in place for the appropriate administration of allowable medication to animals.Does the standard include criteria on medication?"},{"@id":"sustainability:procedures_to_prevent_the_spread_of_animal_disease","@type":["rdf:Property","owl:DatatypeProperty"],"rdfs:label":"procedures_to_prevent_the_spread_of_animal_disease","schema:rangeIncludes":{"@id":"xsd:boolean"},"schema:domainIncludes":{"@id":"sustainability:Livestock"},"rdfs:comment":"Does the standard require establishment and implementation of procedures to prevent the spread of animal disease?"},{"@id":"sustainability:waste_management_general_principle","@type":["rdf:Property","owl:DatatypeProperty"],"rdfs:label":"waste_management_general_principle","schema:rangeIncludes":{"@id":"xsd:string"},"schema:domainIncludes":{"@id":"sustainability:Waste"},"rdfs:comment":"Does the standard include criteria on waste management in the production phase?"},{"@id":"sustainability:prevention_of_run_off_of_waste_chemicals_mineral_and_organic_substances","@type":["rdf:Property","owl:DatatypeProperty"],"rdfs:label":"prevention_of_run_off_of_waste_chemicals_mineral_and_organic_substances","schema:rangeIncludes":{"@id":"xsd:boolean"},"schema:domainIncludes":{"@id":"sustainability:Waste"},"rdfs:comment":"Does the standard require preventative measures to be in place to avoid run-off of waste chemicals, mineral and organic substances into watercourses?"},{"@id":"sustainability:air_quality_pollution_monitoring","@type":["rdf:Property","owl:DatatypeProperty"],"rdfs:label":"air_quality_pollution_monitoring","schema:rangeIncludes":{"@id":"sustainability:AirQualityPollutionMonitoring"},"schema:domainIncludes":{"@id":"sustainability:Waste"},"rdfs:comment":"Systems in place for the measurement, monitoring and reduction of emissions.Does the standard include criteria on air pollution?"},{"@id":"sustainability:air_pollution_along_the_textiles_production_process_ssct","@type":["rdf:Property","owl:DatatypeProperty"],"rdfs:label":"air_pollution_along_the_textiles_production_process_ssct","schema:rangeIncludes":{"@id":"sustainability:AirPollutionAlongTheTextilesProductionProcessSsct"},"schema:domainIncludes":{"@id":"sustainability:Waste"},"rdfs:comment":"For which production phase does the standard include criteria on air pollution?"},{"@id":"sustainability:s_and_nox_emissions_for_paper_industry_ssct","@type":["rdf:Property","owl:DatatypeProperty"],"rdfs:label":"s_and_nox_emissions_for_paper_industry_ssct","schema:rangeIncludes":{"@id":"xsd:boolean"},"schema:domainIncludes":{"@id":"sustainability:Waste"},"rdfs:comment":"Does the standard include criteria on threshold values of Sulphur (S) and NOx emissions to air?"},{"@id":"sustainability:pollution_incidents_mitigation_procedures_for_risks_monitoring_and_records_keeping","@type":["rdf:Property","owl:DatatypeProperty"],"rdfs:label":"pollution_incidents_mitigation_procedures_for_risks_monitoring_and_records_keeping","schema:rangeIncludes":{"@id":"xsd:boolean"},"schema:domainIncludes":{"@id":"sustainability:Waste"},"rdfs:comment":"Procedures in place for risks monitoring and records keeping of pollution incidents.Does the standard include criteria on specific procedures/controls to deal with pollution incidents (to mitigate environmental impacts)?"},{"@id":"sustainability:mitigation_of_transboundary_effects_of_air_pollution","@type":["rdf:Property","owl:DatatypeProperty"],"rdfs:label":"mitigation_of_transboundary_effects_of_air_pollution","schema:rangeIncludes":{"@id":"xsd:boolean"},"schema:domainIncludes":{"@id":"sustainability:Waste"},"rdfs:comment":"Does the standard require procedures to be in place to mitigate transboundary effects of air pollution?"},{"@id":"sustainability:noise_odour_and_other_pollution_nuisance","@type":["rdf:Property","owl:DatatypeProperty"],"rdfs:label":"noise_odour_and_other_pollution_nuisance","schema:rangeIncludes":{"@id":"xsd:boolean"},"schema:domainIncludes":{"@id":"sustainability:Waste"},"rdfs:comment":"Does the standard include criteria on monitoring and controlling noise, odour and other pollution nuisance?"},{"@id":"sustainability:principles_and_practices_related_to_composting","@type":["rdf:Property","owl:DatatypeProperty"],"rdfs:label":"principles_and_practices_related_to_composting","schema:rangeIncludes":{"@id":"xsd:boolean"},"schema:domainIncludes":{"@id":"sustainability:Waste"},"rdfs:comment":"Does the standard require biodegradation of organic matter waste (composting)?"},{"@id":"sustainability:principles_and_practices_related_to_tailings","@type":["rdf:Property","owl:DatatypeProperty"],"rdfs:label":"principles_and_practices_related_to_tailings","schema:rangeIncludes":{"@id":"xsd:boolean"},"schema:domainIncludes":{"@id":"sustainability:Waste"},"rdfs:comment":"Does the standard require safe treatment of tailings (e.g. isolated impoundments)?"},{"@id":"sustainability:principles_and_practices_related_to_packaging","@type":["rdf:Property","owl:DatatypeProperty"],"rdfs:label":"principles_and_practices_related_to_packaging","schema:rangeIncludes":{"@id":"xsd:boolean"},"schema:domainIncludes":{"@id":"sustainability:Waste"},"rdfs:comment":"Does the standard include criteria related to packaging of products in various segments of the value chain (e.g. environmental critical materials used for packaging)."},{"@id":"sustainability:waste_management_principles","@type":["rdf:Property","owl:DatatypeProperty"],"rdfs:label":"waste_management_principles","schema:rangeIncludes":{"@id":"xsd:boolean"},"schema:domainIncludes":{"@id":"sustainability:Waste"},"rdfs:comment":"Is there a general principle outlined in the standard that addresses waste management?"},{"@id":"sustainability:waste_disposal_incl_solid_waste_non_solid_waste_excl_hazardous_waste","@type":["rdf:Property","owl:DatatypeProperty"],"rdfs:label":"waste_disposal_incl_solid_waste_non_solid_waste_excl_hazardous_waste","schema:rangeIncludes":{"@id":"xsd:boolean"},"schema:domainIncludes":{"@id":"sustainability:Waste"},"rdfs:comment":"Does the standard include criteria related to the proper disposal of waste (incl. solid waste, non-solid waste, excl. hazardous waste)?"},{"@id":"sustainability:specific_disposal_of_hazardous_waste","@type":["rdf:Property","owl:DatatypeProperty"],"rdfs:label":"specific_disposal_of_hazardous_waste","schema:rangeIncludes":{"@id":"xsd:boolean"},"schema:domainIncludes":{"@id":"sustainability:Waste"},"rdfs:comment":"Does the standard include criteria on safe disposal of hazardous waste?"},{"@id":"sustainability:specific_requirements_for_handling_disposal_of_waste_by_third_parties","@type":["rdf:Property","owl:DatatypeProperty"],"rdfs:label":"specific_requirements_for_handling_disposal_of_waste_by_third_parties","schema:rangeIncludes":{"@id":"sustainability:SpecificRequirementsForHandlingDisposalOfWasteByThirdParties"},"schema:domainIncludes":{"@id":"sustainability:Waste"},"rdfs:comment":"Does the standard include criteria on handling or disposal of waste by third parties?"},{"@id":"sustainability:practices_related_to_the_use_of_fire_to_eliminate_waste","@type":["rdf:Property","owl:DatatypeProperty"],"rdfs:label":"practices_related_to_the_use_of_fire_to_eliminate_waste","schema:rangeIncludes":{"@id":"sustainability:PracticesRelatedToTheUseOfFireToEliminateWaste"},"schema:domainIncludes":{"@id":"sustainability:Waste"},"rdfs:comment":"Does the standard include criteria on the restiction or prohibition of uncontrolled on-site waste burning?"},{"@id":"sustainability:principles_and_practices_related_to_avoidance_of_uncontrolled_waste_landfilling","@type":["rdf:Property","owl:DatatypeProperty"],"rdfs:label":"principles_and_practices_related_to_avoidance_of_uncontrolled_waste_landfilling","schema:rangeIncludes":{"@id":"sustainability:PrinciplesAndPracticesRelatedToAvoidanceOfUncontrolledWasteLandfilling"},"schema:domainIncludes":{"@id":"sustainability:Waste"},"rdfs:comment":"Does the standard include criteria on uncontrolled waste landfilling?"},{"@id":"sustainability:other_waste_management","@type":["rdf:Property","owl:DatatypeProperty"],"rdfs:label":"other_waste_management","schema:rangeIncludes":{"@id":"xsd:boolean"},"schema:domainIncludes":{"@id":"sustainability:Waste"},"rdfs:comment":"Does the standard include other criteria related to waste management not addressed above?"},{"@id":"sustainability:environmental_friendly_purchasing_policy","@type":["rdf:Property","owl:DatatypeProperty"],"rdfs:label":"environmental_friendly_purchasing_policy","schema:rangeIncludes":{"@id":"xsd:boolean"},"schema:domainIncludes":{"@id":"sustainability:Waste"},"rdfs:comment":"Does the standard require an environmental friendly purchasing policy?"},{"@id":"sustainability:disposables_measured_reduced","@type":["rdf:Property","owl:DatatypeProperty"],"rdfs:label":"disposables_measured_reduced","schema:rangeIncludes":{"@id":"xsd:boolean"},"schema:domainIncludes":{"@id":"sustainability:Waste"},"rdfs:comment":"Does the standard require the monitoring, measurement and reduction of disposable products?"},{"@id":"sustainability:disposal_of_the_product_ssct_paper_specific","@type":["rdf:Property","owl:DatatypeProperty"],"rdfs:label":"disposal_of_the_product_ssct_paper_specific","schema:rangeIncludes":{"@id":"xsd:boolean"},"schema:domainIncludes":{"@id":"sustainability:Waste"},"rdfs:comment":"Does the standard include criteria on the provision of consumer information on product disposal?"},{"@id":"sustainability:treatment_and_use_of_solid_waste","@type":["rdf:Property","owl:DatatypeProperty"],"rdfs:label":"treatment_and_use_of_solid_waste","schema:rangeIncludes":{"@id":"xsd:boolean"},"schema:domainIncludes":{"@id":"sustainability:Waste"},"rdfs:comment":"Does the standard include criteria on solid waste management?"},{"@id":"sustainability:monitoring_and_measuring_solid_waste_volumes","@type":["rdf:Property","owl:DatatypeProperty"],"rdfs:label":"monitoring_and_measuring_solid_waste_volumes","schema:rangeIncludes":{"@id":"sustainability:MonitoringAndMeasuringSolidWasteVolumes"},"schema:domainIncludes":{"@id":"sustainability:Waste"},"rdfs:comment":"Does the standard include criteria on volumes of waste?"},{"@id":"sustainability:reducing_solid_waste_volumes","@type":["rdf:Property","owl:DatatypeProperty"],"rdfs:label":"reducing_solid_waste_volumes","schema:rangeIncludes":{"@id":"xsd:boolean"},"schema:domainIncludes":{"@id":"sustainability:Waste"},"rdfs:comment":"Does the standard require reductions on volumes of solid waste produced?"},{"@id":"sustainability:monitoring_and_measuring_waste_toxicity","@type":["rdf:Property","owl:DatatypeProperty"],"rdfs:label":"monitoring_and_measuring_waste_toxicity","schema:rangeIncludes":{"@id":"sustainability:MonitoringAndMeasuringWasteToxicity"},"schema:domainIncludes":{"@id":"sustainability:Waste"},"rdfs:comment":"Does the standard include criteria on the management of toxicity of waste?"},{"@id":"sustainability:reducing_re_use_recycle_solid_waste","@type":["rdf:Property","owl:DatatypeProperty"],"rdfs:label":"reducing_re_use_recycle_solid_waste","schema:rangeIncludes":{"@id":"xsd:boolean"},"schema:domainIncludes":{"@id":"sustainability:Waste"},"rdfs:comment":"Does the standard include criteria on re-using or recycling waste on-site?"},{"@id":"sustainability:treatment_and_use_of_non_solid_waste","@type":["rdf:Property","owl:DatatypeProperty"],"rdfs:label":"treatment_and_use_of_non_solid_waste","schema:rangeIncludes":{"@id":"xsd:boolean"},"schema:domainIncludes":{"@id":"sustainability:Waste"},"rdfs:comment":"Does the standard have requirements on the treatment and use of non-solid waste?"},{"@id":"sustainability:waste_segregation","@type":["rdf:Property","owl:DatatypeProperty"],"rdfs:label":"waste_segregation","schema:rangeIncludes":{"@id":"xsd:boolean"},"schema:domainIncludes":{"@id":"sustainability:Waste"},"rdfs:comment":"Processes in place for the segregation of different waste streams generated from operations.Does the standard include criteria on waste segregation?"},{"@id":"sustainability:water_resources_monitoring_use_and_consumption","@type":["rdf:Property","owl:DatatypeProperty"],"rdfs:label":"water_resources_monitoring_use_and_consumption","schema:rangeIncludes":{"@id":"sustainability:WaterResourcesMonitoringUseAndConsumption"},"schema:domainIncludes":{"@id":"sustainability:Water"},"rdfs:comment":"Does the standard include criteria on water consumption management?"},{"@id":"sustainability:surface_and_ground_water_contamination_pollution","@type":["rdf:Property","owl:DatatypeProperty"],"rdfs:label":"surface_and_ground_water_contamination_pollution","schema:rangeIncludes":{"@id":"xsd:boolean"},"schema:domainIncludes":{"@id":"sustainability:Water"},"rdfs:comment":"Does the standard include criteria on the prevention of surface and ground water contamination/pollution?"},{"@id":"sustainability:mitigation_of_transboundary_effects_of_water_pollution","@type":["rdf:Property","owl:DatatypeProperty"],"rdfs:label":"mitigation_of_transboundary_effects_of_water_pollution","schema:rangeIncludes":{"@id":"xsd:boolean"},"schema:domainIncludes":{"@id":"sustainability:Water"},"rdfs:comment":"Does the standard include requirements to mitigate the transboundary effects of water pollution"},{"@id":"sustainability:quality_of_water_used_in_production_agriculture_forestry","@type":["rdf:Property","owl:DatatypeProperty"],"rdfs:label":"quality_of_water_used_in_production_agriculture_forestry","schema:rangeIncludes":{"@id":"sustainability:QualityOfWaterUsedInProductionAgricultureForestry"},"schema:domainIncludes":{"@id":"sustainability:Water"},"rdfs:comment":"Does the standard include criteria on quality of input water used for production (agriculture, forestry)?"},{"@id":"sustainability:principles_and_practices_related_to_water_disposal_storage","@type":["rdf:Property","owl:DatatypeProperty"],"rdfs:label":"principles_and_practices_related_to_water_disposal_storage","schema:rangeIncludes":{"@id":"xsd:boolean"},"schema:domainIncludes":{"@id":"sustainability:Water"},"rdfs:comment":"Does the standard include criteria on proper disposal and storage of grey waters?"},{"@id":"sustainability:water_extraction_irrigation","@type":["rdf:Property","owl:DatatypeProperty"],"rdfs:label":"water_extraction_irrigation","schema:rangeIncludes":{"@id":"xsd:boolean"},"schema:domainIncludes":{"@id":"sustainability:Water"},"rdfs:comment":"Does the standard include requirements on groundwater extraction and irrigation efficiency?"},{"@id":"sustainability:natural_wetlands_are_maintained_in_undrained_conditions","@type":["rdf:Property","owl:DatatypeProperty"],"rdfs:label":"natural_wetlands_are_maintained_in_undrained_conditions","schema:rangeIncludes":{"@id":"xsd:boolean"},"schema:domainIncludes":{"@id":"sustainability:Water"},"rdfs:comment":"Does the standard include requirements on maintaining wetlands in undrained conditions?"},{"@id":"sustainability:water_usage_records_keeping","@type":["rdf:Property","owl:DatatypeProperty"],"rdfs:label":"water_usage_records_keeping","schema:rangeIncludes":{"@id":"xsd:boolean"},"schema:domainIncludes":{"@id":"sustainability:Water"},"rdfs:comment":"Does the standard include requirements on maintaining records on the amount of water used?"},{"@id":"sustainability:other_water","@type":["rdf:Property","owl:DatatypeProperty"],"rdfs:label":"other_water","schema:rangeIncludes":{"@id":"xsd:string"},"schema:domainIncludes":{"@id":"sustainability:Water"},"rdfs:comment":"Does the standard include other requirements related to water not covered above?"},{"@id":"sustainability:water_management_plan","@type":["rdf:Property","owl:DatatypeProperty"],"rdfs:label":"water_management_plan","schema:rangeIncludes":{"@id":"xsd:boolean"},"schema:domainIncludes":{"@id":"sustainability:Water"},"rdfs:comment":"Does the standard require a management plan for water use and quality?"},{"@id":"sustainability:water_dependencies_and_water_scarcity","@type":["rdf:Property","owl:DatatypeProperty"],"rdfs:label":"water_dependencies_and_water_scarcity","schema:rangeIncludes":{"@id":"xsd:boolean"},"schema:domainIncludes":{"@id":"sustainability:Water"},"rdfs:comment":"Does the standard include requirements on water use in areas of scarcity or high risk?"},{"@id":"sustainability:water_reuse_recycling_and_harvesting","@type":["rdf:Property","owl:DatatypeProperty"],"rdfs:label":"water_reuse_recycling_and_harvesting","schema:rangeIncludes":{"@id":"xsd:boolean"},"schema:domainIncludes":{"@id":"sustainability:Water"},"rdfs:comment":"Does the standard include criteria on reusing/recycling or harvesting water to reduce water use?"},{"@id":"sustainability:wastewater_quality_management_and_treatment","@type":["rdf:Property","owl:DatatypeProperty"],"rdfs:label":"wastewater_quality_management_and_treatment","schema:rangeIncludes":{"@id":"sustainability:WastewaterQualityManagementAndTreatment"},"schema:domainIncludes":{"@id":"sustainability:Water"},"rdfs:comment":"Does the standard include criteria on wastewater quality management and treatment?"},{"@id":"sustainability:limitations_of_wastewater_volume","@type":["rdf:Property","owl:DatatypeProperty"],"rdfs:label":"limitations_of_wastewater_volume","schema:rangeIncludes":{"@id":"sustainability:LimitationsOfWastewaterVolume"},"schema:domainIncludes":{"@id":"sustainability:Water"},"rdfs:comment":"Does the standard include criteria on limitations of wastewater volumes?"},{"@id":"sustainability:wastewater_basic_parameters_for_textile_industry","@type":["rdf:Property","owl:DatatypeProperty"],"rdfs:label":"wastewater_basic_parameters_for_textile_industry","schema:rangeIncludes":{"@id":"sustainability:WastewaterBasicParametersForTextileIndustry"},"schema:domainIncludes":{"@id":"sustainability:Water"},"rdfs:comment":"Does the standard include threshold values on wastewater parameters of COD, pH, temperature?"},{"@id":"sustainability:wastewater_advanced_parameters_for_textile_industry","@type":["rdf:Property","owl:DatatypeProperty"],"rdfs:label":"wastewater_advanced_parameters_for_textile_industry","schema:rangeIncludes":{"@id":"sustainability:WastewaterAdvancedParametersForTextileIndustry"},"schema:domainIncludes":{"@id":"sustainability:Water"},"rdfs:comment":"Does the standard require threshold values on wastewater parameters of BOD, AOX, N, P, sulphite, ammonium nitrogen and chrome, copper, nickel, zinc, tin?"},{"@id":"sustainability:wastewater_parameters_for_paper_industry","@type":["rdf:Property","owl:DatatypeProperty"],"rdfs:label":"wastewater_parameters_for_paper_industry","schema:rangeIncludes":{"@id":"sustainability:WastewaterParametersForPaperIndustry"},"schema:domainIncludes":{"@id":"sustainability:Water"},"rdfs:comment":"Does the standard require threshold values on wastewater parameters of COD and P?"},{"@id":"sustainability:energy_consumption_monitoring_recording","@type":["rdf:Property","owl:DatatypeProperty"],"rdfs:label":"energy_consumption_monitoring_recording","schema:rangeIncludes":{"@id":"sustainability:EnergyConsumptionMonitoringRecording"},"schema:domainIncludes":{"@id":"sustainability:Energy"},"rdfs:comment":"Does the standard include criteria on energy consumption in the production phase?"},{"@id":"sustainability:use_of_biofuels","@type":["rdf:Property","owl:DatatypeProperty"],"rdfs:label":"use_of_biofuels","schema:rangeIncludes":{"@id":"xsd:boolean"},"schema:domainIncludes":{"@id":"sustainability:Energy"},"rdfs:comment":"Does the standard include criteria on the use of biofuels for energy use in operational practices?"},{"@id":"sustainability:use_of_non_renewable_energies","@type":["rdf:Property","owl:DatatypeProperty"],"rdfs:label":"use_of_non_renewable_energies","schema:rangeIncludes":{"@id":"xsd:boolean"},"schema:domainIncludes":{"@id":"sustainability:Energy"},"rdfs:comment":"Does the standard include requirements for the reduction in use of non-renewable energies in production practices?"},{"@id":"sustainability:use_of_non_renewable_energies_general_principle","@type":["rdf:Property","owl:DatatypeProperty"],"rdfs:label":"use_of_non_renewable_energies_general_principle","schema:rangeIncludes":{"@id":"xsd:boolean"},"schema:domainIncludes":{"@id":"sustainability:Energy"},"rdfs:comment":"Does the standard include a general principle on the use of non-renewable energies?"},{"@id":"sustainability:other_energy_consumption_and_management","@type":["rdf:Property","owl:DatatypeProperty"],"rdfs:label":"other_energy_consumption_and_management","schema:rangeIncludes":{"@id":"xsd:string"},"schema:domainIncludes":{"@id":"sustainability:Energy"},"rdfs:comment":"Does the standard include additional criteria on energy consumption and management not addressed above?"},{"@id":"sustainability:the_application_of_a_set_of_clean_production_practices","@type":["rdf:Property","owl:DatatypeProperty"],"rdfs:label":"the_application_of_a_set_of_clean_production_practices","schema:rangeIncludes":{"@id":"xsd:boolean"},"schema:domainIncludes":{"@id":"sustainability:Energy"},"rdfs:comment":"Does the standard include requirements on the application of a set of clean production practices?"},{"@id":"sustainability:criteria_to_reduce_use_of_energy_resources","@type":["rdf:Property","owl:DatatypeProperty"],"rdfs:label":"criteria_to_reduce_use_of_energy_resources","schema:rangeIncludes":{"@id":"xsd:boolean"},"schema:domainIncludes":{"@id":"sustainability:Energy"},"rdfs:comment":"Does the standard include requirements related to the reduction in use of energy resources?"},{"@id":"sustainability:storage_of_energy_incl_fuel_electricity","@type":["rdf:Property","owl:DatatypeProperty"],"rdfs:label":"storage_of_energy_incl_fuel_electricity","schema:rangeIncludes":{"@id":"xsd:boolean"},"schema:domainIncludes":{"@id":"sustainability:Energy"},"rdfs:comment":"Does the standard include requirements related to storage of energy (incl. fuel and electricity)?"},{"@id":"sustainability:use_of_alternative_energies_including_solar_wind_etc","@type":["rdf:Property","owl:DatatypeProperty"],"rdfs:label":"use_of_alternative_energies_including_solar_wind_etc","schema:rangeIncludes":{"@id":"xsd:boolean"},"schema:domainIncludes":{"@id":"sustainability:Energy"},"rdfs:comment":"Does the standard include a general principle on renewable energy usage?"},{"@id":"sustainability:use_of_solar_energy","@type":["rdf:Property","owl:DatatypeProperty"],"rdfs:label":"use_of_solar_energy","schema:rangeIncludes":{"@id":"xsd:boolean"},"schema:domainIncludes":{"@id":"sustainability:Energy"},"rdfs:comment":"Does the standard include criteria on the use of solar energy?"},{"@id":"sustainability:use_of_hydropower_energy","@type":["rdf:Property","owl:DatatypeProperty"],"rdfs:label":"use_of_hydropower_energy","schema:rangeIncludes":{"@id":"xsd:boolean"},"schema:domainIncludes":{"@id":"sustainability:Energy"},"rdfs:comment":"Does the standard include criteria on the use of hydropower energy?"},{"@id":"sustainability:use_of_wind_energy","@type":["rdf:Property","owl:DatatypeProperty"],"rdfs:label":"use_of_wind_energy","schema:rangeIncludes":{"@id":"xsd:boolean"},"schema:domainIncludes":{"@id":"sustainability:Energy"},"rdfs:comment":"Does the standard include criteria on the use of wind energy in production practices?"},{"@id":"sustainability:use_of_wood_based_energy","@type":["rdf:Property","owl:DatatypeProperty"],"rdfs:label":"use_of_wood_based_energy","schema:rangeIncludes":{"@id":"xsd:boolean"},"schema:domainIncludes":{"@id":"sustainability:Energy"},"rdfs:comment":"Does the standard include criteria on the use of wood-based energy?"},{"@id":"sustainability:carbon_policies_general_principle","@type":["rdf:Property","owl:DatatypeProperty"],"rdfs:label":"carbon_policies_general_principle","schema:rangeIncludes":{"@id":"xsd:string"},"schema:domainIncludes":{"@id":"sustainability:ClimateCarbon"},"rdfs:comment":"General principle on carbon policies.Does the standard include a general principle on carbon policies?"},{"@id":"sustainability:the_protection_of_high_carbon_landscapes_land_with_high_carbon_stock_hcs","@type":["rdf:Property","owl:DatatypeProperty"],"rdfs:label":"the_protection_of_high_carbon_landscapes_land_with_high_carbon_stock_hcs","schema:rangeIncludes":{"@id":"sustainability:TheProtectionOfHighCarbonLandscapesLandWithHighCarbonStockHcs"},"schema:domainIncludes":{"@id":"sustainability:ClimateCarbon"},"rdfs:comment":"Does the standard include criteria on high carbon landscapes (above and/or below ground carbon stocks)?"},{"@id":"sustainability:using_offsets","@type":["rdf:Property","owl:DatatypeProperty"],"rdfs:label":"using_offsets","schema:rangeIncludes":{"@id":"xsd:boolean"},"schema:domainIncludes":{"@id":"sustainability:ClimateCarbon"},"rdfs:comment":"Does the standard include requirements for the purchase of carbon offsets?"},{"@id":"sustainability:specific_climate_adaptation_activities","@type":["rdf:Property","owl:DatatypeProperty"],"rdfs:label":"specific_climate_adaptation_activities","schema:rangeIncludes":{"@id":"xsd:boolean"},"schema:domainIncludes":{"@id":"sustainability:ClimateCarbon"},"rdfs:comment":"Does the standard include criteria on specific climate adaptation activities?"},{"@id":"sustainability:carbon_neutrality","@type":["rdf:Property","owl:DatatypeProperty"],"rdfs:label":"carbon_neutrality","schema:rangeIncludes":{"@id":"xsd:boolean"},"schema:domainIncludes":{"@id":"sustainability:ClimateCarbon"},"rdfs:comment":"Does the standard require implementation of a \"Carbon neutrality\" objective in operation activities?"},{"@id":"sustainability:carbon_standards_specific_offset_externalities","@type":["rdf:Property","owl:DatatypeProperty"],"rdfs:label":"carbon_standards_specific_offset_externalities","schema:rangeIncludes":{"@id":"xsd:boolean"},"schema:domainIncludes":{"@id":"sustainability:ClimateCarbon"},"rdfs:comment":"Does the standard include requirements regarding offset externalities linked to carbon offsets?"},{"@id":"sustainability:carbon_standards_specific_additionality_tests","@type":["rdf:Property","owl:DatatypeProperty"],"rdfs:label":"carbon_standards_specific_additionality_tests","schema:rangeIncludes":{"@id":"xsd:boolean"},"schema:domainIncludes":{"@id":"sustainability:ClimateCarbon"},"rdfs:comment":"Does the standard include requirements regarding additionality tests?"},{"@id":"sustainability:carbon_standards_specific_registry_of_carbon_project","@type":["rdf:Property","owl:DatatypeProperty"],"rdfs:label":"carbon_standards_specific_registry_of_carbon_project","schema:rangeIncludes":{"@id":"xsd:boolean"},"schema:domainIncludes":{"@id":"sustainability:ClimateCarbon"},"rdfs:comment":"Does the standard include explicit requirements regarding the carbon offset registry?"},{"@id":"sustainability:carbon_standards_specific_type_of_project","@type":["rdf:Property","owl:DatatypeProperty"],"rdfs:label":"carbon_standards_specific_type_of_project","schema:rangeIncludes":{"@id":"xsd:boolean"},"schema:domainIncludes":{"@id":"sustainability:ClimateCarbon"},"rdfs:comment":"Does the standard include explicit requirements regarding the project types which may be part of carbon offsets?"},{"@id":"sustainability:carbon_standards_specific_crediting_periods","@type":["rdf:Property","owl:DatatypeProperty"],"rdfs:label":"carbon_standards_specific_crediting_periods","schema:rangeIncludes":{"@id":"xsd:boolean"},"schema:domainIncludes":{"@id":"sustainability:ClimateCarbon"},"rdfs:comment":"Does the standard include explicit requirements regarding the crediting period of the carbon offsets?"},{"@id":"sustainability:other_carbon_policies_and_management","@type":["rdf:Property","owl:DatatypeProperty"],"rdfs:label":"other_carbon_policies_and_management","schema:rangeIncludes":{"@id":"xsd:string"},"schema:domainIncludes":{"@id":"sustainability:ClimateCarbon"},"rdfs:comment":"Does the standard include additional criteria on carbon policies and management not addressed in above criteria?"},{"@id":"sustainability:monitoring_ghg_carbon_emissions","@type":["rdf:Property","owl:DatatypeProperty"],"rdfs:label":"monitoring_ghg_carbon_emissions","schema:rangeIncludes":{"@id":"sustainability:MonitoringGhgCarbonEmissions"},"schema:domainIncludes":{"@id":"sustainability:ClimateCarbon"},"rdfs:comment":"Does the standard include criteria on (non-energy) greenhouse gas emissions?"},{"@id":"sustainability:requirements_to_perform_analysis_of_possible_alternatives_to_reduce_ghg_emissions","@type":["rdf:Property","owl:DatatypeProperty"],"rdfs:label":"requirements_to_perform_analysis_of_possible_alternatives_to_reduce_ghg_emissions","schema:rangeIncludes":{"@id":"xsd:boolean"},"schema:domainIncludes":{"@id":"sustainability:ClimateCarbon"},"rdfs:comment":"Does the standard include requirements for analyses of alternative operation methods aimed at reducing GHG emissions?"},{"@id":"sustainability:requirements_to_quantify_ghg_emissions","@type":["rdf:Property","owl:DatatypeProperty"],"rdfs:label":"requirements_to_quantify_ghg_emissions","schema:rangeIncludes":{"@id":"xsd:boolean"},"schema:domainIncludes":{"@id":"sustainability:ClimateCarbon"},"rdfs:comment":"Does the standard include requirements to quantify GHG emissions?"},{"@id":"sustainability:reducing_ghg_emissions","@type":["rdf:Property","owl:DatatypeProperty"],"rdfs:label":"reducing_ghg_emissions","schema:rangeIncludes":{"@id":"xsd:boolean"},"schema:domainIncludes":{"@id":"sustainability:ClimateCarbon"},"rdfs:comment":"Does the standard include requirements for the reduction of GHG emissions?"},{"@id":"sustainability:sequestration_of_green_house_gases","@type":["rdf:Property","owl:DatatypeProperty"],"rdfs:label":"sequestration_of_green_house_gases","schema:rangeIncludes":{"@id":"xsd:boolean"},"schema:domainIncludes":{"@id":"sustainability:ClimateCarbon"},"rdfs:comment":"Does the standard include specific requirements for the sequestration of green-house gases?"},{"@id":"sustainability:sequestration_of_green_house_gases_general_principle","@type":["rdf:Property","owl:DatatypeProperty"],"rdfs:label":"sequestration_of_green_house_gases_general_principle","schema:rangeIncludes":{"@id":"xsd:boolean"},"schema:domainIncludes":{"@id":"sustainability:ClimateCarbon"},"rdfs:comment":"Does the standard include a general principle on the sequestration of green-house gases?"},{"@id":"sustainability:soil_or_trees_sequestration","@type":["rdf:Property","owl:DatatypeProperty"],"rdfs:label":"soil_or_trees_sequestration","schema:rangeIncludes":{"@id":"xsd:boolean"},"schema:domainIncludes":{"@id":"sustainability:ClimateCarbon"},"rdfs:comment":"Does the standard include requirements for soil or tree sequestration of green-house gases?"},{"@id":"sustainability:high_carbon_stock_areas_monitoring_and_management","@type":["rdf:Property","owl:DatatypeProperty"],"rdfs:label":"high_carbon_stock_areas_monitoring_and_management","schema:rangeIncludes":{"@id":"xsd:boolean"},"schema:domainIncludes":{"@id":"sustainability:ClimateCarbon"},"rdfs:comment":"Does the standard include requirements for the monitoring and management of High Carbon Stock areas?"},{"@id":"sustainability:the_use_of_synthetic_pesticides","@type":["rdf:Property","owl:DatatypeProperty"],"rdfs:label":"the_use_of_synthetic_pesticides","schema:rangeIncludes":{"@id":"sustainability:TheUseOfSyntheticPesticides"},"schema:domainIncludes":{"@id":"sustainability:SsctAndOther"},"rdfs:comment":"Does the standard include criteria on synthetic pesticides?"},{"@id":"sustainability:the_use_of_chlorine_gas_as_bleaching_agent","@type":["rdf:Property","owl:DatatypeProperty"],"rdfs:label":"the_use_of_chlorine_gas_as_bleaching_agent","schema:rangeIncludes":{"@id":"sustainability:TheUseOfChlorineGasAsBleachingAgent"},"schema:domainIncludes":{"@id":"sustainability:SsctAndOther"},"rdfs:comment":"Does the standard include criteria on the use of chlorine gas, elemental chlorine, chloroorganic compounds as bleaching agent?"},{"@id":"sustainability:chemicals_described_as_a_risk_to_the_environment","@type":["rdf:Property","owl:DatatypeProperty"],"rdfs:label":"chemicals_described_as_a_risk_to_the_environment","schema:rangeIncludes":{"@id":"sustainability:ChemicalsDescribedAsARiskToTheEnvironment"},"schema:domainIncludes":{"@id":"sustainability:SsctAndOther"},"rdfs:comment":"Does the standard include criteria on H statements H400, H410, H411?"},{"@id":"sustainability:chemicals_described_as_a_risk_to_human_health","@type":["rdf:Property","owl:DatatypeProperty"],"rdfs:label":"chemicals_described_as_a_risk_to_human_health","schema:rangeIncludes":{"@id":"sustainability:ChemicalsDescribedAsARiskToHumanHealth"},"schema:domainIncludes":{"@id":"sustainability:SsctAndOther"},"rdfs:comment":"Does the standard include criteria on H statements H300, H310, H330, H340, H341, H350, H351, H360, H361, H370, H371?"},{"@id":"sustainability:testing_the_final_product_regarding_accumulation_of_chemical_residues","@type":["rdf:Property","owl:DatatypeProperty"],"rdfs:label":"testing_the_final_product_regarding_accumulation_of_chemical_residues","schema:rangeIncludes":{"@id":"sustainability:TestingTheFinalProductRegardingAccumulationOfChemicalResidues"},"schema:domainIncludes":{"@id":"sustainability:SsctAndOther"},"rdfs:comment":"Does the standard include criteria on testing the final product regarding residues of chemicals?"},{"@id":"sustainability:biological_control_to_prevent_or_suppress_harmful_organisms","@type":["rdf:Property","owl:DatatypeProperty"],"rdfs:label":"biological_control_to_prevent_or_suppress_harmful_organisms","schema:rangeIncludes":{"@id":"xsd:boolean"},"schema:domainIncludes":{"@id":"sustainability:SsctAndOther"},"rdfs:comment":"Does the standard include criteria on biological control to prevent or suppress harmful organisms?"},{"@id":"sustainability:the_monitoring_harmful_organisms_by_observations_in_the_field","@type":["rdf:Property","owl:DatatypeProperty"],"rdfs:label":"the_monitoring_harmful_organisms_by_observations_in_the_field","schema:rangeIncludes":{"@id":"xsd:boolean"},"schema:domainIncludes":{"@id":"sustainability:SsctAndOther"},"rdfs:comment":"Does the standard include criteria on regularly monitoring harmful organisms by observations in the field or warning, forecasting and early diagnosis systems (e.g. traps)"},{"@id":"sustainability:the_principle_to_use_pesticides_as_last_resort_only","@type":["rdf:Property","owl:DatatypeProperty"],"rdfs:label":"the_principle_to_use_pesticides_as_last_resort_only","schema:rangeIncludes":{"@id":"xsd:boolean"},"schema:domainIncludes":{"@id":"sustainability:SsctAndOther"},"rdfs:comment":"Does the standard include criteria on the principle to use pesticides as last resort only?"},{"@id":"sustainability:the_production_of_natural_fibres","@type":["rdf:Property","owl:DatatypeProperty"],"rdfs:label":"the_production_of_natural_fibres","schema:rangeIncludes":{"@id":"sustainability:TheProductionOfNaturalFibres"},"schema:domainIncludes":{"@id":"sustainability:SsctAndOther"},"rdfs:comment":"Does the standard include criteria on the production of natural fibres?"},{"@id":"sustainability:the_production_of_synthetic_fibers","@type":["rdf:Property","owl:DatatypeProperty"],"rdfs:label":"the_production_of_synthetic_fibers","schema:rangeIncludes":{"@id":"sustainability:TheProductionOfSyntheticFibers"},"schema:domainIncludes":{"@id":"sustainability:SsctAndOther"},"rdfs:comment":"Does the standard include criteria on the production of synthetic fibers?"},{"@id":"sustainability:the_usage_of_recycled_fibres","@type":["rdf:Property","owl:DatatypeProperty"],"rdfs:label":"the_usage_of_recycled_fibres","schema:rangeIncludes":{"@id":"sustainability:TheUsageOfRecycledFibres"},"schema:domainIncludes":{"@id":"sustainability:SsctAndOther"},"rdfs:comment":"Does the standard include criteria on the usage of recycled material?"},{"@id":"sustainability:on_synthetic_fertilizers","@type":["rdf:Property","owl:DatatypeProperty"],"rdfs:label":"on_synthetic_fertilizers","schema:rangeIncludes":{"@id":"sustainability:OnSyntheticFertilizers"},"schema:domainIncludes":{"@id":"sustainability:SsctAndOther"},"rdfs:comment":"Does the standard include criteria on synthetic fertilizers?"},{"@id":"sustainability:the_use_of_wooden_fibres","@type":["rdf:Property","owl:DatatypeProperty"],"rdfs:label":"the_use_of_wooden_fibres","schema:rangeIncludes":{"@id":"sustainability:TheUseOfWoodenFibres"},"schema:domainIncludes":{"@id":"sustainability:SsctAndOther"},"rdfs:comment":"Does the standard include criteria on the use of wooden fibres?"},{"@id":"sustainability:energy_consumption_in_the_production_phase","@type":["rdf:Property","owl:DatatypeProperty"],"rdfs:label":"energy_consumption_in_the_production_phase","schema:rangeIncludes":{"@id":"sustainability:EnergyConsumptionInTheProductionPhase"},"schema:domainIncludes":{"@id":"sustainability:SsctAndOther"},"rdfs:comment":"Does the standard include criteria on energy consumption in the production phase?"},{"@id":"sustainability:the_usage_of_renewable_energy_in_the_production_phase_of_the_hardware","@type":["rdf:Property","owl:DatatypeProperty"],"rdfs:label":"the_usage_of_renewable_energy_in_the_production_phase_of_the_hardware","schema:rangeIncludes":{"@id":"sustainability:TheUsageOfRenewableEnergyInTheProductionPhaseOfTheHardware"},"schema:domainIncludes":{"@id":"sustainability:SsctAndOther"},"rdfs:comment":"Does the standard include criteria on the usage of renewable energy in the production phase of the hardware?"},{"@id":"sustainability:f_ghg_emissions","@type":["rdf:Property","owl:DatatypeProperty"],"rdfs:label":"f_ghg_emissions","schema:rangeIncludes":{"@id":"sustainability:FGhgEmissions"},"schema:domainIncludes":{"@id":"sustainability:SsctAndOther"},"rdfs:comment":"Does the standard include criteria on F-GHG emissions?"},{"@id":"sustainability:power_consumption_and_power_management_during_the_use_phase","@type":["rdf:Property","owl:DatatypeProperty"],"rdfs:label":"power_consumption_and_power_management_during_the_use_phase","schema:rangeIncludes":{"@id":"sustainability:PowerConsumptionAndPowerManagementDuringTheUsePhase"},"schema:domainIncludes":{"@id":"sustainability:SsctAndOther"},"rdfs:comment":"Does the standard include criteria on power consumption and power management (during the use phase)?"},{"@id":"sustainability:providing_information_concerning_possible_power_savings_to_the_user","@type":["rdf:Property","owl:DatatypeProperty"],"rdfs:label":"providing_information_concerning_possible_power_savings_to_the_user","schema:rangeIncludes":{"@id":"xsd:boolean"},"schema:domainIncludes":{"@id":"sustainability:SsctAndOther"},"rdfs:comment":"Does the standard include criteria on providing information concerning possible power savings to the user?"},{"@id":"sustainability:h_statements_h340_h341_h350_h351_h360_h361","@type":["rdf:Property","owl:DatatypeProperty"],"rdfs:label":"h_statements_h340_h341_h350_h351_h360_h361","schema:rangeIncludes":{"@id":"sustainability:HStatementsH340H341H350H351H360H361"},"schema:domainIncludes":{"@id":"sustainability:SsctAndOther"},"rdfs:comment":"Does the standard include criteria on H statements H340, H341, H350, H351, H360, H361?"},{"@id":"sustainability:the_use_of_mercury_cadmium_lead_chromium_vi","@type":["rdf:Property","owl:DatatypeProperty"],"rdfs:label":"the_use_of_mercury_cadmium_lead_chromium_vi","schema:rangeIncludes":{"@id":"sustainability:TheUseOfMercuryCadmiumLeadChromiumVi"},"schema:domainIncludes":{"@id":"sustainability:SsctAndOther"},"rdfs:comment":"Does the standard include criteria on the use of mercury, cadmium, lead, chromium VI?"},{"@id":"sustainability:the_use_of_flame_retardants","@type":["rdf:Property","owl:DatatypeProperty"],"rdfs:label":"the_use_of_flame_retardants","schema:rangeIncludes":{"@id":"sustainability:TheUseOfFlameRetardants"},"schema:domainIncludes":{"@id":"sustainability:SsctAndOther"},"rdfs:comment":"Does the standard include criteria on the use of flame retardants?"},{"@id":"sustainability:the_use_of_plasticizers_with_adverse_environmental_and_health_impact","@type":["rdf:Property","owl:DatatypeProperty"],"rdfs:label":"the_use_of_plasticizers_with_adverse_environmental_and_health_impact","schema:rangeIncludes":{"@id":"sustainability:TheUseOfPlasticizersWithAdverseEnvironmentalAndHealthImpact"},"schema:domainIncludes":{"@id":"sustainability:SsctAndOther"},"rdfs:comment":"Does the standard include criteria on the use of plasticizers with adverse environmental and health impact?"},{"@id":"sustainability:the_use_of_biocides_in_the_finishing_process","@type":["rdf:Property","owl:DatatypeProperty"],"rdfs:label":"the_use_of_biocides_in_the_finishing_process","schema:rangeIncludes":{"@id":"sustainability:TheUseOfBiocidesInTheFinishingProcess"},"schema:domainIncludes":{"@id":"sustainability:SsctAndOther"},"rdfs:comment":"Does the standard include criteria on the use of biocides in the finishing process?"},{"@id":"sustainability:the_use_of_polymers_containing_halogens","@type":["rdf:Property","owl:DatatypeProperty"],"rdfs:label":"the_use_of_polymers_containing_halogens","schema:rangeIncludes":{"@id":"sustainability:TheUseOfPolymersContainingHalogens"},"schema:domainIncludes":{"@id":"sustainability:SsctAndOther"},"rdfs:comment":"Does the standard include criteria on the use of polymers containing halogens?"},{"@id":"sustainability:clear_coding_of_used_materials","@type":["rdf:Property","owl:DatatypeProperty"],"rdfs:label":"clear_coding_of_used_materials","schema:rangeIncludes":{"@id":"xsd:boolean"},"schema:domainIncludes":{"@id":"sustainability:SsctAndOther"},"rdfs:comment":"Does the standard include criteria on clear coding of used materials?"},{"@id":"sustainability:the_recyclability_of_plastics_used","@type":["rdf:Property","owl:DatatypeProperty"],"rdfs:label":"the_recyclability_of_plastics_used","schema:rangeIncludes":{"@id":"sustainability:TheRecyclabilityOfPlasticsUsed"},"schema:domainIncludes":{"@id":"sustainability:SsctAndOther"},"rdfs:comment":"Does the standard include criteria on the recyclability of plastics used?"},{"@id":"sustainability:disassembly_of_the_product_for_recycling","@type":["rdf:Property","owl:DatatypeProperty"],"rdfs:label":"disassembly_of_the_product_for_recycling","schema:rangeIncludes":{"@id":"xsd:boolean"},"schema:domainIncludes":{"@id":"sustainability:SsctAndOther"},"rdfs:comment":"Does the standard include criteria on disassembly of the product for recycling?"},{"@id":"sustainability:a_take_back_system_for_the_product","@type":["rdf:Property","owl:DatatypeProperty"],"rdfs:label":"a_take_back_system_for_the_product","schema:rangeIncludes":{"@id":"xsd:boolean"},"schema:domainIncludes":{"@id":"sustainability:SsctAndOther"},"rdfs:comment":"Does the standard include criteria on a take back system for the product?"},{"@id":"sustainability:environmental_responsible_mining_practices","@type":["rdf:Property","owl:DatatypeProperty"],"rdfs:label":"environmental_responsible_mining_practices","schema:rangeIncludes":{"@id":"sustainability:EnvironmentalResponsibleMiningPractices"},"schema:domainIncludes":{"@id":"sustainability:SsctAndOther"},"rdfs:comment":"Does the standard include criteria on environmental responsible mining practices?"},{"@id":"sustainability:the_use_of_recycled_material_in_the_packaging","@type":["rdf:Property","owl:DatatypeProperty"],"rdfs:label":"the_use_of_recycled_material_in_the_packaging","schema:rangeIncludes":{"@id":"sustainability:TheUseOfRecycledMaterialInThePackaging"},"schema:domainIncludes":{"@id":"sustainability:SsctAndOther"},"rdfs:comment":"Does the standard include criteria on the use of recycled material in the packaging?"},{"@id":"sustainability:the_use_of_postconsumer_recycled_content_in_the_product","@type":["rdf:Property","owl:DatatypeProperty"],"rdfs:label":"the_use_of_postconsumer_recycled_content_in_the_product","schema:rangeIncludes":{"@id":"sustainability:TheUseOfPostconsumerRecycledContentInTheProduct"},"schema:domainIncludes":{"@id":"sustainability:SsctAndOther"},"rdfs:comment":"Does the standard include criteria on the use of postconsumer recycled content in the product?"},{"@id":"sustainability:noise_emissions_during_the_use_phase","@type":["rdf:Property","owl:DatatypeProperty"],"rdfs:label":"noise_emissions_during_the_use_phase","schema:rangeIncludes":{"@id":"xsd:boolean"},"schema:domainIncludes":{"@id":"sustainability:SsctAndOther"},"rdfs:comment":"Does the standard include criteria on noise emissions during the use phase?"},{"@id":"sustainability:environmental_management_instruments_like_emas_or_iso14001","@type":["rdf:Property","owl:DatatypeProperty"],"rdfs:label":"environmental_management_instruments_like_emas_or_iso14001","schema:rangeIncludes":{"@id":"sustainability:EnvironmentalManagementInstrumentsLikeEmasOrIso14001"},"schema:domainIncludes":{"@id":"sustainability:SsctAndOther"},"rdfs:comment":"Does the standard include criteria on environmental management instruments like EMAS or ISO 14001?"},{"@id":"sustainability:the_use_of_formaldehyde","@type":["rdf:Property","owl:DatatypeProperty"],"rdfs:label":"the_use_of_formaldehyde","schema:rangeIncludes":{"@id":"sustainability:TheUseOfFormaldehyde"},"schema:domainIncludes":{"@id":"sustainability:SsctAndOther"},"rdfs:comment":"Does the standard include criteria on the use of formaldehyde?"},{"@id":"sustainability:an_additional_lifetime_guarantee_for_the_product_beyond_the_legal_obligations","@type":["rdf:Property","owl:DatatypeProperty"],"rdfs:label":"an_additional_lifetime_guarantee_for_the_product_beyond_the_legal_obligations","schema:rangeIncludes":{"@id":"sustainability:AnAdditionalLifetimeGuaranteeForTheProductBeyondTheLegalObligations"},"schema:domainIncludes":{"@id":"sustainability:SsctAndOther"},"rdfs:comment":"Does the standard include criteria on an additional lifetime guarantee for the product beyond the legal obligations?"},{"@id":"sustainability:the_quality_durability_of_specific_components","@type":["rdf:Property","owl:DatatypeProperty"],"rdfs:label":"the_quality_durability_of_specific_components","schema:rangeIncludes":{"@id":"xsd:boolean"},"schema:domainIncludes":{"@id":"sustainability:SsctAndOther"},"rdfs:comment":"Does the standard include criteria on the quality / durability of specific components?"},{"@id":"sustainability:a_modular_design_of_the_product","@type":["rdf:Property","owl:DatatypeProperty"],"rdfs:label":"a_modular_design_of_the_product","schema:rangeIncludes":{"@id":"xsd:boolean"},"schema:domainIncludes":{"@id":"sustainability:SsctAndOther"},"rdfs:comment":"Does the standard include criteria on a modular design of the product?"},{"@id":"sustainability:the_availability_of_spare_parts_for_the_product","@type":["rdf:Property","owl:DatatypeProperty"],"rdfs:label":"the_availability_of_spare_parts_for_the_product","schema:rangeIncludes":{"@id":"sustainability:TheAvailabilityOfSparePartsForTheProduct"},"schema:domainIncludes":{"@id":"sustainability:SsctAndOther"},"rdfs:comment":"Does the standard include criteria on the availability of spare parts for the product?"},{"@id":"sustainability:properties_of_the_battery","@type":["rdf:Property","owl:DatatypeProperty"],"rdfs:label":"properties_of_the_battery","schema:rangeIncludes":{"@id":"xsd:boolean"},"schema:domainIncludes":{"@id":"sustainability:SsctAndOther"},"rdfs:comment":"Does the standard include criteria on properties of the battery?"},{"@id":"sustainability:expansion_facilities_of_the_product","@type":["rdf:Property","owl:DatatypeProperty"],"rdfs:label":"expansion_facilities_of_the_product","schema:rangeIncludes":{"@id":"xsd:boolean"},"schema:domainIncludes":{"@id":"sustainability:SsctAndOther"},"rdfs:comment":"Does the standard include criteria on expansion facilities of the product?"},{"@id":"sustainability:repairability_upgradeability_and_usage_of_the_battery_to_the_user","@type":["rdf:Property","owl:DatatypeProperty"],"rdfs:label":"repairability_upgradeability_and_usage_of_the_battery_to_the_user","schema:rangeIncludes":{"@id":"xsd:boolean"},"schema:domainIncludes":{"@id":"sustainability:SsctAndOther"},"rdfs:comment":"Does the standard include criteria on providing information concerning reparability, upgradeability and usage of the battery to the user?"},{"@id":"sustainability:conflict_minerals","@type":["rdf:Property","owl:DatatypeProperty"],"rdfs:label":"conflict_minerals","schema:rangeIncludes":{"@id":"xsd:boolean"},"schema:domainIncludes":{"@id":"sustainability:SsctAndOther"},"rdfs:comment":"Does the standard include criteria on conflict minerals?"},{"@id":"sustainability:compliance_with_all_ilo_core_labour_standards_are_verified_by_a_third_party","@type":["rdf:Property","owl:DatatypeProperty"],"rdfs:label":"compliance_with_all_ilo_core_labour_standards_are_verified_by_a_third_party","schema:rangeIncludes":{"@id":"xsd:boolean"},"schema:domainIncludes":{"@id":"sustainability:SsctAndOther"},"rdfs:comment":"Does the standard require that (at least) compliance with all ILO core labour standards are verified by a third party?"},{"@id":"sustainability:forced_and_compulsory_labour_as_defined_in_ilo105","@type":["rdf:Property","owl:DatatypeProperty"],"rdfs:label":"forced_and_compulsory_labour_as_defined_in_ilo105","schema:rangeIncludes":{"@id":"xsd:boolean"},"schema:domainIncludes":{"@id":"sustainability:SsctAndOther"},"rdfs:comment":"Does the standard prohibit forced and compulsory labour as defined in ILO 105?"},{"@id":"sustainability:the_use_of_nanomaterials","@type":["rdf:Property","owl:DatatypeProperty"],"rdfs:label":"the_use_of_nanomaterials","schema:rangeIncludes":{"@id":"sustainability:TheUseOfNanomaterials"},"schema:domainIncludes":{"@id":"sustainability:SsctAndOther"},"rdfs:comment":"Does the standard include criteria on the use of nanomaterials?"},{"@id":"sustainability:requirements_to_train_workers_on_labour_rights","@type":["rdf:Property","owl:DatatypeProperty"],"rdfs:label":"requirements_to_train_workers_on_labour_rights","schema:rangeIncludes":{"@id":"xsd:boolean"},"schema:domainIncludes":{"@id":"sustainability:SsctAndOther"},"rdfs:comment":"Does the standard include requirements to train workers on labour rights?"},{"@id":"sustainability:setting_up_policies_or_procedures_to_manage_basic_labour_rights_in_the_workplace","@type":["rdf:Property","owl:DatatypeProperty"],"rdfs:label":"setting_up_policies_or_procedures_to_manage_basic_labour_rights_in_the_workplace","schema:rangeIncludes":{"@id":"xsd:boolean"},"schema:domainIncludes":{"@id":"sustainability:SsctAndOther"},"rdfs:comment":"Does the standard include requirements on setting up policies or procedures to manage basic labour rights in the workplace?"},{"@id":"sustainability:the_biodegradability_of_substances","@type":["rdf:Property","owl:DatatypeProperty"],"rdfs:label":"the_biodegradability_of_substances","schema:rangeIncludes":{"@id":"xsd:boolean"},"schema:domainIncludes":{"@id":"sustainability:SsctAndOther"},"rdfs:comment":"Does the standard include criteria on biodegradability of substances?"},{"@id":"sustainability:the_use_of_dyes_or_pigments_based_on_lead_copper_chromium_nickel_and_aluminum","@type":["rdf:Property","owl:DatatypeProperty"],"rdfs:label":"the_use_of_dyes_or_pigments_based_on_lead_copper_chromium_nickel_and_aluminum","schema:rangeIncludes":{"@id":"sustainability:TheUseOfDyesOrPigmentsBasedOnLeadCopperChromiumNickelAndAluminum"},"schema:domainIncludes":{"@id":"sustainability:SsctAndOther"},"rdfs:comment":"Does the standard include criteria on the use of dyes or pigments based on lead copper, chromium, nickel, cadmium and aluminum?"},{"@id":"sustainability:the_use_of_azo_dyes_that_may_cleave_aromatic_amines_which_are_harmful_to_human_health","@type":["rdf:Property","owl:DatatypeProperty"],"rdfs:label":"the_use_of_azo_dyes_that_may_cleave_aromatic_amines_which_are_harmful_to_human_health","schema:rangeIncludes":{"@id":"sustainability:TheUseOfAzoDyesThatMayCleaveAromaticAminesWhichAreHarmfulToHumanHealth"},"schema:domainIncludes":{"@id":"sustainability:SsctAndOther"},"rdfs:comment":"Does the standard include criteria on the use of azo dyes that may cleave aromatic amines which are harmful to human health?"},{"@id":"sustainability:human_rights_and_local_communities_general_principle","@type":["rdf:Property","owl:DatatypeProperty"],"rdfs:label":"human_rights_and_local_communities_general_principle","schema:rangeIncludes":{"@id":"xsd:string"},"schema:domainIncludes":{"@id":"sustainability:HumanRights"},"rdfs:comment":"Does the standard address basic culture and human rights as defined by the UN Universal Declaration of Human Rights?"},{"@id":"sustainability:gender_policies_and_best_practices","@type":["rdf:Property","owl:DatatypeProperty"],"rdfs:label":"gender_policies_and_best_practices","schema:rangeIncludes":{"@id":"xsd:boolean"},"schema:domainIncludes":{"@id":"sustainability:HumanRights"},"rdfs:comment":"Does the standard require policy development and implentation of initiatives that promote gender equality?"},{"@id":"sustainability:women_s_access_to_health_and_safety_services","@type":["rdf:Property","owl:DatatypeProperty"],"rdfs:label":"women_s_access_to_health_and_safety_services","schema:rangeIncludes":{"@id":"xsd:boolean"},"schema:domainIncludes":{"@id":"sustainability:HumanRights"},"rdfs:comment":"Does the standard include criteria related to women specific health and safety issues?"},{"@id":"sustainability:factoring_gender_considerations_in_impacts_and_risks_assessment_of_production","@type":["rdf:Property","owl:DatatypeProperty"],"rdfs:label":"factoring_gender_considerations_in_impacts_and_risks_assessment_of_production","schema:rangeIncludes":{"@id":"xsd:boolean"},"schema:domainIncludes":{"@id":"sustainability:HumanRights"},"rdfs:comment":"Does the standard require the inclusion of gender considerations in impacts and risks assessments of the unit of operation"},{"@id":"sustainability:factoring_gender_considerations_in_stakeholder_engagement_process","@type":["rdf:Property","owl:DatatypeProperty"],"rdfs:label":"factoring_gender_considerations_in_stakeholder_engagement_process","schema:rangeIncludes":{"@id":"xsd:boolean"},"schema:domainIncludes":{"@id":"sustainability:HumanRights"},"rdfs:comment":"Does the standard require equal inclusion on the basis of gender in the stakeholder engagement process"},{"@id":"sustainability:indigenous_peoples_as_defined_in_ilo_convention169","@type":["rdf:Property","owl:DatatypeProperty"],"rdfs:label":"indigenous_peoples_as_defined_in_ilo_convention169","schema:rangeIncludes":{"@id":"xsd:boolean"},"schema:domainIncludes":{"@id":"sustainability:HumanRights"},"rdfs:comment":"Does the standard include criteria on the rights of indigenous and tribal peoples as defined in ILO 169?"},{"@id":"sustainability:the_protection_of_minority_rights_of_indigenous_peoples","@type":["rdf:Property","owl:DatatypeProperty"],"rdfs:label":"the_protection_of_minority_rights_of_indigenous_peoples","schema:rangeIncludes":{"@id":"xsd:boolean"},"schema:domainIncludes":{"@id":"sustainability:HumanRights"},"rdfs:comment":"Does the standard include criteria addressing protection of minority rights of indigenous peoples?"},{"@id":"sustainability:the_protection_of_minority_rights_of_marginalized_groups","@type":["rdf:Property","owl:DatatypeProperty"],"rdfs:label":"the_protection_of_minority_rights_of_marginalized_groups","schema:rangeIncludes":{"@id":"xsd:boolean"},"schema:domainIncludes":{"@id":"sustainability:HumanRights"},"rdfs:comment":"Does the standard include criteria on the protection of minority rights of marginalized groups?"},{"@id":"sustainability:socio_cultural_sites","@type":["rdf:Property","owl:DatatypeProperty"],"rdfs:label":"socio_cultural_sites","schema:rangeIncludes":{"@id":"sustainability:SocioCulturalSites"},"schema:domainIncludes":{"@id":"sustainability:HumanRights"},"rdfs:comment":"Does the standard include criteria on the protection of local historical, archaeological, cultural, and spiritual properties and sites?"},{"@id":"sustainability:historical_cultural_and_archeological_artifacts_trade","@type":["rdf:Property","owl:DatatypeProperty"],"rdfs:label":"historical_cultural_and_archeological_artifacts_trade","schema:rangeIncludes":{"@id":"xsd:boolean"},"schema:domainIncludes":{"@id":"sustainability:HumanRights"},"rdfs:comment":"Does the standard include criteria relating to the trade of historical, cultural and archeological artifacts?"},{"@id":"sustainability:using_local_art_architecture_and_or_cultural_heritage_in_design_for_commercial_purposes","@type":["rdf:Property","owl:DatatypeProperty"],"rdfs:label":"using_local_art_architecture_and_or_cultural_heritage_in_design_for_commercial_purposes","schema:rangeIncludes":{"@id":"xsd:boolean"},"schema:domainIncludes":{"@id":"sustainability:HumanRights"},"rdfs:comment":"Does the standard include criteria on using local art, architecture and/or cultural heritage in design / for commercial purposes"},{"@id":"sustainability:basic_human_rights_and_local_communities_engagement","@type":["rdf:Property","owl:DatatypeProperty"],"rdfs:label":"basic_human_rights_and_local_communities_engagement","schema:rangeIncludes":{"@id":"xsd:boolean"},"schema:domainIncludes":{"@id":"sustainability:HumanRights"},"rdfs:comment":"Does the standard require that producers consult and engage in dialogue with local communities?"},{"@id":"sustainability:internationally_recognized_legally_protected_sites_and_cultural_heritage","@type":["rdf:Property","owl:DatatypeProperty"],"rdfs:label":"internationally_recognized_legally_protected_sites_and_cultural_heritage","schema:rangeIncludes":{"@id":"xsd:boolean"},"schema:domainIncludes":{"@id":"sustainability:HumanRights"},"rdfs:comment":"Does the standard include criteria on the ackowledgement and protection of internationally recognized/legally protected sites of cultural and religious significance."},{"@id":"sustainability:community_access_to_cultural_heritage","@type":["rdf:Property","owl:DatatypeProperty"],"rdfs:label":"community_access_to_cultural_heritage","schema:rangeIncludes":{"@id":"xsd:boolean"},"schema:domainIncludes":{"@id":"sustainability:HumanRights"},"rdfs:comment":"Does the standard include criteria relating to community access to cultural heritage sites?"},{"@id":"sustainability:behavior_guidelines_for_access_to_and_use_of_natural_resources_cultural_sites","@type":["rdf:Property","owl:DatatypeProperty"],"rdfs:label":"behavior_guidelines_for_access_to_and_use_of_natural_resources_cultural_sites","schema:rangeIncludes":{"@id":"xsd:boolean"},"schema:domainIncludes":{"@id":"sustainability:HumanRights"},"rdfs:comment":"Does the standard require that interpretive materials and behavior guidelines pertaining to resource use are made available for workers and visitors?"},{"@id":"sustainability:local_access_to_historical_cultural_archeological_and_spiritually_important_properties_and_sites","@type":["rdf:Property","owl:DatatypeProperty"],"rdfs:label":"local_access_to_historical_cultural_archeological_and_spiritually_important_properties_and_sites","schema:rangeIncludes":{"@id":"xsd:boolean"},"schema:domainIncludes":{"@id":"sustainability:HumanRights"},"rdfs:comment":"Does the standard include criteria on maintaining local access to historical, cultural, archeological and spiritually important properties and sites?"},{"@id":"sustainability:establishment_of_a_code_of_conduct_for_working_with_local_and_indigenous_communities","@type":["rdf:Property","owl:DatatypeProperty"],"rdfs:label":"establishment_of_a_code_of_conduct_for_working_with_local_and_indigenous_communities","schema:rangeIncludes":{"@id":"xsd:boolean"},"schema:domainIncludes":{"@id":"sustainability:HumanRights"},"rdfs:comment":"Standard includes criteria relating to establishment of a code of conduct for working with local and indigenous communities"},{"@id":"sustainability:services_and_benefits_offered_to_communities_beyond_the_business_operations_education_health_sanitation","@type":["rdf:Property","owl:DatatypeProperty"],"rdfs:label":"services_and_benefits_offered_to_communities_beyond_the_business_operations_education_health_sanitation","schema:rangeIncludes":{"@id":"xsd:boolean"},"schema:domainIncludes":{"@id":"sustainability:HumanRights"},"rdfs:comment":"Does the standard include criteria related to the active support of community development"},{"@id":"sustainability:compensation_for_use_of_local_communities_facilities","@type":["rdf:Property","owl:DatatypeProperty"],"rdfs:label":"compensation_for_use_of_local_communities_facilities","schema:rangeIncludes":{"@id":"sustainability:CompensationForUseOfLocalCommunitiesFacilities"},"schema:domainIncludes":{"@id":"sustainability:HumanRights"},"rdfs:comment":"Does the standard include criteria on compensation mechanisms for the utilization of traditional knowledge?"},{"@id":"sustainability:engagement_consultation_with_local_communities","@type":["rdf:Property","owl:DatatypeProperty"],"rdfs:label":"engagement_consultation_with_local_communities","schema:rangeIncludes":{"@id":"xsd:boolean"},"schema:domainIncludes":{"@id":"sustainability:HumanRights"},"rdfs:comment":"Does the standard require the unit of operation to engage and consult with local communities regarding changes or impacts from business activities on local resources and communities?"},{"@id":"sustainability:land_title_and_use_rights","@type":["rdf:Property","owl:DatatypeProperty"],"rdfs:label":"land_title_and_use_rights","schema:rangeIncludes":{"@id":"xsd:boolean"},"schema:domainIncludes":{"@id":"sustainability:HumanRights"},"rdfs:comment":"Does the standard explicitly address the issue of legal land title and use rights, such as land ownership issues etc."},{"@id":"sustainability:supporting_local_communities_economic_development","@type":["rdf:Property","owl:DatatypeProperty"],"rdfs:label":"supporting_local_communities_economic_development","schema:rangeIncludes":{"@id":"xsd:boolean"},"schema:domainIncludes":{"@id":"sustainability:HumanRights"},"rdfs:comment":"Does the standard require the unit of operation support economic development of local communities by providing opportunities for local employment and provision of services?"},{"@id":"sustainability:assessing_possible_impacts_of_production_practices_on_food_security","@type":["rdf:Property","owl:DatatypeProperty"],"rdfs:label":"assessing_possible_impacts_of_production_practices_on_food_security","schema:rangeIncludes":{"@id":"xsd:boolean"},"schema:domainIncludes":{"@id":"sustainability:HumanRights"},"rdfs:comment":"Does the standard include criteria on food security assessments in the case of significant land use changes or changes in land tenure/ ownership?"},{"@id":"sustainability:hiring_workers_from_local_communities","@type":["rdf:Property","owl:DatatypeProperty"],"rdfs:label":"hiring_workers_from_local_communities","schema:rangeIncludes":{"@id":"xsd:boolean"},"schema:domainIncludes":{"@id":"sustainability:HumanRights"},"rdfs:comment":"Does the standard include criteria relating to hiring workers from local communities?"},{"@id":"sustainability:purchasing_local_materials_goods_products_and_services","@type":["rdf:Property","owl:DatatypeProperty"],"rdfs:label":"purchasing_local_materials_goods_products_and_services","schema:rangeIncludes":{"@id":"xsd:boolean"},"schema:domainIncludes":{"@id":"sustainability:HumanRights"},"rdfs:comment":"Does the standard include criteria promoting the purchase of local materials, goods, products and services (e.g. Implements a \"buy local\" policy)?"},{"@id":"sustainability:traditional_and_cultural_production_practices","@type":["rdf:Property","owl:DatatypeProperty"],"rdfs:label":"traditional_and_cultural_production_practices","schema:rangeIncludes":{"@id":"xsd:boolean"},"schema:domainIncludes":{"@id":"sustainability:HumanRights"},"rdfs:comment":"Does the standard include criteria relating to respecting traditional and cultural production practices of indigenous/minority groups?"},{"@id":"sustainability:grievance_mechanisms_for_affected_communities","@type":["rdf:Property","owl:DatatypeProperty"],"rdfs:label":"grievance_mechanisms_for_affected_communities","schema:rangeIncludes":{"@id":"sustainability:GrievanceMechanismsForAffectedCommunities"},"schema:domainIncludes":{"@id":"sustainability:HumanRights"},"rdfs:comment":"Does the standard include criteria to address grievances and provide fair compensation for negative impacts of operations on local communities and individuals?"},{"@id":"sustainability:conduct_of_security_personnel_towards_communities","@type":["rdf:Property","owl:DatatypeProperty"],"rdfs:label":"conduct_of_security_personnel_towards_communities","schema:rangeIncludes":{"@id":"xsd:boolean"},"schema:domainIncludes":{"@id":"sustainability:HumanRights"},"rdfs:comment":"Does the standard include criteria relating to the development of a code of conduct for security personnel and their interaction with local communities?"},{"@id":"sustainability:assessment_of_impacts_of_local_activities_on_human_rights_issues_such_as_health_safety_and_security","@type":["rdf:Property","owl:DatatypeProperty"],"rdfs:label":"assessment_of_impacts_of_local_activities_on_human_rights_issues_such_as_health_safety_and_security","schema:rangeIncludes":{"@id":"xsd:boolean"},"schema:domainIncludes":{"@id":"sustainability:HumanRights"},"rdfs:comment":"Does the standard require the unit of operation to conduct an impacts assessment of business operations on the health, safety and security of local communities, and take measures to minimize and mitigate any negative impacts from operations on those surrounding communities."},{"@id":"sustainability:impact_assessment_on_access_to_basic_services_for_local_communities","@type":["rdf:Property","owl:DatatypeProperty"],"rdfs:label":"impact_assessment_on_access_to_basic_services_for_local_communities","schema:rangeIncludes":{"@id":"xsd:boolean"},"schema:domainIncludes":{"@id":"sustainability:HumanRights"},"rdfs:comment":"Does the standard require an assessment of impacts from business activities on access to basic services for local communities, as well as implement measures to resolve related disputes?"},{"@id":"sustainability:involuntary_resettlement_physical_displacement_and_or_economic_displacement","@type":["rdf:Property","owl:DatatypeProperty"],"rdfs:label":"involuntary_resettlement_physical_displacement_and_or_economic_displacement","schema:rangeIncludes":{"@id":"xsd:boolean"},"schema:domainIncludes":{"@id":"sustainability:HumanRights"},"rdfs:comment":"Does the standard include criteria relating to involuntary resettlement, physical displacement and/or economic displacement resulting from business operations?"},{"@id":"sustainability:compensation_and_benefits_for_displaced_persons","@type":["rdf:Property","owl:DatatypeProperty"],"rdfs:label":"compensation_and_benefits_for_displaced_persons","schema:rangeIncludes":{"@id":"xsd:boolean"},"schema:domainIncludes":{"@id":"sustainability:HumanRights"},"rdfs:comment":"Does the standard require the unit of operation to have in place a resettlement action plan designed to provide compensation and benefits for displaced persons?"},{"@id":"sustainability:planning_implementation_of_resettlement_activities","@type":["rdf:Property","owl:DatatypeProperty"],"rdfs:label":"planning_implementation_of_resettlement_activities","schema:rangeIncludes":{"@id":"xsd:boolean"},"schema:domainIncludes":{"@id":"sustainability:HumanRights"},"rdfs:comment":"Does the standard require the unit of operation to have in place a resettlement action plan for planning and implementing fair resettlement activities for affected communities/persons?"},{"@id":"sustainability:production_practices_promoting_healthy_high_nutritional_value_foods","@type":["rdf:Property","owl:DatatypeProperty"],"rdfs:label":"production_practices_promoting_healthy_high_nutritional_value_foods","schema:rangeIncludes":{"@id":"xsd:boolean"},"schema:domainIncludes":{"@id":"sustainability:HumanRights"},"rdfs:comment":"Does the standard include criteria on production practices promoting healthy and nutrient rich food?"},{"@id":"sustainability:livelihood_restoration_for_displaced_persons","@type":["rdf:Property","owl:DatatypeProperty"],"rdfs:label":"livelihood_restoration_for_displaced_persons","schema:rangeIncludes":{"@id":"xsd:boolean"},"schema:domainIncludes":{"@id":"sustainability:HumanRights"},"rdfs:comment":"Does the standard require the unit of operation to have in place a livelihood restoration policy?"},{"@id":"sustainability:hazardous_chemicals_reach","@type":["rdf:Property","owl:DatatypeProperty"],"rdfs:label":"hazardous_chemicals_reach","schema:rangeIncludes":{"@id":"xsd:boolean"},"schema:domainIncludes":{"@id":"sustainability:HumanRights"},"rdfs:comment":"Does the standard require compliance with REACH"},{"@id":"sustainability:free_prior_and_informed_consent_fpic_of_local_communities","@type":["rdf:Property","owl:DatatypeProperty"],"rdfs:label":"free_prior_and_informed_consent_fpic_of_local_communities","schema:rangeIncludes":{"@id":"xsd:boolean"},"schema:domainIncludes":{"@id":"sustainability:HumanRights"},"rdfs:comment":"Does the standard include criteria to seek Free, Prior and Informed Consent (FPIC) of local communities?"},{"@id":"sustainability:requirement_to_identify_legal_and_customary_rights_of_tenure","@type":["rdf:Property","owl:DatatypeProperty"],"rdfs:label":"requirement_to_identify_legal_and_customary_rights_of_tenure","schema:rangeIncludes":{"@id":"xsd:boolean"},"schema:domainIncludes":{"@id":"sustainability:HumanRights"},"rdfs:comment":"Does the standard include criteria on the identification of legal and customary rights of tenure (incl. access and use of other parties that apply on the production/management unit)"},{"@id":"sustainability:activities_not_adversely_affecting_local_communities_access_to_livelihoods","@type":["rdf:Property","owl:DatatypeProperty"],"rdfs:label":"activities_not_adversely_affecting_local_communities_access_to_livelihoods","schema:rangeIncludes":{"@id":"xsd:string"},"schema:domainIncludes":{"@id":"sustainability:HumanRights"},"rdfs:comment":"Does the standard have processes in place for maintaining access to livelihoods for surrounding communities?"},{"@id":"sustainability:production_practices_that_reduce_food_and_feed_waste","@type":["rdf:Property","owl:DatatypeProperty"],"rdfs:label":"production_practices_that_reduce_food_and_feed_waste","schema:rangeIncludes":{"@id":"xsd:boolean"},"schema:domainIncludes":{"@id":"sustainability:HumanRights"},"rdfs:comment":"Does the standard include criteria on food and feed loss in subsequent stages of the food supply chain?"},{"@id":"sustainability:the_promotion_enhancement_of_education","@type":["rdf:Property","owl:DatatypeProperty"],"rdfs:label":"the_promotion_enhancement_of_education","schema:rangeIncludes":{"@id":"xsd:boolean"},"schema:domainIncludes":{"@id":"sustainability:HumanRights"},"rdfs:comment":"Does the standard include the promotion/enhancement of education?"},{"@id":"sustainability:the_promotion_enhancement_of_medical_care_services","@type":["rdf:Property","owl:DatatypeProperty"],"rdfs:label":"the_promotion_enhancement_of_medical_care_services","schema:rangeIncludes":{"@id":"xsd:boolean"},"schema:domainIncludes":{"@id":"sustainability:HumanRights"},"rdfs:comment":"Does the standard include criteria requiring access to medical care for workers and their families"},{"@id":"sustainability:the_promotion_enhancement_of_housing_and_sanitary_facilities","@type":["rdf:Property","owl:DatatypeProperty"],"rdfs:label":"the_promotion_enhancement_of_housing_and_sanitary_facilities","schema:rangeIncludes":{"@id":"xsd:boolean"},"schema:domainIncludes":{"@id":"sustainability:HumanRights"},"rdfs:comment":"Does the standard include criteria related to the provision of housing and sanitary facilities for workers and their families."},{"@id":"sustainability:gender_issues_general_principle","@type":["rdf:Property","owl:DatatypeProperty"],"rdfs:label":"gender_issues_general_principle","schema:rangeIncludes":{"@id":"xsd:boolean"},"schema:domainIncludes":{"@id":"sustainability:HumanRights"},"rdfs:comment":"Does the standard include a general principle addressing gender issues when interacting with local communities?"},{"@id":"sustainability:working_conditions_overarching_principles","@type":["rdf:Property","owl:DatatypeProperty"],"rdfs:label":"working_conditions_overarching_principles","schema:rangeIncludes":{"@id":"xsd:string"},"schema:domainIncludes":{"@id":"sustainability:ConditionsOfWork"},"rdfs:comment":"Does the standard address issues and rights related to workers and hired labors?"},{"@id":"sustainability:publicly_available_evacuation_procedures","@type":["rdf:Property","owl:DatatypeProperty"],"rdfs:label":"publicly_available_evacuation_procedures","schema:rangeIncludes":{"@id":"xsd:boolean"},"schema:domainIncludes":{"@id":"sustainability:ConditionsOfWork"},"rdfs:comment":"Does the standard make publicly available to all workers and visitors manuals on management of emergencies and accidents?"},{"@id":"sustainability:emergency_exists_maintenance","@type":["rdf:Property","owl:DatatypeProperty"],"rdfs:label":"emergency_exists_maintenance","schema:rangeIncludes":{"@id":"xsd:boolean"},"schema:domainIncludes":{"@id":"sustainability:ConditionsOfWork"},"rdfs:comment":"Does the standard include explicit criteria on the maintenance of emergency exists?"},{"@id":"sustainability:training_on_health_safety_issues","@type":["rdf:Property","owl:DatatypeProperty"],"rdfs:label":"training_on_health_safety_issues","schema:rangeIncludes":{"@id":"xsd:boolean"},"schema:domainIncludes":{"@id":"sustainability:ConditionsOfWork"},"rdfs:comment":"Does the standard include criteria on training for health and safety at work"},{"@id":"sustainability:occupational_health_and_safety_as_defined_in_ilo155","@type":["rdf:Property","owl:DatatypeProperty"],"rdfs:label":"occupational_health_and_safety_as_defined_in_ilo155","schema:rangeIncludes":{"@id":"sustainability:OccupationalHealthAndSafetyAsDefinedInIlo155"},"schema:domainIncludes":{"@id":"sustainability:ConditionsOfWork"},"rdfs:comment":"Does the standard include criteria on occupational health and safety, as defined in ILO 155?"},{"@id":"sustainability:workplace_safety","@type":["rdf:Property","owl:DatatypeProperty"],"rdfs:label":"workplace_safety","schema:rangeIncludes":{"@id":"xsd:boolean"},"schema:domainIncludes":{"@id":"sustainability:ConditionsOfWork"},"rdfs:comment":"Does the standard include criteria relating to safe work environment?"},{"@id":"sustainability:safety_equipments_personal_protective_equipment_ppe","@type":["rdf:Property","owl:DatatypeProperty"],"rdfs:label":"safety_equipments_personal_protective_equipment_ppe","schema:rangeIncludes":{"@id":"xsd:boolean"},"schema:domainIncludes":{"@id":"sustainability:ConditionsOfWork"},"rdfs:comment":"Does the standard require the provision of appropriate safety equipment and PPE"},{"@id":"sustainability:maintenance_of_safety_of_machinery_equipment_and_materials","@type":["rdf:Property","owl:DatatypeProperty"],"rdfs:label":"maintenance_of_safety_of_machinery_equipment_and_materials","schema:rangeIncludes":{"@id":"xsd:boolean"},"schema:domainIncludes":{"@id":"sustainability:ConditionsOfWork"},"rdfs:comment":"Does the standard include criteria on the maintenance of equipment and machinery to ensure their proper and efficient functioning."},{"@id":"sustainability:emergency_first_aid_kits","@type":["rdf:Property","owl:DatatypeProperty"],"rdfs:label":"emergency_first_aid_kits","schema:rangeIncludes":{"@id":"xsd:boolean"},"schema:domainIncludes":{"@id":"sustainability:ConditionsOfWork"},"rdfs:comment":"Does the standard include criteria relating to emergency first aid kits"},{"@id":"sustainability:safety_procedures_for_handling_chemicals","@type":["rdf:Property","owl:DatatypeProperty"],"rdfs:label":"safety_procedures_for_handling_chemicals","schema:rangeIncludes":{"@id":"xsd:boolean"},"schema:domainIncludes":{"@id":"sustainability:ConditionsOfWork"},"rdfs:comment":"Does the standard include criteria relating to the safe handling of chemicals at work?"},{"@id":"sustainability:monitoring_of_accidents_records","@type":["rdf:Property","owl:DatatypeProperty"],"rdfs:label":"monitoring_of_accidents_records","schema:rangeIncludes":{"@id":"xsd:boolean"},"schema:domainIncludes":{"@id":"sustainability:ConditionsOfWork"},"rdfs:comment":"Does the standard require the monitoring of accidents records?"},{"@id":"sustainability:women_s_rights_at_work","@type":["rdf:Property","owl:DatatypeProperty"],"rdfs:label":"women_s_rights_at_work","schema:rangeIncludes":{"@id":"xsd:boolean"},"schema:domainIncludes":{"@id":"sustainability:ConditionsOfWork"},"rdfs:comment":"Does the standard include explicit criteria to protect women rights at work?"},{"@id":"sustainability:training_of_workers_on_procedures_to_deal_with_accidents","@type":["rdf:Property","owl:DatatypeProperty"],"rdfs:label":"training_of_workers_on_procedures_to_deal_with_accidents","schema:rangeIncludes":{"@id":"xsd:boolean"},"schema:domainIncludes":{"@id":"sustainability:ConditionsOfWork"},"rdfs:comment":"Does the standard require the provision of trainings for workers on procedures to deal with accidents"},{"@id":"sustainability:regular_medical_checks","@type":["rdf:Property","owl:DatatypeProperty"],"rdfs:label":"regular_medical_checks","schema:rangeIncludes":{"@id":"xsd:boolean"},"schema:domainIncludes":{"@id":"sustainability:ConditionsOfWork"},"rdfs:comment":"Does the standard include criteria on the provision of regular medical checks for workers (including farmers)?"},{"@id":"sustainability:workers_access_to_safe_drinking_water","@type":["rdf:Property","owl:DatatypeProperty"],"rdfs:label":"workers_access_to_safe_drinking_water","schema:rangeIncludes":{"@id":"xsd:boolean"},"schema:domainIncludes":{"@id":"sustainability:ConditionsOfWork"},"rdfs:comment":"Does the standard include criteria relating to workers’ access to safe drinking water?"},{"@id":"sustainability:workers_access_to_decent_sanitary_facilities_at_work_showers_wc_changing_rooms_etc","@type":["rdf:Property","owl:DatatypeProperty"],"rdfs:label":"workers_access_to_decent_sanitary_facilities_at_work_showers_wc_changing_rooms_etc","schema:rangeIncludes":{"@id":"xsd:boolean"},"schema:domainIncludes":{"@id":"sustainability:ConditionsOfWork"},"rdfs:comment":"Does the standard require workers to have access to decent sanitary facilities in the workplace?"},{"@id":"sustainability:workplace_conditions_air_quality_lighting_noise","@type":["rdf:Property","owl:DatatypeProperty"],"rdfs:label":"workplace_conditions_air_quality_lighting_noise","schema:rangeIncludes":{"@id":"sustainability:WorkplaceConditionsAirQualityLightingNoise"},"schema:domainIncludes":{"@id":"sustainability:ConditionsOfWork"},"rdfs:comment":"Does the standard include requirements on workplace conditions (air quality, ligthing, noise…)?"},{"@id":"sustainability:safe_and_appropriate_housing_conditions_incl_dormitories_and_canteens_for_workers","@type":["rdf:Property","owl:DatatypeProperty"],"rdfs:label":"safe_and_appropriate_housing_conditions_incl_dormitories_and_canteens_for_workers","schema:rangeIncludes":{"@id":"xsd:boolean"},"schema:domainIncludes":{"@id":"sustainability:ConditionsOfWork"},"rdfs:comment":"Does the standard require safe and appropriate housing conditions (including dormitories and canteens) for workers ?"},{"@id":"sustainability:workers_entitlement_to_breaks_e_g_meal_breaks","@type":["rdf:Property","owl:DatatypeProperty"],"rdfs:label":"workers_entitlement_to_breaks_e_g_meal_breaks","schema:rangeIncludes":{"@id":"xsd:boolean"},"schema:domainIncludes":{"@id":"sustainability:ConditionsOfWork"},"rdfs:comment":"Does the standard require entitlement to breaks (e.g. meal breaks) for workers"},{"@id":"sustainability:workers_access_to_basic_medical_services","@type":["rdf:Property","owl:DatatypeProperty"],"rdfs:label":"workers_access_to_basic_medical_services","schema:rangeIncludes":{"@id":"sustainability:WorkersAccessToBasicMedicalServices"},"schema:domainIncludes":{"@id":"sustainability:ConditionsOfWork"},"rdfs:comment":"Does the standard include criteria on the access to basic medical services for workers?"},{"@id":"sustainability:policies_that_prohibit_the_use_of_physical_violence_intimidation_etc","@type":["rdf:Property","owl:DatatypeProperty"],"rdfs:label":"policies_that_prohibit_the_use_of_physical_violence_intimidation_etc","schema:rangeIncludes":{"@id":"xsd:boolean"},"schema:domainIncludes":{"@id":"sustainability:ConditionsOfWork"},"rdfs:comment":"Does the standard prohibit harassment or abuse of workers?"},{"@id":"sustainability:keeping_records_of_disciplinary_measures","@type":["rdf:Property","owl:DatatypeProperty"],"rdfs:label":"keeping_records_of_disciplinary_measures","schema:rangeIncludes":{"@id":"xsd:boolean"},"schema:domainIncludes":{"@id":"sustainability:ConditionsOfWork"},"rdfs:comment":"Does the standard include criteria relating to keeping records of disciplinary measures"},{"@id":"sustainability:sexual_exploitation_harassment","@type":["rdf:Property","owl:DatatypeProperty"],"rdfs:label":"sexual_exploitation_harassment","schema:rangeIncludes":{"@id":"xsd:boolean"},"schema:domainIncludes":{"@id":"sustainability:ConditionsOfWork"},"rdfs:comment":"Does the standard incllude explicit criteria to protect permanent and temporary workers from any type of sexual exploitation or harassment?"},{"@id":"sustainability:security_issues_role_and_behavior_of_security_guards","@type":["rdf:Property","owl:DatatypeProperty"],"rdfs:label":"security_issues_role_and_behavior_of_security_guards","schema:rangeIncludes":{"@id":"xsd:boolean"},"schema:domainIncludes":{"@id":"sustainability:ConditionsOfWork"},"rdfs:comment":"Does the standard require the implementation of policies relating to security issues / role and behavior of security guards"},{"@id":"sustainability:privacy_protection","@type":["rdf:Property","owl:DatatypeProperty"],"rdfs:label":"privacy_protection","schema:rangeIncludes":{"@id":"xsd:boolean"},"schema:domainIncludes":{"@id":"sustainability:ConditionsOfWork"},"rdfs:comment":"Does the standard require policies to be in place for privacy protection"},{"@id":"sustainability:worst_forms_of_child_labor_ilo182","@type":["rdf:Property","owl:DatatypeProperty"],"rdfs:label":"worst_forms_of_child_labor_ilo182","schema:rangeIncludes":{"@id":"xsd:boolean"},"schema:domainIncludes":{"@id":"sustainability:ConditionsOfWork"},"rdfs:comment":"Does the standard prohibit the worst forms of child labour as defined under ILO 182?"},{"@id":"sustainability:other_conditions_of_work","@type":["rdf:Property","owl:DatatypeProperty"],"rdfs:label":"other_conditions_of_work","schema:rangeIncludes":{"@id":"xsd:string"},"schema:domainIncludes":{"@id":"sustainability:ConditionsOfWork"},"rdfs:comment":"Does the standard include other work/labor rights not covered in previous list"},{"@id":"sustainability:safety_at_work_ilo184","@type":["rdf:Property","owl:DatatypeProperty"],"rdfs:label":"safety_at_work_ilo184","schema:rangeIncludes":{"@id":"sustainability:SafetyAtWorkIlo184"},"schema:domainIncludes":{"@id":"sustainability:ConditionsOfWork"},"rdfs:comment":"Does the standard address requirements for safety at work related to workers' health and safety, as defined in ILO 184?"},{"@id":"sustainability:safety_at_work_legal_compliance","@type":["rdf:Property","owl:DatatypeProperty"],"rdfs:label":"safety_at_work_legal_compliance","schema:rangeIncludes":{"@id":"xsd:boolean"},"schema:domainIncludes":{"@id":"sustainability:ConditionsOfWork"},"rdfs:comment":"Does the standard explicitely require the unit of operation to comply with all international and legal requirements related to safety at work?"},{"@id":"sustainability:electrical_equipments_safety","@type":["rdf:Property","owl:DatatypeProperty"],"rdfs:label":"electrical_equipments_safety","schema:rangeIncludes":{"@id":"xsd:boolean"},"schema:domainIncludes":{"@id":"sustainability:ConditionsOfWork"},"rdfs:comment":"Does the standard require regular and proper maintenance of electrical equipment?"},{"@id":"sustainability:policies_in_place_for_verification_and_maintenance_of_buildings_safety","@type":["rdf:Property","owl:DatatypeProperty"],"rdfs:label":"policies_in_place_for_verification_and_maintenance_of_buildings_safety","schema:rangeIncludes":{"@id":"xsd:boolean"},"schema:domainIncludes":{"@id":"sustainability:ConditionsOfWork"},"rdfs:comment":"Does the standard include criteria on the verification and maintenance of buidling safety."},{"@id":"sustainability:fire_preparedness_drills_equipment_signs","@type":["rdf:Property","owl:DatatypeProperty"],"rdfs:label":"fire_preparedness_drills_equipment_signs","schema:rangeIncludes":{"@id":"xsd:boolean"},"schema:domainIncludes":{"@id":"sustainability:ConditionsOfWork"},"rdfs:comment":"Does the standard include criteria on fire preparedness (e.g. drills, equipment, signs, etc."},{"@id":"sustainability:documented_emergency_management_plan","@type":["rdf:Property","owl:DatatypeProperty"],"rdfs:label":"documented_emergency_management_plan","schema:rangeIncludes":{"@id":"xsd:boolean"},"schema:domainIncludes":{"@id":"sustainability:ConditionsOfWork"},"rdfs:comment":"Does the standard require the unit of operation to have in place an emergency management plan"},{"@id":"sustainability:conditions_of_employment_general_principle","@type":["rdf:Property","owl:DatatypeProperty"],"rdfs:label":"conditions_of_employment_general_principle","schema:rangeIncludes":{"@id":"xsd:string"},"schema:domainIncludes":{"@id":"sustainability:Employment"},"rdfs:comment":"Does the standard have a general principle on conditions of employment"},{"@id":"sustainability:workers_access_to_medical_insurance","@type":["rdf:Property","owl:DatatypeProperty"],"rdfs:label":"workers_access_to_medical_insurance","schema:rangeIncludes":{"@id":"xsd:boolean"},"schema:domainIncludes":{"@id":"sustainability:Employment"},"rdfs:comment":"Does the standard address requirements for medical insurance in the workplace"},{"@id":"sustainability:human_resources_management_general_principle","@type":["rdf:Property","owl:DatatypeProperty"],"rdfs:label":"human_resources_management_general_principle","schema:rangeIncludes":{"@id":"xsd:boolean"},"schema:domainIncludes":{"@id":"sustainability:Employment"},"rdfs:comment":"Does the standard include criteria related to the management of human resources"},{"@id":"sustainability:employment_hiring_practices_legal_compliance","@type":["rdf:Property","owl:DatatypeProperty"],"rdfs:label":"employment_hiring_practices_legal_compliance","schema:rangeIncludes":{"@id":"xsd:boolean"},"schema:domainIncludes":{"@id":"sustainability:Employment"},"rdfs:comment":"Does the standard require the unit of operation to comply with national regulation on employment / hiring practices?"},{"@id":"sustainability:migrant_workers_employment_and_contract_management","@type":["rdf:Property","owl:DatatypeProperty"],"rdfs:label":"migrant_workers_employment_and_contract_management","schema:rangeIncludes":{"@id":"xsd:boolean"},"schema:domainIncludes":{"@id":"sustainability:Employment"},"rdfs:comment":"Does the standard include criteria on migrant workers' employment and contract management regarding the protection of their labour rights"},{"@id":"sustainability:workforce_reduction_policies_and_practices_legal_compliance","@type":["rdf:Property","owl:DatatypeProperty"],"rdfs:label":"workforce_reduction_policies_and_practices_legal_compliance","schema:rangeIncludes":{"@id":"xsd:boolean"},"schema:domainIncludes":{"@id":"sustainability:Employment"},"rdfs:comment":"Does the standard require legal compliance with workforce reduction policies and practices"},{"@id":"sustainability:payroll_records_and_pay_slips","@type":["rdf:Property","owl:DatatypeProperty"],"rdfs:label":"payroll_records_and_pay_slips","schema:rangeIncludes":{"@id":"xsd:boolean"},"schema:domainIncludes":{"@id":"sustainability:Employment"},"rdfs:comment":"Does the standard include criteria relating to payroll records and pay slips"},{"@id":"sustainability:workers_performance_for_promotion_trainings","@type":["rdf:Property","owl:DatatypeProperty"],"rdfs:label":"workers_performance_for_promotion_trainings","schema:rangeIncludes":{"@id":"xsd:boolean"},"schema:domainIncludes":{"@id":"sustainability:Employment"},"rdfs:comment":"Does the standard include criteria relating to workers' performance assessment (for promotion, trainings…)"},{"@id":"sustainability:illegal_excessive_deductions_or_fees_incl_recruitment_fees","@type":["rdf:Property","owl:DatatypeProperty"],"rdfs:label":"illegal_excessive_deductions_or_fees_incl_recruitment_fees","schema:rangeIncludes":{"@id":"xsd:boolean"},"schema:domainIncludes":{"@id":"sustainability:Employment"},"rdfs:comment":"Does the standard include criteria preventing the illegal or excessive deduction of recruitment fees (including visa fees)"},{"@id":"sustainability:workers_equipment_costs_incl_uniforms","@type":["rdf:Property","owl:DatatypeProperty"],"rdfs:label":"workers_equipment_costs_incl_uniforms","schema:rangeIncludes":{"@id":"xsd:boolean"},"schema:domainIncludes":{"@id":"sustainability:Employment"},"rdfs:comment":"Does the standard include criteria relating to workers equipment costs (incl. uniforms)"},{"@id":"sustainability:retention_of_workers_documentation_id_passport","@type":["rdf:Property","owl:DatatypeProperty"],"rdfs:label":"retention_of_workers_documentation_id_passport","schema:rangeIncludes":{"@id":"xsd:boolean"},"schema:domainIncludes":{"@id":"sustainability:Employment"},"rdfs:comment":"Does the standard prohibit the withholding of workers' documents?"},{"@id":"sustainability:existence_of_publicly_available_policy_defining_workers_rights","@type":["rdf:Property","owl:DatatypeProperty"],"rdfs:label":"existence_of_publicly_available_policy_defining_workers_rights","schema:rangeIncludes":{"@id":"xsd:boolean"},"schema:domainIncludes":{"@id":"sustainability:Employment"},"rdfs:comment":"Does the standard require the unit of operaton to develop and make publicly available a policy defining workers' rights"},{"@id":"sustainability:use_of_legally_binding_labour_contracts_in_written_form","@type":["rdf:Property","owl:DatatypeProperty"],"rdfs:label":"use_of_legally_binding_labour_contracts_in_written_form","schema:rangeIncludes":{"@id":"xsd:boolean"},"schema:domainIncludes":{"@id":"sustainability:Employment"},"rdfs:comment":"Does the standard require formal written contracts versus verbal agreements"},{"@id":"sustainability:scope_of_workers_rights_and_benefits_applicable_equally_to_all_types_of_workers","@type":["rdf:Property","owl:DatatypeProperty"],"rdfs:label":"scope_of_workers_rights_and_benefits_applicable_equally_to_all_types_of_workers","schema:rangeIncludes":{"@id":"xsd:boolean"},"schema:domainIncludes":{"@id":"sustainability:Employment"},"rdfs:comment":"Does the standard require that workers' rights and benefits apply equally to all types of workers"},{"@id":"sustainability:distinct_home_workers","@type":["rdf:Property","owl:DatatypeProperty"],"rdfs:label":"distinct_home_workers","schema:rangeIncludes":{"@id":"xsd:boolean"},"schema:domainIncludes":{"@id":"sustainability:Employment"},"rdfs:comment":"Does the standard has specific policies and criteria related to the use of home-workers"},{"@id":"sustainability:equal_rights_and_benefits_applicable_to_full_time_and_sub_contract_workers","@type":["rdf:Property","owl:DatatypeProperty"],"rdfs:label":"equal_rights_and_benefits_applicable_to_full_time_and_sub_contract_workers","schema:rangeIncludes":{"@id":"xsd:boolean"},"schema:domainIncludes":{"@id":"sustainability:Employment"},"rdfs:comment":"Do the standard's rights and benefits for workers also apply to sub-contracted labour?"},{"@id":"sustainability:workers_mobility_and_freedom_of_movement","@type":["rdf:Property","owl:DatatypeProperty"],"rdfs:label":"workers_mobility_and_freedom_of_movement","schema:rangeIncludes":{"@id":"xsd:boolean"},"schema:domainIncludes":{"@id":"sustainability:Employment"},"rdfs:comment":"Does the standard include criteria on the freedom of movement of employees?"},{"@id":"sustainability:paid_leave_general_policy_public_holidays_annual_leave_sick_leave_casual_leave","@type":["rdf:Property","owl:DatatypeProperty"],"rdfs:label":"paid_leave_general_policy_public_holidays_annual_leave_sick_leave_casual_leave","schema:rangeIncludes":{"@id":"sustainability:PaidLeaveGeneralPolicyPublicHolidaysAnnualLeaveSickLeaveCasualLeave"},"schema:domainIncludes":{"@id":"sustainability:Employment"},"rdfs:comment":"Does the standard require a general policy on the number and types of leave days, including public holidays and annual leave?"},{"@id":"sustainability:1_rest_day_off_in7_days_period_or_more_stringent_policy","@type":["rdf:Property","owl:DatatypeProperty"],"rdfs:label":"1_rest_day_off_in7_days_period_or_more_stringent_policy","schema:rangeIncludes":{"@id":"xsd:boolean"},"schema:domainIncludes":{"@id":"sustainability:Employment"},"rdfs:comment":"Does the standard require that all workers have the right to at least one rest day in 7-days period"},{"@id":"sustainability:specific_maternity_paternity_leave_days","@type":["rdf:Property","owl:DatatypeProperty"],"rdfs:label":"specific_maternity_paternity_leave_days","schema:rangeIncludes":{"@id":"sustainability:SpecificMaternityPaternityLeaveDays"},"schema:domainIncludes":{"@id":"sustainability:Employment"},"rdfs:comment":"Does the standard include criteria on the right to maternity leave (as defined in ILO 183)?"},{"@id":"sustainability:specific_special_leave_sickness_marriage_paternity_family_leave","@type":["rdf:Property","owl:DatatypeProperty"],"rdfs:label":"specific_special_leave_sickness_marriage_paternity_family_leave","schema:rangeIncludes":{"@id":"xsd:boolean"},"schema:domainIncludes":{"@id":"sustainability:Employment"},"rdfs:comment":"Does the standard include criteria related to special leave days, including sickness, marriage, family leave"},{"@id":"sustainability:fair_and_timely_payment_of_wages","@type":["rdf:Property","owl:DatatypeProperty"],"rdfs:label":"fair_and_timely_payment_of_wages","schema:rangeIncludes":{"@id":"sustainability:FairAndTimelyPaymentOfWages"},"schema:domainIncludes":{"@id":"sustainability:Employment"},"rdfs:comment":"Does the standard require wages to be paid in a timely, regular and convenient manner understood by all employees?"},{"@id":"sustainability:voluntary_employment_no_forced_labor_ilo29105","@type":["rdf:Property","owl:DatatypeProperty"],"rdfs:label":"voluntary_employment_no_forced_labor_ilo29105","schema:rangeIncludes":{"@id":"xsd:boolean"},"schema:domainIncludes":{"@id":"sustainability:Employment"},"rdfs:comment":"Does the standard prohibit forced and compulsory labour as defined in ILO 29 and ILO 105?"},{"@id":"sustainability:pensions_and_social_security_benefits","@type":["rdf:Property","owl:DatatypeProperty"],"rdfs:label":"pensions_and_social_security_benefits","schema:rangeIncludes":{"@id":"xsd:boolean"},"schema:domainIncludes":{"@id":"sustainability:Employment"},"rdfs:comment":"Does the standard require the provision of pensions and social security benefits"},{"@id":"sustainability:waivers_national_exemptions_to_full_scope_coverage_of_social_benefits_for_all_employees","@type":["rdf:Property","owl:DatatypeProperty"],"rdfs:label":"waivers_national_exemptions_to_full_scope_coverage_of_social_benefits_for_all_employees","schema:rangeIncludes":{"@id":"xsd:boolean"},"schema:domainIncludes":{"@id":"sustainability:Employment"},"rdfs:comment":"Does the standard address waivers/national exemptions to full scope coverage of social benefits for all employees"},{"@id":"sustainability:transportation_of_workers_to_production_site","@type":["rdf:Property","owl:DatatypeProperty"],"rdfs:label":"transportation_of_workers_to_production_site","schema:rangeIncludes":{"@id":"xsd:boolean"},"schema:domainIncludes":{"@id":"sustainability:Employment"},"rdfs:comment":"Does the standard include criteria related to the transportation of workers from their living place to the production site"},{"@id":"sustainability:securing_a_minimum_wage_based_on_sector_or_region_specificities","@type":["rdf:Property","owl:DatatypeProperty"],"rdfs:label":"securing_a_minimum_wage_based_on_sector_or_region_specificities","schema:rangeIncludes":{"@id":"xsd:boolean"},"schema:domainIncludes":{"@id":"sustainability:Employment"},"rdfs:comment":"Does the standard has specific criteria to ensure workers are paid minimum legal wages based on sector or region specificities?"},{"@id":"sustainability:living_wage_based_on_sector_or_region_specificities","@type":["rdf:Property","owl:DatatypeProperty"],"rdfs:label":"living_wage_based_on_sector_or_region_specificities","schema:rangeIncludes":{"@id":"xsd:boolean"},"schema:domainIncludes":{"@id":"sustainability:Employment"},"rdfs:comment":"Does the standard require paying wages sufficient to meet basic needs of the worker and his or her family (living wage)?"},{"@id":"sustainability:wage_compensation_issues_and_policies_forced_days_of_lock_outs_meetings_outside_pay_time","@type":["rdf:Property","owl:DatatypeProperty"],"rdfs:label":"wage_compensation_issues_and_policies_forced_days_of_lock_outs_meetings_outside_pay_time","schema:rangeIncludes":{"@id":"xsd:boolean"},"schema:domainIncludes":{"@id":"sustainability:Employment"},"rdfs:comment":"Does the standard address wage compensation issues and policies for workers?"},{"@id":"sustainability:child_labor_and_minimum_age_ilo138","@type":["rdf:Property","owl:DatatypeProperty"],"rdfs:label":"child_labor_and_minimum_age_ilo138","schema:rangeIncludes":{"@id":"xsd:boolean"},"schema:domainIncludes":{"@id":"sustainability:Employment"},"rdfs:comment":"Does the standard include criteria on the prohibition of child labour as defined under ILO 138?"},{"@id":"sustainability:child_labour_legal_compliance_policy","@type":["rdf:Property","owl:DatatypeProperty"],"rdfs:label":"child_labour_legal_compliance_policy","schema:rangeIncludes":{"@id":"xsd:boolean"},"schema:domainIncludes":{"@id":"sustainability:Employment"},"rdfs:comment":"Does the standard require legal compliance with child labour regulations?"},{"@id":"sustainability:maintaining_age_records_of_workers","@type":["rdf:Property","owl:DatatypeProperty"],"rdfs:label":"maintaining_age_records_of_workers","schema:rangeIncludes":{"@id":"xsd:boolean"},"schema:domainIncludes":{"@id":"sustainability:Employment"},"rdfs:comment":"Does the standard require keeping age records of workers?"},{"@id":"sustainability:child_labour_remediation_policy_including_assistance_to_child_workers_and_their_families","@type":["rdf:Property","owl:DatatypeProperty"],"rdfs:label":"child_labour_remediation_policy_including_assistance_to_child_workers_and_their_families","schema:rangeIncludes":{"@id":"xsd:boolean"},"schema:domainIncludes":{"@id":"sustainability:Employment"},"rdfs:comment":"Does the standard require that assistance be provided to replaced child workers upon compliance with the standard?"},{"@id":"sustainability:waivers_national_exemptions_to_maximum_working_hours","@type":["rdf:Property","owl:DatatypeProperty"],"rdfs:label":"waivers_national_exemptions_to_maximum_working_hours","schema:rangeIncludes":{"@id":"xsd:boolean"},"schema:domainIncludes":{"@id":"sustainability:Employment"},"rdfs:comment":"Does the standard include criteria on waivers / national exemptions to maximum working hours?"},{"@id":"sustainability:hiring_and_employing_young_workers","@type":["rdf:Property","owl:DatatypeProperty"],"rdfs:label":"hiring_and_employing_young_workers","schema:rangeIncludes":{"@id":"xsd:boolean"},"schema:domainIncludes":{"@id":"sustainability:Employment"},"rdfs:comment":"Does the standard include criteria on hiring and employing young workers?"},{"@id":"sustainability:good_conditions_of_work_for_young_workers","@type":["rdf:Property","owl:DatatypeProperty"],"rdfs:label":"good_conditions_of_work_for_young_workers","schema:rangeIncludes":{"@id":"xsd:boolean"},"schema:domainIncludes":{"@id":"sustainability:Employment"},"rdfs:comment":"Does the standard require good working conditions for young workers"},{"@id":"sustainability:young_workers_working_hours","@type":["rdf:Property","owl:DatatypeProperty"],"rdfs:label":"young_workers_working_hours","schema:rangeIncludes":{"@id":"xsd:boolean"},"schema:domainIncludes":{"@id":"sustainability:Employment"},"rdfs:comment":"Does the standard address young workers' working hours"},{"@id":"sustainability:training_programs_for_young_workers","@type":["rdf:Property","owl:DatatypeProperty"],"rdfs:label":"training_programs_for_young_workers","schema:rangeIncludes":{"@id":"xsd:boolean"},"schema:domainIncludes":{"@id":"sustainability:Employment"},"rdfs:comment":"Does the standard promote young workers' access to training approved by the competent authority"},{"@id":"sustainability:young_workers_access_to_effective_grievance_mechanisms","@type":["rdf:Property","owl:DatatypeProperty"],"rdfs:label":"young_workers_access_to_effective_grievance_mechanisms","schema:rangeIncludes":{"@id":"xsd:boolean"},"schema:domainIncludes":{"@id":"sustainability:Employment"},"rdfs:comment":"Does the standard address issues relating to young workers' access to effective grievance mechanisms"},{"@id":"sustainability:young_workers_trained_on_occupational_health_and_safety","@type":["rdf:Property","owl:DatatypeProperty"],"rdfs:label":"young_workers_trained_on_occupational_health_and_safety","schema:rangeIncludes":{"@id":"xsd:boolean"},"schema:domainIncludes":{"@id":"sustainability:Employment"},"rdfs:comment":"Does the standard require training on Occupational Health and Safety for young workers"},{"@id":"sustainability:equal_remuneration_ilo100","@type":["rdf:Property","owl:DatatypeProperty"],"rdfs:label":"equal_remuneration_ilo100","schema:rangeIncludes":{"@id":"xsd:boolean"},"schema:domainIncludes":{"@id":"sustainability:Employment"},"rdfs:comment":"Does the standard includes criteria related to equal remuneration, as defined by ILO 100?"},{"@id":"sustainability:maximum_working_hours","@type":["rdf:Property","owl:DatatypeProperty"],"rdfs:label":"maximum_working_hours","schema:rangeIncludes":{"@id":"xsd:boolean"},"schema:domainIncludes":{"@id":"sustainability:Employment"},"rdfs:comment":"Does the standard include criteria on working hours, as defined in ILO Convention 1?"},{"@id":"sustainability:hours_of_work_overtime_monitoring","@type":["rdf:Property","owl:DatatypeProperty"],"rdfs:label":"hours_of_work_overtime_monitoring","schema:rangeIncludes":{"@id":"xsd:boolean"},"schema:domainIncludes":{"@id":"sustainability:Employment"},"rdfs:comment":"Does the standard include criteria related to hours of work and overtime monitoring"},{"@id":"sustainability:other_the_conditions_of_employment","@type":["rdf:Property","owl:DatatypeProperty"],"rdfs:label":"other_the_conditions_of_employment","schema:rangeIncludes":{"@id":"xsd:string"},"schema:domainIncludes":{"@id":"sustainability:Employment"},"rdfs:comment":"Does the standard address other conditions of employment not covered above"},{"@id":"sustainability:right_to_refuse_overtime","@type":["rdf:Property","owl:DatatypeProperty"],"rdfs:label":"right_to_refuse_overtime","schema:rangeIncludes":{"@id":"xsd:boolean"},"schema:domainIncludes":{"@id":"sustainability:Employment"},"rdfs:comment":"Does the standard explicitely state that workers have the right to refuse overtime"},{"@id":"sustainability:overtime_is_voluntary_and_compensated","@type":["rdf:Property","owl:DatatypeProperty"],"rdfs:label":"overtime_is_voluntary_and_compensated","schema:rangeIncludes":{"@id":"xsd:boolean"},"schema:domainIncludes":{"@id":"sustainability:Employment"},"rdfs:comment":"Does the standard require compensation for overtime?"},{"@id":"sustainability:the_use_of_prison_labor","@type":["rdf:Property","owl:DatatypeProperty"],"rdfs:label":"the_use_of_prison_labor","schema:rangeIncludes":{"@id":"xsd:boolean"},"schema:domainIncludes":{"@id":"sustainability:Employment"},"rdfs:comment":"Does the standard include criteria related to voluntary prison labou"},{"@id":"sustainability:use_of_formal_format_or_template_for_labour_contracts","@type":["rdf:Property","owl:DatatypeProperty"],"rdfs:label":"use_of_formal_format_or_template_for_labour_contracts","schema:rangeIncludes":{"@id":"xsd:boolean"},"schema:domainIncludes":{"@id":"sustainability:Employment"},"rdfs:comment":"Does the standard require a formal format or template for labour contracts in which all rights and obligations of workers are defined?"},{"@id":"sustainability:workers_compensation_for_medical_costs_in_case_of_work_related_accidents","@type":["rdf:Property","owl:DatatypeProperty"],"rdfs:label":"workers_compensation_for_medical_costs_in_case_of_work_related_accidents","schema:rangeIncludes":{"@id":"sustainability:WorkersCompensationForMedicalCostsInCaseOfWorkRelatedAccidents"},"schema:domainIncludes":{"@id":"sustainability:Employment"},"rdfs:comment":"Does the standard require compensation payments/ covering of costs in case of work related accidents and injuries?"},{"@id":"sustainability:freedom_of_association_ilo87","@type":["rdf:Property","owl:DatatypeProperty"],"rdfs:label":"freedom_of_association_ilo87","schema:rangeIncludes":{"@id":"xsd:boolean"},"schema:domainIncludes":{"@id":"sustainability:HumanDevelopment"},"rdfs:comment":"Does the standard promote the right to freedom of association, as defined in ILO 87?"},{"@id":"sustainability:formation_of_workers_representation_in_countries_where_freedom_of_association_and_collective_bargaining_is_not_supported_by_legislation","@type":["rdf:Property","owl:DatatypeProperty"],"rdfs:label":"formation_of_workers_representation_in_countries_where_freedom_of_association_and_collective_bargaining_is_not_supported_by_legislation","schema:rangeIncludes":{"@id":"sustainability:FormationOfWorkersRepresentationInCountriesWhereFreedomOfAssociationAndCollectiveBargainingIsNotSupportedByLegislation"},"schema:domainIncludes":{"@id":"sustainability:HumanDevelopment"},"rdfs:comment":"Does the standard include criteria on the formation of workers representations where freedom of association is restricted by law?"},{"@id":"sustainability:workers_awareness_of_procedures_and_best_practices","@type":["rdf:Property","owl:DatatypeProperty"],"rdfs:label":"workers_awareness_of_procedures_and_best_practices","schema:rangeIncludes":{"@id":"xsd:boolean"},"schema:domainIncludes":{"@id":"sustainability:HumanDevelopment"},"rdfs:comment":"Does the standard require that workers are made aware of procedures and best practices?"},{"@id":"sustainability:policies_and_procedures_to_address_workers_grievances","@type":["rdf:Property","owl:DatatypeProperty"],"rdfs:label":"policies_and_procedures_to_address_workers_grievances","schema:rangeIncludes":{"@id":"xsd:boolean"},"schema:domainIncludes":{"@id":"sustainability:HumanDevelopment"},"rdfs:comment":"Does the standard require worker grievance mechanisms to be in place?"},{"@id":"sustainability:gender_policies_at_work_general_principles","@type":["rdf:Property","owl:DatatypeProperty"],"rdfs:label":"gender_policies_at_work_general_principles","schema:rangeIncludes":{"@id":"xsd:boolean"},"schema:domainIncludes":{"@id":"sustainability:HumanDevelopment"},"rdfs:comment":"Does the standard include a general principle addressing gender policies at work"},{"@id":"sustainability:gender_policies_family_friendly_policies_to_increase_the_labour_force_participation_of_women","@type":["rdf:Property","owl:DatatypeProperty"],"rdfs:label":"gender_policies_family_friendly_policies_to_increase_the_labour_force_participation_of_women","schema:rangeIncludes":{"@id":"xsd:boolean"},"schema:domainIncludes":{"@id":"sustainability:HumanDevelopment"},"rdfs:comment":"Does the standard promote active female participation through the implementation of family friendly policies"},{"@id":"sustainability:gender_policies_development_assistance_policies_which_promote_the_economic_role_of_women","@type":["rdf:Property","owl:DatatypeProperty"],"rdfs:label":"gender_policies_development_assistance_policies_which_promote_the_economic_role_of_women","schema:rangeIncludes":{"@id":"xsd:boolean"},"schema:domainIncludes":{"@id":"sustainability:HumanDevelopment"},"rdfs:comment":"Does the standard encourage the implementation of development assistance policies aimed at promoting the economic role of women"},{"@id":"sustainability:gender_policies_upgrading_the_status_of_and_wages_for_traditional_areas_of_women_s_work","@type":["rdf:Property","owl:DatatypeProperty"],"rdfs:label":"gender_policies_upgrading_the_status_of_and_wages_for_traditional_areas_of_women_s_work","schema:rangeIncludes":{"@id":"xsd:boolean"},"schema:domainIncludes":{"@id":"sustainability:HumanDevelopment"},"rdfs:comment":"Does the standard promote upgrading the status of and wages for traditional areas of women's work (e.g. employment conditions, increased degree of professionalisation, higher pay and more training and career opportunities)"},{"@id":"sustainability:gender_policies_incentives_to_women_to_develop_their_careers_e_g_specific_training","@type":["rdf:Property","owl:DatatypeProperty"],"rdfs:label":"gender_policies_incentives_to_women_to_develop_their_careers_e_g_specific_training","schema:rangeIncludes":{"@id":"xsd:boolean"},"schema:domainIncludes":{"@id":"sustainability:HumanDevelopment"},"rdfs:comment":"Does the standard promote incentives for women to develop their careers (e.g. training)"},{"@id":"sustainability:gender_policies_increased_access_to_finance_and_support_services_for_women_entrepreneurs","@type":["rdf:Property","owl:DatatypeProperty"],"rdfs:label":"gender_policies_increased_access_to_finance_and_support_services_for_women_entrepreneurs","schema:rangeIncludes":{"@id":"xsd:boolean"},"schema:domainIncludes":{"@id":"sustainability:HumanDevelopment"},"rdfs:comment":"Does the standard promote the implementation of gender policies to increase access to finance and support services for women entrepreneurs"},{"@id":"sustainability:gender_policies_integration_of_women_migrants_into_labor_force","@type":["rdf:Property","owl:DatatypeProperty"],"rdfs:label":"gender_policies_integration_of_women_migrants_into_labor_force","schema:rangeIncludes":{"@id":"xsd:boolean"},"schema:domainIncludes":{"@id":"sustainability:HumanDevelopment"},"rdfs:comment":"Does the standard encourage the integration of women migrants into labor force"},{"@id":"sustainability:collective_bargaining_ilo98","@type":["rdf:Property","owl:DatatypeProperty"],"rdfs:label":"collective_bargaining_ilo98","schema:rangeIncludes":{"@id":"xsd:boolean"},"schema:domainIncludes":{"@id":"sustainability:HumanDevelopment"},"rdfs:comment":"Does the standard promote the right to collective bargaining, as defined in ILO 98?"},{"@id":"sustainability:policies_and_procedures_to_monitor_workers_satisfaction_at_work","@type":["rdf:Property","owl:DatatypeProperty"],"rdfs:label":"policies_and_procedures_to_monitor_workers_satisfaction_at_work","schema:rangeIncludes":{"@id":"xsd:boolean"},"schema:domainIncludes":{"@id":"sustainability:HumanDevelopment"},"rdfs:comment":"Does the standard require processes to be in place for the monitoring of workers' satisfaction in the workplace?"},{"@id":"sustainability:other_empowerment_of_workers","@type":["rdf:Property","owl:DatatypeProperty"],"rdfs:label":"other_empowerment_of_workers","schema:rangeIncludes":{"@id":"xsd:string"},"schema:domainIncludes":{"@id":"sustainability:HumanDevelopment"},"rdfs:comment":"Does the standard address other social/human rights issues not covered in previous criteria"},{"@id":"sustainability:no_discrimination_at_work_ilo111","@type":["rdf:Property","owl:DatatypeProperty"],"rdfs:label":"no_discrimination_at_work_ilo111","schema:rangeIncludes":{"@id":"xsd:boolean"},"schema:domainIncludes":{"@id":"sustainability:HumanDevelopment"},"rdfs:comment":"Does the standard require adherence to non-discrimination in the workplace, as defined in ILO 111?"},{"@id":"sustainability:non_discrimination_based_on_gender","@type":["rdf:Property","owl:DatatypeProperty"],"rdfs:label":"non_discrimination_based_on_gender","schema:rangeIncludes":{"@id":"xsd:boolean"},"schema:domainIncludes":{"@id":"sustainability:HumanDevelopment"},"rdfs:comment":"Does the standard require policies and/ or processes in place that prevent discrimination based specifically on gender in the workplace?"},{"@id":"sustainability:non_discrimination_of_persons_with_disabilities","@type":["rdf:Property","owl:DatatypeProperty"],"rdfs:label":"non_discrimination_of_persons_with_disabilities","schema:rangeIncludes":{"@id":"xsd:boolean"},"schema:domainIncludes":{"@id":"sustainability:HumanDevelopment"},"rdfs:comment":"Does the standard include criteria on the non-discrimination of persons with disabilities"},{"@id":"sustainability:ensuring_participation_of_women_minorities_in_management","@type":["rdf:Property","owl:DatatypeProperty"],"rdfs:label":"ensuring_participation_of_women_minorities_in_management","schema:rangeIncludes":{"@id":"xsd:boolean"},"schema:domainIncludes":{"@id":"sustainability:HumanDevelopment"},"rdfs:comment":"Does the standard promote participation of women and/or minorities in management"},{"@id":"sustainability:workers_access_to_training_programs","@type":["rdf:Property","owl:DatatypeProperty"],"rdfs:label":"workers_access_to_training_programs","schema:rangeIncludes":{"@id":"xsd:boolean"},"schema:domainIncludes":{"@id":"sustainability:HumanDevelopment"},"rdfs:comment":"Does the standard include criteria on the provision of professional training for workers?"},{"@id":"sustainability:apprentice_programs_for_young_workers","@type":["rdf:Property","owl:DatatypeProperty"],"rdfs:label":"apprentice_programs_for_young_workers","schema:rangeIncludes":{"@id":"xsd:boolean"},"schema:domainIncludes":{"@id":"sustainability:HumanDevelopment"},"rdfs:comment":"Does the standard promote the provision of apprentice programs for young workers"},{"@id":"sustainability:joint_committees_trade_unions_labour_associations","@type":["rdf:Property","owl:DatatypeProperty"],"rdfs:label":"joint_committees_trade_unions_labour_associations","schema:rangeIncludes":{"@id":"xsd:boolean"},"schema:domainIncludes":{"@id":"sustainability:HumanDevelopment"},"rdfs:comment":"Does the standard explicitly require workers' to have input into management processes through joint committees or similar mechanism"},{"@id":"sustainability:business_operations_economic_viability_general_principle","@type":["rdf:Property","owl:DatatypeProperty"],"rdfs:label":"business_operations_economic_viability_general_principle","schema:rangeIncludes":{"@id":"xsd:string"},"schema:domainIncludes":{"@id":"sustainability:EconomicViability"},"rdfs:comment":"Does the standard system include a general principle on the financial resiliance (business viability) of the unit of operation?"},{"@id":"sustainability:fair_competition","@type":["rdf:Property","owl:DatatypeProperty"],"rdfs:label":"fair_competition","schema:rangeIncludes":{"@id":"xsd:boolean"},"schema:domainIncludes":{"@id":"sustainability:EconomicViability"},"rdfs:comment":"Does the standard system cover issues relating to fair competition"},{"@id":"sustainability:production_efficiency_productivity","@type":["rdf:Property","owl:DatatypeProperty"],"rdfs:label":"production_efficiency_productivity","schema:rangeIncludes":{"@id":"xsd:boolean"},"schema:domainIncludes":{"@id":"sustainability:EconomicViability"},"rdfs:comment":"Does the standard system include criteria on improving production efficiency / productivity?"},{"@id":"sustainability:diversification_of_business_operations","@type":["rdf:Property","owl:DatatypeProperty"],"rdfs:label":"diversification_of_business_operations","schema:rangeIncludes":{"@id":"xsd:boolean"},"schema:domainIncludes":{"@id":"sustainability:EconomicViability"},"rdfs:comment":"Does the standard system require consideration of options for business diversification?"},{"@id":"sustainability:long_term_sustainability_management_plan_continuous_improvement","@type":["rdf:Property","owl:DatatypeProperty"],"rdfs:label":"long_term_sustainability_management_plan_continuous_improvement","schema:rangeIncludes":{"@id":"xsd:boolean"},"schema:domainIncludes":{"@id":"sustainability:EconomicViability"},"rdfs:comment":"Does the standard include criteria on management plans for continuous improvement?"},{"@id":"sustainability:administration_and_management_business_plan","@type":["rdf:Property","owl:DatatypeProperty"],"rdfs:label":"administration_and_management_business_plan","schema:rangeIncludes":{"@id":"xsd:boolean"},"schema:domainIncludes":{"@id":"sustainability:EconomicViability"},"rdfs:comment":"Does the standard have a general principle on administration and management"},{"@id":"sustainability:environment_and_social_e_s_management_systems_general_principles","@type":["rdf:Property","owl:DatatypeProperty"],"rdfs:label":"environment_and_social_e_s_management_systems_general_principles","schema:rangeIncludes":{"@id":"xsd:string"},"schema:domainIncludes":{"@id":"sustainability:SustainabilityManagement"},"rdfs:comment":"Does the standard have a general principle related to Environment and Social (E&S) Management Systems"},{"@id":"sustainability:organizational_capacity_for_continuous_improvement_of_environmental_and_social_management","@type":["rdf:Property","owl:DatatypeProperty"],"rdfs:label":"organizational_capacity_for_continuous_improvement_of_environmental_and_social_management","schema:rangeIncludes":{"@id":"xsd:boolean"},"schema:domainIncludes":{"@id":"sustainability:SustainabilityManagement"},"rdfs:comment":"Does the standard address issues relating to organizational capacity for continuous improvement of environmental and social (E&S) management"},{"@id":"sustainability:procedures_to_monitor_and_measure_effectiveness_of_e_s_management_systems","@type":["rdf:Property","owl:DatatypeProperty"],"rdfs:label":"procedures_to_monitor_and_measure_effectiveness_of_e_s_management_systems","schema:rangeIncludes":{"@id":"xsd:boolean"},"schema:domainIncludes":{"@id":"sustainability:SustainabilityManagement"},"rdfs:comment":"Does the standard require procedures to be in place that effectively monitor and measure the effectiveness of E&S management systems?"},{"@id":"sustainability:reporting_on_and_making_publicly_available_e_s_management_systems","@type":["rdf:Property","owl:DatatypeProperty"],"rdfs:label":"reporting_on_and_making_publicly_available_e_s_management_systems","schema:rangeIncludes":{"@id":"xsd:boolean"},"schema:domainIncludes":{"@id":"sustainability:SustainabilityManagement"},"rdfs:comment":"Does the standard require reporting and making publicly available E&S management system reports"},{"@id":"sustainability:emergency_response_plans_or_strategies_to_climate_related_hazards","@type":["rdf:Property","owl:DatatypeProperty"],"rdfs:label":"emergency_response_plans_or_strategies_to_climate_related_hazards","schema:rangeIncludes":{"@id":"xsd:boolean"},"schema:domainIncludes":{"@id":"sustainability:SustainabilityManagement"},"rdfs:comment":"Does the standard include criteria on emergency response plans or strategies to climate related hazards?"},{"@id":"sustainability:evacuation_safety_procedure","@type":["rdf:Property","owl:DatatypeProperty"],"rdfs:label":"evacuation_safety_procedure","schema:rangeIncludes":{"@id":"xsd:boolean"},"schema:domainIncludes":{"@id":"sustainability:SustainabilityManagement"},"rdfs:comment":"Does the standard include criteria on evacuation safety procedures?"},{"@id":"sustainability:stakeholder_analysis_and_engagement_planning_in_e_s_management_systems","@type":["rdf:Property","owl:DatatypeProperty"],"rdfs:label":"stakeholder_analysis_and_engagement_planning_in_e_s_management_systems","schema:rangeIncludes":{"@id":"xsd:boolean"},"schema:domainIncludes":{"@id":"sustainability:SustainabilityManagement"},"rdfs:comment":""},{"@id":"sustainability:verification_of_mandatory_certificates_and_permits_e_g_water_use_rights_land_use_rights_etc","@type":["rdf:Property","owl:DatatypeProperty"],"rdfs:label":"verification_of_mandatory_certificates_and_permits_e_g_water_use_rights_land_use_rights_etc","schema:rangeIncludes":{"@id":"xsd:boolean"},"schema:domainIncludes":{"@id":"sustainability:SustainabilityManagement"},"rdfs:comment":"Does the standard include criteria to ensure that relevant and up-to-date permits are held (such as water use rights or land use titles)?"},{"@id":"sustainability:occupation_health_and_safety_ohs_management_system","@type":["rdf:Property","owl:DatatypeProperty"],"rdfs:label":"occupation_health_and_safety_ohs_management_system","schema:rangeIncludes":{"@id":"xsd:boolean"},"schema:domainIncludes":{"@id":"sustainability:SustainabilityManagement"},"rdfs:comment":"Does the standard require policies and procedures to manage health and safety in the workplace?"},{"@id":"sustainability:establishing_and_making_publicly_available_the_management_unit_csr_policy","@type":["rdf:Property","owl:DatatypeProperty"],"rdfs:label":"establishing_and_making_publicly_available_the_management_unit_csr_policy","schema:rangeIncludes":{"@id":"xsd:boolean"},"schema:domainIncludes":{"@id":"sustainability:SustainabilityManagement"},"rdfs:comment":"Does the standard require corporate social responsibility to be an explicit integral part of the organization’s mission or policy statement(s)"},{"@id":"sustainability:staff_training_on_sustainability_issues_environment_social_economic_quality_culture_health_and_safety","@type":["rdf:Property","owl:DatatypeProperty"],"rdfs:label":"staff_training_on_sustainability_issues_environment_social_economic_quality_culture_health_and_safety","schema:rangeIncludes":{"@id":"xsd:boolean"},"schema:domainIncludes":{"@id":"sustainability:SustainabilityManagement"},"rdfs:comment":"Does the standard promote sustainability trainings for all workers"},{"@id":"sustainability:establishing_and_making_publicly_available_the_management_unit_internal_control_system","@type":["rdf:Property","owl:DatatypeProperty"],"rdfs:label":"establishing_and_making_publicly_available_the_management_unit_internal_control_system","schema:rangeIncludes":{"@id":"xsd:boolean"},"schema:domainIncludes":{"@id":"sustainability:SustainabilityManagement"},"rdfs:comment":"Does the standard include explicit requirements to establish and manage an internal control system which shall be responsible for the smooth implementation of the standards requirements"},{"@id":"sustainability:respect_the_natural_or_cultural_heritage_surroundings","@type":["rdf:Property","owl:DatatypeProperty"],"rdfs:label":"respect_the_natural_or_cultural_heritage_surroundings","schema:rangeIncludes":{"@id":"xsd:boolean"},"schema:domainIncludes":{"@id":"sustainability:SustainabilityManagement"},"rdfs:comment":"Does the standard include criteria related to the respect of natural or cultural heritage surroundings in siting, design, impact assessment, and land  rights and acquisition (e.g. tourism sector)"},{"@id":"sustainability:use_of_locally_appropriate_principles_for_scenic_sites","@type":["rdf:Property","owl:DatatypeProperty"],"rdfs:label":"use_of_locally_appropriate_principles_for_scenic_sites","schema:rangeIncludes":{"@id":"xsd:boolean"},"schema:domainIncludes":{"@id":"sustainability:SustainabilityManagement"},"rdfs:comment":"Does the standard include criteria related to locally appropriate principles of sustainable construction"},{"@id":"sustainability:provision_of_access_for_persons_or_workers_with_special_needs","@type":["rdf:Property","owl:DatatypeProperty"],"rdfs:label":"provision_of_access_for_persons_or_workers_with_special_needs","schema:rangeIncludes":{"@id":"xsd:boolean"},"schema:domainIncludes":{"@id":"sustainability:SustainabilityManagement"},"rdfs:comment":"Does the standard require provision of special access facilities to production sites for persons or workers with special needs"},{"@id":"sustainability:other_administration_and_management_issues","@type":["rdf:Property","owl:DatatypeProperty"],"rdfs:label":"other_administration_and_management_issues","schema:rangeIncludes":{"@id":"xsd:string"},"schema:domainIncludes":{"@id":"sustainability:SustainabilityManagement"},"rdfs:comment":"Does the standard include other administration and management related requirements not listed previously"},{"@id":"sustainability:assess_risks_and_impacts_on_water_usage","@type":["rdf:Property","owl:DatatypeProperty"],"rdfs:label":"assess_risks_and_impacts_on_water_usage","schema:rangeIncludes":{"@id":"xsd:boolean"},"schema:domainIncludes":{"@id":"sustainability:SustainabilityManagement"},"rdfs:comment":"Does the standard include criteria on the assessment of risks and impacts on water usage"},{"@id":"sustainability:risks_and_impacts_on_water_levels_of_water_resources_used_surface_and_or_ground_water","@type":["rdf:Property","owl:DatatypeProperty"],"rdfs:label":"risks_and_impacts_on_water_levels_of_water_resources_used_surface_and_or_ground_water","schema:rangeIncludes":{"@id":"sustainability:RisksAndImpactsOnWaterLevelsOfWaterResourcesUsedSurfaceAndOrGroundWater"},"schema:domainIncludes":{"@id":"sustainability:SustainabilityManagement"},"rdfs:comment":"Does the standard include explicit criteria on impacts assessment of water levels of surface and/or ground water?"},{"@id":"sustainability:risks_and_impacts_on_water_quality_of_water_resources_used_surface_and_or_ground_water","@type":["rdf:Property","owl:DatatypeProperty"],"rdfs:label":"risks_and_impacts_on_water_quality_of_water_resources_used_surface_and_or_ground_water","schema:rangeIncludes":{"@id":"sustainability:RisksAndImpactsOnWaterQualityOfWaterResourcesUsedSurfaceAndOrGroundWater"},"schema:domainIncludes":{"@id":"sustainability:SustainabilityManagement"},"rdfs:comment":"Does the standard include explicit criteria on impacts assessment of the quality of surface and/or ground water?"},{"@id":"sustainability:environmental_risks_and_impacts","@type":["rdf:Property","owl:DatatypeProperty"],"rdfs:label":"environmental_risks_and_impacts","schema:rangeIncludes":{"@id":"sustainability:EnvironmentalRisksAndImpacts"},"schema:domainIncludes":{"@id":"sustainability:SustainabilityManagement"},"rdfs:comment":"Does the standard include criteria on assessing the environmental risks and impacts of production/operations prior to any significant intensification or expansion of business operations/cultivation and infrastructure?"},{"@id":"sustainability:risks_and_impacts_on_soil_resources_condition","@type":["rdf:Property","owl:DatatypeProperty"],"rdfs:label":"risks_and_impacts_on_soil_resources_condition","schema:rangeIncludes":{"@id":"xsd:boolean"},"schema:domainIncludes":{"@id":"sustainability:SustainabilityManagement"},"rdfs:comment":"Does the standard require an assessment of risks and impacts on soil resources condition"},{"@id":"sustainability:risks_and_impacts_on_biodiversity_in_as_well_as_outside_management_or_production_unit","@type":["rdf:Property","owl:DatatypeProperty"],"rdfs:label":"risks_and_impacts_on_biodiversity_in_as_well_as_outside_management_or_production_unit","schema:rangeIncludes":{"@id":"xsd:boolean"},"schema:domainIncludes":{"@id":"sustainability:SustainabilityManagement"},"rdfs:comment":"Does the standard require a biodiversity management plan to continuously manage impacts during the extraction phase?"},{"@id":"sustainability:environment_and_social_risks_mitigation_and_performance_improvement","@type":["rdf:Property","owl:DatatypeProperty"],"rdfs:label":"environment_and_social_risks_mitigation_and_performance_improvement","schema:rangeIncludes":{"@id":"xsd:boolean"},"schema:domainIncludes":{"@id":"sustainability:SustainabilityManagement"},"rdfs:comment":"Does the standard include criteria on environment and social risks mitigation and performance improvement"},{"@id":"sustainability:market_data_and_analysis","@type":["rdf:Property","owl:DatatypeProperty"],"rdfs:label":"market_data_and_analysis","schema:rangeIncludes":{"@id":"xsd:string"},"schema:domainIncludes":{"@id":"sustainability:SupplyChain"},"rdfs:comment":"Standard includes requirements related to recording market information and sharing it with the standard system"},{"@id":"sustainability:distribution_networks_and_access_to_markets_buyers","@type":["rdf:Property","owl:DatatypeProperty"],"rdfs:label":"distribution_networks_and_access_to_markets_buyers","schema:rangeIncludes":{"@id":"xsd:boolean"},"schema:domainIncludes":{"@id":"sustainability:SupplyChain"},"rdfs:comment":"Standard includes criteria related to other market access issues not included in previous list"},{"@id":"sustainability:non_discriminatory_lending_practices","@type":["rdf:Property","owl:DatatypeProperty"],"rdfs:label":"non_discriminatory_lending_practices","schema:rangeIncludes":{"@id":"xsd:boolean"},"schema:domainIncludes":{"@id":"sustainability:SupplyChain"},"rdfs:comment":"Standard includes criteria related to promote or put in place non-discriminatory lending practices"},{"@id":"sustainability:lending_practices_promoting_local_entities","@type":["rdf:Property","owl:DatatypeProperty"],"rdfs:label":"lending_practices_promoting_local_entities","schema:rangeIncludes":{"@id":"xsd:boolean"},"schema:domainIncludes":{"@id":"sustainability:SupplyChain"},"rdfs:comment":"Does the standard system encourage lending practices that promote local entities"},{"@id":"sustainability:access_and_selection_of_inputs_and_varieties_traditional_versus_improved_engineered","@type":["rdf:Property","owl:DatatypeProperty"],"rdfs:label":"access_and_selection_of_inputs_and_varieties_traditional_versus_improved_engineered","schema:rangeIncludes":{"@id":"xsd:boolean"},"schema:domainIncludes":{"@id":"sustainability:SupplyChain"},"rdfs:comment":"Does the standard promote access and selection of inputs and varieties (traditional versus improved/engineered)"},{"@id":"sustainability:traceability_of_inputs_varieties_and_records_of_materials_used","@type":["rdf:Property","owl:DatatypeProperty"],"rdfs:label":"traceability_of_inputs_varieties_and_records_of_materials_used","schema:rangeIncludes":{"@id":"xsd:boolean"},"schema:domainIncludes":{"@id":"sustainability:SupplyChain"},"rdfs:comment":"Does the standard address issues relating to traceability of inputs / varieties and records of materials used"},{"@id":"sustainability:access_to_technology_and_innovation","@type":["rdf:Property","owl:DatatypeProperty"],"rdfs:label":"access_to_technology_and_innovation","schema:rangeIncludes":{"@id":"xsd:boolean"},"schema:domainIncludes":{"@id":"sustainability:SupplyChain"},"rdfs:comment":"Does the standard promote access to technology and innovation"},{"@id":"sustainability:infrastructure_transport_storage_testing_laboratories","@type":["rdf:Property","owl:DatatypeProperty"],"rdfs:label":"infrastructure_transport_storage_testing_laboratories","schema:rangeIncludes":{"@id":"xsd:boolean"},"schema:domainIncludes":{"@id":"sustainability:SupplyChain"},"rdfs:comment":"Does the standard require appropriate conditions (temperature, maintenance, servicing) in infrastructure (transport, storage, testing laboratories)"},{"@id":"sustainability:responsible_intensification_expansion_of_cultivation_or_infrastructures","@type":["rdf:Property","owl:DatatypeProperty"],"rdfs:label":"responsible_intensification_expansion_of_cultivation_or_infrastructures","schema:rangeIncludes":{"@id":"xsd:boolean"},"schema:domainIncludes":{"@id":"sustainability:SupplyChain"},"rdfs:comment":"Does the standard promote (responsible) intensification / expansion of cultivation or infrastructures"},{"@id":"sustainability:monitoring_measure_of_customer_client_satisfaction","@type":["rdf:Property","owl:DatatypeProperty"],"rdfs:label":"monitoring_measure_of_customer_client_satisfaction","schema:rangeIncludes":{"@id":"xsd:boolean"},"schema:domainIncludes":{"@id":"sustainability:SupplyChain"},"rdfs:comment":"Does the standard include criteria related to measures of customers satisfaction"},{"@id":"sustainability:clients_staff_and_suppliers_to_consider_sustainability_issues_reduce_ghg_emissions_waste_water_use","@type":["rdf:Property","owl:DatatypeProperty"],"rdfs:label":"clients_staff_and_suppliers_to_consider_sustainability_issues_reduce_ghg_emissions_waste_water_use","schema:rangeIncludes":{"@id":"xsd:boolean"},"schema:domainIncludes":{"@id":"sustainability:SupplyChain"},"rdfs:comment":"Does the standard system requier the development and implementation of policies that encourage clients, staff and suppliers to consider sustainability issues"},{"@id":"sustainability:supply_chain_stakeholders_mapping","@type":["rdf:Property","owl:DatatypeProperty"],"rdfs:label":"supply_chain_stakeholders_mapping","schema:rangeIncludes":{"@id":"xsd:boolean"},"schema:domainIncludes":{"@id":"sustainability:SupplyChain"},"rdfs:comment":"Criteria providing a framework to reinforce the links between supply chain actors and making it more robust (e.g. via contracts and responsibilities sharing…)"},{"@id":"sustainability:fair_marketing_based_on_factual_and_unbiased_information","@type":["rdf:Property","owl:DatatypeProperty"],"rdfs:label":"fair_marketing_based_on_factual_and_unbiased_information","schema:rangeIncludes":{"@id":"xsd:boolean"},"schema:domainIncludes":{"@id":"sustainability:SupplyChain"},"rdfs:comment":"Does the standard include criteria related to policies and rules for marketing materials used by the assessee (quality/accuracy of the marketing materials)"},{"@id":"sustainability:group_organization_and_management_for_example_cooperatives","@type":["rdf:Property","owl:DatatypeProperty"],"rdfs:label":"group_organization_and_management_for_example_cooperatives","schema:rangeIncludes":{"@id":"xsd:boolean"},"schema:domainIncludes":{"@id":"sustainability:SupplyChain"},"rdfs:comment":"Does the standard system encourage the formation of different types of organization and management (for example cooperatives"},{"@id":"sustainability:distinct_subcontracting_disclosure_of_prior_approval_auditor_s_access_to","@type":["rdf:Property","owl:DatatypeProperty"],"rdfs:label":"distinct_subcontracting_disclosure_of_prior_approval_auditor_s_access_to","schema:rangeIncludes":{"@id":"xsd:boolean"},"schema:domainIncludes":{"@id":"sustainability:SupplyChain"},"rdfs:comment":"Does the standard include criteria on clear policies and fair process for subcontracting"},{"@id":"sustainability:local_micro_businesses_incubation_facilitation","@type":["rdf:Property","owl:DatatypeProperty"],"rdfs:label":"local_micro_businesses_incubation_facilitation","schema:rangeIncludes":{"@id":"xsd:boolean"},"schema:domainIncludes":{"@id":"sustainability:SupplyChain"},"rdfs:comment":"Does the standard include criteria related to local micro businesses/incubation/facilitation"},{"@id":"sustainability:setting_up_specific_delivery_times_for_suppliers_and_related_possible_sanctions_for_late_delivery","@type":["rdf:Property","owl:DatatypeProperty"],"rdfs:label":"setting_up_specific_delivery_times_for_suppliers_and_related_possible_sanctions_for_late_delivery","schema:rangeIncludes":{"@id":"xsd:boolean"},"schema:domainIncludes":{"@id":"sustainability:SupplyChain"},"rdfs:comment":"Does the standard include criteria on establishing specific delivery times for suppliers and processes for late delivery?"},{"@id":"sustainability:access_to_financial_services_payment_credit_savings_subsidies","@type":["rdf:Property","owl:DatatypeProperty"],"rdfs:label":"access_to_financial_services_payment_credit_savings_subsidies","schema:rangeIncludes":{"@id":"xsd:boolean"},"schema:domainIncludes":{"@id":"sustainability:SupplyChain"},"rdfs:comment":"Standard explicitly includes information on applicants’ access to finance/credit to the applicant, and the standard organization has a role to play"},{"@id":"sustainability:guarantee_of_premium_on_sales_of_certified_product","@type":["rdf:Property","owl:DatatypeProperty"],"rdfs:label":"guarantee_of_premium_on_sales_of_certified_product","schema:rangeIncludes":{"@id":"xsd:boolean"},"schema:domainIncludes":{"@id":"sustainability:SupplyChain"},"rdfs:comment":"Does the standard require price premiums to be paid to producers"},{"@id":"sustainability:minimum_price_guarantees","@type":["rdf:Property","owl:DatatypeProperty"],"rdfs:label":"minimum_price_guarantees","schema:rangeIncludes":{"@id":"xsd:boolean"},"schema:domainIncludes":{"@id":"sustainability:SupplyChain"},"rdfs:comment":"Does the standard addresses issues relating to minimum price guarantees"},{"@id":"sustainability:setting_up_contracts_with_traders","@type":["rdf:Property","owl:DatatypeProperty"],"rdfs:label":"setting_up_contracts_with_traders","schema:rangeIncludes":{"@id":"xsd:boolean"},"schema:domainIncludes":{"@id":"sustainability:SupplyChain"},"rdfs:comment":"Does the standard require written contracts with traders to be issued"},{"@id":"sustainability:inclusion_of_suppliers_sustainability_strategy","@type":["rdf:Property","owl:DatatypeProperty"],"rdfs:label":"inclusion_of_suppliers_sustainability_strategy","schema:rangeIncludes":{"@id":"xsd:boolean"},"schema:domainIncludes":{"@id":"sustainability:SupplyChain"},"rdfs:comment":"Does the standard's requirements for rights and benefits for workers also apply to input suppliers?"},{"@id":"sustainability:supply_chain_responsibility_beyond_primary_production","@type":["rdf:Property","owl:DatatypeProperty"],"rdfs:label":"supply_chain_responsibility_beyond_primary_production","schema:rangeIncludes":{"@id":"sustainability:SupplyChainResponsibilityBeyondPrimaryProduction"},"schema:domainIncludes":{"@id":"sustainability:SupplyChain"},"rdfs:comment":"Does the standard include criteria for the production processes beyond primary production?"},{"@id":"sustainability:advance_payments_requests","@type":["rdf:Property","owl:DatatypeProperty"],"rdfs:label":"advance_payments_requests","schema:rangeIncludes":{"@id":"xsd:boolean"},"schema:domainIncludes":{"@id":"sustainability:SupplyChain"},"rdfs:comment":"Standard addresses issues related to advance payments including pre-financing"},{"@id":"sustainability:quality_policy_general_requirements","@type":["rdf:Property","owl:DatatypeProperty"],"rdfs:label":"quality_policy_general_requirements","schema:rangeIncludes":{"@id":"xsd:string"},"schema:domainIncludes":{"@id":"sustainability:QualityManagement"},"rdfs:comment":"Does the standard includes general requirements on quality management for products and services"},{"@id":"sustainability:using_organic_inputs_to_production","@type":["rdf:Property","owl:DatatypeProperty"],"rdfs:label":"using_organic_inputs_to_production","schema:rangeIncludes":{"@id":"xsd:boolean"},"schema:domainIncludes":{"@id":"sustainability:QualityManagement"},"rdfs:comment":"Does the standard include criteria related to using organic inputs to production"},{"@id":"sustainability:energy_used_during_manufacturing_processes","@type":["rdf:Property","owl:DatatypeProperty"],"rdfs:label":"energy_used_during_manufacturing_processes","schema:rangeIncludes":{"@id":"xsd:boolean"},"schema:domainIncludes":{"@id":"sustainability:QualityManagement"},"rdfs:comment":"Does the standard include criteria related to efficient energy use during the manufacturing process"},{"@id":"sustainability:energy_efficiency_of_production_process","@type":["rdf:Property","owl:DatatypeProperty"],"rdfs:label":"energy_efficiency_of_production_process","schema:rangeIncludes":{"@id":"xsd:boolean"},"schema:domainIncludes":{"@id":"sustainability:QualityManagement"},"rdfs:comment":"Does the standard include criteria related to efficient energy use during the production process"},{"@id":"sustainability:energy_efficiency_of_final_product_during_consumption","@type":["rdf:Property","owl:DatatypeProperty"],"rdfs:label":"energy_efficiency_of_final_product_during_consumption","schema:rangeIncludes":{"@id":"xsd:boolean"},"schema:domainIncludes":{"@id":"sustainability:QualityManagement"},"rdfs:comment":"Does the standard include criteria related to energy efficiency of final product during consumption"},{"@id":"sustainability:energy_efficiency_of_final_product_during_end_of_life","@type":["rdf:Property","owl:DatatypeProperty"],"rdfs:label":"energy_efficiency_of_final_product_during_end_of_life","schema:rangeIncludes":{"@id":"xsd:boolean"},"schema:domainIncludes":{"@id":"sustainability:QualityManagement"},"rdfs:comment":"Does the standard include criteria related to energy efficiency of final product during end-of-life"},{"@id":"sustainability:quality_of_products_packaging_and_transportation","@type":["rdf:Property","owl:DatatypeProperty"],"rdfs:label":"quality_of_products_packaging_and_transportation","schema:rangeIncludes":{"@id":"xsd:boolean"},"schema:domainIncludes":{"@id":"sustainability:QualityManagement"},"rdfs:comment":"Does the standard include criteria related to the quality of packaging and transportation of products"},{"@id":"sustainability:quality_of_product_storage_facilities_warehouses_containers_etc","@type":["rdf:Property","owl:DatatypeProperty"],"rdfs:label":"quality_of_product_storage_facilities_warehouses_containers_etc","schema:rangeIncludes":{"@id":"xsd:boolean"},"schema:domainIncludes":{"@id":"sustainability:QualityManagement"},"rdfs:comment":"Does the standard include criteria related to the quality of product storage facilities (warehouses, containers etc) - excl. Food products specific criteria"},{"@id":"sustainability:quality_manual_available_to_staff_workers","@type":["rdf:Property","owl:DatatypeProperty"],"rdfs:label":"quality_manual_available_to_staff_workers","schema:rangeIncludes":{"@id":"xsd:boolean"},"schema:domainIncludes":{"@id":"sustainability:QualityManagement"},"rdfs:comment":"Does the standard require that there is a quality manual available to staff/workers"},{"@id":"sustainability:control_process_established_and_documented","@type":["rdf:Property","owl:DatatypeProperty"],"rdfs:label":"control_process_established_and_documented","schema:rangeIncludes":{"@id":"xsd:boolean"},"schema:domainIncludes":{"@id":"sustainability:QualityManagement"},"rdfs:comment":"Does the standard require that control processes are established and documented within the Quality Management System"},{"@id":"sustainability:traceability_and_records_keeping","@type":["rdf:Property","owl:DatatypeProperty"],"rdfs:label":"traceability_and_records_keeping","schema:rangeIncludes":{"@id":"xsd:boolean"},"schema:domainIncludes":{"@id":"sustainability:QualityManagement"},"rdfs:comment":"Does the standard require that the Quality Management System include traceability and records-keeping"},{"@id":"sustainability:quality_compliance_to_national_and_international_legislation","@type":["rdf:Property","owl:DatatypeProperty"],"rdfs:label":"quality_compliance_to_national_and_international_legislation","schema:rangeIncludes":{"@id":"xsd:boolean"},"schema:domainIncludes":{"@id":"sustainability:QualityManagement"},"rdfs:comment":"Does the standard requires that a quality management system complies with national and international legislation"},{"@id":"sustainability:procedures_established_and_monitored","@type":["rdf:Property","owl:DatatypeProperty"],"rdfs:label":"procedures_established_and_monitored","schema:rangeIncludes":{"@id":"xsd:boolean"},"schema:domainIncludes":{"@id":"sustainability:QualityManagement"},"rdfs:comment":"Does the standard require that procedures are established and monitored within the Quality Management System"},{"@id":"sustainability:customer_focus_performance_indicators","@type":["rdf:Property","owl:DatatypeProperty"],"rdfs:label":"customer_focus_performance_indicators","schema:rangeIncludes":{"@id":"xsd:boolean"},"schema:domainIncludes":{"@id":"sustainability:QualityManagement"},"rdfs:comment":"Does the standard require that the Quality Management System has a customer focus"},{"@id":"sustainability:complaint_management_system_implemented","@type":["rdf:Property","owl:DatatypeProperty"],"rdfs:label":"complaint_management_system_implemented","schema:rangeIncludes":{"@id":"xsd:boolean"},"schema:domainIncludes":{"@id":"sustainability:QualityManagement"},"rdfs:comment":"Does the standard require that the Quality Management System includes a complaint management system"},{"@id":"sustainability:complaints_records_keeping","@type":["rdf:Property","owl:DatatypeProperty"],"rdfs:label":"complaints_records_keeping","schema:rangeIncludes":{"@id":"xsd:boolean"},"schema:domainIncludes":{"@id":"sustainability:QualityManagement"},"rdfs:comment":"Does the standard require that the Quality Management System maintain records on complaints"},{"@id":"sustainability:control_process_periodic_review_and_assessment","@type":["rdf:Property","owl:DatatypeProperty"],"rdfs:label":"control_process_periodic_review_and_assessment","schema:rangeIncludes":{"@id":"xsd:boolean"},"schema:domainIncludes":{"@id":"sustainability:QualityManagement"},"rdfs:comment":"Does the standard require that the unit of operations has a periodic review and assessment of its Quality Management System control processes"},{"@id":"sustainability:internal_audit_self_assessment_system_established_and_monitored","@type":["rdf:Property","owl:DatatypeProperty"],"rdfs:label":"internal_audit_self_assessment_system_established_and_monitored","schema:rangeIncludes":{"@id":"xsd:boolean"},"schema:domainIncludes":{"@id":"sustainability:QualityManagement"},"rdfs:comment":"Does the standard require that the unit of operation establish a system for regular internal audits / self assessments of its Quality Management System and to monitor the system accordingly"},{"@id":"sustainability:incidences_monitoring_and_records_keeping","@type":["rdf:Property","owl:DatatypeProperty"],"rdfs:label":"incidences_monitoring_and_records_keeping","schema:rangeIncludes":{"@id":"xsd:boolean"},"schema:domainIncludes":{"@id":"sustainability:QualityManagement"},"rdfs:comment":"Does the standard require that Quality Management System monitors and maintains records of incidences"},{"@id":"sustainability:corrective_actions_implemented_and_documented","@type":["rdf:Property","owl:DatatypeProperty"],"rdfs:label":"corrective_actions_implemented_and_documented","schema:rangeIncludes":{"@id":"xsd:boolean"},"schema:domainIncludes":{"@id":"sustainability:QualityManagement"},"rdfs:comment":"Does the standard require that a unit of operation's Quality Management System implements and documents corrective actions in response to non-conformities"},{"@id":"sustainability:quality_risk_assessment_and_hazard_control_procedures","@type":["rdf:Property","owl:DatatypeProperty"],"rdfs:label":"quality_risk_assessment_and_hazard_control_procedures","schema:rangeIncludes":{"@id":"xsd:boolean"},"schema:domainIncludes":{"@id":"sustainability:QualityManagement"},"rdfs:comment":"Does the standard body require that a quality management system has risk assessment and hazard control procedures in place"},{"@id":"sustainability:quality_documentation_and_monitoring_procedures","@type":["rdf:Property","owl:DatatypeProperty"],"rdfs:label":"quality_documentation_and_monitoring_procedures","schema:rangeIncludes":{"@id":"xsd:boolean"},"schema:domainIncludes":{"@id":"sustainability:QualityManagement"},"rdfs:comment":"Does the standard body require that the quality management system of a unit of operation involves documentation and monitoring procedures"},{"@id":"sustainability:quality_technical_specifications","@type":["rdf:Property","owl:DatatypeProperty"],"rdfs:label":"quality_technical_specifications","schema:rangeIncludes":{"@id":"xsd:boolean"},"schema:domainIncludes":{"@id":"sustainability:QualityManagement"},"rdfs:comment":"Does the standard body require that the quality management system follow specific technical specifications applying to the production process/final product or service development/delivery"},{"@id":"sustainability:product_safety_specifications_excl_food_safety","@type":["rdf:Property","owl:DatatypeProperty"],"rdfs:label":"product_safety_specifications_excl_food_safety","schema:rangeIncludes":{"@id":"xsd:boolean"},"schema:domainIncludes":{"@id":"sustainability:QualityManagement"},"rdfs:comment":"Does the standard include criteria related to product safety (excluding issues covering food safety)"},{"@id":"sustainability:testing_quality_of_inputs_to_production","@type":["rdf:Property","owl:DatatypeProperty"],"rdfs:label":"testing_quality_of_inputs_to_production","schema:rangeIncludes":{"@id":"xsd:boolean"},"schema:domainIncludes":{"@id":"sustainability:QualityManagement"},"rdfs:comment":"Does the standard include criteria related to testing quality of inputs to production"},{"@id":"sustainability:testing_quality_of_semi_final_products","@type":["rdf:Property","owl:DatatypeProperty"],"rdfs:label":"testing_quality_of_semi_final_products","schema:rangeIncludes":{"@id":"xsd:boolean"},"schema:domainIncludes":{"@id":"sustainability:QualityManagement"},"rdfs:comment":"Does the standard include criteria related to testing quality of semi-final products"},{"@id":"sustainability:testing_quality_of_final_products","@type":["rdf:Property","owl:DatatypeProperty"],"rdfs:label":"testing_quality_of_final_products","schema:rangeIncludes":{"@id":"xsd:boolean"},"schema:domainIncludes":{"@id":"sustainability:QualityManagement"},"rdfs:comment":"Does the standard include criteria related to testing quality of final products"},{"@id":"sustainability:defined_controlled_and_monitored_technical_processes_for_non_food_manufactured_products","@type":["rdf:Property","owl:DatatypeProperty"],"rdfs:label":"defined_controlled_and_monitored_technical_processes_for_non_food_manufactured_products","schema:rangeIncludes":{"@id":"xsd:boolean"},"schema:domainIncludes":{"@id":"sustainability:QualityManagement"},"rdfs:comment":"Does the standard require that the quality management system has defined, controlled and monitored technical processes for non-food manufactured products"},{"@id":"sustainability:production_site_specifications_established_and_monitored_through_inspections","@type":["rdf:Property","owl:DatatypeProperty"],"rdfs:label":"production_site_specifications_established_and_monitored_through_inspections","schema:rangeIncludes":{"@id":"xsd:boolean"},"schema:domainIncludes":{"@id":"sustainability:QualityManagement"},"rdfs:comment":"Does the standard require that the quality management system has established production site specifications which are regularly monitored by inspection"},{"@id":"sustainability:waste_management_system_established_and_monitored_volume_toxicity_discharge","@type":["rdf:Property","owl:DatatypeProperty"],"rdfs:label":"waste_management_system_established_and_monitored_volume_toxicity_discharge","schema:rangeIncludes":{"@id":"xsd:boolean"},"schema:domainIncludes":{"@id":"sustainability:QualityManagement"},"rdfs:comment":"Does the standard require that the quality management system has an established waste management system, which is regularly monitored"},{"@id":"sustainability:water_usage_management_system_established_and_monitored_volume_quality_use_re_use_and_recycling_wastewater_discharge","@type":["rdf:Property","owl:DatatypeProperty"],"rdfs:label":"water_usage_management_system_established_and_monitored_volume_quality_use_re_use_and_recycling_wastewater_discharge","schema:rangeIncludes":{"@id":"xsd:boolean"},"schema:domainIncludes":{"@id":"sustainability:QualityManagement"},"rdfs:comment":"Does the standard require that the quality management system has an established water usage management system, which is regularly monitored"},{"@id":"sustainability:chemicals_usage_management_system_established_and_monitored_volume_quality_prohibited_substances_storage_and_hazardous_waste_discharge","@type":["rdf:Property","owl:DatatypeProperty"],"rdfs:label":"chemicals_usage_management_system_established_and_monitored_volume_quality_prohibited_substances_storage_and_hazardous_waste_discharge","schema:rangeIncludes":{"@id":"xsd:boolean"},"schema:domainIncludes":{"@id":"sustainability:QualityManagement"},"rdfs:comment":"Does the standard require that the quality management system has an established chemicals usage management system, which is regularly monitored"},{"@id":"sustainability:risk_assessment_for_contamination_of_non_food_products","@type":["rdf:Property","owl:DatatypeProperty"],"rdfs:label":"risk_assessment_for_contamination_of_non_food_products","schema:rangeIncludes":{"@id":"xsd:boolean"},"schema:domainIncludes":{"@id":"sustainability:QualityManagement"},"rdfs:comment":"Does the standard require that the quality management system involves a risk assessment for contamination of non-food products?"},{"@id":"sustainability:food_products_compliance_to_national_and_international_legislation","@type":["rdf:Property","owl:DatatypeProperty"],"rdfs:label":"food_products_compliance_to_national_and_international_legislation","schema:rangeIncludes":{"@id":"xsd:boolean"},"schema:domainIncludes":{"@id":"sustainability:QualityManagement"},"rdfs:comment":"Does the standard require compliance with national and international legislation on food products"},{"@id":"sustainability:food_safety_complaints_and_non_conformities_records_keeping","@type":["rdf:Property","owl:DatatypeProperty"],"rdfs:label":"food_safety_complaints_and_non_conformities_records_keeping","schema:rangeIncludes":{"@id":"xsd:boolean"},"schema:domainIncludes":{"@id":"sustainability:QualityManagement"},"rdfs:comment":"Does the standard require records keeping of food safety complaints and non-conformities"},{"@id":"sustainability:food_safety_non_conformities_corrective_action_plan_established","@type":["rdf:Property","owl:DatatypeProperty"],"rdfs:label":"food_safety_non_conformities_corrective_action_plan_established","schema:rangeIncludes":{"@id":"xsd:boolean"},"schema:domainIncludes":{"@id":"sustainability:QualityManagement"},"rdfs:comment":"Does the standard require the establishment of a corrective action plan on food safety non-conformities"},{"@id":"sustainability:food_safety_procedures_established_and_documented","@type":["rdf:Property","owl:DatatypeProperty"],"rdfs:label":"food_safety_procedures_established_and_documented","schema:rangeIncludes":{"@id":"xsd:boolean"},"schema:domainIncludes":{"@id":"sustainability:QualityManagement"},"rdfs:comment":"Does the standard require that food safety procedures are established and documented"},{"@id":"sustainability:food_safety_instructions_including_hygiene_requirements_established_and_communicated_to_staff_workers","@type":["rdf:Property","owl:DatatypeProperty"],"rdfs:label":"food_safety_instructions_including_hygiene_requirements_established_and_communicated_to_staff_workers","schema:rangeIncludes":{"@id":"xsd:boolean"},"schema:domainIncludes":{"@id":"sustainability:QualityManagement"},"rdfs:comment":"Does the standard require that food safety instructions, including hygiene requirements, are established and communicated to staff / workers"},{"@id":"sustainability:hygiene_instructions_clearly_signed_and_communicated_to_external_visitors","@type":["rdf:Property","owl:DatatypeProperty"],"rdfs:label":"hygiene_instructions_clearly_signed_and_communicated_to_external_visitors","schema:rangeIncludes":{"@id":"xsd:boolean"},"schema:domainIncludes":{"@id":"sustainability:QualityManagement"},"rdfs:comment":"Does the standard require that hygiene instructions are clearly signed and communicated to external visitors"},{"@id":"sustainability:food_safety_training_for_all_staff_handling_food_products","@type":["rdf:Property","owl:DatatypeProperty"],"rdfs:label":"food_safety_training_for_all_staff_handling_food_products","schema:rangeIncludes":{"@id":"xsd:boolean"},"schema:domainIncludes":{"@id":"sustainability:QualityManagement"},"rdfs:comment":"Does the standard require training for all staff handling food products"},{"@id":"sustainability:food_safety_incidences_management_procedures_established_and_communicated_to_staff_workers","@type":["rdf:Property","owl:DatatypeProperty"],"rdfs:label":"food_safety_incidences_management_procedures_established_and_communicated_to_staff_workers","schema:rangeIncludes":{"@id":"xsd:boolean"},"schema:domainIncludes":{"@id":"sustainability:QualityManagement"},"rdfs:comment":"Does the standard require that food safety incidences management procedures are established and communicated to staff / workers"},{"@id":"sustainability:food_safety_incidences_management_plan_testing_and_regular_training_of_staff_workers","@type":["rdf:Property","owl:DatatypeProperty"],"rdfs:label":"food_safety_incidences_management_plan_testing_and_regular_training_of_staff_workers","schema:rangeIncludes":{"@id":"xsd:boolean"},"schema:domainIncludes":{"@id":"sustainability:QualityManagement"},"rdfs:comment":"Does the standard require testing of the food safety incidences management plan and regular training for its procedures to staff / workers"},{"@id":"sustainability:food_safety_incidences_records_keeping","@type":["rdf:Property","owl:DatatypeProperty"],"rdfs:label":"food_safety_incidences_records_keeping","schema:rangeIncludes":{"@id":"xsd:boolean"},"schema:domainIncludes":{"@id":"sustainability:QualityManagement"},"rdfs:comment":"Does the standard require records to be maintained for food safety incidences"},{"@id":"sustainability:food_safety_incidences_external_communication_plan","@type":["rdf:Property","owl:DatatypeProperty"],"rdfs:label":"food_safety_incidences_external_communication_plan","schema:rangeIncludes":{"@id":"xsd:boolean"},"schema:domainIncludes":{"@id":"sustainability:QualityManagement"},"rdfs:comment":"Does the standard require a food safety incidences external communication plan"},{"@id":"sustainability:inputs_purchasing_policies_and_suppliers_clearance_process_established_and_monitored","@type":["rdf:Property","owl:DatatypeProperty"],"rdfs:label":"inputs_purchasing_policies_and_suppliers_clearance_process_established_and_monitored","schema:rangeIncludes":{"@id":"xsd:boolean"},"schema:domainIncludes":{"@id":"sustainability:TechnicalSpecifications"},"rdfs:comment":"Does the standard body require that a Quality Management System has established and monitored inputs purchasing policies and suppliers' clearance processes"},{"@id":"sustainability:technical_processes_for_manufacturing_processing_of_non_food_products","@type":["rdf:Property","owl:DatatypeProperty"],"rdfs:label":"technical_processes_for_manufacturing_processing_of_non_food_products","schema:rangeIncludes":{"@id":"xsd:boolean"},"schema:domainIncludes":{"@id":"sustainability:TechnicalSpecifications"},"rdfs:comment":"Does the standard have requirements related to technical processes for manufacturing / processing of non-food products"},{"@id":"sustainability:final_products_technical_specifications_and_suitability_of_non_food_products","@type":["rdf:Property","owl:DatatypeProperty"],"rdfs:label":"final_products_technical_specifications_and_suitability_of_non_food_products","schema:rangeIncludes":{"@id":"xsd:boolean"},"schema:domainIncludes":{"@id":"sustainability:TechnicalSpecifications"},"rdfs:comment":"Does the standard have requirements related to final products technical specifications and suitability of non-food products"},{"@id":"sustainability:assess_final_product_potential_for_re_use_and_recycling_of_non_food_products","@type":["rdf:Property","owl:DatatypeProperty"],"rdfs:label":"assess_final_product_potential_for_re_use_and_recycling_of_non_food_products","schema:rangeIncludes":{"@id":"xsd:boolean"},"schema:domainIncludes":{"@id":"sustainability:TechnicalSpecifications"},"rdfs:comment":"Does the standard have criteria for the assessment of final product potential for re-use and recycling of non-food products"},{"@id":"sustainability:does_the_standard_cover_the_quality_of_textiles","@type":["rdf:Property","owl:DatatypeProperty"],"rdfs:label":"does_the_standard_cover_the_quality_of_textiles","schema:rangeIncludes":{"@id":"sustainability:DoesTheStandardCoverTheQualityOfTextiles"},"schema:domainIncludes":{"@id":"sustainability:TechnicalSpecifications"},"rdfs:comment":"Does the standard cover criteria on the quality of textiles?"},{"@id":"sustainability:does_the_standard_include_the_suitability_of_use","@type":["rdf:Property","owl:DatatypeProperty"],"rdfs:label":"does_the_standard_include_the_suitability_of_use","schema:rangeIncludes":{"@id":"xsd:boolean"},"schema:domainIncludes":{"@id":"sustainability:TechnicalSpecifications"},"rdfs:comment":"Does the standard include criteria on the suitability of the product for the intended purpose?"},{"@id":"sustainability:quality_management_systems_transportation_of_non_food_products","@type":["rdf:Property","owl:DatatypeProperty"],"rdfs:label":"quality_management_systems_transportation_of_non_food_products","schema:rangeIncludes":{"@id":"xsd:boolean"},"schema:domainIncludes":{"@id":"sustainability:TraceabilityAndRecall"},"rdfs:comment":"Does the standard include criteria on the transportation of non-food products?"},{"@id":"sustainability:traceability_system_established_and_monitored","@type":["rdf:Property","owl:DatatypeProperty"],"rdfs:label":"traceability_system_established_and_monitored","schema:rangeIncludes":{"@id":"xsd:boolean"},"schema:domainIncludes":[{"@id":"sustainability:TraceabilityAndRecall"},{"@id":"sustainability:TracebilityRecallAndAllergens"}],"rdfs:comment":"Does the standard require that a traceability system is established and monitored for non-food products"},{"@id":"sustainability:traceability_records_maintained_through_entire_chain_of_production","@type":["rdf:Property","owl:DatatypeProperty"],"rdfs:label":"traceability_records_maintained_through_entire_chain_of_production","schema:rangeIncludes":{"@id":"xsd:boolean"},"schema:domainIncludes":[{"@id":"sustainability:TraceabilityAndRecall"},{"@id":"sustainability:TracebilityRecallAndAllergens"}],"rdfs:comment":"Does the standard require that traceability records are maintained through the entire chain of production for non-food products"},{"@id":"sustainability:labeling_system_of_all_inputs_through_entire_production_chain","@type":["rdf:Property","owl:DatatypeProperty"],"rdfs:label":"labeling_system_of_all_inputs_through_entire_production_chain","schema:rangeIncludes":{"@id":"xsd:boolean"},"schema:domainIncludes":[{"@id":"sustainability:TraceabilityAndRecall"},{"@id":"sustainability:TracebilityRecallAndAllergens"}],"rdfs:comment":"Does the standard require the implementation of a labeling system of all inputs through entire production chain for non-food products"},{"@id":"sustainability:product_recall_policy_established_tested_and_monitored","@type":["rdf:Property","owl:DatatypeProperty"],"rdfs:label":"product_recall_policy_established_tested_and_monitored","schema:rangeIncludes":{"@id":"xsd:boolean"},"schema:domainIncludes":[{"@id":"sustainability:TraceabilityAndRecall"},{"@id":"sustainability:TracebilityRecallAndAllergens"}],"rdfs:comment":"Does the standard require that a product recall policy is established, tested and monitored?"},{"@id":"sustainability:identity_preservation_model_established_and_monitored_modus_operandi","@type":["rdf:Property","owl:DatatypeProperty"],"rdfs:label":"identity_preservation_model_established_and_monitored_modus_operandi","schema:rangeIncludes":{"@id":"xsd:boolean"},"schema:domainIncludes":[{"@id":"sustainability:TraceabilityAndRecall"},{"@id":"sustainability:TracebilityRecallAndAllergens"}],"rdfs:comment":"Does the standard require that the Identity preservation model is established and monitored for the traceability of non-food products"},{"@id":"sustainability:segregation_model_established_and_monitored_modus_operandi","@type":["rdf:Property","owl:DatatypeProperty"],"rdfs:label":"segregation_model_established_and_monitored_modus_operandi","schema:rangeIncludes":{"@id":"xsd:boolean"},"schema:domainIncludes":[{"@id":"sustainability:TraceabilityAndRecall"},{"@id":"sustainability:TracebilityRecallAndAllergens"}],"rdfs:comment":"Does the standard require that the segregation model is established and monitored for the traceability of non-food products"},{"@id":"sustainability:establishing_and_implementation_of_a_t_t_system_focused_on_a_quick_identification_separation_blocking_and_withdrawal_from_market","@type":["rdf:Property","owl:DatatypeProperty"],"rdfs:label":"establishing_and_implementation_of_a_t_t_system_focused_on_a_quick_identification_separation_blocking_and_withdrawal_from_market","schema:rangeIncludes":{"@id":"xsd:boolean"},"schema:domainIncludes":{"@id":"sustainability:TraceabilityAndRecall"},"rdfs:comment":"Establishing and implementation of a T&T system focused on a quick identification, separation, blocking and withdrawal from market"},{"@id":"sustainability:communication_including_list_of_stakeholders_both_internally_as_externally","@type":["rdf:Property","owl:DatatypeProperty"],"rdfs:label":"communication_including_list_of_stakeholders_both_internally_as_externally","schema:rangeIncludes":{"@id":"xsd:boolean"},"schema:domainIncludes":{"@id":"sustainability:TraceabilityAndRecall"},"rdfs:comment":"Criteria for communication including list of stakeholders (both internally as externally)"},{"@id":"sustainability:notification_of_clients","@type":["rdf:Property","owl:DatatypeProperty"],"rdfs:label":"notification_of_clients","schema:rangeIncludes":{"@id":"xsd:boolean"},"schema:domainIncludes":{"@id":"sustainability:TraceabilityAndRecall"},"rdfs:comment":"Notification of clients"},{"@id":"sustainability:notification_of_competent_authority","@type":["rdf:Property","owl:DatatypeProperty"],"rdfs:label":"notification_of_competent_authority","schema:rangeIncludes":{"@id":"xsd:boolean"},"schema:domainIncludes":{"@id":"sustainability:TraceabilityAndRecall"},"rdfs:comment":"Notification of Competent Authority"},{"@id":"sustainability:notification_of_certification_body","@type":["rdf:Property","owl:DatatypeProperty"],"rdfs:label":"notification_of_certification_body","schema:rangeIncludes":{"@id":"xsd:boolean"},"schema:domainIncludes":{"@id":"sustainability:TraceabilityAndRecall"},"rdfs:comment":"Notification of certification body"},{"@id":"sustainability:notification_of_scheme_manager","@type":["rdf:Property","owl:DatatypeProperty"],"rdfs:label":"notification_of_scheme_manager","schema:rangeIncludes":{"@id":"xsd:boolean"},"schema:domainIncludes":{"@id":"sustainability:TraceabilityAndRecall"},"rdfs:comment":"Notification of scheme manager"},{"@id":"sustainability:continuous_update_of_recall_procedure","@type":["rdf:Property","owl:DatatypeProperty"],"rdfs:label":"continuous_update_of_recall_procedure","schema:rangeIncludes":{"@id":"xsd:boolean"},"schema:domainIncludes":{"@id":"sustainability:TraceabilityAndRecall"},"rdfs:comment":"Continuous update of recall procedure"},{"@id":"sustainability:a_procedure_to_evaluate_executed_recalls_and_define_improvements","@type":["rdf:Property","owl:DatatypeProperty"],"rdfs:label":"a_procedure_to_evaluate_executed_recalls_and_define_improvements","schema:rangeIncludes":{"@id":"xsd:boolean"},"schema:domainIncludes":{"@id":"sustainability:TraceabilityAndRecall"},"rdfs:comment":"A procedure to evaluate executed recalls and define improvements"},{"@id":"sustainability:performance_of_a_recall_simulation_with_a_risk_based_frequency","@type":["rdf:Property","owl:DatatypeProperty"],"rdfs:label":"performance_of_a_recall_simulation_with_a_risk_based_frequency","schema:rangeIncludes":{"@id":"xsd:boolean"},"schema:domainIncludes":{"@id":"sustainability:TraceabilityAndRecall"},"rdfs:comment":"Performance of a recall simulation with a risk based frequency"},{"@id":"sustainability:performance_of_a_recall_simulation_at_least_once_a_year","@type":["rdf:Property","owl:DatatypeProperty"],"rdfs:label":"performance_of_a_recall_simulation_at_least_once_a_year","schema:rangeIncludes":{"@id":"xsd:boolean"},"schema:domainIncludes":{"@id":"sustainability:TraceabilityAndRecall"},"rdfs:comment":"Performance of a recall simulation at least once a year"},{"@id":"sustainability:a_procedure_to_evaluate_the_recall_simulation","@type":["rdf:Property","owl:DatatypeProperty"],"rdfs:label":"a_procedure_to_evaluate_the_recall_simulation","schema:rangeIncludes":{"@id":"xsd:boolean"},"schema:domainIncludes":{"@id":"sustainability:TraceabilityAndRecall"},"rdfs:comment":"A procedure to evaluate the recall simulation"},{"@id":"sustainability:record_at_least_relevant_information_related_to_received_products_downstream_and_suppliers","@type":["rdf:Property","owl:DatatypeProperty"],"rdfs:label":"record_at_least_relevant_information_related_to_received_products_downstream_and_suppliers","schema:rangeIncludes":{"@id":"xsd:boolean"},"schema:domainIncludes":{"@id":"sustainability:TraceabilityAndRecall"},"rdfs:comment":"Record at least relevant information related to received products (downstream) and suppliers"},{"@id":"sustainability:establishing_a_crisis_management_team","@type":["rdf:Property","owl:DatatypeProperty"],"rdfs:label":"establishing_a_crisis_management_team","schema:rangeIncludes":{"@id":"xsd:boolean"},"schema:domainIncludes":{"@id":"sustainability:TraceabilityAndRecall"},"rdfs:comment":"Establishing a crisis management team"},{"@id":"sustainability:record_at_least_relevant_information_related_to_delivered_products_upstream_and_customers","@type":["rdf:Property","owl:DatatypeProperty"],"rdfs:label":"record_at_least_relevant_information_related_to_delivered_products_upstream_and_customers","schema:rangeIncludes":{"@id":"xsd:boolean"},"schema:domainIncludes":{"@id":"sustainability:TraceabilityAndRecall"},"rdfs:comment":"Record at least relevant information related to delivered products (upstream) and customers"},{"@id":"sustainability:implementation_a_system_for_internal_t_t","@type":["rdf:Property","owl:DatatypeProperty"],"rdfs:label":"implementation_a_system_for_internal_t_t","schema:rangeIncludes":{"@id":"xsd:boolean"},"schema:domainIncludes":{"@id":"sustainability:TraceabilityAndRecall"},"rdfs:comment":"Implementation a system for internal T&T"},{"@id":"sustainability:provision_of_relevant_information_about_products_and_their_delivery","@type":["rdf:Property","owl:DatatypeProperty"],"rdfs:label":"provision_of_relevant_information_about_products_and_their_delivery","schema:rangeIncludes":{"@id":"xsd:boolean"},"schema:domainIncludes":{"@id":"sustainability:TraceabilityAndRecall"},"rdfs:comment":"Provision of relevant information about products and their delivery"},{"@id":"sustainability:provision_of_relevant_information_about_products_and_their_delivery_within_a_certain_time_limit","@type":["rdf:Property","owl:DatatypeProperty"],"rdfs:label":"provision_of_relevant_information_about_products_and_their_delivery_within_a_certain_time_limit","schema:rangeIncludes":{"@id":"xsd:boolean"},"schema:domainIncludes":{"@id":"sustainability:TraceabilityAndRecall"},"rdfs:comment":"Provision of relevant information about products and their delivery within a certain time limit"},{"@id":"sustainability:establishing_a_recall_team_including_roles_tasks_responsibilities_and_mandates","@type":["rdf:Property","owl:DatatypeProperty"],"rdfs:label":"establishing_a_recall_team_including_roles_tasks_responsibilities_and_mandates","schema:rangeIncludes":{"@id":"xsd:boolean"},"schema:domainIncludes":{"@id":"sustainability:TraceabilityAndRecall"},"rdfs:comment":"Establishing a recall team including roles, tasks, responsibilities and mandates."},{"@id":"sustainability:a_recall_team_including_provision_of_all_necessary_means","@type":["rdf:Property","owl:DatatypeProperty"],"rdfs:label":"a_recall_team_including_provision_of_all_necessary_means","schema:rangeIncludes":{"@id":"xsd:boolean"},"schema:domainIncludes":{"@id":"sustainability:TraceabilityAndRecall"},"rdfs:comment":"Criteria for a recall team including provision of all necessary means"},{"@id":"sustainability:recall","@type":["rdf:Property","owl:DatatypeProperty"],"rdfs:label":"recall","schema:rangeIncludes":{"@id":"xsd:boolean"},"schema:domainIncludes":{"@id":"sustainability:TraceabilityAndRecall"},"rdfs:comment":"Criteria for recall"},{"@id":"sustainability:mass_balance_model_established_and_monitored_modus_operandi","@type":["rdf:Property","owl:DatatypeProperty"],"rdfs:label":"mass_balance_model_established_and_monitored_modus_operandi","schema:rangeIncludes":{"@id":"xsd:boolean"},"schema:domainIncludes":[{"@id":"sustainability:StaffRequirements"},{"@id":"sustainability:TracebilityRecallAndAllergens"}],"rdfs:comment":"Does the standard require that the mass balance model is established and monitored for the traceability of non-food products"},{"@id":"sustainability:workers_staff_skills_requirements","@type":["rdf:Property","owl:DatatypeProperty"],"rdfs:label":"workers_staff_skills_requirements","schema:rangeIncludes":{"@id":"xsd:boolean"},"schema:domainIncludes":{"@id":"sustainability:StaffRequirements"},"rdfs:comment":"Does the standard include criteria on the skill requirements for manufacturing workers"},{"@id":"sustainability:workers_staff_training_programs","@type":["rdf:Property","owl:DatatypeProperty"],"rdfs:label":"workers_staff_training_programs","schema:rangeIncludes":{"@id":"xsd:boolean"},"schema:domainIncludes":{"@id":"sustainability:StaffRequirements"},"rdfs:comment":"Does the standard include criteria on staff training programs for manufacturing workers"},{"@id":"sustainability:workers_staff_protective_clothing","@type":["rdf:Property","owl:DatatypeProperty"],"rdfs:label":"workers_staff_protective_clothing","schema:rangeIncludes":{"@id":"xsd:boolean"},"schema:domainIncludes":{"@id":"sustainability:StaffRequirements"},"rdfs:comment":"Does the standard include criteria on protective clothing for manufacturing workers"},{"@id":"sustainability:general_principle_about_food_safety","@type":["rdf:Property","owl:DatatypeProperty"],"rdfs:label":"general_principle_about_food_safety","schema:rangeIncludes":{"@id":"xsd:string"},"schema:domainIncludes":{"@id":"sustainability:SafetyHaccpSystem"},"rdfs:comment":"Does the standard include a general principle on food safety"},{"@id":"sustainability:general_principle_about_irradiation","@type":["rdf:Property","owl:DatatypeProperty"],"rdfs:label":"general_principle_about_irradiation","schema:rangeIncludes":{"@id":"xsd:boolean"},"schema:domainIncludes":{"@id":"sustainability:SafetyHaccpSystem"},"rdfs:comment":"Does the standard include a general principle on the irradiation of food products"},{"@id":"sustainability:general_principle_about_chilling_storage_and_transportation","@type":["rdf:Property","owl:DatatypeProperty"],"rdfs:label":"general_principle_about_chilling_storage_and_transportation","schema:rangeIncludes":{"@id":"xsd:boolean"},"schema:domainIncludes":{"@id":"sustainability:SafetyHaccpSystem"},"rdfs:comment":"Does the standard include a general principle on the chilling, storage and transportation of food products"},{"@id":"sustainability:transportation_of_food_products","@type":["rdf:Property","owl:DatatypeProperty"],"rdfs:label":"transportation_of_food_products","schema:rangeIncludes":{"@id":"xsd:boolean"},"schema:domainIncludes":{"@id":"sustainability:SafetyHaccpSystem"},"rdfs:comment":"Does the standard include criteria related to the transportation of food products"},{"@id":"sustainability:haccp_principle1_is_a_hazard_analysis_conducted_for_each_process_step_in_the_manufacturing_of_the_food_item","@type":["rdf:Property","owl:DatatypeProperty"],"rdfs:label":"haccp_principle1_is_a_hazard_analysis_conducted_for_each_process_step_in_the_manufacturing_of_the_food_item","schema:rangeIncludes":{"@id":"xsd:boolean"},"schema:domainIncludes":{"@id":"sustainability:SafetyHaccpSystem"},"rdfs:comment":"Does the standard include criteria related to HACCP Principle 1 (Conduct a Hazard Analysis)"},{"@id":"sustainability:haccp_principle2_if_the_hazard_analysis_indicates_any_hazards_present_within_the_food_manufacturing_process_are_critical_control_points_ccps_identified","@type":["rdf:Property","owl:DatatypeProperty"],"rdfs:label":"haccp_principle2_if_the_hazard_analysis_indicates_any_hazards_present_within_the_food_manufacturing_process_are_critical_control_points_ccps_identified","schema:rangeIncludes":{"@id":"xsd:boolean"},"schema:domainIncludes":{"@id":"sustainability:SafetyHaccpSystem"},"rdfs:comment":"Does the standard include criteria related to HACCP Principle 2 (Determine the Critical Control Points (CCPs))"},{"@id":"sustainability:haccp_principle3_are_critical_limits_established_for_each_ccp","@type":["rdf:Property","owl:DatatypeProperty"],"rdfs:label":"haccp_principle3_are_critical_limits_established_for_each_ccp","schema:rangeIncludes":{"@id":"xsd:boolean"},"schema:domainIncludes":{"@id":"sustainability:SafetyHaccpSystem"},"rdfs:comment":"Does the standard include criteria related to HACCP Principle 3 (Establish Critical Limits for each CCP)"},{"@id":"sustainability:haccp_principle4_are_monitoring_procedures_established_for_each_ccp","@type":["rdf:Property","owl:DatatypeProperty"],"rdfs:label":"haccp_principle4_are_monitoring_procedures_established_for_each_ccp","schema:rangeIncludes":{"@id":"xsd:boolean"},"schema:domainIncludes":{"@id":"sustainability:SafetyHaccpSystem"},"rdfs:comment":"Does the standard include criteria related to HACCP Principle 4 (Establish a Monitoring System for each CCP)"},{"@id":"sustainability:haccp_principle5_are_corrective_actions_established_for_each_ccp_in_the_event_critical_limits_are_exceeded","@type":["rdf:Property","owl:DatatypeProperty"],"rdfs:label":"haccp_principle5_are_corrective_actions_established_for_each_ccp_in_the_event_critical_limits_are_exceeded","schema:rangeIncludes":{"@id":"xsd:boolean"},"schema:domainIncludes":{"@id":"sustainability:SafetyHaccpSystem"},"rdfs:comment":"Does the standard include criteria related to HACCP Principle 5 (Establish a Corrective Action Plan)"},{"@id":"sustainability:haccp_principle6_are_verification_procedures_established","@type":["rdf:Property","owl:DatatypeProperty"],"rdfs:label":"haccp_principle6_are_verification_procedures_established","schema:rangeIncludes":{"@id":"xsd:boolean"},"schema:domainIncludes":{"@id":"sustainability:SafetyHaccpSystem"},"rdfs:comment":"Does the standard include criteria related to HACCP Principle 6 (Establish Verification Procedures)"},{"@id":"sustainability:haccp_principle7_are_record_keeping_and_documentation_for_haccp_procedures_established","@type":["rdf:Property","owl:DatatypeProperty"],"rdfs:label":"haccp_principle7_are_record_keeping_and_documentation_for_haccp_procedures_established","schema:rangeIncludes":{"@id":"xsd:boolean"},"schema:domainIncludes":{"@id":"sustainability:SafetyHaccpSystem"},"rdfs:comment":"Does the standard include criteria related to HACCP Principle 7 (Establish HACCP Documentation and Record Keeping and Review)"},{"@id":"sustainability:haccp_existence_of_a_haccp_system","@type":["rdf:Property","owl:DatatypeProperty"],"rdfs:label":"haccp_existence_of_a_haccp_system","schema:rangeIncludes":{"@id":"xsd:boolean"},"schema:domainIncludes":{"@id":"sustainability:SafetyHaccpSystem"},"rdfs:comment":"Does the standard require that the unit of operation has an established HACCP system"},{"@id":"sustainability:haccp_system_team_composed_of_multidisciplinary_skills","@type":["rdf:Property","owl:DatatypeProperty"],"rdfs:label":"haccp_system_team_composed_of_multidisciplinary_skills","schema:rangeIncludes":{"@id":"xsd:boolean"},"schema:domainIncludes":{"@id":"sustainability:SafetyHaccpSystem"},"rdfs:comment":"Does the standard require that the HACCP team is composed of multi-disciplinary skills"},{"@id":"sustainability:haccp_system_team_leader_mandatory_training","@type":["rdf:Property","owl:DatatypeProperty"],"rdfs:label":"haccp_system_team_leader_mandatory_training","schema:rangeIncludes":{"@id":"xsd:boolean"},"schema:domainIncludes":{"@id":"sustainability:SafetyHaccpSystem"},"rdfs:comment":"Does the standard require mandatory training for the HACCP team leader"},{"@id":"sustainability:haccp_system_critical_control_points_critical_limits_monitoring_procedures_established_and_monitored","@type":["rdf:Property","owl:DatatypeProperty"],"rdfs:label":"haccp_system_critical_control_points_critical_limits_monitoring_procedures_established_and_monitored","schema:rangeIncludes":{"@id":"xsd:boolean"},"schema:domainIncludes":{"@id":"sustainability:SafetyHaccpSystem"},"rdfs:comment":"Does the standard require that critical control points, critical limits and monitoring procedures are established and monitored according to the HACCP system"},{"@id":"sustainability:haccp_system_established_documented_and_monitored_corrective_actions","@type":["rdf:Property","owl:DatatypeProperty"],"rdfs:label":"haccp_system_established_documented_and_monitored_corrective_actions","schema:rangeIncludes":{"@id":"xsd:boolean"},"schema:domainIncludes":{"@id":"sustainability:SafetyHaccpSystem"},"rdfs:comment":"Does the standard require that corrective actions are established, documented and monitored according to the HACCP system"},{"@id":"sustainability:haccp_system_procedures_in_place_to_verify_efficiency_of_the_haccp_system","@type":["rdf:Property","owl:DatatypeProperty"],"rdfs:label":"haccp_system_procedures_in_place_to_verify_efficiency_of_the_haccp_system","schema:rangeIncludes":{"@id":"xsd:boolean"},"schema:domainIncludes":{"@id":"sustainability:SafetyHaccpSystem"},"rdfs:comment":"Does the standard require that procedures are in place to verify efficiency of the HACCP system"},{"@id":"sustainability:established_and_documented_policy_relating_to_control_measures_implemented_to_mitigate_food_safety_hazards","@type":["rdf:Property","owl:DatatypeProperty"],"rdfs:label":"established_and_documented_policy_relating_to_control_measures_implemented_to_mitigate_food_safety_hazards","schema:rangeIncludes":{"@id":"xsd:boolean"},"schema:domainIncludes":{"@id":"sustainability:SafetyHaccpSystem"},"rdfs:comment":"Does the standard require an established and documented policy relating to control measures implemented to mitigate food safety hazards"},{"@id":"sustainability:established_and_documented_policy_relating_to_food_contamination","@type":["rdf:Property","owl:DatatypeProperty"],"rdfs:label":"established_and_documented_policy_relating_to_food_contamination","schema:rangeIncludes":{"@id":"xsd:boolean"},"schema:domainIncludes":{"@id":"sustainability:SafetyHaccpSystem"},"rdfs:comment":"Does the standard require an established and documented policy relating to mitigation of threats of food contamination"},{"@id":"sustainability:contamination_in_food_harvesting","@type":["rdf:Property","owl:DatatypeProperty"],"rdfs:label":"contamination_in_food_harvesting","schema:rangeIncludes":{"@id":"xsd:boolean"},"schema:domainIncludes":{"@id":"sustainability:SafetyHaccpSystem"},"rdfs:comment":"Does the standard include criteria related to mitigation of threats of contamination in food harvesting"},{"@id":"sustainability:contamination_in_food_handling_incl_washing","@type":["rdf:Property","owl:DatatypeProperty"],"rdfs:label":"contamination_in_food_handling_incl_washing","schema:rangeIncludes":{"@id":"xsd:boolean"},"schema:domainIncludes":{"@id":"sustainability:SafetyHaccpSystem"},"rdfs:comment":"Does the standard include criteria related to mitigation of threats of contamination in food handling (incl. washing)"},{"@id":"sustainability:contamination_in_food_transportation","@type":["rdf:Property","owl:DatatypeProperty"],"rdfs:label":"contamination_in_food_transportation","schema:rangeIncludes":{"@id":"xsd:boolean"},"schema:domainIncludes":{"@id":"sustainability:SafetyHaccpSystem"},"rdfs:comment":"Does the standard include criteria related to mitigation of threats of contamination in food transportation"},{"@id":"sustainability:contamination_in_food_processing","@type":["rdf:Property","owl:DatatypeProperty"],"rdfs:label":"contamination_in_food_processing","schema:rangeIncludes":{"@id":"xsd:boolean"},"schema:domainIncludes":{"@id":"sustainability:SafetyHaccpSystem"},"rdfs:comment":"Does the standard include criteria related to mitigation of threats of contamination in food processing"},{"@id":"sustainability:contamination_in_food_packaging","@type":["rdf:Property","owl:DatatypeProperty"],"rdfs:label":"contamination_in_food_packaging","schema:rangeIncludes":{"@id":"xsd:boolean"},"schema:domainIncludes":{"@id":"sustainability:SafetyHaccpSystem"},"rdfs:comment":"Does the standard include criteria related to mitigation of threats of contamination in food packaging"},{"@id":"sustainability:site_location","@type":["rdf:Property","owl:DatatypeProperty"],"rdfs:label":"site_location","schema:rangeIncludes":{"@id":"xsd:boolean"},"schema:domainIncludes":{"@id":"sustainability:ProductionSite"},"rdfs:comment":"Does the standard address production site location as a critical control point of the food management system"},{"@id":"sustainability:site_and_facilities_disinfection_procedures","@type":["rdf:Property","owl:DatatypeProperty"],"rdfs:label":"site_and_facilities_disinfection_procedures","schema:rangeIncludes":{"@id":"xsd:boolean"},"schema:domainIncludes":{"@id":"sustainability:ProductionSite"},"rdfs:comment":"Does the standard require that the food production site has site and facilities disinfection procedures"},{"@id":"sustainability:staff_facilities_hand_washing_and_toilets_hygiene_requirements","@type":["rdf:Property","owl:DatatypeProperty"],"rdfs:label":"staff_facilities_hand_washing_and_toilets_hygiene_requirements","schema:rangeIncludes":{"@id":"xsd:boolean"},"schema:domainIncludes":{"@id":"sustainability:ProductionSite"},"rdfs:comment":"Does the standard include requirements for hand washing and toilet hygiene for staff facilities in the food production site"},{"@id":"sustainability:staff_facilities_changing_facilities_lockers_and_catering_specifications","@type":["rdf:Property","owl:DatatypeProperty"],"rdfs:label":"staff_facilities_changing_facilities_lockers_and_catering_specifications","schema:rangeIncludes":{"@id":"xsd:boolean"},"schema:domainIncludes":{"@id":"sustainability:ProductionSite"},"rdfs:comment":"Does the standard require that staff changing facilities, lockers and catering areas follow proper specifications for food production sites"},{"@id":"sustainability:staff_facilities_eating_places_segregated_from_production_areas","@type":["rdf:Property","owl:DatatypeProperty"],"rdfs:label":"staff_facilities_eating_places_segregated_from_production_areas","schema:rangeIncludes":{"@id":"xsd:boolean"},"schema:domainIncludes":{"@id":"sustainability:ProductionSite"},"rdfs:comment":"Does the standard require that staff eating places are segregated from production areas in the food production site"},{"@id":"sustainability:food_feed_production_site_pest_control_procedures","@type":["rdf:Property","owl:DatatypeProperty"],"rdfs:label":"food_feed_production_site_pest_control_procedures","schema:rangeIncludes":{"@id":"xsd:boolean"},"schema:domainIncludes":{"@id":"sustainability:ProductionSite"},"rdfs:comment":"Does the standard require that the food production site has pest control procedures in place"},{"@id":"sustainability:access_to_the_site","@type":["rdf:Property","owl:DatatypeProperty"],"rdfs:label":"access_to_the_site","schema:rangeIncludes":{"@id":"xsd:boolean"},"schema:domainIncludes":{"@id":"sustainability:ProductionSite"},"rdfs:comment":"Does the standard include criteria related to controlled access to the food production site"},{"@id":"sustainability:risk_assessment_of_site_and_processes_risks_of_contamination","@type":["rdf:Property","owl:DatatypeProperty"],"rdfs:label":"risk_assessment_of_site_and_processes_risks_of_contamination","schema:rangeIncludes":{"@id":"xsd:boolean"},"schema:domainIncludes":{"@id":"sustainability:ProductionSite"},"rdfs:comment":"Does the standard require a risk assessment of the production site and processes (risks of contamination)"},{"@id":"sustainability:food_harvesting_processing_utensils_cleaned_disinfected_sanitized_maintained_and_protected_from_contamination","@type":["rdf:Property","owl:DatatypeProperty"],"rdfs:label":"food_harvesting_processing_utensils_cleaned_disinfected_sanitized_maintained_and_protected_from_contamination","schema:rangeIncludes":{"@id":"xsd:boolean"},"schema:domainIncludes":{"@id":"sustainability:ProductionSite"},"rdfs:comment":"Does the standard require that food harvesting/processing utensils are cleaned, disinfected/sanitized, maintained and protected from contamination"},{"@id":"sustainability:site_construction_materials_appropriate_risks_of_contamination","@type":["rdf:Property","owl:DatatypeProperty"],"rdfs:label":"site_construction_materials_appropriate_risks_of_contamination","schema:rangeIncludes":{"@id":"xsd:boolean"},"schema:domainIncludes":{"@id":"sustainability:ProductionSite"},"rdfs:comment":"Does the standard require that the production site is constructed using appropriate materials to avoid risk of food contamination"},{"@id":"sustainability:water_supply_volume_and_quality_monitored","@type":["rdf:Property","owl:DatatypeProperty"],"rdfs:label":"water_supply_volume_and_quality_monitored","schema:rangeIncludes":{"@id":"xsd:boolean"},"schema:domainIncludes":{"@id":"sustainability:ProductionSite"},"rdfs:comment":"Does the standard require monitoring of volumes and quality of water supply to the food production site"},{"@id":"sustainability:waste_management_system_volume_toxicity_recycling_discharge","@type":["rdf:Property","owl:DatatypeProperty"],"rdfs:label":"waste_management_system_volume_toxicity_recycling_discharge","schema:rangeIncludes":{"@id":"xsd:boolean"},"schema:domainIncludes":{"@id":"sustainability:ProductionSite"},"rdfs:comment":"Does the standard require that the food production site has a waste management system (volume, toxicity, recycling, discharge)"},{"@id":"sustainability:waste_water_drainage_discharge_re_using_recycling_processes","@type":["rdf:Property","owl:DatatypeProperty"],"rdfs:label":"waste_water_drainage_discharge_re_using_recycling_processes","schema:rangeIncludes":{"@id":"xsd:boolean"},"schema:domainIncludes":{"@id":"sustainability:ProductionSite"},"rdfs:comment":"Does the standard require that the food production site has waste water drainage, discharge, re-using and recycling processes"},{"@id":"sustainability:site_and_facilities_cleaning_procedures","@type":["rdf:Property","owl:DatatypeProperty"],"rdfs:label":"site_and_facilities_cleaning_procedures","schema:rangeIncludes":{"@id":"xsd:boolean"},"schema:domainIncludes":{"@id":"sustainability:ProductionSite"},"rdfs:comment":"Does the standard require that the food production site has site and facilities cleaning procedures"},{"@id":"sustainability:gmo_handling_procedures_and_staff_training","@type":["rdf:Property","owl:DatatypeProperty"],"rdfs:label":"gmo_handling_procedures_and_staff_training","schema:rangeIncludes":{"@id":"xsd:boolean"},"schema:domainIncludes":{"@id":"sustainability:TracebilityRecallAndAllergens"},"rdfs:comment":"Does the standard require GMO handling procedures and staff training to be in place"},{"@id":"sustainability:gmo_inputs_selection_and_technical_specifications","@type":["rdf:Property","owl:DatatypeProperty"],"rdfs:label":"gmo_inputs_selection_and_technical_specifications","schema:rangeIncludes":{"@id":"xsd:boolean"},"schema:domainIncludes":{"@id":"sustainability:TracebilityRecallAndAllergens"},"rdfs:comment":"Does the standard require technical specifications and inputs selection of GMOs for food production"},{"@id":"sustainability:allergen_handling_procedures_and_staff_training","@type":["rdf:Property","owl:DatatypeProperty"],"rdfs:label":"allergen_handling_procedures_and_staff_training","schema:rangeIncludes":{"@id":"xsd:boolean"},"schema:domainIncludes":{"@id":"sustainability:TracebilityRecallAndAllergens"},"rdfs:comment":"Does the standard require allergen handling procedures and staff training"},{"@id":"sustainability:allergen_inputs_selection_and_technical_specifications","@type":["rdf:Property","owl:DatatypeProperty"],"rdfs:label":"allergen_inputs_selection_and_technical_specifications","schema:rangeIncludes":{"@id":"xsd:boolean"},"schema:domainIncludes":{"@id":"sustainability:TracebilityRecallAndAllergens"},"rdfs:comment":"Does the standard require technical specifications and inputs selection of allergens for food production"},{"@id":"sustainability:risk_of_contamination_from_raw_material_control_of_inputs_and_ingredients","@type":["rdf:Property","owl:DatatypeProperty"],"rdfs:label":"risk_of_contamination_from_raw_material_control_of_inputs_and_ingredients","schema:rangeIncludes":{"@id":"xsd:boolean"},"schema:domainIncludes":{"@id":"sustainability:ForeignBodiesAndContamination"},"rdfs:comment":"Does the standard require the control of inputs and ingredients to avoid risk of contamination from raw material in food production"},{"@id":"sustainability:contamination_waste_disposal_contamination_risk_assessment_and_discharge_procedures","@type":["rdf:Property","owl:DatatypeProperty"],"rdfs:label":"contamination_waste_disposal_contamination_risk_assessment_and_discharge_procedures","schema:rangeIncludes":{"@id":"xsd:boolean"},"schema:domainIncludes":{"@id":"sustainability:ForeignBodiesAndContamination"},"rdfs:comment":"Does the standard require a risk assessment for waste disposal contamination and discharge procedures to be in place to avoid risk of contamination in the food production system"},{"@id":"sustainability:contamination_foreign_body_control_detector_monitoring_procedures","@type":["rdf:Property","owl:DatatypeProperty"],"rdfs:label":"contamination_foreign_body_control_detector_monitoring_procedures","schema:rangeIncludes":{"@id":"xsd:boolean"},"schema:domainIncludes":{"@id":"sustainability:ForeignBodiesAndContamination"},"rdfs:comment":"Does the standard require foreign body control & detection monitoring procedures to be in place for the production of food"},{"@id":"sustainability:food_products_handling_general_policy","@type":["rdf:Property","owl:DatatypeProperty"],"rdfs:label":"food_products_handling_general_policy","schema:rangeIncludes":{"@id":"xsd:boolean"},"schema:domainIncludes":{"@id":"sustainability:ForeignBodiesAndContamination"},"rdfs:comment":"Does the standard require the unit of operations to have a general policy on the handling of food products"},{"@id":"sustainability:food_products_handling_equipment_specifications_maintenance_and_testing","@type":["rdf:Property","owl:DatatypeProperty"],"rdfs:label":"food_products_handling_equipment_specifications_maintenance_and_testing","schema:rangeIncludes":{"@id":"xsd:boolean"},"schema:domainIncludes":{"@id":"sustainability:ForeignBodiesAndContamination"},"rdfs:comment":"Does the standard require specifications, maintenance and testing to be in place for all equipment used in the handling of food"},{"@id":"sustainability:food_products_handling_storage_facilities_specifications_hygiene_maintenance_and_verification","@type":["rdf:Property","owl:DatatypeProperty"],"rdfs:label":"food_products_handling_storage_facilities_specifications_hygiene_maintenance_and_verification","schema:rangeIncludes":{"@id":"xsd:boolean"},"schema:domainIncludes":{"@id":"sustainability:ForeignBodiesAndContamination"},"rdfs:comment":"Does the standard include criteria on storage facilities specifications, hygiene maintenance and verification in the handling of food"},{"@id":"sustainability:food_products_handling_storage_conditions_hygiene_requirements_and_verification_processes","@type":["rdf:Property","owl:DatatypeProperty"],"rdfs:label":"food_products_handling_storage_conditions_hygiene_requirements_and_verification_processes","schema:rangeIncludes":{"@id":"xsd:boolean"},"schema:domainIncludes":{"@id":"sustainability:ForeignBodiesAndContamination"},"rdfs:comment":"Does the standard include criteria on storage conditions, hygiene requirements and verification processes in the handling of food"},{"@id":"sustainability:food_products_handling_packaging_and_labeling_requirements","@type":["rdf:Property","owl:DatatypeProperty"],"rdfs:label":"food_products_handling_packaging_and_labeling_requirements","schema:rangeIncludes":{"@id":"xsd:boolean"},"schema:domainIncludes":{"@id":"sustainability:ForeignBodiesAndContamination"},"rdfs:comment":"Does the standard include packaging and label requirements for the handling of food"},{"@id":"sustainability:semi_final_product_specifications_and_controls_of_risk_foreign_bodies","@type":["rdf:Property","owl:DatatypeProperty"],"rdfs:label":"semi_final_product_specifications_and_controls_of_risk_foreign_bodies","schema:rangeIncludes":{"@id":"xsd:boolean"},"schema:domainIncludes":{"@id":"sustainability:ForeignBodiesAndContamination"},"rdfs:comment":"Does the standard require product specifications and controls for the risk of foreign bodies in semi-final production"},{"@id":"sustainability:final_product_specifications_and_controls_for_contamination","@type":["rdf:Property","owl:DatatypeProperty"],"rdfs:label":"final_product_specifications_and_controls_for_contamination","schema:rangeIncludes":{"@id":"xsd:boolean"},"schema:domainIncludes":{"@id":"sustainability:ForeignBodiesAndContamination"},"rdfs:comment":"Does the standard require final product specifications and controls for contamination for food products"},{"@id":"sustainability:harvested_semi_processed_products_packaging_protection_against_contamination","@type":["rdf:Property","owl:DatatypeProperty"],"rdfs:label":"harvested_semi_processed_products_packaging_protection_against_contamination","schema:rangeIncludes":{"@id":"xsd:boolean"},"schema:domainIncludes":{"@id":"sustainability:ForeignBodiesAndContamination"},"rdfs:comment":"Does the standard include criteria related to packaging protection against contaminants for harvested / semi-processed products?"},{"@id":"sustainability:harvested_semi_processed_final_products_treatment_before_retail","@type":["rdf:Property","owl:DatatypeProperty"],"rdfs:label":"harvested_semi_processed_final_products_treatment_before_retail","schema:rangeIncludes":{"@id":"xsd:boolean"},"schema:domainIncludes":{"@id":"sustainability:ForeignBodiesAndContamination"},"rdfs:comment":"Does the standard include criteria on the treatment of harvested / semi-processed / final products before retail"},{"@id":"sustainability:contamination_glass_and_wood_foreign_bodies_inspection","@type":["rdf:Property","owl:DatatypeProperty"],"rdfs:label":"contamination_glass_and_wood_foreign_bodies_inspection","schema:rangeIncludes":{"@id":"xsd:boolean"},"schema:domainIncludes":{"@id":"sustainability:ForeignBodiesAndContamination"},"rdfs:comment":"Does the standard require procedures to be in place for the protection and inspection of glass and wood foreign body contaminants in the food production system"},{"@id":"sustainability:contamination_water_contamination_mitigation_controls_and_procedures","@type":["rdf:Property","owl:DatatypeProperty"],"rdfs:label":"contamination_water_contamination_mitigation_controls_and_procedures","schema:rangeIncludes":{"@id":"xsd:boolean"},"schema:domainIncludes":{"@id":"sustainability:ForeignBodiesAndContamination"},"rdfs:comment":"Does the standard require water contamination mitigation controls and procedures in the food production system"},{"@id":"sustainability:contamination_chemical_storage","@type":["rdf:Property","owl:DatatypeProperty"],"rdfs:label":"contamination_chemical_storage","schema:rangeIncludes":{"@id":"xsd:boolean"},"schema:domainIncludes":{"@id":"sustainability:ForeignBodiesAndContamination"},"rdfs:comment":"Does the standard include criteria on chemical storage to avoid contamination in the food production system"},{"@id":"sustainability:contamination_site_and_equipment_inspection","@type":["rdf:Property","owl:DatatypeProperty"],"rdfs:label":"contamination_site_and_equipment_inspection","schema:rangeIncludes":{"@id":"xsd:boolean"},"schema:domainIncludes":{"@id":"sustainability:ForeignBodiesAndContamination"},"rdfs:comment":"Does the standard require site and equipment inspection in the food production system"},{"@id":"sustainability:food_production_process_control_raw_material_intermediate_final_product_specifications","@type":["rdf:Property","owl:DatatypeProperty"],"rdfs:label":"food_production_process_control_raw_material_intermediate_final_product_specifications","schema:rangeIncludes":{"@id":"xsd:boolean"},"schema:domainIncludes":{"@id":"sustainability:ProcessAndProductControl"},"rdfs:comment":"Does the standard require specifications to be available for all raw materials, intermediate and final food products"},{"@id":"sustainability:food_production_process_control_product_transportation_procedures","@type":["rdf:Property","owl:DatatypeProperty"],"rdfs:label":"food_production_process_control_product_transportation_procedures","schema:rangeIncludes":{"@id":"xsd:boolean"},"schema:domainIncludes":{"@id":"sustainability:ProcessAndProductControl"},"rdfs:comment":"Does the standard require control processes to be in place for product transportation procedures"},{"@id":"sustainability:food_production_process_control_product_development_process","@type":["rdf:Property","owl:DatatypeProperty"],"rdfs:label":"food_production_process_control_product_development_process","schema:rangeIncludes":{"@id":"xsd:boolean"},"schema:domainIncludes":{"@id":"sustainability:ProcessAndProductControl"},"rdfs:comment":"Does the standard require control processes to be in place for food product development"},{"@id":"sustainability:food_feed_production_process_control_nutritional_requirements","@type":["rdf:Property","owl:DatatypeProperty"],"rdfs:label":"food_feed_production_process_control_nutritional_requirements","schema:rangeIncludes":{"@id":"xsd:boolean"},"schema:domainIncludes":{"@id":"sustainability:ProcessAndProductControl"},"rdfs:comment":"Does the standard require control processes for nutritional requirements to be in place for food / feed production"},{"@id":"sustainability:food_production_process_control_packaging_material_procedures","@type":["rdf:Property","owl:DatatypeProperty"],"rdfs:label":"food_production_process_control_packaging_material_procedures","schema:rangeIncludes":{"@id":"xsd:boolean"},"schema:domainIncludes":{"@id":"sustainability:ProcessAndProductControl"},"rdfs:comment":"Does the standard require control processes to be in place for packaging material and procedures"},{"@id":"sustainability:food_production_process_control_product_analysis_and_testing","@type":["rdf:Property","owl:DatatypeProperty"],"rdfs:label":"food_production_process_control_product_analysis_and_testing","schema:rangeIncludes":{"@id":"xsd:boolean"},"schema:domainIncludes":{"@id":"sustainability:ProcessAndProductControl"},"rdfs:comment":"Does the standard require control processes to be in place for food product analysis and testing"},{"@id":"sustainability:food_feed_production_process_control_health_and_nutrition_requirements","@type":["rdf:Property","owl:DatatypeProperty"],"rdfs:label":"food_feed_production_process_control_health_and_nutrition_requirements","schema:rangeIncludes":{"@id":"xsd:boolean"},"schema:domainIncludes":{"@id":"sustainability:ProcessAndProductControl"},"rdfs:comment":"Does the standard require control processes to be in place for food / feed health and nutritional requirements"},{"@id":"sustainability:food_production_process_control_quantity_control_procedures","@type":["rdf:Property","owl:DatatypeProperty"],"rdfs:label":"food_production_process_control_quantity_control_procedures","schema:rangeIncludes":{"@id":"xsd:boolean"},"schema:domainIncludes":{"@id":"sustainability:ProcessAndProductControl"},"rdfs:comment":"Does the standard require control processes to be in place for quantity control"},{"@id":"sustainability:food_production_process_control_management_of_non_conforming_products","@type":["rdf:Property","owl:DatatypeProperty"],"rdfs:label":"food_production_process_control_management_of_non_conforming_products","schema:rangeIncludes":{"@id":"xsd:boolean"},"schema:domainIncludes":{"@id":"sustainability:ProcessAndProductControl"},"rdfs:comment":"Does the standard require control processes to be in place for management of non-conforming products"},{"@id":"sustainability:food_production_process_control_verification_calibration_of_monitoring_devices","@type":["rdf:Property","owl:DatatypeProperty"],"rdfs:label":"food_production_process_control_verification_calibration_of_monitoring_devices","schema:rangeIncludes":{"@id":"xsd:boolean"},"schema:domainIncludes":{"@id":"sustainability:ProcessAndProductControl"},"rdfs:comment":"Does the standard require control processes to be in place for verification/calibration of monitoring devices"},{"@id":"sustainability:food_production_personnel_skills_training_records","@type":["rdf:Property","owl:DatatypeProperty"],"rdfs:label":"food_production_personnel_skills_training_records","schema:rangeIncludes":{"@id":"xsd:boolean"},"schema:domainIncludes":{"@id":"sustainability:WorkersRequirements"},"rdfs:comment":"Does the standard address personnel skills and require records of training for food production workers"},{"@id":"sustainability:food_production_workers_staff_training_programs","@type":["rdf:Property","owl:DatatypeProperty"],"rdfs:label":"food_production_workers_staff_training_programs","schema:rangeIncludes":{"@id":"xsd:boolean"},"schema:domainIncludes":{"@id":"sustainability:WorkersRequirements"},"rdfs:comment":"Does the standard require the unit of operations to provide training programs for food production workers/staff"},{"@id":"sustainability:food_production_personal_hygiene","@type":["rdf:Property","owl:DatatypeProperty"],"rdfs:label":"food_production_personal_hygiene","schema:rangeIncludes":{"@id":"xsd:boolean"},"schema:domainIncludes":{"@id":"sustainability:WorkersRequirements"},"rdfs:comment":"Does the standard require that all workers / staff comply with good personal hygiene practices"},{"@id":"sustainability:food_production_medical_screening","@type":["rdf:Property","owl:DatatypeProperty"],"rdfs:label":"food_production_medical_screening","schema:rangeIncludes":{"@id":"xsd:boolean"},"schema:domainIncludes":{"@id":"sustainability:WorkersRequirements"},"rdfs:comment":"Does the standard require that all food production workers / staff undergo medical screening prior to working with food"},{"@id":"sustainability:food_production_protective_clothing","@type":["rdf:Property","owl:DatatypeProperty"],"rdfs:label":"food_production_protective_clothing","schema:rangeIncludes":{"@id":"xsd:boolean"},"schema:domainIncludes":{"@id":"sustainability:WorkersRequirements"},"rdfs:comment":"Does the standard require that all food production workers / staff wear protective clothing"},{"@id":"sustainability:definition_of_scope","@type":["rdf:Property","owl:DatatypeProperty"],"rdfs:label":"definition_of_scope","schema:rangeIncludes":{"@id":"xsd:string"},"schema:domainIncludes":{"@id":"sustainability:ManagementSystem"},"rdfs:comment":"Definition of scope"},{"@id":"sustainability:determination_of_all_necessary_inspections_monitoring_and_measurements","@type":["rdf:Property","owl:DatatypeProperty"],"rdfs:label":"determination_of_all_necessary_inspections_monitoring_and_measurements","schema:rangeIncludes":{"@id":"xsd:boolean"},"schema:domainIncludes":{"@id":"sustainability:ManagementSystem"},"rdfs:comment":"Determination of all necessary inspections, monitoring and measurements"},{"@id":"sustainability:implementation_of_actions_to_achieve_planned_results","@type":["rdf:Property","owl:DatatypeProperty"],"rdfs:label":"implementation_of_actions_to_achieve_planned_results","schema:rangeIncludes":{"@id":"xsd:boolean"},"schema:domainIncludes":{"@id":"sustainability:ManagementSystem"},"rdfs:comment":"Implementation of actions to achieve planned results"},{"@id":"sustainability:compliance_with_all_relevant_legal_feed_safety_requirements","@type":["rdf:Property","owl:DatatypeProperty"],"rdfs:label":"compliance_with_all_relevant_legal_feed_safety_requirements","schema:rangeIncludes":{"@id":"xsd:boolean"},"schema:domainIncludes":{"@id":"sustainability:ManagementSystem"},"rdfs:comment":"Compliance with all relevant legal feed safety requirements"},{"@id":"sustainability:keep_up_with_all_relevant_legal_developments","@type":["rdf:Property","owl:DatatypeProperty"],"rdfs:label":"keep_up_with_all_relevant_legal_developments","schema:rangeIncludes":{"@id":"xsd:boolean"},"schema:domainIncludes":{"@id":"sustainability:ManagementSystem"},"rdfs:comment":"Keep up with all relevant legal developments"},{"@id":"sustainability:communication_within_the_organisation_and_upstream_downstream_in_the_chain","@type":["rdf:Property","owl:DatatypeProperty"],"rdfs:label":"communication_within_the_organisation_and_upstream_downstream_in_the_chain","schema:rangeIncludes":{"@id":"xsd:boolean"},"schema:domainIncludes":{"@id":"sustainability:ManagementSystem"},"rdfs:comment":"Communication within the organisation and upstream/downstream in the chain"},{"@id":"sustainability:determination_of_processes_and_their_interactions","@type":["rdf:Property","owl:DatatypeProperty"],"rdfs:label":"determination_of_processes_and_their_interactions","schema:rangeIncludes":{"@id":"xsd:boolean"},"schema:domainIncludes":{"@id":"sustainability:ManagementSystem"},"rdfs:comment":"Determination of processes and their interactions"},{"@id":"sustainability:identification_of_all_critical_elements_in_the_processes","@type":["rdf:Property","owl:DatatypeProperty"],"rdfs:label":"identification_of_all_critical_elements_in_the_processes","schema:rangeIncludes":{"@id":"xsd:boolean"},"schema:domainIncludes":{"@id":"sustainability:ManagementSystem"},"rdfs:comment":"Identification of all critical elements in the processes"},{"@id":"sustainability:determination_of_criteria_and_methods_to_ensure_effective_operation","@type":["rdf:Property","owl:DatatypeProperty"],"rdfs:label":"determination_of_criteria_and_methods_to_ensure_effective_operation","schema:rangeIncludes":{"@id":"xsd:boolean"},"schema:domainIncludes":{"@id":"sustainability:ManagementSystem"},"rdfs:comment":"Determination of criteria and methods to ensure effective operation"},{"@id":"sustainability:determination_of_criteria_and_methods_to_control_the_risks","@type":["rdf:Property","owl:DatatypeProperty"],"rdfs:label":"determination_of_criteria_and_methods_to_control_the_risks","schema:rangeIncludes":{"@id":"xsd:boolean"},"schema:domainIncludes":{"@id":"sustainability:ManagementSystem"},"rdfs:comment":"Determination of criteria and methods to control the risks"},{"@id":"sustainability:establish_and_implement_prerequisite_programmes","@type":["rdf:Property","owl:DatatypeProperty"],"rdfs:label":"establish_and_implement_prerequisite_programmes","schema:rangeIncludes":{"@id":"xsd:boolean"},"schema:domainIncludes":{"@id":"sustainability:ManagementSystem"},"rdfs:comment":"Establish and implement prerequisite programmes"},{"@id":"sustainability:establish_and_implement_a_haccp_plan","@type":["rdf:Property","owl:DatatypeProperty"],"rdfs:label":"establish_and_implement_a_haccp_plan","schema:rangeIncludes":{"@id":"xsd:boolean"},"schema:domainIncludes":{"@id":"sustainability:ManagementSystem"},"rdfs:comment":"Establish and implement a HACCP-plan"},{"@id":"sustainability:availability_of_information_to_support_correct_operation_and_control","@type":["rdf:Property","owl:DatatypeProperty"],"rdfs:label":"availability_of_information_to_support_correct_operation_and_control","schema:rangeIncludes":{"@id":"xsd:boolean"},"schema:domainIncludes":{"@id":"sustainability:ManagementSystem"},"rdfs:comment":"Availability of information to support correct operation and control"},{"@id":"sustainability:availability_of_resources","@type":["rdf:Property","owl:DatatypeProperty"],"rdfs:label":"availability_of_resources","schema:rangeIncludes":{"@id":"xsd:boolean"},"schema:domainIncludes":{"@id":"sustainability:ManagementSystem"},"rdfs:comment":"Availability of resources"},{"@id":"sustainability:specification_of_feed_products_and_or_feed_services_covered_under_the_scope","@type":["rdf:Property","owl:DatatypeProperty"],"rdfs:label":"specification_of_feed_products_and_or_feed_services_covered_under_the_scope","schema:rangeIncludes":{"@id":"xsd:boolean"},"schema:domainIncludes":{"@id":"sustainability:Specifications"},"rdfs:comment":"Specification of feed products and/or feed services covered under the scope"},{"@id":"sustainability:specification_of_legal_aspects","@type":["rdf:Property","owl:DatatypeProperty"],"rdfs:label":"specification_of_legal_aspects","schema:rangeIncludes":{"@id":"xsd:boolean"},"schema:domainIncludes":{"@id":"sustainability:Specifications"},"rdfs:comment":"Specification of legal aspects"},{"@id":"sustainability:specification_of_locations_and_sites_covered_under_the_scope","@type":["rdf:Property","owl:DatatypeProperty"],"rdfs:label":"specification_of_locations_and_sites_covered_under_the_scope","schema:rangeIncludes":{"@id":"xsd:boolean"},"schema:domainIncludes":{"@id":"sustainability:Specifications"},"rdfs:comment":"Specification of locations and sites covered under the scope"},{"@id":"sustainability:specification_of_processes_covered_under_the_scope","@type":["rdf:Property","owl:DatatypeProperty"],"rdfs:label":"specification_of_processes_covered_under_the_scope","schema:rangeIncludes":{"@id":"xsd:boolean"},"schema:domainIncludes":{"@id":"sustainability:Specifications"},"rdfs:comment":"Specification of processes covered under the scope"},{"@id":"sustainability:specification_of_outsourced_activities_covered_under_the_scope","@type":["rdf:Property","owl:DatatypeProperty"],"rdfs:label":"specification_of_outsourced_activities_covered_under_the_scope","schema:rangeIncludes":{"@id":"xsd:boolean"},"schema:domainIncludes":{"@id":"sustainability:Specifications"},"rdfs:comment":"Specification of outsourced activities covered under the scope"},{"@id":"sustainability:specification_of_exclusions","@type":["rdf:Property","owl:DatatypeProperty"],"rdfs:label":"specification_of_exclusions","schema:rangeIncludes":{"@id":"xsd:boolean"},"schema:domainIncludes":{"@id":"sustainability:Specifications"},"rdfs:comment":"Specification of exclusions"},{"@id":"sustainability:documentation_of_the_policy_and_related_feed_objectives","@type":["rdf:Property","owl:DatatypeProperty"],"rdfs:label":"documentation_of_the_policy_and_related_feed_objectives","schema:rangeIncludes":{"@id":"xsd:boolean"},"schema:domainIncludes":{"@id":"sustainability:Documentation"},"rdfs:comment":"Documentation of the policy and related feed objectives"},{"@id":"sustainability:safe_storage_of_data","@type":["rdf:Property","owl:DatatypeProperty"],"rdfs:label":"safe_storage_of_data","schema:rangeIncludes":{"@id":"xsd:boolean"},"schema:domainIncludes":{"@id":"sustainability:Documentation"},"rdfs:comment":"Safe storage of data"},{"@id":"sustainability:documentation_of_the_scope_description_as_specified_above","@type":["rdf:Property","owl:DatatypeProperty"],"rdfs:label":"documentation_of_the_scope_description_as_specified_above","schema:rangeIncludes":{"@id":"xsd:boolean"},"schema:domainIncludes":{"@id":"sustainability:Documentation"},"rdfs:comment":"Documentation of the scope description (as specified above)"},{"@id":"sustainability:documentation_of_the_required_procedures_and_instructions","@type":["rdf:Property","owl:DatatypeProperty"],"rdfs:label":"documentation_of_the_required_procedures_and_instructions","schema:rangeIncludes":{"@id":"xsd:boolean"},"schema:domainIncludes":{"@id":"sustainability:Documentation"},"rdfs:comment":"Documentation of the required procedures and instructions"},{"@id":"sustainability:documentation_of_other_documents_needed_to_ensure_an_effective_operation_of_fms","@type":["rdf:Property","owl:DatatypeProperty"],"rdfs:label":"documentation_of_other_documents_needed_to_ensure_an_effective_operation_of_fms","schema:rangeIncludes":{"@id":"xsd:boolean"},"schema:domainIncludes":{"@id":"sustainability:Documentation"},"rdfs:comment":"Documentation of other documents needed to ensure an effective operation of FMS"},{"@id":"sustainability:documentation_of_the_structure_of_the_controlled_documentation_system","@type":["rdf:Property","owl:DatatypeProperty"],"rdfs:label":"documentation_of_the_structure_of_the_controlled_documentation_system","schema:rangeIncludes":{"@id":"xsd:boolean"},"schema:domainIncludes":{"@id":"sustainability:Documentation"},"rdfs:comment":"Documentation of the structure of the controlled documentation system"},{"@id":"sustainability:a_procedure_to_draft_approve_issue_review_update_implement_and_control_the_documents","@type":["rdf:Property","owl:DatatypeProperty"],"rdfs:label":"a_procedure_to_draft_approve_issue_review_update_implement_and_control_the_documents","schema:rangeIncludes":{"@id":"xsd:boolean"},"schema:domainIncludes":{"@id":"sustainability:Documentation"},"rdfs:comment":"A procedure to draft, approve, issue, review, update, implement and control the documents."},{"@id":"sustainability:a_procedure_to_register_and_store_data_and_records","@type":["rdf:Property","owl:DatatypeProperty"],"rdfs:label":"a_procedure_to_register_and_store_data_and_records","schema:rangeIncludes":{"@id":"xsd:boolean"},"schema:domainIncludes":{"@id":"sustainability:Documentation"},"rdfs:comment":"A procedure to register and store data and records"},{"@id":"sustainability:a_procedure_to_guarantee_security_of_data_to_exclude_unauthorised_and_unwanted_change_of_data_and_to_exclude_fraud","@type":["rdf:Property","owl:DatatypeProperty"],"rdfs:label":"a_procedure_to_guarantee_security_of_data_to_exclude_unauthorised_and_unwanted_change_of_data_and_to_exclude_fraud","schema:rangeIncludes":{"@id":"xsd:boolean"},"schema:domainIncludes":{"@id":"sustainability:Documentation"},"rdfs:comment":"A procedure to guarantee security of data; to exclude unauthorised and unwanted change of data and to exclude fraud"},{"@id":"sustainability:a_time_period_for_retaining_records","@type":["rdf:Property","owl:DatatypeProperty"],"rdfs:label":"a_time_period_for_retaining_records","schema:rangeIncludes":{"@id":"xsd:boolean"},"schema:domainIncludes":{"@id":"sustainability:Documentation"},"rdfs:comment":"A time period for retaining records"},{"@id":"sustainability:demonstration_of_commitment_to_feed_safety_assurance","@type":["rdf:Property","owl:DatatypeProperty"],"rdfs:label":"demonstration_of_commitment_to_feed_safety_assurance","schema:rangeIncludes":{"@id":"xsd:boolean"},"schema:domainIncludes":{"@id":"sustainability:ManagementResponsibility"},"rdfs:comment":"Demonstration of commitment to feed safety assurance"},{"@id":"sustainability:definition_of_a_policy_which_includes_activities_needed_to_achieve_feed_safety_and_quality_requirements_of_customers","@type":["rdf:Property","owl:DatatypeProperty"],"rdfs:label":"definition_of_a_policy_which_includes_activities_needed_to_achieve_feed_safety_and_quality_requirements_of_customers","schema:rangeIncludes":{"@id":"xsd:boolean"},"schema:domainIncludes":{"@id":"sustainability:ManagementResponsibility"},"rdfs:comment":"Definition of a policy which includes activities needed to achieve feed safety and quality requirements of customers"},{"@id":"sustainability:definition_of_smart_objectives_related_to_the_policy","@type":["rdf:Property","owl:DatatypeProperty"],"rdfs:label":"definition_of_smart_objectives_related_to_the_policy","schema:rangeIncludes":{"@id":"xsd:boolean"},"schema:domainIncludes":{"@id":"sustainability:ManagementResponsibility"},"rdfs:comment":"Definition of smart objectives related to the policy"},{"@id":"sustainability:creation_of_awareness_in_the_organization_about_importance_of_feed_safety_assurance","@type":["rdf:Property","owl:DatatypeProperty"],"rdfs:label":"creation_of_awareness_in_the_organization_about_importance_of_feed_safety_assurance","schema:rangeIncludes":{"@id":"xsd:boolean"},"schema:domainIncludes":{"@id":"sustainability:ManagementResponsibility"},"rdfs:comment":"Creation of awareness in the organization about importance of feed safety assurance"},{"@id":"sustainability:operation_of_an_effective_fms","@type":["rdf:Property","owl:DatatypeProperty"],"rdfs:label":"operation_of_an_effective_fms","schema:rangeIncludes":{"@id":"xsd:boolean"},"schema:domainIncludes":{"@id":"sustainability:ManagementResponsibility"},"rdfs:comment":"Operation of an effective FMS"},{"@id":"sustainability:job_descriptions_addressing_responsibilities_and_authorities_regarding_feed_safety_assurance","@type":["rdf:Property","owl:DatatypeProperty"],"rdfs:label":"job_descriptions_addressing_responsibilities_and_authorities_regarding_feed_safety_assurance","schema:rangeIncludes":{"@id":"xsd:boolean"},"schema:domainIncludes":{"@id":"sustainability:ManagementResponsibility"},"rdfs:comment":"Job descriptions, addressing responsibilities and authorities regarding feed safety assurance"},{"@id":"sustainability:an_organogram","@type":["rdf:Property","owl:DatatypeProperty"],"rdfs:label":"an_organogram","schema:rangeIncludes":{"@id":"xsd:boolean"},"schema:domainIncludes":{"@id":"sustainability:ManagementResponsibility"},"rdfs:comment":"An organogram"},{"@id":"sustainability:establishing_a_haccp_team","@type":["rdf:Property","owl:DatatypeProperty"],"rdfs:label":"establishing_a_haccp_team","schema:rangeIncludes":{"@id":"xsd:boolean"},"schema:domainIncludes":{"@id":"sustainability:ManagementResponsibility"},"rdfs:comment":"Establishing a HACCP team"},{"@id":"sustainability:assurance_that_all_relevant_departments_are_represented_in_the_haccp_team","@type":["rdf:Property","owl:DatatypeProperty"],"rdfs:label":"assurance_that_all_relevant_departments_are_represented_in_the_haccp_team","schema:rangeIncludes":{"@id":"xsd:boolean"},"schema:domainIncludes":{"@id":"sustainability:ManagementResponsibility"},"rdfs:comment":"Assurance that all relevant departments are represented in the HACCP team"},{"@id":"sustainability:definition_of_skills_and_competences_for_each_member_of_the_haccp_team","@type":["rdf:Property","owl:DatatypeProperty"],"rdfs:label":"definition_of_skills_and_competences_for_each_member_of_the_haccp_team","schema:rangeIncludes":{"@id":"xsd:boolean"},"schema:domainIncludes":{"@id":"sustainability:ManagementResponsibility"},"rdfs:comment":"Definition of skills and competences for each member of the HACCP-team"},{"@id":"sustainability:appointment_of_a_haccp_team_leader","@type":["rdf:Property","owl:DatatypeProperty"],"rdfs:label":"appointment_of_a_haccp_team_leader","schema:rangeIncludes":{"@id":"xsd:boolean"},"schema:domainIncludes":{"@id":"sustainability:ManagementResponsibility"},"rdfs:comment":"Appointment of a HACCP team leader"},{"@id":"sustainability:internal_communication_of_the_importance_of_feed_safety_assurance","@type":["rdf:Property","owl:DatatypeProperty"],"rdfs:label":"internal_communication_of_the_importance_of_feed_safety_assurance","schema:rangeIncludes":{"@id":"xsd:boolean"},"schema:domainIncludes":{"@id":"sustainability:ManagementResponsibility"},"rdfs:comment":"Internal communication of the importance of feed safety assurance"},{"@id":"sustainability:arrangement_of_external_communication","@type":["rdf:Property","owl:DatatypeProperty"],"rdfs:label":"arrangement_of_external_communication","schema:rangeIncludes":{"@id":"xsd:boolean"},"schema:domainIncludes":{"@id":"sustainability:ManagementResponsibility"},"rdfs:comment":"Arrangement of external communication"},{"@id":"sustainability:arrangement_of_internal_communication","@type":["rdf:Property","owl:DatatypeProperty"],"rdfs:label":"arrangement_of_internal_communication","schema:rangeIncludes":{"@id":"xsd:boolean"},"schema:domainIncludes":{"@id":"sustainability:ManagementResponsibility"},"rdfs:comment":"Arrangement of internal communication"},{"@id":"sustainability:review_of_monitoring_plan","@type":["rdf:Property","owl:DatatypeProperty"],"rdfs:label":"review_of_monitoring_plan","schema:rangeIncludes":{"@id":"xsd:boolean"},"schema:domainIncludes":{"@id":"sustainability:ManagementResponsibility"},"rdfs:comment":"Review of monitoring plan"},{"@id":"sustainability:review_of_external_audit","@type":["rdf:Property","owl:DatatypeProperty"],"rdfs:label":"review_of_external_audit","schema:rangeIncludes":{"@id":"xsd:boolean"},"schema:domainIncludes":{"@id":"sustainability:ManagementResponsibility"},"rdfs:comment":"Review of external audit"},{"@id":"sustainability:review_of_internal_audit","@type":["rdf:Property","owl:DatatypeProperty"],"rdfs:label":"review_of_internal_audit","schema:rangeIncludes":{"@id":"xsd:boolean"},"schema:domainIncludes":{"@id":"sustainability:ManagementResponsibility"},"rdfs:comment":"Review of internal audit"},{"@id":"sustainability:review_of_customer_satisfaction","@type":["rdf:Property","owl:DatatypeProperty"],"rdfs:label":"review_of_customer_satisfaction","schema:rangeIncludes":{"@id":"xsd:boolean"},"schema:domainIncludes":{"@id":"sustainability:ManagementResponsibility"},"rdfs:comment":"Review of customer satisfaction"},{"@id":"sustainability:review_of_verification_report_of_the_fms","@type":["rdf:Property","owl:DatatypeProperty"],"rdfs:label":"review_of_verification_report_of_the_fms","schema:rangeIncludes":{"@id":"xsd:boolean"},"schema:domainIncludes":{"@id":"sustainability:ManagementResponsibility"},"rdfs:comment":"Review of verification report of the FMS"},{"@id":"sustainability:review_of_verification_report_of_the_haccp","@type":["rdf:Property","owl:DatatypeProperty"],"rdfs:label":"review_of_verification_report_of_the_haccp","schema:rangeIncludes":{"@id":"xsd:boolean"},"schema:domainIncludes":{"@id":"sustainability:ManagementResponsibility"},"rdfs:comment":"Review of verification report of the HACCP"},{"@id":"sustainability:review_of_supplier_evaluation","@type":["rdf:Property","owl:DatatypeProperty"],"rdfs:label":"review_of_supplier_evaluation","schema:rangeIncludes":{"@id":"xsd:boolean"},"schema:domainIncludes":{"@id":"sustainability:ManagementResponsibility"},"rdfs:comment":"Review of supplier evaluation"},{"@id":"sustainability:review_of_other_relevant_input_for_mr","@type":["rdf:Property","owl:DatatypeProperty"],"rdfs:label":"review_of_other_relevant_input_for_mr","schema:rangeIncludes":{"@id":"xsd:boolean"},"schema:domainIncludes":{"@id":"sustainability:ManagementResponsibility"},"rdfs:comment":"Review of other relevant input for MR"},{"@id":"sustainability:organize_and_implement_quality_feed_safety_into_the_organization","@type":["rdf:Property","owl:DatatypeProperty"],"rdfs:label":"organize_and_implement_quality_feed_safety_into_the_organization","schema:rangeIncludes":{"@id":"xsd:boolean"},"schema:domainIncludes":{"@id":"sustainability:ManagementResponsibility"},"rdfs:comment":"Organize and implement quality/feed safety into the organization"},{"@id":"sustainability:the_frequency_for_conducting_the_mr","@type":["rdf:Property","owl:DatatypeProperty"],"rdfs:label":"the_frequency_for_conducting_the_mr","schema:rangeIncludes":{"@id":"xsd:boolean"},"schema:domainIncludes":{"@id":"sustainability:ManagementResponsibility"},"rdfs:comment":"The frequency for conducting the MR"},{"@id":"sustainability:decision_of_about_effectiveness_of_the_fms","@type":["rdf:Property","owl:DatatypeProperty"],"rdfs:label":"decision_of_about_effectiveness_of_the_fms","schema:rangeIncludes":{"@id":"xsd:boolean"},"schema:domainIncludes":{"@id":"sustainability:ManagementResponsibility"},"rdfs:comment":"Decision of about effectiveness of the FMS"},{"@id":"sustainability:decision_of_about_improvements","@type":["rdf:Property","owl:DatatypeProperty"],"rdfs:label":"decision_of_about_improvements","schema:rangeIncludes":{"@id":"xsd:boolean"},"schema:domainIncludes":{"@id":"sustainability:ManagementResponsibility"},"rdfs:comment":"Decision of about improvements"},{"@id":"sustainability:review_of_objectives_as_defined_in_the_previous_period","@type":["rdf:Property","owl:DatatypeProperty"],"rdfs:label":"review_of_objectives_as_defined_in_the_previous_period","schema:rangeIncludes":{"@id":"xsd:boolean"},"schema:domainIncludes":{"@id":"sustainability:ManagementResponsibility"},"rdfs:comment":"Review of objectives as defined in the previous period"},{"@id":"sustainability:definition_of_smart_feed_safety_objectives","@type":["rdf:Property","owl:DatatypeProperty"],"rdfs:label":"definition_of_smart_feed_safety_objectives","schema:rangeIncludes":{"@id":"xsd:boolean"},"schema:domainIncludes":{"@id":"sustainability:ManagementResponsibility"},"rdfs:comment":"Definition of SMART feed safety objectives"},{"@id":"sustainability:provision_of_financial_resources_needed_for_improvements","@type":["rdf:Property","owl:DatatypeProperty"],"rdfs:label":"provision_of_financial_resources_needed_for_improvements","schema:rangeIncludes":{"@id":"xsd:boolean"},"schema:domainIncludes":{"@id":"sustainability:ManagementResponsibility"},"rdfs:comment":"Provision of financial resources needed for improvements"},{"@id":"sustainability:provision_of_resources_needed_for_improvements","@type":["rdf:Property","owl:DatatypeProperty"],"rdfs:label":"provision_of_resources_needed_for_improvements","schema:rangeIncludes":{"@id":"xsd:boolean"},"schema:domainIncludes":{"@id":"sustainability:ManagementResponsibility"},"rdfs:comment":"Provision of resources needed for improvements"},{"@id":"sustainability:assigning_a_responsible_person_to_execute_this","@type":["rdf:Property","owl:DatatypeProperty"],"rdfs:label":"assigning_a_responsible_person_to_execute_this","schema:rangeIncludes":{"@id":"xsd:boolean"},"schema:domainIncludes":{"@id":"sustainability:ManagementResponsibility"},"rdfs:comment":"Assigning a responsible person to execute this."},{"@id":"sustainability:definition_of_a_clear_feed_safety_and_quality_statement","@type":["rdf:Property","owl:DatatypeProperty"],"rdfs:label":"definition_of_a_clear_feed_safety_and_quality_statement","schema:rangeIncludes":{"@id":"xsd:boolean"},"schema:domainIncludes":{"@id":"sustainability:ManagementResponsibility"},"rdfs:comment":"Definition of a clear feed safety and quality statement"},{"@id":"sustainability:definition_of_a_policy_which_fits_to_the_size_and_role_of_the_organization","@type":["rdf:Property","owl:DatatypeProperty"],"rdfs:label":"definition_of_a_policy_which_fits_to_the_size_and_role_of_the_organization","schema:rangeIncludes":{"@id":"xsd:boolean"},"schema:domainIncludes":{"@id":"sustainability:ManagementResponsibility"},"rdfs:comment":"Definition of a policy which fits to the size and role of the organization."},{"@id":"sustainability:definition_of_a_policy_which_is_in_compliance_with_legal_market_and_customer_requirements","@type":["rdf:Property","owl:DatatypeProperty"],"rdfs:label":"definition_of_a_policy_which_is_in_compliance_with_legal_market_and_customer_requirements","schema:rangeIncludes":{"@id":"xsd:boolean"},"schema:domainIncludes":{"@id":"sustainability:ManagementResponsibility"},"rdfs:comment":"Definition of a policy which is in compliance with legal, market and customer requirements"},{"@id":"sustainability:definition_of_policy_which_includes_activities_needed_to_achieve_feed_safety_and_quality_regulatory_requirements","@type":["rdf:Property","owl:DatatypeProperty"],"rdfs:label":"definition_of_policy_which_includes_activities_needed_to_achieve_feed_safety_and_quality_regulatory_requirements","schema:rangeIncludes":{"@id":"xsd:boolean"},"schema:domainIncludes":{"@id":"sustainability:ManagementResponsibility"},"rdfs:comment":"Definition of policy which includes activities needed to achieve feed safety and quality regulatory requirements"},{"@id":"sustainability:definition_of_a_policy_which_includes_activities_needed_to_achieve_feed_safety_and_quality_requirements_of_the_market","@type":["rdf:Property","owl:DatatypeProperty"],"rdfs:label":"definition_of_a_policy_which_includes_activities_needed_to_achieve_feed_safety_and_quality_requirements_of_the_market","schema:rangeIncludes":{"@id":"xsd:boolean"},"schema:domainIncludes":{"@id":"sustainability:ManagementResponsibility"},"rdfs:comment":"Definition of a policy which includes activities needed to achieve feed safety and quality requirements of the market"},{"@id":"sustainability:a_procedure_for_managing_internal_complaints_effectively","@type":["rdf:Property","owl:DatatypeProperty"],"rdfs:label":"a_procedure_for_managing_internal_complaints_effectively","schema:rangeIncludes":{"@id":"xsd:boolean"},"schema:domainIncludes":{"@id":"sustainability:VerificationAndImprovement"},"rdfs:comment":"A procedure for managing internal complaints effectively"},{"@id":"sustainability:execution_of_the_internal_audit_at_least_every_year","@type":["rdf:Property","owl:DatatypeProperty"],"rdfs:label":"execution_of_the_internal_audit_at_least_every_year","schema:rangeIncludes":{"@id":"xsd:boolean"},"schema:domainIncludes":{"@id":"sustainability:VerificationAndImprovement"},"rdfs:comment":"Execution of the internal audit at least every year"},{"@id":"sustainability:analysis_of_results_of_all_verification_activities_including_the_results_of_monitoring_plan_complaints_and_internal_audits","@type":["rdf:Property","owl:DatatypeProperty"],"rdfs:label":"analysis_of_results_of_all_verification_activities_including_the_results_of_monitoring_plan_complaints_and_internal_audits","schema:rangeIncludes":{"@id":"xsd:boolean"},"schema:domainIncludes":{"@id":"sustainability:VerificationAndImprovement"},"rdfs:comment":"Analysis of results of all verification activities, including the results of monitoring plan, complaints, and (internal) audits"},{"@id":"sustainability:definition_of_updates_or_improvements_of_the_system","@type":["rdf:Property","owl:DatatypeProperty"],"rdfs:label":"definition_of_updates_or_improvements_of_the_system","schema:rangeIncludes":{"@id":"xsd:boolean"},"schema:domainIncludes":{"@id":"sustainability:VerificationAndImprovement"},"rdfs:comment":"Definition of updates or improvements of the system"},{"@id":"sustainability:communication_of_results_of_verification_activities","@type":["rdf:Property","owl:DatatypeProperty"],"rdfs:label":"communication_of_results_of_verification_activities","schema:rangeIncludes":{"@id":"xsd:boolean"},"schema:domainIncludes":{"@id":"sustainability:VerificationAndImprovement"},"rdfs:comment":"Communication of results of verification activities"},{"@id":"sustainability:assurance_of_possibilities_for_continually_improvement","@type":["rdf:Property","owl:DatatypeProperty"],"rdfs:label":"assurance_of_possibilities_for_continually_improvement","schema:rangeIncludes":{"@id":"xsd:boolean"},"schema:domainIncludes":{"@id":"sustainability:VerificationAndImprovement"},"rdfs:comment":"Assurance of possibilities for continually improvement"},{"@id":"sustainability:assurance_of_continuous_update_of_the_system","@type":["rdf:Property","owl:DatatypeProperty"],"rdfs:label":"assurance_of_continuous_update_of_the_system","schema:rangeIncludes":{"@id":"xsd:boolean"},"schema:domainIncludes":{"@id":"sustainability:VerificationAndImprovement"},"rdfs:comment":"Assurance of continuous update of the system"},{"@id":"sustainability:a_procedure_for_managing_external_complaints_effectively","@type":["rdf:Property","owl:DatatypeProperty"],"rdfs:label":"a_procedure_for_managing_external_complaints_effectively","schema:rangeIncludes":{"@id":"xsd:boolean"},"schema:domainIncludes":{"@id":"sustainability:VerificationAndImprovement"},"rdfs:comment":"A procedure for managing external complaints effectively"},{"@id":"sustainability:a_procedure_for_reviewing_complaints_to_establish_corrective_actions","@type":["rdf:Property","owl:DatatypeProperty"],"rdfs:label":"a_procedure_for_reviewing_complaints_to_establish_corrective_actions","schema:rangeIncludes":{"@id":"xsd:boolean"},"schema:domainIncludes":{"@id":"sustainability:VerificationAndImprovement"},"rdfs:comment":"A procedure for reviewing complaints to establish corrective actions"},{"@id":"sustainability:a_procedure_for_reviewing_complaints_to_establish_preventive_actions","@type":["rdf:Property","owl:DatatypeProperty"],"rdfs:label":"a_procedure_for_reviewing_complaints_to_establish_preventive_actions","schema:rangeIncludes":{"@id":"xsd:boolean"},"schema:domainIncludes":{"@id":"sustainability:VerificationAndImprovement"},"rdfs:comment":"A procedure for reviewing complaints to establish preventive actions"},{"@id":"sustainability:implementation_of_a_complete_internal_audit_programme","@type":["rdf:Property","owl:DatatypeProperty"],"rdfs:label":"implementation_of_a_complete_internal_audit_programme","schema:rangeIncludes":{"@id":"xsd:boolean"},"schema:domainIncludes":{"@id":"sustainability:VerificationAndImprovement"},"rdfs:comment":"Implementation of a complete internal audit programme"},{"@id":"sustainability:the_qualifications_for_internal_auditors","@type":["rdf:Property","owl:DatatypeProperty"],"rdfs:label":"the_qualifications_for_internal_auditors","schema:rangeIncludes":{"@id":"xsd:boolean"},"schema:domainIncludes":{"@id":"sustainability:VerificationAndImprovement"},"rdfs:comment":"The qualifications for internal auditors"},{"@id":"sustainability:assurance_of_independency_and_impartiality_of_auditors","@type":["rdf:Property","owl:DatatypeProperty"],"rdfs:label":"assurance_of_independency_and_impartiality_of_auditors","schema:rangeIncludes":{"@id":"xsd:boolean"},"schema:domainIncludes":{"@id":"sustainability:VerificationAndImprovement"},"rdfs:comment":"Assurance of independency and impartiality of auditors"},{"@id":"sustainability:planning_of_audits_which_cover_all_parts_of_the_system","@type":["rdf:Property","owl:DatatypeProperty"],"rdfs:label":"planning_of_audits_which_cover_all_parts_of_the_system","schema:rangeIncludes":{"@id":"xsd:boolean"},"schema:domainIncludes":{"@id":"sustainability:VerificationAndImprovement"},"rdfs:comment":"Planning of audits which cover all parts of the system"},{"@id":"sustainability:execution_of_the_internal_audit_with_a_risk_based_frequency","@type":["rdf:Property","owl:DatatypeProperty"],"rdfs:label":"execution_of_the_internal_audit_with_a_risk_based_frequency","schema:rangeIncludes":{"@id":"xsd:boolean"},"schema:domainIncludes":{"@id":"sustainability:VerificationAndImprovement"},"rdfs:comment":"Execution of the internal audit with a risk-based frequency"},{"@id":"sustainability:awareness_and_competence_about_feed_safety_assurance","@type":["rdf:Property","owl:DatatypeProperty"],"rdfs:label":"awareness_and_competence_about_feed_safety_assurance","schema:rangeIncludes":{"@id":"xsd:boolean"},"schema:domainIncludes":{"@id":"sustainability:PrerequisiteProgrammes"},"rdfs:comment":"Awareness and competence about feed safety assurance"},{"@id":"sustainability:implementation_of_protective_measures_against_sabotage_vandalism_or_terrorism","@type":["rdf:Property","owl:DatatypeProperty"],"rdfs:label":"implementation_of_protective_measures_against_sabotage_vandalism_or_terrorism","schema:rangeIncludes":{"@id":"xsd:boolean"},"schema:domainIncludes":{"@id":"sustainability:PrerequisiteProgrammes"},"rdfs:comment":"Implementation of protective measures against sabotage, vandalism or terrorism"},{"@id":"sustainability:design_construction_and_maintenance_which_is_fit_for_safe_feed_production_that_results_in_clean_well_facilitating_buildings_and_protect_against_cross_contamination_of_the_feed","@type":["rdf:Property","owl:DatatypeProperty"],"rdfs:label":"design_construction_and_maintenance_which_is_fit_for_safe_feed_production_that_results_in_clean_well_facilitating_buildings_and_protect_against_cross_contamination_of_the_feed","schema:rangeIncludes":{"@id":"xsd:boolean"},"schema:domainIncludes":{"@id":"sustainability:PrerequisiteProgrammes"},"rdfs:comment":"Design, construction and maintenance which is fit for safe feed production that results in clean, well-facilitating buildings and protect against (cross)contamination of the feed"},{"@id":"sustainability:clear_identification_of_buildings","@type":["rdf:Property","owl:DatatypeProperty"],"rdfs:label":"clear_identification_of_buildings","schema:rangeIncludes":{"@id":"xsd:boolean"},"schema:domainIncludes":{"@id":"sustainability:PrerequisiteProgrammes"},"rdfs:comment":"Clear identification of buildings"},{"@id":"sustainability:prevention_of_pests_and_other_animals_to_enter_the_buildings","@type":["rdf:Property","owl:DatatypeProperty"],"rdfs:label":"prevention_of_pests_and_other_animals_to_enter_the_buildings","schema:rangeIncludes":{"@id":"xsd:boolean"},"schema:domainIncludes":{"@id":"sustainability:PrerequisiteProgrammes"},"rdfs:comment":"Prevention of pests and other animals to enter the buildings"},{"@id":"sustainability:assuring_enough_daylight_or_artificial_light_to_guarantee_safe_production_of_feed","@type":["rdf:Property","owl:DatatypeProperty"],"rdfs:label":"assuring_enough_daylight_or_artificial_light_to_guarantee_safe_production_of_feed","schema:rangeIncludes":{"@id":"xsd:boolean"},"schema:domainIncludes":{"@id":"sustainability:PrerequisiteProgrammes"},"rdfs:comment":"Assuring enough daylight or artificial light to guarantee safe production of feed"},{"@id":"sustainability:design_construction_and_maintenance_which_is_fit_for_safe_feed_production_that_results_in_a_dry_clean_well_ventilated_area_protected_from_dust_condensation_or_other_sources_of_cross_contamination","@type":["rdf:Property","owl:DatatypeProperty"],"rdfs:label":"design_construction_and_maintenance_which_is_fit_for_safe_feed_production_that_results_in_a_dry_clean_well_ventilated_area_protected_from_dust_condensation_or_other_sources_of_cross_contamination","schema:rangeIncludes":{"@id":"xsd:boolean"},"schema:domainIncludes":{"@id":"sustainability:PrerequisiteProgrammes"},"rdfs:comment":"Design, construction and maintenance which is fit for safe feed production that results in a dry, clean, well-ventilated area protected from dust, condensation or other sources of (cross)contamination."},{"@id":"sustainability:addressing_possible_cross_contamination_in_the_risk_assessment_to_assure_that_it_is_controlled_and_does_not_exceed_established_limits","@type":["rdf:Property","owl:DatatypeProperty"],"rdfs:label":"addressing_possible_cross_contamination_in_the_risk_assessment_to_assure_that_it_is_controlled_and_does_not_exceed_established_limits","schema:rangeIncludes":{"@id":"xsd:boolean"},"schema:domainIncludes":{"@id":"sustainability:PrerequisiteProgrammes"},"rdfs:comment":"Addressing possible (cross)contamination in the risk assessment to assure that it is controlled and does not exceed established limits"},{"@id":"sustainability:clear_identification_of_the_areas","@type":["rdf:Property","owl:DatatypeProperty"],"rdfs:label":"clear_identification_of_the_areas","schema:rangeIncludes":{"@id":"xsd:boolean"},"schema:domainIncludes":{"@id":"sustainability:PrerequisiteProgrammes"},"rdfs:comment":"Clear identification of the areas"},{"@id":"sustainability:assurance_of_possibilities_to_carry_out_proper_cleaning_maintenance_and_pest_control_programme","@type":["rdf:Property","owl:DatatypeProperty"],"rdfs:label":"assurance_of_possibilities_to_carry_out_proper_cleaning_maintenance_and_pest_control_programme","schema:rangeIncludes":{"@id":"xsd:boolean"},"schema:domainIncludes":{"@id":"sustainability:PrerequisiteProgrammes"},"rdfs:comment":"Assurance of possibilities to carry out proper cleaning, maintenance and pest control programme."},{"@id":"sustainability:design_construction_and_maintenance_of_the_storage_areas_that_results_in_a_dry_clean_well_ventilated_area_protected_from_dust_condensation_or_other_sources_of_cross_contamination","@type":["rdf:Property","owl:DatatypeProperty"],"rdfs:label":"design_construction_and_maintenance_of_the_storage_areas_that_results_in_a_dry_clean_well_ventilated_area_protected_from_dust_condensation_or_other_sources_of_cross_contamination","schema:rangeIncludes":{"@id":"xsd:boolean"},"schema:domainIncludes":{"@id":"sustainability:PrerequisiteProgrammes"},"rdfs:comment":"Design, construction and maintenance of the storage areas that results in a dry, clean, well-ventilated area protected from dust, condensation or other sources of (cross)contamination."},{"@id":"sustainability:training_and_education_especially_about_haccp_and_feed_safety","@type":["rdf:Property","owl:DatatypeProperty"],"rdfs:label":"training_and_education_especially_about_haccp_and_feed_safety","schema:rangeIncludes":{"@id":"xsd:boolean"},"schema:domainIncludes":{"@id":"sustainability:PrerequisiteProgrammes"},"rdfs:comment":"Training and education, especially about HACCP and feed safety"},{"@id":"sustainability:design_construction_and_maintenance_of_the_internal_transport_equipment_that_results_in_clean_well_working_equipment_and_protect_against_cross_contamination_of_the_feed","@type":["rdf:Property","owl:DatatypeProperty"],"rdfs:label":"design_construction_and_maintenance_of_the_internal_transport_equipment_that_results_in_clean_well_working_equipment_and_protect_against_cross_contamination_of_the_feed","schema:rangeIncludes":{"@id":"xsd:boolean"},"schema:domainIncludes":{"@id":"sustainability:PrerequisiteProgrammes"},"rdfs:comment":"Design, construction and maintenance of the internal transport equipment that results in clean, well-working equipment and protect against (cross)contamination of the feed"},{"@id":"sustainability:ensure_clear_identification_of_the_storage_areas_and_the_internal_transport_equipment","@type":["rdf:Property","owl:DatatypeProperty"],"rdfs:label":"ensure_clear_identification_of_the_storage_areas_and_the_internal_transport_equipment","schema:rangeIncludes":{"@id":"xsd:boolean"},"schema:domainIncludes":{"@id":"sustainability:PrerequisiteProgrammes"},"rdfs:comment":"Ensure clear identification of the storage areas and the internal transport equipment."},{"@id":"sustainability:ensure_separation_or_zoning_of_facilities_so_that_safety_of_feeds_is_always_guaranteed","@type":["rdf:Property","owl:DatatypeProperty"],"rdfs:label":"ensure_separation_or_zoning_of_facilities_so_that_safety_of_feeds_is_always_guaranteed","schema:rangeIncludes":{"@id":"xsd:boolean"},"schema:domainIncludes":{"@id":"sustainability:PrerequisiteProgrammes"},"rdfs:comment":"Ensure separation or zoning of facilities so that safety of feeds is always guaranteed"},{"@id":"sustainability:storage_of_feed_medicines_including_storage_facilities_accessibility_and_handling_by_personnel","@type":["rdf:Property","owl:DatatypeProperty"],"rdfs:label":"storage_of_feed_medicines_including_storage_facilities_accessibility_and_handling_by_personnel","schema:rangeIncludes":{"@id":"xsd:boolean"},"schema:domainIncludes":{"@id":"sustainability:PrerequisiteProgrammes"},"rdfs:comment":"Storage of feed medicines including storage facilities, accessibility and handling by personnel"},{"@id":"sustainability:prevention_of_pests_and_other_animals_entering_the_storage_areas","@type":["rdf:Property","owl:DatatypeProperty"],"rdfs:label":"prevention_of_pests_and_other_animals_entering_the_storage_areas","schema:rangeIncludes":{"@id":"xsd:boolean"},"schema:domainIncludes":{"@id":"sustainability:PrerequisiteProgrammes"},"rdfs:comment":"Prevention of pests and other animals entering the storage areas"},{"@id":"sustainability:design_construction_and_maintenance_which_is_fit_for_safe_feed_production_that_results_in_clean_well_working_equipment_and_protect_against_cross_contamination_of_the_feed","@type":["rdf:Property","owl:DatatypeProperty"],"rdfs:label":"design_construction_and_maintenance_which_is_fit_for_safe_feed_production_that_results_in_clean_well_working_equipment_and_protect_against_cross_contamination_of_the_feed","schema:rangeIncludes":{"@id":"xsd:boolean"},"schema:domainIncludes":{"@id":"sustainability:PrerequisiteProgrammes"},"rdfs:comment":"Design, construction and maintenance which is fit for safe feed production that results in clean, well-working equipment and protect against (cross)contamination of the feed."},{"@id":"sustainability:avoidance_of_cross_contamination","@type":["rdf:Property","owl:DatatypeProperty"],"rdfs:label":"avoidance_of_cross_contamination","schema:rangeIncludes":{"@id":"xsd:boolean"},"schema:domainIncludes":{"@id":"sustainability:PrerequisiteProgrammes"},"rdfs:comment":"Avoidance of (cross)contamination"},{"@id":"sustainability:identification_of_any_potential_risk_for_cross_contamination","@type":["rdf:Property","owl:DatatypeProperty"],"rdfs:label":"identification_of_any_potential_risk_for_cross_contamination","schema:rangeIncludes":{"@id":"xsd:boolean"},"schema:domainIncludes":{"@id":"sustainability:PrerequisiteProgrammes"},"rdfs:comment":"Identification of any potential risk for (cross)contamination."},{"@id":"sustainability:facilities_for_personnel_hygiene","@type":["rdf:Property","owl:DatatypeProperty"],"rdfs:label":"facilities_for_personnel_hygiene","schema:rangeIncludes":{"@id":"xsd:boolean"},"schema:domainIncludes":{"@id":"sustainability:PrerequisiteProgrammes"},"rdfs:comment":"Facilities for personnel hygiene"},{"@id":"sustainability:implementation_of_measures_to_control_the_risks_for_cross_contamination","@type":["rdf:Property","owl:DatatypeProperty"],"rdfs:label":"implementation_of_measures_to_control_the_risks_for_cross_contamination","schema:rangeIncludes":{"@id":"xsd:boolean"},"schema:domainIncludes":{"@id":"sustainability:PrerequisiteProgrammes"},"rdfs:comment":"Implementation of measures to control the risks for (cross)contamination"},{"@id":"sustainability:assurance_that_water_and_steam_used_during_feed_production_does_not_cause_any_risk_to_the_safety_of_the_feed","@type":["rdf:Property","owl:DatatypeProperty"],"rdfs:label":"assurance_that_water_and_steam_used_during_feed_production_does_not_cause_any_risk_to_the_safety_of_the_feed","schema:rangeIncludes":{"@id":"xsd:boolean"},"schema:domainIncludes":{"@id":"sustainability:PrerequisiteProgrammes"},"rdfs:comment":"Assurance that water and steam used during feed production does not cause any risk to the safety of the feed"},{"@id":"sustainability:assurance_that_any_processing_aid_used_during_feed_production_does_not_cause_any_risk_to_the_safety_of_the_feed","@type":["rdf:Property","owl:DatatypeProperty"],"rdfs:label":"assurance_that_any_processing_aid_used_during_feed_production_does_not_cause_any_risk_to_the_safety_of_the_feed","schema:rangeIncludes":{"@id":"xsd:boolean"},"schema:domainIncludes":{"@id":"sustainability:PrerequisiteProgrammes"},"rdfs:comment":"Assurance that any processing aid used during feed production does not cause any risk to the safety of the feed"},{"@id":"sustainability:assurance_that_air_and_air_systems_do_not_affect_feed_safety","@type":["rdf:Property","owl:DatatypeProperty"],"rdfs:label":"assurance_that_air_and_air_systems_do_not_affect_feed_safety","schema:rangeIncludes":{"@id":"xsd:boolean"},"schema:domainIncludes":{"@id":"sustainability:PrerequisiteProgrammes"},"rdfs:comment":"Assurance that air and air systems do not affect feed safety."},{"@id":"sustainability:assurance_that_the_packaging_materials_used_do_not_cause_any_risk_to_the_safety_of_the_feed","@type":["rdf:Property","owl:DatatypeProperty"],"rdfs:label":"assurance_that_the_packaging_materials_used_do_not_cause_any_risk_to_the_safety_of_the_feed","schema:rangeIncludes":{"@id":"xsd:boolean"},"schema:domainIncludes":{"@id":"sustainability:PrerequisiteProgrammes"},"rdfs:comment":"Assurance that the packaging materials used do not cause any risk to the safety of the feed"},{"@id":"sustainability:definition_and_implementation_of_a_proper_and_complete_maintenance_programme","@type":["rdf:Property","owl:DatatypeProperty"],"rdfs:label":"definition_and_implementation_of_a_proper_and_complete_maintenance_programme","schema:rangeIncludes":{"@id":"xsd:boolean"},"schema:domainIncludes":{"@id":"sustainability:PrerequisiteProgrammes"},"rdfs:comment":"Definition and implementation of a proper and complete maintenance programme"},{"@id":"sustainability:maintenance_of_all_sites_buildings_areas_and_equipment","@type":["rdf:Property","owl:DatatypeProperty"],"rdfs:label":"maintenance_of_all_sites_buildings_areas_and_equipment","schema:rangeIncludes":{"@id":"xsd:boolean"},"schema:domainIncludes":{"@id":"sustainability:PrerequisiteProgrammes"},"rdfs:comment":"Maintenance of all sites, buildings, areas and equipment"},{"@id":"sustainability:definition_and_implementation_a_proper_and_complete_cleaning_programme","@type":["rdf:Property","owl:DatatypeProperty"],"rdfs:label":"definition_and_implementation_a_proper_and_complete_cleaning_programme","schema:rangeIncludes":{"@id":"xsd:boolean"},"schema:domainIncludes":{"@id":"sustainability:PrerequisiteProgrammes"},"rdfs:comment":"Definition and implementation a proper and complete cleaning programme."},{"@id":"sustainability:cleaning_of_all_sites_buildings_areas_and_equipment","@type":["rdf:Property","owl:DatatypeProperty"],"rdfs:label":"cleaning_of_all_sites_buildings_areas_and_equipment","schema:rangeIncludes":{"@id":"xsd:boolean"},"schema:domainIncludes":{"@id":"sustainability:PrerequisiteProgrammes"},"rdfs:comment":"Cleaning of all sites, buildings, areas and equipment"},{"@id":"sustainability:assurance_that_cleaning_and_sanitizing_agents_do_not_cause_any_risk_to_the_safety_of_the_feed","@type":["rdf:Property","owl:DatatypeProperty"],"rdfs:label":"assurance_that_cleaning_and_sanitizing_agents_do_not_cause_any_risk_to_the_safety_of_the_feed","schema:rangeIncludes":{"@id":"xsd:boolean"},"schema:domainIncludes":{"@id":"sustainability:PrerequisiteProgrammes"},"rdfs:comment":"Assurance that cleaning and sanitizing agents do not cause any risk to the safety of the feed."},{"@id":"sustainability:prohibition_to_eat_drink_and_smoke_in_production_storage_areas","@type":["rdf:Property","owl:DatatypeProperty"],"rdfs:label":"prohibition_to_eat_drink_and_smoke_in_production_storage_areas","schema:rangeIncludes":{"@id":"xsd:boolean"},"schema:domainIncludes":{"@id":"sustainability:PrerequisiteProgrammes"},"rdfs:comment":"Prohibition to eat, drink and smoke in production/storage areas"},{"@id":"sustainability:assurance_that_cleaning_and_sanitizing_agents_comply_with_legal_aspects","@type":["rdf:Property","owl:DatatypeProperty"],"rdfs:label":"assurance_that_cleaning_and_sanitizing_agents_comply_with_legal_aspects","schema:rangeIncludes":{"@id":"xsd:boolean"},"schema:domainIncludes":{"@id":"sustainability:PrerequisiteProgrammes"},"rdfs:comment":"Assurance that cleaning and sanitizing agents comply with legal aspects"},{"@id":"sustainability:water_for_cleaning_or_applications_where_there_is_a_risk_of_indirect_product_contact_to_meet_specified_animal_food_safety_requirements_relevant_to_the_application","@type":["rdf:Property","owl:DatatypeProperty"],"rdfs:label":"water_for_cleaning_or_applications_where_there_is_a_risk_of_indirect_product_contact_to_meet_specified_animal_food_safety_requirements_relevant_to_the_application","schema:rangeIncludes":{"@id":"xsd:boolean"},"schema:domainIncludes":{"@id":"sustainability:PrerequisiteProgrammes"},"rdfs:comment":"Water for cleaning or applications where there is a risk of indirect product contact to meet specified animal food safety requirements relevant to the application"},{"@id":"sustainability:definition_and_implementation_of_a_proper_and_pest_control_programme","@type":["rdf:Property","owl:DatatypeProperty"],"rdfs:label":"definition_and_implementation_of_a_proper_and_pest_control_programme","schema:rangeIncludes":{"@id":"xsd:boolean"},"schema:domainIncludes":{"@id":"sustainability:PrerequisiteProgrammes"},"rdfs:comment":"Definition and implementation of a proper and pest control programme."},{"@id":"sustainability:qualifications_for_personnel_involved_in_the_execution_of_the_pest_control_program","@type":["rdf:Property","owl:DatatypeProperty"],"rdfs:label":"qualifications_for_personnel_involved_in_the_execution_of_the_pest_control_program","schema:rangeIncludes":{"@id":"xsd:boolean"},"schema:domainIncludes":{"@id":"sustainability:PrerequisiteProgrammes"},"rdfs:comment":"Qualifications for personnel involved in the execution of the pest control program"},{"@id":"sustainability:training_of_own_personnel_involved_in_the_execution_of_the_pest_control_program","@type":["rdf:Property","owl:DatatypeProperty"],"rdfs:label":"training_of_own_personnel_involved_in_the_execution_of_the_pest_control_program","schema:rangeIncludes":{"@id":"xsd:boolean"},"schema:domainIncludes":{"@id":"sustainability:PrerequisiteProgrammes"},"rdfs:comment":"Training of own personnel involved in the execution of the pest control program"},{"@id":"sustainability:certification_of_external_people_involved_in_the_execution_of_the_pest_control_program","@type":["rdf:Property","owl:DatatypeProperty"],"rdfs:label":"certification_of_external_people_involved_in_the_execution_of_the_pest_control_program","schema:rangeIncludes":{"@id":"xsd:boolean"},"schema:domainIncludes":{"@id":"sustainability:PrerequisiteProgrammes"},"rdfs:comment":"Certification of external people involved in the execution of the pest control program"},{"@id":"sustainability:keeping_all_sites_buildings_areas_and_equipment_free_of_pests_and_other_animals","@type":["rdf:Property","owl:DatatypeProperty"],"rdfs:label":"keeping_all_sites_buildings_areas_and_equipment_free_of_pests_and_other_animals","schema:rangeIncludes":{"@id":"xsd:boolean"},"schema:domainIncludes":{"@id":"sustainability:PrerequisiteProgrammes"},"rdfs:comment":"Keeping all sites, buildings, areas and equipment free of pests and other animals"},{"@id":"sustainability:prevention_of_pest_and_other_animals_to_enter_buildings_and_areas","@type":["rdf:Property","owl:DatatypeProperty"],"rdfs:label":"prevention_of_pest_and_other_animals_to_enter_buildings_and_areas","schema:rangeIncludes":{"@id":"xsd:boolean"},"schema:domainIncludes":{"@id":"sustainability:PrerequisiteProgrammes"},"rdfs:comment":"Prevention of pest and other animals to enter buildings and areas"},{"@id":"sustainability:identification_collection_removal_and_disposal_of_waste_in_such_a_way_that_cross_contamination_is_prevented","@type":["rdf:Property","owl:DatatypeProperty"],"rdfs:label":"identification_collection_removal_and_disposal_of_waste_in_such_a_way_that_cross_contamination_is_prevented","schema:rangeIncludes":{"@id":"xsd:boolean"},"schema:domainIncludes":{"@id":"sustainability:PrerequisiteProgrammes"},"rdfs:comment":"Identification, collection, removal and disposal of waste in such a way that (cross)contamination is prevented"},{"@id":"sustainability:prevention_of_cross_contamination_with_validated_procedures","@type":["rdf:Property","owl:DatatypeProperty"],"rdfs:label":"prevention_of_cross_contamination_with_validated_procedures","schema:rangeIncludes":{"@id":"xsd:boolean"},"schema:domainIncludes":{"@id":"sustainability:PrerequisiteProgrammes"},"rdfs:comment":"Prevention of cross-contamination with validated procedures"},{"@id":"sustainability:provision_of_protective_clothing_equipment_if_there_is_potential_risk_for_cross_contamination","@type":["rdf:Property","owl:DatatypeProperty"],"rdfs:label":"provision_of_protective_clothing_equipment_if_there_is_potential_risk_for_cross_contamination","schema:rangeIncludes":{"@id":"xsd:boolean"},"schema:domainIncludes":{"@id":"sustainability:PrerequisiteProgrammes"},"rdfs:comment":"Provision of protective clothing/equipment if there is potential risk for (cross)contamination"},{"@id":"sustainability:prevention_of_cross_contamination_of_feed_medicines_with_validated_procedures","@type":["rdf:Property","owl:DatatypeProperty"],"rdfs:label":"prevention_of_cross_contamination_of_feed_medicines_with_validated_procedures","schema:rangeIncludes":{"@id":"xsd:boolean"},"schema:domainIncludes":{"@id":"sustainability:PrerequisiteProgrammes"},"rdfs:comment":"Prevention of cross-contamination of feed medicines with validated procedures"},{"@id":"sustainability:a_design_construction_and_maintenance_which_is_fit_for_safe_feed_production","@type":["rdf:Property","owl:DatatypeProperty"],"rdfs:label":"a_design_construction_and_maintenance_which_is_fit_for_safe_feed_production","schema:rangeIncludes":{"@id":"xsd:boolean"},"schema:domainIncludes":{"@id":"sustainability:PrerequisiteProgrammes"},"rdfs:comment":"A design, construction and maintenance which is fit for safe feed production"},{"@id":"sustainability:facilities_for_eating_and_drinking","@type":["rdf:Property","owl:DatatypeProperty"],"rdfs:label":"facilities_for_eating_and_drinking","schema:rangeIncludes":{"@id":"xsd:boolean"},"schema:domainIncludes":{"@id":"sustainability:PrerequisiteProgrammes"},"rdfs:comment":"Facilities for eating and drinking"},{"@id":"sustainability:controlled_access_to_the_site_including_visitors","@type":["rdf:Property","owl:DatatypeProperty"],"rdfs:label":"controlled_access_to_the_site_including_visitors","schema:rangeIncludes":{"@id":"xsd:boolean"},"schema:domainIncludes":{"@id":"sustainability:PrerequisiteProgrammes"},"rdfs:comment":"Controlled access to the site, including visitors."},{"@id":"sustainability:overview_of_all_suppliers_and_services","@type":["rdf:Property","owl:DatatypeProperty"],"rdfs:label":"overview_of_all_suppliers_and_services","schema:rangeIncludes":{"@id":"xsd:boolean"},"schema:domainIncludes":{"@id":"sustainability:Purchase"},"rdfs:comment":"Overview of all suppliers and services"},{"@id":"sustainability:specifications_of_raw_materials_and_services","@type":["rdf:Property","owl:DatatypeProperty"],"rdfs:label":"specifications_of_raw_materials_and_services","schema:rangeIncludes":{"@id":"xsd:boolean"},"schema:domainIncludes":{"@id":"sustainability:Purchase"},"rdfs:comment":"Specifications of raw materials and services"},{"@id":"sustainability:specifications_of_suppliers","@type":["rdf:Property","owl:DatatypeProperty"],"rdfs:label":"specifications_of_suppliers","schema:rangeIncludes":{"@id":"xsd:boolean"},"schema:domainIncludes":{"@id":"sustainability:Purchase"},"rdfs:comment":"Specifications of suppliers"},{"@id":"sustainability:assessment_of_potential_supplier","@type":["rdf:Property","owl:DatatypeProperty"],"rdfs:label":"assessment_of_potential_supplier","schema:rangeIncludes":{"@id":"xsd:boolean"},"schema:domainIncludes":{"@id":"sustainability:Purchase"},"rdfs:comment":"Assessment of (potential) supplier"},{"@id":"sustainability:assessment_of_liability_and_credibility_of_a_supplier","@type":["rdf:Property","owl:DatatypeProperty"],"rdfs:label":"assessment_of_liability_and_credibility_of_a_supplier","schema:rangeIncludes":{"@id":"xsd:boolean"},"schema:domainIncludes":{"@id":"sustainability:Purchase"},"rdfs:comment":"Assessment of liability and credibility of a supplier"},{"@id":"sustainability:a_system_to_approve_the_ingredient_supplier_combination","@type":["rdf:Property","owl:DatatypeProperty"],"rdfs:label":"a_system_to_approve_the_ingredient_supplier_combination","schema:rangeIncludes":{"@id":"xsd:boolean"},"schema:domainIncludes":{"@id":"sustainability:Purchase"},"rdfs:comment":"A system to approve the ingredient - supplier combination"},{"@id":"sustainability:lay_down_of_agreements_in_a_contract","@type":["rdf:Property","owl:DatatypeProperty"],"rdfs:label":"lay_down_of_agreements_in_a_contract","schema:rangeIncludes":{"@id":"xsd:boolean"},"schema:domainIncludes":[{"@id":"sustainability:Purchase"},{"@id":"sustainability:OutsourcedActivities"}],"rdfs:comment":"Lay down of agreements in a contract"},{"@id":"sustainability:re_assessment_of_suppliers_periodically_supplier_evaluation","@type":["rdf:Property","owl:DatatypeProperty"],"rdfs:label":"re_assessment_of_suppliers_periodically_supplier_evaluation","schema:rangeIncludes":{"@id":"xsd:boolean"},"schema:domainIncludes":{"@id":"sustainability:Purchase"},"rdfs:comment":"Re-assessment of suppliers periodically (supplier-evaluation)"},{"@id":"sustainability:recording_of_all_purchasing_activities","@type":["rdf:Property","owl:DatatypeProperty"],"rdfs:label":"recording_of_all_purchasing_activities","schema:rangeIncludes":{"@id":"xsd:boolean"},"schema:domainIncludes":{"@id":"sustainability:Purchase"},"rdfs:comment":"Recording of all purchasing activities"},{"@id":"sustainability:establishing_flowcharts_of_the_whole_production_including_reception_of_goods_production_packaging_storage_and_transport","@type":["rdf:Property","owl:DatatypeProperty"],"rdfs:label":"establishing_flowcharts_of_the_whole_production_including_reception_of_goods_production_packaging_storage_and_transport","schema:rangeIncludes":{"@id":"xsd:boolean"},"schema:domainIncludes":{"@id":"sustainability:Production"},"rdfs:comment":"Establishing flowcharts of the whole production including reception of goods, production, packaging, storage and transport."},{"@id":"sustainability:use_of_medicated_rework_only_in_feed_with_the_same_medication_and_in_compliance_with_legal_requirements","@type":["rdf:Property","owl:DatatypeProperty"],"rdfs:label":"use_of_medicated_rework_only_in_feed_with_the_same_medication_and_in_compliance_with_legal_requirements","schema:rangeIncludes":{"@id":"xsd:boolean"},"schema:domainIncludes":{"@id":"sustainability:Production"},"rdfs:comment":"Use of medicated rework only in feed with the same medication and in compliance with legal requirements"},{"@id":"sustainability:proper_identification_of_rework","@type":["rdf:Property","owl:DatatypeProperty"],"rdfs:label":"proper_identification_of_rework","schema:rangeIncludes":{"@id":"xsd:boolean"},"schema:domainIncludes":{"@id":"sustainability:Production"},"rdfs:comment":"Proper identification of rework"},{"@id":"sustainability:record_usage_of_rework_t_t","@type":["rdf:Property","owl:DatatypeProperty"],"rdfs:label":"record_usage_of_rework_t_t","schema:rangeIncludes":{"@id":"xsd:boolean"},"schema:domainIncludes":{"@id":"sustainability:Production"},"rdfs:comment":"Record usage of rework (T&T)"},{"@id":"sustainability:establishing_and_implementation_of_procedures_to_plan_and_control_production","@type":["rdf:Property","owl:DatatypeProperty"],"rdfs:label":"establishing_and_implementation_of_procedures_to_plan_and_control_production","schema:rangeIncludes":{"@id":"xsd:boolean"},"schema:domainIncludes":{"@id":"sustainability:Production"},"rdfs:comment":"Establishing and implementation of procedures to plan and control production"},{"@id":"sustainability:assurance_that_produced_products_meet_the_specified_criteria_including_the_feed_safety_standards","@type":["rdf:Property","owl:DatatypeProperty"],"rdfs:label":"assurance_that_produced_products_meet_the_specified_criteria_including_the_feed_safety_standards","schema:rangeIncludes":{"@id":"xsd:boolean"},"schema:domainIncludes":{"@id":"sustainability:Production"},"rdfs:comment":"Assurance that produced products meet the specified criteria including the feed safety standards"},{"@id":"sustainability:assurance_that_potential_risks_related_to_drying_especially_direct_drying_are_identified_and_controlled","@type":["rdf:Property","owl:DatatypeProperty"],"rdfs:label":"assurance_that_potential_risks_related_to_drying_especially_direct_drying_are_identified_and_controlled","schema:rangeIncludes":{"@id":"xsd:boolean"},"schema:domainIncludes":{"@id":"sustainability:Production"},"rdfs:comment":"Assurance that potential risks related to drying, especially direct drying, are identified and controlled:"},{"@id":"sustainability:assurance_that_defined_risks_related_to_dosing_weighing_mixing_pelleting_extruding_expanding_are_identified_and_controlled","@type":["rdf:Property","owl:DatatypeProperty"],"rdfs:label":"assurance_that_defined_risks_related_to_dosing_weighing_mixing_pelleting_extruding_expanding_are_identified_and_controlled","schema:rangeIncludes":{"@id":"xsd:boolean"},"schema:domainIncludes":{"@id":"sustainability:Production"},"rdfs:comment":"Assurance that defined risks related to dosing, weighing, mixing, pelleting, extruding, expanding are identified and controlled:"},{"@id":"sustainability:assurance_that_validated_procedures_including_measurements_are_in_place_to_control_unintended_cross_contamination_of_products_that_affect_the_safety_of_the_feed","@type":["rdf:Property","owl:DatatypeProperty"],"rdfs:label":"assurance_that_validated_procedures_including_measurements_are_in_place_to_control_unintended_cross_contamination_of_products_that_affect_the_safety_of_the_feed","schema:rangeIncludes":{"@id":"xsd:boolean"},"schema:domainIncludes":{"@id":"sustainability:Production"},"rdfs:comment":"Assurance that validated procedures including measurements are in place to control unintended (cross)contamination of products that affect the safety of the feed."},{"@id":"sustainability:establishing_a_procedure_and_implement_measurements_to_define_if_and_how_the_rework_shall_be_used_before_the_rework_is_entering_the_site","@type":["rdf:Property","owl:DatatypeProperty"],"rdfs:label":"establishing_a_procedure_and_implement_measurements_to_define_if_and_how_the_rework_shall_be_used_before_the_rework_is_entering_the_site","schema:rangeIncludes":{"@id":"xsd:boolean"},"schema:domainIncludes":{"@id":"sustainability:Production"},"rdfs:comment":"Establishing a procedure and implement measurements to define if and how the rework shall be used before the rework is entering the site"},{"@id":"sustainability:correct_handling_and_use_of_rework_related_to_safety_traceability_and_legal_requirements","@type":["rdf:Property","owl:DatatypeProperty"],"rdfs:label":"correct_handling_and_use_of_rework_related_to_safety_traceability_and_legal_requirements","schema:rangeIncludes":{"@id":"xsd:boolean"},"schema:domainIncludes":{"@id":"sustainability:Production"},"rdfs:comment":"Correct handling and use of rework related to safety, traceability and legal requirements"},{"@id":"sustainability:specification_of_the_outsourced_activity","@type":["rdf:Property","owl:DatatypeProperty"],"rdfs:label":"specification_of_the_outsourced_activity","schema:rangeIncludes":{"@id":"xsd:boolean"},"schema:domainIncludes":{"@id":"sustainability:OutsourcedActivities"},"rdfs:comment":"Specification of the outsourced activity"},{"@id":"sustainability:assessment_of_potential_contractor","@type":["rdf:Property","owl:DatatypeProperty"],"rdfs:label":"assessment_of_potential_contractor","schema:rangeIncludes":{"@id":"xsd:boolean"},"schema:domainIncludes":{"@id":"sustainability:OutsourcedActivities"},"rdfs:comment":"Assessment of (potential) contractor"},{"@id":"sustainability:assessment_of_liability_and_credibility_of_a_contractor","@type":["rdf:Property","owl:DatatypeProperty"],"rdfs:label":"assessment_of_liability_and_credibility_of_a_contractor","schema:rangeIncludes":{"@id":"xsd:boolean"},"schema:domainIncludes":{"@id":"sustainability:OutsourcedActivities"},"rdfs:comment":"Assessment of liability and credibility of a contractor"},{"@id":"sustainability:re_assessment_of_suppliers_periodically","@type":["rdf:Property","owl:DatatypeProperty"],"rdfs:label":"re_assessment_of_suppliers_periodically","schema:rangeIncludes":{"@id":"xsd:boolean"},"schema:domainIncludes":{"@id":"sustainability:OutsourcedActivities"},"rdfs:comment":"Re-assessment of suppliers periodically"},{"@id":"sustainability:monitoring_analysing_products_produced_by_services_provided_by_contractors_in_relation_to_agreed_specifications","@type":["rdf:Property","owl:DatatypeProperty"],"rdfs:label":"monitoring_analysing_products_produced_by_services_provided_by_contractors_in_relation_to_agreed_specifications","schema:rangeIncludes":{"@id":"xsd:boolean"},"schema:domainIncludes":{"@id":"sustainability:OutsourcedActivities"},"rdfs:comment":"Monitoring (analysing) products produced by /services provided by contractors in relation to agreed specifications"},{"@id":"sustainability:evaluation_of_contractors_and_their_services_related_to_defined_agreements","@type":["rdf:Property","owl:DatatypeProperty"],"rdfs:label":"evaluation_of_contractors_and_their_services_related_to_defined_agreements","schema:rangeIncludes":{"@id":"xsd:boolean"},"schema:domainIncludes":{"@id":"sustainability:OutsourcedActivities"},"rdfs:comment":"Evaluation of contractors and their services related to defined agreements"},{"@id":"sustainability:establish_procedures_to_ensure_that_formulation_of_diets_does_not_introduce_any_feed_safety_risks","@type":["rdf:Property","owl:DatatypeProperty"],"rdfs:label":"establish_procedures_to_ensure_that_formulation_of_diets_does_not_introduce_any_feed_safety_risks","schema:rangeIncludes":{"@id":"xsd:boolean"},"schema:domainIncludes":{"@id":"sustainability:Formulation"},"rdfs:comment":"Establish procedures to ensure that formulation of diets does not introduce any feed safety risks"},{"@id":"sustainability:establish_procedure_how_to_communicate_formula_s_to_the_production_area_in_such_a_way_that_there_is_no_feed_safety_risk_introduced","@type":["rdf:Property","owl:DatatypeProperty"],"rdfs:label":"establish_procedure_how_to_communicate_formula_s_to_the_production_area_in_such_a_way_that_there_is_no_feed_safety_risk_introduced","schema:rangeIncludes":{"@id":"xsd:boolean"},"schema:domainIncludes":{"@id":"sustainability:Formulation"},"rdfs:comment":"Establish procedure how to communicate formula's to the production-area in such a way that there is no feed safety risk introduced"},{"@id":"sustainability:labeling_of_products_in_compliance_with_applicable_legal_requirements","@type":["rdf:Property","owl:DatatypeProperty"],"rdfs:label":"labeling_of_products_in_compliance_with_applicable_legal_requirements","schema:rangeIncludes":{"@id":"xsd:boolean"},"schema:domainIncludes":{"@id":"sustainability:Labeling"},"rdfs:comment":"Labeling of products in compliance with applicable legal requirements"},{"@id":"sustainability:registration_and_managing_non_conformities","@type":["rdf:Property","owl:DatatypeProperty"],"rdfs:label":"registration_and_managing_non_conformities","schema:rangeIncludes":{"@id":"xsd:boolean"},"schema:domainIncludes":{"@id":"sustainability:ControlOfNonConformity"},"rdfs:comment":"Registration and managing non-conformities"},{"@id":"sustainability:assessment_of_non_conformities_to_define_if_they_need_follow_up","@type":["rdf:Property","owl:DatatypeProperty"],"rdfs:label":"assessment_of_non_conformities_to_define_if_they_need_follow_up","schema:rangeIncludes":{"@id":"xsd:boolean"},"schema:domainIncludes":{"@id":"sustainability:ControlOfNonConformity"},"rdfs:comment":"Assessment of non-conformities to define if they need follow up"},{"@id":"sustainability:immediate_prevention_of_the_production_and_delivery_of_a_product_when_critical_limits_are_exceeded","@type":["rdf:Property","owl:DatatypeProperty"],"rdfs:label":"immediate_prevention_of_the_production_and_delivery_of_a_product_when_critical_limits_are_exceeded","schema:rangeIncludes":{"@id":"xsd:boolean"},"schema:domainIncludes":{"@id":"sustainability:ControlOfNonConformity"},"rdfs:comment":"Immediate prevention of the production and delivery of a product when critical limits are exceeded"},{"@id":"sustainability:prevention_of_unintended_use_of_materials_that_do_not_comply_with_relevant_specifications","@type":["rdf:Property","owl:DatatypeProperty"],"rdfs:label":"prevention_of_unintended_use_of_materials_that_do_not_comply_with_relevant_specifications","schema:rangeIncludes":{"@id":"xsd:boolean"},"schema:domainIncludes":{"@id":"sustainability:ControlOfNonConformity"},"rdfs:comment":"Prevention of unintended use of materials that do not comply with relevant specifications"},{"@id":"sustainability:elimination_of_the_cause_of_the_non_conformity","@type":["rdf:Property","owl:DatatypeProperty"],"rdfs:label":"elimination_of_the_cause_of_the_non_conformity","schema:rangeIncludes":{"@id":"xsd:boolean"},"schema:domainIncludes":{"@id":"sustainability:ControlOfNonConformity"},"rdfs:comment":"Elimination of the cause of the non-conformity"},{"@id":"sustainability:periodically_evaluation_of_non_conformities_and_corrective_action_for_improvement_of_the_fms","@type":["rdf:Property","owl:DatatypeProperty"],"rdfs:label":"periodically_evaluation_of_non_conformities_and_corrective_action_for_improvement_of_the_fms","schema:rangeIncludes":{"@id":"xsd:boolean"},"schema:domainIncludes":{"@id":"sustainability:ControlOfNonConformity"},"rdfs:comment":"Periodically evaluation of non-conformities and corrective action for improvement of the FMS"},{"@id":"sustainability:prevention_non_conformities","@type":["rdf:Property","owl:DatatypeProperty"],"rdfs:label":"prevention_non_conformities","schema:rangeIncludes":{"@id":"xsd:boolean"},"schema:domainIncludes":{"@id":"sustainability:ControlOfNonConformity"},"rdfs:comment":"Prevention non-conformities"},{"@id":"sustainability:establish_management_commitment","@type":["rdf:Property","owl:DatatypeProperty"],"rdfs:label":"establish_management_commitment","schema:rangeIncludes":{"@id":"xsd:boolean"},"schema:domainIncludes":{"@id":"sustainability:Haccp"},"rdfs:comment":"Establish management commitment"},{"@id":"sustainability:identification_of_all_potential_hazards","@type":["rdf:Property","owl:DatatypeProperty"],"rdfs:label":"identification_of_all_potential_hazards","schema:rangeIncludes":{"@id":"xsd:boolean"},"schema:domainIncludes":{"@id":"sustainability:Haccp"},"rdfs:comment":"Identification of all potential hazards"},{"@id":"sustainability:definition_of_occurrence_and_severity_including_calculation_matrix","@type":["rdf:Property","owl:DatatypeProperty"],"rdfs:label":"definition_of_occurrence_and_severity_including_calculation_matrix","schema:rangeIncludes":{"@id":"xsd:boolean"},"schema:domainIncludes":{"@id":"sustainability:Haccp"},"rdfs:comment":"Definition of occurrence and severity including calculation-matrix"},{"@id":"sustainability:conducting_a_hazard_analysis","@type":["rdf:Property","owl:DatatypeProperty"],"rdfs:label":"conducting_a_hazard_analysis","schema:rangeIncludes":{"@id":"xsd:boolean"},"schema:domainIncludes":{"@id":"sustainability:Haccp"},"rdfs:comment":"Conducting a hazard analysis"},{"@id":"sustainability:likely_occurrence","@type":["rdf:Property","owl:DatatypeProperty"],"rdfs:label":"likely_occurrence","schema:rangeIncludes":{"@id":"xsd:boolean"},"schema:domainIncludes":{"@id":"sustainability:Haccp"},"rdfs:comment":"Likely occurrence"},{"@id":"sustainability:severity","@type":["rdf:Property","owl:DatatypeProperty"],"rdfs:label":"severity","schema:rangeIncludes":{"@id":"xsd:boolean"},"schema:domainIncludes":{"@id":"sustainability:Haccp"},"rdfs:comment":"Severity"},{"@id":"sustainability:definition_of_control_measures","@type":["rdf:Property","owl:DatatypeProperty"],"rdfs:label":"definition_of_control_measures","schema:rangeIncludes":{"@id":"xsd:boolean"},"schema:domainIncludes":{"@id":"sustainability:Haccp"},"rdfs:comment":"Definition of control measures"},{"@id":"sustainability:determination_of_ccp_s","@type":["rdf:Property","owl:DatatypeProperty"],"rdfs:label":"determination_of_ccp_s","schema:rangeIncludes":{"@id":"xsd:boolean"},"schema:domainIncludes":{"@id":"sustainability:Haccp"},"rdfs:comment":"Determination of CCP_x0019_ s"},{"@id":"sustainability:establishing_critical_limits","@type":["rdf:Property","owl:DatatypeProperty"],"rdfs:label":"establishing_critical_limits","schema:rangeIncludes":{"@id":"xsd:boolean"},"schema:domainIncludes":{"@id":"sustainability:Haccp"},"rdfs:comment":"Establishing critical limits"},{"@id":"sustainability:validation_of_the_haccp_by_independent_qualified_personal","@type":["rdf:Property","owl:DatatypeProperty"],"rdfs:label":"validation_of_the_haccp_by_independent_qualified_personal","schema:rangeIncludes":{"@id":"xsd:boolean"},"schema:domainIncludes":{"@id":"sustainability:Haccp"},"rdfs:comment":"Validation of the HACCP by independent, qualified personal"},{"@id":"sustainability:assurance_that_every_ccp_is_monitored_and_in_control","@type":["rdf:Property","owl:DatatypeProperty"],"rdfs:label":"assurance_that_every_ccp_is_monitored_and_in_control","schema:rangeIncludes":{"@id":"xsd:boolean"},"schema:domainIncludes":{"@id":"sustainability:Haccp"},"rdfs:comment":"Assurance that every CCP is monitored and in control"},{"@id":"sustainability:assembling_a_haccp_team","@type":["rdf:Property","owl:DatatypeProperty"],"rdfs:label":"assembling_a_haccp_team","schema:rangeIncludes":{"@id":"xsd:boolean"},"schema:domainIncludes":{"@id":"sustainability:Haccp"},"rdfs:comment":"Assembling a HACCP team"},{"@id":"sustainability:assurance_that_every_other_hazard_is_adequately_monitored","@type":["rdf:Property","owl:DatatypeProperty"],"rdfs:label":"assurance_that_every_other_hazard_is_adequately_monitored","schema:rangeIncludes":{"@id":"xsd:boolean"},"schema:domainIncludes":{"@id":"sustainability:Haccp"},"rdfs:comment":"Assurance that every other hazard is adequately monitored"},{"@id":"sustainability:responsibilities_methods_frequencies_evaluation_and_follow_up_of_results","@type":["rdf:Property","owl:DatatypeProperty"],"rdfs:label":"responsibilities_methods_frequencies_evaluation_and_follow_up_of_results","schema:rangeIncludes":{"@id":"xsd:boolean"},"schema:domainIncludes":{"@id":"sustainability:Haccp"},"rdfs:comment":"Responsibilities, methods, frequencies, evaluation and follow-up of results"},{"@id":"sustainability:establishing_corrective_actions","@type":["rdf:Property","owl:DatatypeProperty"],"rdfs:label":"establishing_corrective_actions","schema:rangeIncludes":{"@id":"xsd:boolean"},"schema:domainIncludes":{"@id":"sustainability:Haccp"},"rdfs:comment":"Establishing corrective actions"},{"@id":"sustainability:verification_of_the_haccp_plan_including_frequency","@type":["rdf:Property","owl:DatatypeProperty"],"rdfs:label":"verification_of_the_haccp_plan_including_frequency","schema:rangeIncludes":{"@id":"xsd:boolean"},"schema:domainIncludes":{"@id":"sustainability:Haccp"},"rdfs:comment":"Verification of the HACCP plan including frequency"},{"@id":"sustainability:records_of_data_to_demonstrate_effectiveness_in_controlling_the_hazards","@type":["rdf:Property","owl:DatatypeProperty"],"rdfs:label":"records_of_data_to_demonstrate_effectiveness_in_controlling_the_hazards","schema:rangeIncludes":{"@id":"xsd:boolean"},"schema:domainIncludes":{"@id":"sustainability:Haccp"},"rdfs:comment":"Records of data to demonstrate effectiveness in controlling the hazards"},{"@id":"sustainability:assessment_whether_and_how_the_haccp_plan_needs_update","@type":["rdf:Property","owl:DatatypeProperty"],"rdfs:label":"assessment_whether_and_how_the_haccp_plan_needs_update","schema:rangeIncludes":{"@id":"xsd:boolean"},"schema:domainIncludes":{"@id":"sustainability:Haccp"},"rdfs:comment":"Assessment whether and how the HACCP plan needs update"},{"@id":"sustainability:validation_of_the_haccp_plan_after_each_update","@type":["rdf:Property","owl:DatatypeProperty"],"rdfs:label":"validation_of_the_haccp_plan_after_each_update","schema:rangeIncludes":{"@id":"xsd:boolean"},"schema:domainIncludes":{"@id":"sustainability:Haccp"},"rdfs:comment":"Validation of the HACCP plan after each update"},{"@id":"sustainability:appoint_a_haccp_team_leader","@type":["rdf:Property","owl:DatatypeProperty"],"rdfs:label":"appoint_a_haccp_team_leader","schema:rangeIncludes":{"@id":"xsd:boolean"},"schema:domainIncludes":{"@id":"sustainability:Haccp"},"rdfs:comment":"Appoint a HACCP-team leader"},{"@id":"sustainability:define_roles_responsibilities_and_mandates","@type":["rdf:Property","owl:DatatypeProperty"],"rdfs:label":"define_roles_responsibilities_and_mandates","schema:rangeIncludes":{"@id":"xsd:boolean"},"schema:domainIncludes":{"@id":"sustainability:Haccp"},"rdfs:comment":"Define roles, responsibilities and mandates"},{"@id":"sustainability:scope_definition_and_description","@type":["rdf:Property","owl:DatatypeProperty"],"rdfs:label":"scope_definition_and_description","schema:rangeIncludes":{"@id":"xsd:boolean"},"schema:domainIncludes":{"@id":"sustainability:Haccp"},"rdfs:comment":"Scope definition and description"},{"@id":"sustainability:specification_of_feed","@type":["rdf:Property","owl:DatatypeProperty"],"rdfs:label":"specification_of_feed","schema:rangeIncludes":{"@id":"xsd:boolean"},"schema:domainIncludes":{"@id":"sustainability:Haccp"},"rdfs:comment":"Specification of feed"},{"@id":"sustainability:specification_of_intended_use","@type":["rdf:Property","owl:DatatypeProperty"],"rdfs:label":"specification_of_intended_use","schema:rangeIncludes":{"@id":"xsd:boolean"},"schema:domainIncludes":{"@id":"sustainability:Haccp"},"rdfs:comment":"Specification of intended use"},{"@id":"sustainability:specification_of_the_process_flow_diagram","@type":["rdf:Property","owl:DatatypeProperty"],"rdfs:label":"specification_of_the_process_flow_diagram","schema:rangeIncludes":{"@id":"xsd:boolean"},"schema:domainIncludes":{"@id":"sustainability:Haccp"},"rdfs:comment":"Specification of the process (flow diagram)"},{"@id":"sustainability:implementation_of_the_prerequisite_programmes","@type":["rdf:Property","owl:DatatypeProperty"],"rdfs:label":"implementation_of_the_prerequisite_programmes","schema:rangeIncludes":{"@id":"xsd:boolean"},"schema:domainIncludes":{"@id":"sustainability:Haccp"},"rdfs:comment":"Implementation of the prerequisite programmes"},{"@id":"sustainability:definition_of_all_monitoring_activities_to_demonstrate_control_the_ccp_s","@type":["rdf:Property","owl:DatatypeProperty"],"rdfs:label":"definition_of_all_monitoring_activities_to_demonstrate_control_the_ccp_s","schema:rangeIncludes":{"@id":"xsd:boolean"},"schema:domainIncludes":{"@id":"sustainability:MonitoringAndVerification"},"rdfs:comment":"Definition of all monitoring activities to demonstrate control the CCP's"},{"@id":"sustainability:establish_a_quarantine_procedure_based_on_risk_assessment","@type":["rdf:Property","owl:DatatypeProperty"],"rdfs:label":"establish_a_quarantine_procedure_based_on_risk_assessment","schema:rangeIncludes":{"@id":"xsd:boolean"},"schema:domainIncludes":{"@id":"sustainability:MonitoringAndVerification"},"rdfs:comment":"Establish a quarantine procedure based on risk assessment"},{"@id":"sustainability:implementation_of_a_release_procedure","@type":["rdf:Property","owl:DatatypeProperty"],"rdfs:label":"implementation_of_a_release_procedure","schema:rangeIncludes":{"@id":"xsd:boolean"},"schema:domainIncludes":{"@id":"sustainability:MonitoringAndVerification"},"rdfs:comment":"Implementation of a release procedure"},{"@id":"sustainability:sampling_procedures_for_incoming_goods_finished_products_and_products_during_production","@type":["rdf:Property","owl:DatatypeProperty"],"rdfs:label":"sampling_procedures_for_incoming_goods_finished_products_and_products_during_production","schema:rangeIncludes":{"@id":"xsd:boolean"},"schema:domainIncludes":{"@id":"sustainability:MonitoringAndVerification"},"rdfs:comment":"Sampling procedures for incoming goods, finished products and products during production"},{"@id":"sustainability:establish_sampling_frequency","@type":["rdf:Property","owl:DatatypeProperty"],"rdfs:label":"establish_sampling_frequency","schema:rangeIncludes":{"@id":"xsd:boolean"},"schema:domainIncludes":{"@id":"sustainability:MonitoringAndVerification"},"rdfs:comment":"Establish sampling frequency"},{"@id":"sustainability:qualifications_for_persons_involved_in_sampling","@type":["rdf:Property","owl:DatatypeProperty"],"rdfs:label":"qualifications_for_persons_involved_in_sampling","schema:rangeIncludes":{"@id":"xsd:boolean"},"schema:domainIncludes":{"@id":"sustainability:MonitoringAndVerification"},"rdfs:comment":"Qualifications for persons involved in sampling"},{"@id":"sustainability:training_of_personal","@type":["rdf:Property","owl:DatatypeProperty"],"rdfs:label":"training_of_personal","schema:rangeIncludes":{"@id":"xsd:boolean"},"schema:domainIncludes":{"@id":"sustainability:MonitoringAndVerification"},"rdfs:comment":"Training of personal"},{"@id":"sustainability:sampling_equipment","@type":["rdf:Property","owl:DatatypeProperty"],"rdfs:label":"sampling_equipment","schema:rangeIncludes":{"@id":"xsd:boolean"},"schema:domainIncludes":{"@id":"sustainability:MonitoringAndVerification"},"rdfs:comment":"Sampling equipment"},{"@id":"sustainability:sampling_methods","@type":["rdf:Property","owl:DatatypeProperty"],"rdfs:label":"sampling_methods","schema:rangeIncludes":{"@id":"xsd:boolean"},"schema:domainIncludes":{"@id":"sustainability:MonitoringAndVerification"},"rdfs:comment":"Sampling methods"},{"@id":"sustainability:storage_conditions_for_samples","@type":["rdf:Property","owl:DatatypeProperty"],"rdfs:label":"storage_conditions_for_samples","schema:rangeIncludes":{"@id":"xsd:boolean"},"schema:domainIncludes":{"@id":"sustainability:MonitoringAndVerification"},"rdfs:comment":"Storage conditions for samples"},{"@id":"sustainability:minimum_storage_period_for_samples","@type":["rdf:Property","owl:DatatypeProperty"],"rdfs:label":"minimum_storage_period_for_samples","schema:rangeIncludes":{"@id":"xsd:boolean"},"schema:domainIncludes":{"@id":"sustainability:MonitoringAndVerification"},"rdfs:comment":"Minimum storage period for samples"},{"@id":"sustainability:verification_of_the_effectiveness_of_the_prp_s","@type":["rdf:Property","owl:DatatypeProperty"],"rdfs:label":"verification_of_the_effectiveness_of_the_prp_s","schema:rangeIncludes":{"@id":"xsd:boolean"},"schema:domainIncludes":{"@id":"sustainability:MonitoringAndVerification"},"rdfs:comment":"Verification of the effectiveness of the PRP's"},{"@id":"sustainability:laboratory_general_qualifications","@type":["rdf:Property","owl:DatatypeProperty"],"rdfs:label":"laboratory_general_qualifications","schema:rangeIncludes":{"@id":"xsd:boolean"},"schema:domainIncludes":{"@id":"sustainability:MonitoringAndVerification"},"rdfs:comment":"Laboratory (general qualifications)"},{"@id":"sustainability:accreditation_of_laboratory","@type":["rdf:Property","owl:DatatypeProperty"],"rdfs:label":"accreditation_of_laboratory","schema:rangeIncludes":{"@id":"xsd:boolean"},"schema:domainIncludes":{"@id":"sustainability:MonitoringAndVerification"},"rdfs:comment":"Accreditation of laboratory"},{"@id":"sustainability:methods_of_analysis","@type":["rdf:Property","owl:DatatypeProperty"],"rdfs:label":"methods_of_analysis","schema:rangeIncludes":{"@id":"xsd:boolean"},"schema:domainIncludes":{"@id":"sustainability:MonitoringAndVerification"},"rdfs:comment":"Methods of analysis"},{"@id":"sustainability:accreditation_of_methods","@type":["rdf:Property","owl:DatatypeProperty"],"rdfs:label":"accreditation_of_methods","schema:rangeIncludes":{"@id":"xsd:boolean"},"schema:domainIncludes":{"@id":"sustainability:MonitoringAndVerification"},"rdfs:comment":"Accreditation of methods"},{"@id":"sustainability:contracts_to_lay_down_agreements","@type":["rdf:Property","owl:DatatypeProperty"],"rdfs:label":"contracts_to_lay_down_agreements","schema:rangeIncludes":{"@id":"xsd:boolean"},"schema:domainIncludes":{"@id":"sustainability:MonitoringAndVerification"},"rdfs:comment":"Contracts to lay down agreements"},{"@id":"sustainability:assessment_of_laboratory_and_contracts","@type":["rdf:Property","owl:DatatypeProperty"],"rdfs:label":"assessment_of_laboratory_and_contracts","schema:rangeIncludes":{"@id":"xsd:boolean"},"schema:domainIncludes":{"@id":"sustainability:MonitoringAndVerification"},"rdfs:comment":"Assessment of laboratory and contracts"},{"@id":"sustainability:evaluation_of_laboratories","@type":["rdf:Property","owl:DatatypeProperty"],"rdfs:label":"evaluation_of_laboratories","schema:rangeIncludes":{"@id":"xsd:boolean"},"schema:domainIncludes":{"@id":"sustainability:MonitoringAndVerification"},"rdfs:comment":"Evaluation of laboratories"},{"@id":"sustainability:proper_working_of_measuring_equipment","@type":["rdf:Property","owl:DatatypeProperty"],"rdfs:label":"proper_working_of_measuring_equipment","schema:rangeIncludes":{"@id":"xsd:boolean"},"schema:domainIncludes":{"@id":"sustainability:MonitoringAndVerification"},"rdfs:comment":"Proper working of measuring equipment"},{"@id":"sustainability:maintenance_of_measuring_equipment","@type":["rdf:Property","owl:DatatypeProperty"],"rdfs:label":"maintenance_of_measuring_equipment","schema:rangeIncludes":{"@id":"xsd:boolean"},"schema:domainIncludes":{"@id":"sustainability:MonitoringAndVerification"},"rdfs:comment":"Maintenance of measuring equipment"},{"@id":"sustainability:calibration_of_measuring_equipment","@type":["rdf:Property","owl:DatatypeProperty"],"rdfs:label":"calibration_of_measuring_equipment","schema:rangeIncludes":{"@id":"xsd:boolean"},"schema:domainIncludes":{"@id":"sustainability:MonitoringAndVerification"},"rdfs:comment":"Calibration of measuring equipment"},{"@id":"sustainability:verification_of_the_effectiveness_all_other_procedures","@type":["rdf:Property","owl:DatatypeProperty"],"rdfs:label":"verification_of_the_effectiveness_all_other_procedures","schema:rangeIncludes":{"@id":"xsd:boolean"},"schema:domainIncludes":{"@id":"sustainability:MonitoringAndVerification"},"rdfs:comment":"Verification of the effectiveness all other procedures"},{"@id":"sustainability:record_all_monitoring_results","@type":["rdf:Property","owl:DatatypeProperty"],"rdfs:label":"record_all_monitoring_results","schema:rangeIncludes":{"@id":"xsd:boolean"},"schema:domainIncludes":{"@id":"sustainability:MonitoringAndVerification"},"rdfs:comment":"Record all monitoring results"},{"@id":"sustainability:analysis_of_all_monitoring_results","@type":["rdf:Property","owl:DatatypeProperty"],"rdfs:label":"analysis_of_all_monitoring_results","schema:rangeIncludes":{"@id":"xsd:boolean"},"schema:domainIncludes":{"@id":"sustainability:MonitoringAndVerification"},"rdfs:comment":"Analysis of all monitoring results"},{"@id":"sustainability:review_of_the_monitoring_results","@type":["rdf:Property","owl:DatatypeProperty"],"rdfs:label":"review_of_the_monitoring_results","schema:rangeIncludes":{"@id":"xsd:boolean"},"schema:domainIncludes":{"@id":"sustainability:MonitoringAndVerification"},"rdfs:comment":"Review of the monitoring results"},{"@id":"sustainability:establish_monitoring_of_incoming_goods_including_frequency_and_analysis_based_on_risk_assessment","@type":["rdf:Property","owl:DatatypeProperty"],"rdfs:label":"establish_monitoring_of_incoming_goods_including_frequency_and_analysis_based_on_risk_assessment","schema:rangeIncludes":{"@id":"xsd:boolean"},"schema:domainIncludes":{"@id":"sustainability:MonitoringAndVerification"},"rdfs:comment":"Establish monitoring of incoming goods including frequency and analysis based on risk assessment"},{"@id":"sustainability:a_check_on_incoming_products_on_compliance_with_product_specification","@type":["rdf:Property","owl:DatatypeProperty"],"rdfs:label":"a_check_on_incoming_products_on_compliance_with_product_specification","schema:rangeIncludes":{"@id":"xsd:boolean"},"schema:domainIncludes":{"@id":"sustainability:MonitoringAndVerification"},"rdfs:comment":"A check on incoming products on compliance with product specification"},{"@id":"sustainability:verification_on_product_characteristics_by_means_of_analysis","@type":["rdf:Property","owl:DatatypeProperty"],"rdfs:label":"verification_on_product_characteristics_by_means_of_analysis","schema:rangeIncludes":{"@id":"xsd:boolean"},"schema:domainIncludes":{"@id":"sustainability:MonitoringAndVerification"},"rdfs:comment":"Verification on product characteristics by means of analysis"},{"@id":"sustainability:ethics_general_policy_or_set_of_principles","@type":["rdf:Property","owl:DatatypeProperty"],"rdfs:label":"ethics_general_policy_or_set_of_principles","schema:rangeIncludes":{"@id":"xsd:string"},"schema:domainIncludes":{"@id":"sustainability:AntiCorruption"},"rdfs:comment":"Does the standard include a general principle on ethical issues"},{"@id":"sustainability:anti_bribery_internal_controls_records_keeping_m_e","@type":["rdf:Property","owl:DatatypeProperty"],"rdfs:label":"anti_bribery_internal_controls_records_keeping_m_e","schema:rangeIncludes":{"@id":"xsd:boolean"},"schema:domainIncludes":{"@id":"sustainability:AntiCorruption"},"rdfs:comment":"Does the standard require internal controls, records keeping, M&E of anti-bribery policies?"},{"@id":"sustainability:anti_bribery_external_reporting_and_communication","@type":["rdf:Property","owl:DatatypeProperty"],"rdfs:label":"anti_bribery_external_reporting_and_communication","schema:rangeIncludes":{"@id":"xsd:boolean"},"schema:domainIncludes":{"@id":"sustainability:AntiCorruption"},"rdfs:comment":"Does the standard require external reporting and communication of anti-bribery policies?"},{"@id":"sustainability:anti_bribery_mitigation_and_corrective_actions","@type":["rdf:Property","owl:DatatypeProperty"],"rdfs:label":"anti_bribery_mitigation_and_corrective_actions","schema:rangeIncludes":{"@id":"xsd:boolean"},"schema:domainIncludes":{"@id":"sustainability:AntiCorruption"},"rdfs:comment":"Does the standard require policies on mitigative and corrective actions for anti-bribery"},{"@id":"sustainability:transparency_across_types_of_information_obtained_during_audit_discrepancies_between_the_interviews_and_types_of_records","@type":["rdf:Property","owl:DatatypeProperty"],"rdfs:label":"transparency_across_types_of_information_obtained_during_audit_discrepancies_between_the_interviews_and_types_of_records","schema:rangeIncludes":{"@id":"xsd:boolean"},"schema:domainIncludes":{"@id":"sustainability:AntiCorruption"},"rdfs:comment":"Does the standard system require transparent practices to help alleviate discrepencies in information obtained during audits (documentation and observed practices)"},{"@id":"sustainability:audit_access_general_policy_auditor_s_freedom_of_access_to_facility_grounds_workers_production_areas","@type":["rdf:Property","owl:DatatypeProperty"],"rdfs:label":"audit_access_general_policy_auditor_s_freedom_of_access_to_facility_grounds_workers_production_areas","schema:rangeIncludes":{"@id":"xsd:boolean"},"schema:domainIncludes":{"@id":"sustainability:AntiCorruption"},"rdfs:comment":"Does the standard system require that auditors have freedom of access to all on-site activities"},{"@id":"sustainability:denial_of_audit_access_auditor_prevented_from_fulfilling_full_scope_audit_requirements","@type":["rdf:Property","owl:DatatypeProperty"],"rdfs:label":"denial_of_audit_access_auditor_prevented_from_fulfilling_full_scope_audit_requirements","schema:rangeIncludes":{"@id":"xsd:boolean"},"schema:domainIncludes":{"@id":"sustainability:AntiCorruption"},"rdfs:comment":"Does the standard system require measures to be taken to ensure that auditors are not prevented from fulfilling the full scope of audit requirements"},{"@id":"sustainability:monitoring_following_up_on_bribery_corruption_allegations","@type":["rdf:Property","owl:DatatypeProperty"],"rdfs:label":"monitoring_following_up_on_bribery_corruption_allegations","schema:rangeIncludes":{"@id":"xsd:boolean"},"schema:domainIncludes":{"@id":"sustainability:AntiCorruption"},"rdfs:comment":"Does the standard include criteria related to monitoring and follow-up actions on allegations"},{"@id":"sustainability:records_keeping_practices_allegations_fraud_grievances_historical_fines","@type":["rdf:Property","owl:DatatypeProperty"],"rdfs:label":"records_keeping_practices_allegations_fraud_grievances_historical_fines","schema:rangeIncludes":{"@id":"xsd:boolean"},"schema:domainIncludes":{"@id":"sustainability:AntiCorruption"},"rdfs:comment":"Does the standard include criteria related to keeping records of historical fines, issues with business partners, accounting problems"},{"@id":"sustainability:verification_of_business_license_and_legality_of_activities_settlement","@type":["rdf:Property","owl:DatatypeProperty"],"rdfs:label":"verification_of_business_license_and_legality_of_activities_settlement","schema:rangeIncludes":{"@id":"xsd:boolean"},"schema:domainIncludes":{"@id":"sustainability:AntiCorruption"},"rdfs:comment":"Does the standard include criteria on business legality?"},{"@id":"sustainability:intellectual_property_or_customer_information_protection","@type":["rdf:Property","owl:DatatypeProperty"],"rdfs:label":"intellectual_property_or_customer_information_protection","schema:rangeIncludes":{"@id":"xsd:boolean"},"schema:domainIncludes":{"@id":"sustainability:AntiCorruption"},"rdfs:comment":"Does the standard system require intellectual property or customer information protection"},{"@id":"sustainability:corruption_bribery_prevention","@type":["rdf:Property","owl:DatatypeProperty"],"rdfs:label":"corruption_bribery_prevention","schema:rangeIncludes":{"@id":"xsd:boolean"},"schema:domainIncludes":{"@id":"sustainability:AntiCorruption"},"rdfs:comment":"Does the standard promote the prevention of bribery"},{"@id":"sustainability:anti_bribery_procedures_and_risk_assessment","@type":["rdf:Property","owl:DatatypeProperty"],"rdfs:label":"anti_bribery_procedures_and_risk_assessment","schema:rangeIncludes":{"@id":"xsd:boolean"},"schema:domainIncludes":{"@id":"sustainability:AntiCorruption"},"rdfs:comment":"Does the standard require the implementation of anti-bribery procedures and risk-assessment"},{"@id":"sustainability:anti_bribery_political_contributions","@type":["rdf:Property","owl:DatatypeProperty"],"rdfs:label":"anti_bribery_political_contributions","schema:rangeIncludes":{"@id":"xsd:boolean"},"schema:domainIncludes":{"@id":"sustainability:AntiCorruption"},"rdfs:comment":"Does the standard address issues related to bribery through political contributions"},{"@id":"sustainability:anti_bribery_charitable_contributions_and_sponsorships","@type":["rdf:Property","owl:DatatypeProperty"],"rdfs:label":"anti_bribery_charitable_contributions_and_sponsorships","schema:rangeIncludes":{"@id":"xsd:boolean"},"schema:domainIncludes":{"@id":"sustainability:AntiCorruption"},"rdfs:comment":"Does the standard address issues related to bribery in the acceptance of charitable contributions and sponsorships"},{"@id":"sustainability:anti_bribery_facilitation_payments","@type":["rdf:Property","owl:DatatypeProperty"],"rdfs:label":"anti_bribery_facilitation_payments","schema:rangeIncludes":{"@id":"xsd:boolean"},"schema:domainIncludes":{"@id":"sustainability:AntiCorruption"},"rdfs:comment":"Does the standard require the establishment of procedures to avoid making facilitation payments to third parties"},{"@id":"sustainability:anti_bribery_gifts_hospitality_and_expenses","@type":["rdf:Property","owl:DatatypeProperty"],"rdfs:label":"anti_bribery_gifts_hospitality_and_expenses","schema:rangeIncludes":{"@id":"xsd:boolean"},"schema:domainIncludes":{"@id":"sustainability:AntiCorruption"},"rdfs:comment":"Does the standard address issues related to bribery in the acceptance of gifts, hospitality and expenses paid"},{"@id":"sustainability:anti_bribery_due_diligence_assessment_of_business_partners_incl_subsidiaries_and_contractors","@type":["rdf:Property","owl:DatatypeProperty"],"rdfs:label":"anti_bribery_due_diligence_assessment_of_business_partners_incl_subsidiaries_and_contractors","schema:rangeIncludes":{"@id":"xsd:boolean"},"schema:domainIncludes":{"@id":"sustainability:AntiCorruption"},"rdfs:comment":"Does the standard require due diligence of business partners, including subsidiaries and contractors?"},{"@id":"sustainability:anti_bribery_staff_workers_awareness_training_and_support","@type":["rdf:Property","owl:DatatypeProperty"],"rdfs:label":"anti_bribery_staff_workers_awareness_training_and_support","schema:rangeIncludes":{"@id":"xsd:boolean"},"schema:domainIncludes":{"@id":"sustainability:AntiCorruption"},"rdfs:comment":"Does the standard include criteria on training workers on issues of corruption and bribery?"},{"@id":"sustainability:compliance_to_international_conventions_is_required_and_assessed_regardless_of_official_ratification_by_the_country_of_operations","@type":["rdf:Property","owl:DatatypeProperty"],"rdfs:label":"compliance_to_international_conventions_is_required_and_assessed_regardless_of_official_ratification_by_the_country_of_operations","schema:rangeIncludes":{"@id":"xsd:boolean"},"schema:domainIncludes":{"@id":"sustainability:ComplianceToLegislation"},"rdfs:comment":"Does the standard explicitly address issues of legal compliance at local, regional and national levels"},{"@id":"sustainability:compliance_to_national_and_regional_environmental_laws_and_regulations","@type":["rdf:Property","owl:DatatypeProperty"],"rdfs:label":"compliance_to_national_and_regional_environmental_laws_and_regulations","schema:rangeIncludes":{"@id":"sustainability:ComplianceToNationalAndRegionalEnvironmentalLawsAndRegulations"},"schema:domainIncludes":{"@id":"sustainability:ComplianceToLegislation"},"rdfs:comment":"Does the standard require compliance with all relevant local, regional and national environmental laws and regulations?"},{"@id":"sustainability:explicit_policy_or_set_of_criteria_addressing_cultural_and_religion_rights","@type":["rdf:Property","owl:DatatypeProperty"],"rdfs:label":"explicit_policy_or_set_of_criteria_addressing_cultural_and_religion_rights","schema:rangeIncludes":{"@id":"xsd:boolean"},"schema:domainIncludes":{"@id":"sustainability:ComplianceToLegislation"},"rdfs:comment":"Does the standard system require an explicit policy or set of criteria addressing cultural and religion rights"},{"@id":"sustainability:obligation_to_comply_with_relevant_local_regional_and_national_laws_and_regulations_including_legal_land_tenure_title_having_legal_rights_to_use_the_production_or_management_unit","@type":["rdf:Property","owl:DatatypeProperty"],"rdfs:label":"obligation_to_comply_with_relevant_local_regional_and_national_laws_and_regulations_including_legal_land_tenure_title_having_legal_rights_to_use_the_production_or_management_unit","schema:rangeIncludes":{"@id":"xsd:boolean"},"schema:domainIncludes":{"@id":"sustainability:ComplianceToLegislation"},"rdfs:comment":"Does the standard include a requirement for compliance with relevant local, regional and national laws and regulations pertaining to land and production entitlements?"},{"@id":"sustainability:compliance_with_local_zoning_and_protected_or_heritage_area_regulations_and_laws","@type":["rdf:Property","owl:DatatypeProperty"],"rdfs:label":"compliance_with_local_zoning_and_protected_or_heritage_area_regulations_and_laws","schema:rangeIncludes":{"@id":"xsd:boolean"},"schema:domainIncludes":{"@id":"sustainability:ComplianceToLegislation"},"rdfs:comment":"Does the standard include criteria related to local zoning and protected or heritage area requirements (e.g. tourism sector)"}]}