{"@context":{"rdf":"http://www.w3.org/1999/02/22-rdf-syntax-ns#","owl":"http://www.w3.org/2002/07/owl#","rdfs":"http://www.w3.org/2000/01/rdf-schema#","schema":"https://schema.org/","unece":"https://jargon.sh/user/unece/uncefact/v/0.0.2/artefacts/jsonld/render.jsonld#","traceabilityEvents":"https://jargon.sh/user/unece/traceabilityEvents/v/working/artefacts/jsonld/render.jsonld#"},"@graph":[{"rdfs:label":"ActionCode","@type":"rdfs:Class","@id":"traceabilityEvents:ActionCode","rdfs:comment":""},{"@id":"traceabilityEvents:ActionCode#observe","@type":"traceabilityEvents:ActionCode","traceabilityEvents:Name":"observe","rdfs:comment":"Theentityinquestionhasnotbeenchanged:ithasneitherbeencreated,addedto,destroyed,orremovedfrom."},{"@id":"traceabilityEvents:ActionCode#add","@type":"traceabilityEvents:ActionCode","traceabilityEvents:Name":"add","rdfs:comment":"The entity in question has been created or added to."},{"@id":"traceabilityEvents:ActionCode#delete","@type":"traceabilityEvents:ActionCode","traceabilityEvents:Name":"delete","rdfs:comment":"The entity in question has been removed from or destroyed altogether."},{"rdfs:label":"assessmentLevel","@type":"rdfs:Class","@id":"traceabilityEvents:assessmentLevel","rdfs:comment":""},{"@id":"traceabilityEvents:assessmentLevel#self-assessed","@type":"traceabilityEvents:assessmentLevel","rdf:value":"self-assessed"},{"@id":"traceabilityEvents:assessmentLevel#independent-certifier","@type":"traceabilityEvents:assessmentLevel","rdf:value":"independent-certifier"},{"rdfs:label":"BusinessStepCode","@type":"rdfs:Class","@id":"traceabilityEvents:BusinessStepCode","rdfs:comment":""},{"@id":"traceabilityEvents:BusinessStepCode#commissioning","@type":"traceabilityEvents:BusinessStepCode","traceabilityEvents:Name":"commissioning","rdfs:comment":"Process of associating an instance-level identifier (such as an EPC) with a specific object, or the process of associating a class-level identifier, not previously used, with one or more objects. A tag may have been encoded and applied in this step, or may have been previously encoded. commissioning is applied to this association of object and serialised identifier, regardless of industry/sector"},{"@id":"traceabilityEvents:BusinessStepCode#inspecting","@type":"traceabilityEvents:BusinessStepCode","traceabilityEvents:Name":"inspecting","rdfs:comment":"Process of reviewing objects to address potential physical or documentation defects. In contrast to sampled objects, inspected objects remain viable in the supply chain."},{"@id":"traceabilityEvents:BusinessStepCode#shipping","@type":"traceabilityEvents:BusinessStepCode","traceabilityEvents:Name":"shipping","rdfs:comment":"ndicates the overall process of staging_outbound, loading and departing. It may be used when more\ngranular process step information is unknown or inaccessible. It may indicate a final event from a shipping point."},{"@id":"traceabilityEvents:BusinessStepCode#packing","@type":"traceabilityEvents:BusinessStepCode","traceabilityEvents:Name":"packing","rdfs:comment":"Denotes a specific activity within a business process that includes putting objects into a larger container – usually for shipping. Aggregation of one unit to another typically occurs at this point."},{"@id":"traceabilityEvents:BusinessStepCode#unpacking","@type":"traceabilityEvents:BusinessStepCode","traceabilityEvents:Name":"unpacking","rdfs:comment":"Denotes a specific activity within a business process that includes removing products (individuals, inners, cases, pallets) from a larger container – usually after receiving or accepting. Disaggregation of one unit from another typically occurs at this point."},{"rdfs:label":"DispositionCode","@type":"rdfs:Class","@id":"traceabilityEvents:DispositionCode","rdfs:comment":""},{"@id":"traceabilityEvents:DispositionCode#active","@type":"traceabilityEvents:DispositionCode","traceabilityEvents:Name":"active","rdfs:comment":"A commissioned object has just been introduced into the supply chain."},{"@id":"traceabilityEvents:DispositionCode#expired","@type":"traceabilityEvents:DispositionCode","traceabilityEvents:Name":"expired","rdfs:comment":"Object's expiration date is in the past."},{"@id":"traceabilityEvents:DispositionCode#disposed","@type":"traceabilityEvents:DispositionCode","traceabilityEvents:Name":"disposed","rdfs:comment":"Object has been returned for disposal."},{"@id":"traceabilityEvents:DispositionCode#conformant","@type":"traceabilityEvents:DispositionCode","traceabilityEvents:Name":"conformant","rdfs:comment":"Outcome of a successful/passed inspection in an inspecting or repairing step."},{"@id":"traceabilityEvents:DispositionCode#non_conformant","@type":"traceabilityEvents:DispositionCode","traceabilityEvents:Name":"non_conformant","rdfs:comment":"Outcome of an unsuccessful/failed inspection in an inspecting or repairing step."},{"@id":"traceabilityEvents:DispositionCode#in-transit","@type":"traceabilityEvents:DispositionCode","traceabilityEvents:Name":"in-transit","rdfs:comment":"Object being shipped between two trading partners."},{"@id":"traceabilityEvents:DispositionCode#dispensed","@type":"traceabilityEvents:DispositionCode","traceabilityEvents:Name":"dispensed","rdfs:comment":"A full quantity of product is distributed to a final customer or consumed in a manufacturing process."},{"rdfs:label":"DocumentTypeCode","@type":"rdfs:Class","@id":"traceabilityEvents:DocumentTypeCode","rdfs:comment":""},{"@id":"traceabilityEvents:DocumentTypeCode#bol","@type":"traceabilityEvents:DocumentTypeCode","traceabilityEvents:Name":"bol","rdfs:comment":"Bill of Lading or airway bill. A document issued by a carrier to a shipper, listing and acknowledging receipt of goods for transport and specifying terms of\ndelivery."},{"@id":"traceabilityEvents:DocumentTypeCode#cert","@type":"traceabilityEvents:DocumentTypeCode","traceabilityEvents:Name":"cert","rdfs:comment":"Certificate. A document confirming certain characteristics of an object (e.g. product), person, or organisation, typically issued by a third party"},{"@id":"traceabilityEvents:DocumentTypeCode#desadv","@type":"traceabilityEvents:DocumentTypeCode","traceabilityEvents:Name":"desadv","rdfs:comment":"Despatch Advice. A document/message by means of which the seller or consignor informs the consignee about the despatch of goods. Also called\nan “Advanced Shipment Notice,” but the value desadv is always used regardless of local nomenclature."},{"@id":"traceabilityEvents:DocumentTypeCode#inv","@type":"traceabilityEvents:DocumentTypeCode","traceabilityEvents:Name":"inv","rdfs:comment":"Invoice. A document/message claiming payment for goods or services supplied under conditions agreed by the seller and buyer."},{"@id":"traceabilityEvents:DocumentTypeCode#po","@type":"traceabilityEvents:DocumentTypeCode","traceabilityEvents:Name":"po","rdfs:comment":"Purchase Order. A document/message that specifies details for goods and services ordered under conditions agreed by the seller and buyer."},{"rdfs:label":"EventType","@type":"rdfs:Class","@id":"traceabilityEvents:EventType","rdfs:comment":""},{"@id":"traceabilityEvents:EventType#object","@type":"traceabilityEvents:EventType","traceabilityEvents:Name":"object","rdf:value":"","rdfs:comment":""},{"@id":"traceabilityEvents:EventType#transaction","@type":"traceabilityEvents:EventType","traceabilityEvents:Name":"transaction","rdf:value":null,"rdfs:comment":null},{"@id":"traceabilityEvents:EventType#aggregation","@type":"traceabilityEvents:EventType","traceabilityEvents:Name":"aggregation","rdf:value":null,"rdfs:comment":null},{"@id":"traceabilityEvents:EventType#transformation","@type":"traceabilityEvents:EventType","traceabilityEvents:Name":"transformation","rdf:value":null,"rdfs:comment":null},{"rdfs:label":"itcPillar","@type":"rdfs:Class","@id":"traceabilityEvents:itcPillar","rdfs:comment":""},{"@id":"traceabilityEvents:itcPillar#environment","@type":"traceabilityEvents:itcPillar","rdf:value":"environment"},{"@id":"traceabilityEvents:itcPillar#social","@type":"traceabilityEvents:itcPillar","rdf:value":"social"},{"@id":"traceabilityEvents:itcPillar#ethics","@type":"traceabilityEvents:itcPillar","rdf:value":"ethics"},{"@id":"traceabilityEvents:itcPillar#quality","@type":"traceabilityEvents:itcPillar","rdf:value":"quality"},{"rdfs:label":"VerificationOutcome","@type":"rdfs:Class","@id":"traceabilityEvents:VerificationOutcome","rdfs:comment":""},{"@id":"traceabilityEvents:VerificationOutcome#Valid","@type":"traceabilityEvents:VerificationOutcome","traceabilityEvents:Code":"Valid","rdfs:comment":"Event data was verified by the counter party"},{"@id":"traceabilityEvents:VerificationOutcome#Partial","@type":"traceabilityEvents:VerificationOutcome","traceabilityEvents:Code":"Partial","rdfs:comment":"Event data was partially verified"},{"@id":"traceabilityEvents:VerificationOutcome#Invalid","@type":"traceabilityEvents:VerificationOutcome","traceabilityEvents:Code":"Invalid","rdfs:comment":"Event data was declared invalid by the counter party"},{"rdfs:label":"verificationRole","@type":"rdfs:Class","@id":"traceabilityEvents:verificationRole","rdfs:comment":""},{"@id":"traceabilityEvents:verificationRole#businessPartner","@type":"traceabilityEvents:verificationRole","traceabilityEvents:Name":"businessPartner","rdfs:comment":""},{"@id":"traceabilityEvents:verificationRole#certifier","@type":"traceabilityEvents:verificationRole","traceabilityEvents:Name":"certifier","rdfs:comment":null},{"@id":"traceabilityEvents:Event","@type":"rdfs:Class","rdfs:label":"Event","schema:source":{"@id":"Event"},"rdfs:comment":"This abstract event structure provides a common language to describe supply chain events such as shipments, inspections, manufacturing processes, etc. There are four types of EPCIS event but this is an abstract class represenitng all common properties of an EPCIS event.  "},{"@id":"traceabilityEvents:VerificationCallback","@type":"rdfs:Class","rdfs:label":"VerificationCallback","schema:source":{"@id":"VerificationCallback"},"rdfs:comment":"Data structure for a call-back verification service. consumer provides an event structre to be verified, service returns that structure for the same event as known to the verifier together with a uniqu verificationID, date time stamp, and outcome "},{"@id":"traceabilityEvents:Document","@type":"rdfs:Class","rdfs:label":"Document","schema:source":{"@id":"Document"},"rdfs:comment":"A Secure binary document store.  "},{"@id":"traceabilityEvents:ObjectEvent","@type":"rdfs:Class","rdfs:label":"ObjectEvent","schema:source":{"@id":"ObjectEvent"},"rdfs:subClassOf":"traceabilityEvents:Event","rdfs:comment":"Object represents an event that happened to one or more physical or digital objects - such as an inspection or certification of a product or shipment. The physucal objects may be identified either as specific items (eg a unique consignment number) or as a quantified amount of a product class (eg 100Kg of cotton yarn)"},{"@id":"traceabilityEvents:AggregationEvent","@type":"rdfs:Class","rdfs:label":"AggregationEvent","schema:source":{"@id":"AggregationEvent"},"rdfs:subClassOf":"traceabilityEvents:Event","rdfs:comment":"Aggregation represents an event that happened to one or more objects that are physically aggregated together (physically constrained to be in the same place at the same time, as when cases are aggregated to a pallet).  This event is also used to represent de-aggregation (eg unpacking) when businessStepCode is unpacking."},{"@id":"traceabilityEvents:TransactionEvent","@type":"rdfs:Class","rdfs:label":"TransactionEvent","schema:source":{"@id":"TransactionEvent"},"rdfs:subClassOf":"traceabilityEvents:Event","rdfs:comment":"Transaction represents an event in which one or more objects become associated or disassociated with one or more identified business transactions - such as the purchase / shipment of goods between buyer and seller."},{"@id":"traceabilityEvents:TransformationEvent","@type":"rdfs:Class","rdfs:label":"TransformationEvent","schema:source":{"@id":"TransformationEvent"},"rdfs:subClassOf":"traceabilityEvents:Event","rdfs:comment":"Transformation represents an event in which input objects are fully or partially consumed and output objects are produced, such that any of the input objects may have contributed to all of the output objects - for example consuming bales of cotton to produce yarn."},{"@id":"traceabilityEvents:QuantityElement","@type":"rdfs:Class","rdfs:label":"QuantityElement","schema:source":{"@id":"QuantityElement"},"rdfs:comment":"The quantity elment is used to define the quantities (eg 100), units of measure (eg Kg) and product class (eg GTIN or other class identifier) of products that are inputs or outputs or the subject of supply chain events.  "},{"@id":"traceabilityEvents:TradeTransaction","@type":"rdfs:Class","rdfs:label":"TradeTransaction","schema:source":{"@id":"TradeTransaction"},"rdfs:comment":"A trade transaction between two parties such as an invoice, purchase order, or shipping notificaiotn."},{"@id":"traceabilityEvents:CertificationInfo","@type":"rdfs:Class","rdfs:label":"CertificationInfo","schema:source":{"@id":"CertificationInfo"},"rdfs:comment":"Details of a self asssessed or independently verified set of sustainability claims about a product or an establishment."},{"@id":"traceabilityEvents:Item","@type":"rdfs:Class","rdfs:label":"Item","schema:source":{"@id":"Item"},"rdfs:comment":"A specific trade item /product code which could be either a product serial number or a consignment identifier "},{"@id":"traceabilityEvents:Party","@type":"rdfs:Class","rdfs:label":"Party","schema:source":{"@id":"Party"},"rdfs:comment":"A trade party "},{"@id":"traceabilityEvents:BusinessPartner","@type":"rdfs:Class","rdfs:label":"BusinessPartner","schema:source":{"@id":"BusinessPartner"},"rdfs:subClassOf":"traceabilityEvents:Party","rdfs:comment":"The contant details of the party - used for counter party verification callbacks."},{"@id":"traceabilityEvents:eventID","@type":["rdf:Property","owl:DatatypeProperty"],"rdfs:label":"eventID","schema:rangeIncludes":{"@id":"xsd:string"},"schema:domainIncludes":{"@id":"traceabilityEvents:Event"},"rdfs:comment":"The unique identifier of this event - SHOULD be a UUID"},{"@id":"traceabilityEvents:eventType","@type":["rdf:Property","owl:ObjectProperty"],"rdfs:label":"eventType","schema:rangeIncludes":{"@id":"traceabilityEvents:EventType"},"schema:domainIncludes":{"@id":"traceabilityEvents:Event"},"rdfs:comment":"The event type - object, aggregation, transformation, transaction."},{"@id":"traceabilityEvents:eventTime","@type":["rdf:Property","owl:DatatypeProperty"],"rdfs:label":"eventTime","schema:rangeIncludes":{"@id":"xsd:string"},"schema:domainIncludes":{"@id":"traceabilityEvents:Event"},"owl:equivalentProperty":{"@id":"unece:eventTime"},"rdfs:comment":"The ISO-8601 date time when the event occured."},{"@id":"traceabilityEvents:actionCode","@type":["rdf:Property","owl:ObjectProperty"],"rdfs:label":"actionCode","schema:rangeIncludes":{"@id":"traceabilityEvents:ActionCode"},"schema:domainIncludes":{"@id":"traceabilityEvents:Event"},"rdfs:comment":"The Action type says how an event relates to the lifecycle of the entity being described. For example, AggregationEvent is used to capture events related to aggregations of objects, such as cases aggregated to a pallet. Throughout its life, the pallet load participates in many business process steps, each of which may generate an EPCIS event. The action field of each event says how the aggregation itself has changed during the event: have objects been added to the aggregation, have objects been removed from the aggregation, or has the aggregation simply been observed without change to its membership? The action is independent of the bizStep (of type BusinessStepID) which identifies the specific business process step in which the action took place.  allowed values are: - ADD (The entity in question has been created or added to.) - OBSERVE (Theentityinquestionhasnotbeenchanged:ithasneitherbeencreated,addedto,destroyed,orremovedfrom.) - DELETE (The entity in question has been removed from or destroyed altogether.)"},{"@id":"traceabilityEvents:dispositionCode","@type":["rdf:Property","owl:ObjectProperty"],"rdfs:label":"dispositionCode","schema:rangeIncludes":{"@id":"traceabilityEvents:DispositionCode"},"schema:domainIncludes":{"@id":"traceabilityEvents:Event"},"rdfs:comment":"Disposition code is a vocabulary whose elements denote a business state of an object. An example is a code that denotes “recalled\". The disposition field of an event specifies the business condition of the event’s objects, subsequent to the event. The disposition is assumed to hold true until another event indicates a change of disposition. Intervening events that do not specify a disposition field have no effect on the presumed disposition of the object.  The GS1 vocabulary (CBV v2.0) defines 33 possible disposition codes but this specification restricts the options to the minimum set of values that are relevant for supply chain traceability.  "},{"@id":"traceabilityEvents:businessStepCode","@type":["rdf:Property","owl:ObjectProperty"],"rdfs:label":"businessStepCode","schema:rangeIncludes":{"@id":"traceabilityEvents:BusinessStepCode"},"schema:domainIncludes":{"@id":"traceabilityEvents:Event"},"rdfs:comment":"BusinessStepID is a vocabulary whose elements denote steps in business processes. An example is an identifier that denotes “shipping.” The business step field of an event specifies the business context of an event: what business process step was taking place that caused the event to be captured? This specification has chosena 5 of the 41 possible bizstep values defined by GS1 that are appropriate for the sustainbility use case."},{"@id":"traceabilityEvents:readPointId","@type":["rdf:Property","owl:DatatypeProperty"],"rdfs:label":"readPointId","schema:rangeIncludes":{"@id":"xsd:string"},"schema:domainIncludes":{"@id":"traceabilityEvents:Event"},"rdfs:comment":"A Read Point is a discretely recorded location that is meant to identify the most specific place at which an EPCIS event took place. Read Points are determined by the EPCIS Capturing Application, perhaps inferred as a function of logical reader if stationary readers are used, perhaps determined overtly by reading a location tag if the reader is mobile, or in general determined by any other means the EPCIS Capturing Application chooses to use. Conceptually, the Read Point is designed to identify “where objects were at the time of the EPCIS event.”"},{"@id":"traceabilityEvents:locationId","@type":["rdf:Property","owl:DatatypeProperty"],"rdfs:label":"locationId","schema:rangeIncludes":{"@id":"xsd:string"},"schema:domainIncludes":{"@id":"traceabilityEvents:Event"},"rdfs:comment":"A Business Location is a uniquely identified and discretely recorded geospatial location that is meant to designate the specific place where an object is assumed to be following an EPCIS event until it is reported to be at a different Business Location by a subsequent EPCIS event. This specification requires the use of https://maps.google.com/pluscodes/ as geospatial identifiers rather than identifier schemes that cannot be reolved to a geogrpahic point or area."},{"@id":"traceabilityEvents:certification","@type":["rdf:Property","owl:ObjectProperty"],"rdfs:label":"certification","schema:rangeIncludes":{"@id":"traceabilityEvents:CertificationInfo"},"schema:domainIncludes":{"@id":"traceabilityEvents:Event"},"rdfs:comment":"Any test result or certification related to this EPCIS event.Could be self-assessed or independent and has asssociated sustainabiloity claims from the ITC vocabulary."},{"@id":"traceabilityEvents:verficationID","@type":["rdf:Property","owl:DatatypeProperty"],"rdfs:label":"verficationID","schema:rangeIncludes":{"@id":"xsd:string"},"schema:domainIncludes":{"@id":"traceabilityEvents:VerificationCallback"},"rdfs:comment":"The unique ID of of the verification created by the counter party."},{"@id":"traceabilityEvents:verificationDateTime","@type":["rdf:Property","owl:DatatypeProperty"],"rdfs:label":"verificationDateTime","schema:rangeIncludes":{"@id":"xsd:string"},"schema:domainIncludes":{"@id":"traceabilityEvents:VerificationCallback"},"rdfs:comment":"The dateTime stamp of the verification "},{"@id":"traceabilityEvents:verificationOutcome","@type":["rdf:Property","owl:ObjectProperty"],"rdfs:label":"verificationOutcome","schema:rangeIncludes":{"@id":"traceabilityEvents:VerificationOutcome"},"schema:domainIncludes":{"@id":"traceabilityEvents:VerificationCallback"},"rdfs:comment":"The outcome of the counter party verification - returned by the verification callback end point."},{"@id":"traceabilityEvents:verificationData","@type":["rdf:Property","owl:ObjectProperty"],"rdfs:label":"verificationData","schema:rangeIncludes":{"@id":"traceabilityEvents:Event"},"schema:domainIncludes":{"@id":"traceabilityEvents:VerificationCallback"},"rdfs:comment":"The event data that is to be verified by the counter party"},{"@id":"traceabilityEvents:hash","@type":["rdf:Property","owl:DatatypeProperty"],"rdfs:label":"hash","schema:rangeIncludes":{"@id":"xsd:string"},"schema:domainIncludes":{"@id":"traceabilityEvents:Document"},"rdfs:comment":"Multi-hash of the stored document object which is also used as the ID of the document.  "},{"@id":"traceabilityEvents:url","@type":["rdf:Property","owl:DatatypeProperty"],"rdfs:label":"url","schema:rangeIncludes":{"@id":"xsd:string"},"schema:domainIncludes":{"@id":"traceabilityEvents:Document"},"rdfs:comment":"The storage URL of the document which is of the form {path}/{hash}#{key}"},{"@id":"traceabilityEvents:file","@type":["rdf:Property","owl:DatatypeProperty"],"rdfs:label":"file","schema:rangeIncludes":{"@id":"xsd:string"},"schema:domainIncludes":{"@id":"traceabilityEvents:Document"},"rdfs:comment":"Base64 eoncided blob that is the document to be stored."},{"@id":"traceabilityEvents:fileType","@type":["rdf:Property","owl:ObjectProperty"],"rdfs:label":"fileType","schema:rangeIncludes":{"@id":"traceabilityEvents:MIMEType"},"schema:domainIncludes":{"@id":"traceabilityEvents:Document"},"rdfs:comment":"MIME type of stored document"},{"@id":"traceabilityEvents:key","@type":["rdf:Property","owl:DatatypeProperty"],"rdfs:label":"key","schema:rangeIncludes":{"@id":"xsd:string"},"schema:domainIncludes":{"@id":"traceabilityEvents:Document"},"rdfs:comment":"symmetric encryption key used to encrypt the stored document."},{"@id":"traceabilityEvents:itemList","@type":["rdf:Property","owl:ObjectProperty"],"rdfs:label":"itemList","schema:rangeIncludes":{"@id":"traceabilityEvents:Item"},"schema:domainIncludes":[{"@id":"traceabilityEvents:ObjectEvent"},{"@id":"traceabilityEvents:TransactionEvent"}],"rdfs:comment":"A list of uniquely identified items (eg specific items serial numbers or tagged shipments / packages) that are the focus of this object event.  "},{"@id":"traceabilityEvents:quantityList","@type":["rdf:Property","owl:ObjectProperty"],"rdfs:label":"quantityList","schema:rangeIncludes":{"@id":"traceabilityEvents:QuantityElement"},"schema:domainIncludes":[{"@id":"traceabilityEvents:ObjectEvent"},{"@id":"traceabilityEvents:TransactionEvent"}],"rdfs:comment":"A quantified list of product classes (eg GS1 GTINs) that are the focus of this object event"},{"@id":"traceabilityEvents:parentItem","@type":["rdf:Property","owl:ObjectProperty"],"rdfs:label":"parentItem","schema:rangeIncludes":{"@id":"traceabilityEvents:Item"},"schema:domainIncludes":{"@id":"traceabilityEvents:AggregationEvent"},"rdfs:comment":"The unique item identifier that is the result of this aggreation. Typcially a packaging ID used in shipments that represents a box/ pallet / container of contained items."},{"@id":"traceabilityEvents:childItems","@type":["rdf:Property","owl:ObjectProperty"],"rdfs:label":"childItems","schema:rangeIncludes":{"@id":"traceabilityEvents:Item"},"schema:domainIncludes":{"@id":"traceabilityEvents:AggregationEvent"},"rdfs:comment":"The list of child items that have been aggreated into the parent (or disaggregated from the parent). Maybe a list of pckage referneces (eg boxes on a pallet) or may be individual items (eg products in a box)."},{"@id":"traceabilityEvents:childQuantityList","@type":["rdf:Property","owl:ObjectProperty"],"rdfs:label":"childQuantityList","schema:rangeIncludes":{"@id":"traceabilityEvents:QuantityElement"},"schema:domainIncludes":{"@id":"traceabilityEvents:AggregationEvent"},"rdfs:comment":"List of quantified product classes that have been aggregated into the parent.  Used whwn the child items do not have unique identifiers (eg 100 Kg of cotton bales)"},{"@id":"traceabilityEvents:sourceParty","@type":["rdf:Property","owl:ObjectProperty"],"rdfs:label":"sourceParty","schema:rangeIncludes":{"@id":"traceabilityEvents:Party"},"schema:domainIncludes":{"@id":"traceabilityEvents:TransactionEvent"},"rdfs:comment":"The source party for this supply chain transaction - typcially the seller party"},{"@id":"traceabilityEvents:destinationParty","@type":["rdf:Property","owl:ObjectProperty"],"rdfs:label":"destinationParty","schema:rangeIncludes":{"@id":"traceabilityEvents:Party"},"schema:domainIncludes":{"@id":"traceabilityEvents:TransactionEvent"},"rdfs:comment":"The destination party for this supply chain transaction - typcially the buyer party."},{"@id":"traceabilityEvents:transaction","@type":["rdf:Property","owl:ObjectProperty"],"rdfs:label":"transaction","schema:rangeIncludes":{"@id":"traceabilityEvents:TradeTransaction"},"schema:domainIncludes":{"@id":"traceabilityEvents:TransactionEvent"},"rdfs:comment":"The supply chain transaction reference for this transaction event - eg the invoice, order, or despatch advice"},{"@id":"traceabilityEvents:outputItemList","@type":["rdf:Property","owl:ObjectProperty"],"rdfs:label":"outputItemList","schema:rangeIncludes":{"@id":"traceabilityEvents:Item"},"schema:domainIncludes":{"@id":"traceabilityEvents:TransformationEvent"},"rdfs:comment":"The list of uniquely identified items that are the output of this transformation event - for example a list of individually identified bolts of cloth that are the output of a weaving process."},{"@id":"traceabilityEvents:inputItemList","@type":["rdf:Property","owl:ObjectProperty"],"rdfs:label":"inputItemList","schema:rangeIncludes":{"@id":"traceabilityEvents:Item"},"schema:domainIncludes":{"@id":"traceabilityEvents:TransformationEvent"},"rdfs:comment":"The list of uniquely identified items that are the intput of this transformation event - for example a list of individually identified bobbins of yarn that are the input of a weaving process."},{"@id":"traceabilityEvents:inputQuantityList","@type":["rdf:Property","owl:ObjectProperty"],"rdfs:label":"inputQuantityList","schema:rangeIncludes":{"@id":"traceabilityEvents:QuantityElement"},"schema:domainIncludes":{"@id":"traceabilityEvents:TransformationEvent"},"rdfs:comment":"The quantified list of product classes that are the input of this transformation event - usend when each item does not have a unique identity.  for example the weight of raw cotton that is the input to a ginning process."},{"@id":"traceabilityEvents:outputQuantityList","@type":["rdf:Property","owl:ObjectProperty"],"rdfs:label":"outputQuantityList","schema:rangeIncludes":{"@id":"traceabilityEvents:QuantityElement"},"schema:domainIncludes":{"@id":"traceabilityEvents:TransformationEvent"},"rdfs:comment":"The quantified list of product classes that are the output of this transformation event - usend when each item does not have a unique identity.  for example a count of the bales of cleaned cotton that are the output of a ginning process."},{"@id":"traceabilityEvents:processType","@type":["rdf:Property","owl:ObjectProperty"],"rdfs:label":"processType","schema:rangeIncludes":{"@id":"traceabilityEvents:ProcessType"},"schema:domainIncludes":{"@id":"traceabilityEvents:TransformationEvent"},"rdfs:comment":"An industry specific process type code.  "},{"@id":"traceabilityEvents:productClass","@type":["rdf:Property","owl:DatatypeProperty"],"rdfs:label":"productClass","schema:rangeIncludes":{"@id":"xsd:string"},"schema:domainIncludes":{"@id":"traceabilityEvents:QuantityElement"},"owl:equivalentProperty":{"@id":"unece:productClass"},"rdfs:comment":"THe identifier of a product class (as opposed to a product instance) such as a GTIN code for a manufactured product."},{"@id":"traceabilityEvents:quantity","@type":["rdf:Property","owl:DatatypeProperty"],"rdfs:label":"quantity","schema:rangeIncludes":{"@id":"xsd:string"},"schema:domainIncludes":{"@id":"traceabilityEvents:QuantityElement"},"owl:equivalentProperty":{"@id":"unece:quantity"},"rdfs:comment":"The numeric quantity of the product class (eg 100 kg of cotton)"},{"@id":"traceabilityEvents:uom","@type":["rdf:Property","owl:ObjectProperty"],"rdfs:label":"uom","schema:rangeIncludes":{"@id":"traceabilityEvents:UOM"},"schema:domainIncludes":{"@id":"traceabilityEvents:QuantityElement"},"rdfs:comment":"The unit of measure for the quantity value (eg Kg or meters etc) using the UNECE Rec 20 unit of measure codelist."},{"@id":"traceabilityEvents:type","@type":["rdf:Property","owl:ObjectProperty"],"rdfs:label":"type","schema:rangeIncludes":{"@id":"traceabilityEvents:DocumentTypeCode"},"schema:domainIncludes":{"@id":"traceabilityEvents:TradeTransaction"},"rdfs:comment":"The document type representing the trade transaciton. This profile for supply chain traceability defines a simple subset of 5 document types that may be referenced by a transaction event."},{"@id":"traceabilityEvents:identifier","@type":["rdf:Property","owl:DatatypeProperty"],"rdfs:label":"identifier","schema:rangeIncludes":{"@id":"xsd:string"},"schema:domainIncludes":{"@id":"traceabilityEvents:TradeTransaction"},"rdfs:comment":"The identifier of the trade transaction document - eg an invoice number or bill of lading number.  Must be unique for a given source party"},{"@id":"traceabilityEvents:documentURL","@type":["rdf:Property","owl:DatatypeProperty"],"rdfs:label":"documentURL","schema:rangeIncludes":{"@id":"xsd:string"},"schema:domainIncludes":{"@id":"traceabilityEvents:TradeTransaction"},"rdfs:comment":"The URL of the referenced trade document. For privacy and integrity reasons, it is recommended (but not required) that * the documentURL is a hashlink (https://w3c-ccg.github.io/hashlink/) so that if the document the URL is changed then the hash verification will fail.* the document is encrypted for privacy reasons and that the hex encoded symmetric key for decruption is provided as a URL parameter.* the document filename is a GUID so that there is no leakage of possibly identifying information in the URL.https://domain/GUID?h1={document_hash}&key={decryption_key}For examplehttps://docstore.com/ef1e69fbbeaf47b4af97e29c69dc09cf.pdf?h1=zQmWvQxTqbG2Z9HPJgG57jjwR154cKhbtJenbyYTWkjgF3e&key=462D4A614E645267556B587032733576"},{"@id":"traceabilityEvents:certificateID","@type":["rdf:Property","owl:DatatypeProperty"],"rdfs:label":"certificateID","schema:rangeIncludes":{"@id":"xsd:string"},"schema:domainIncludes":{"@id":"traceabilityEvents:CertificationInfo"},"rdfs:comment":"The ID of the certificate document"},{"@id":"traceabilityEvents:referenceStandard","@type":["rdf:Property","owl:DatatypeProperty"],"rdfs:label":"referenceStandard","schema:rangeIncludes":{"@id":"xsd:string"},"schema:domainIncludes":{"@id":"traceabilityEvents:CertificationInfo"},"rdfs:comment":"The identifier (as a URI) of the sustainability standard against whichthe certificate is issued.  For example abvtex.org.br/v4.0"},{"@id":"traceabilityEvents:evidenceURL","@type":["rdf:Property","owl:DatatypeProperty"],"rdfs:label":"evidenceURL","schema:rangeIncludes":{"@id":"xsd:string"},"schema:domainIncludes":{"@id":"traceabilityEvents:CertificationInfo"},"rdfs:comment":"The URL of the certificate document. For privacy and integrity reasons, it is recommended (but not required) that * the documentURL is a hashlink (https://w3c-ccg.github.io/hashlink/) so that if the document the URL is changed then the hash verification will fail.* the document is encrypted for privacy reasons and that the symmetric key for decruption is provided as a URL parameter.* the document filename is a GUID so that there is no leakage of possibly identifying information in the URL.https://domain/GUID?h1={document_hash}&key={decryption_key}For examplehttps://docstore.com/ef1e69fbbeaf47b4af97e29c69dc09cf.pdf?h1=zQmWvQxTqbG2Z9HPJgG57jjwR154cKhbtJenbyYTWkjgF3e&key=462D4A614E645267556B587032733576"},{"@id":"traceabilityEvents:criteriaList","@type":["rdf:Property","owl:DatatypeProperty"],"rdfs:label":"criteriaList","schema:rangeIncludes":{"@id":"xsd:string"},"schema:domainIncludes":{"@id":"traceabilityEvents:CertificationInfo"},"rdfs:comment":"Optional list of specific sustainability criteria that the certificate claims are met."},{"@id":"traceabilityEvents:assessmentLevel","@type":["rdf:Property","owl:ObjectProperty"],"rdfs:label":"assessmentLevel","schema:rangeIncludes":{"@id":"traceabilityEvents:assessmentLevel"},"schema:domainIncludes":{"@id":"traceabilityEvents:CertificationInfo"},"rdfs:comment":"The integrity level of the sustainability claims. Self asssed or independently certified.  "},{"@id":"traceabilityEvents:responsibleAgency","@type":["rdf:Property","owl:ObjectProperty"],"rdfs:label":"responsibleAgency","schema:rangeIncludes":{"@id":"traceabilityEvents:Party"},"schema:domainIncludes":{"@id":"traceabilityEvents:CertificationInfo"},"rdfs:comment":"The issuing authority of the certificate."},{"@id":"traceabilityEvents:itemID","@type":["rdf:Property","owl:DatatypeProperty"],"rdfs:label":"itemID","schema:rangeIncludes":{"@id":"xsd:string"},"schema:domainIncludes":{"@id":"traceabilityEvents:Item"},"rdfs:comment":"The globally unique identifier (eg GS1 GTIN or digital link) of the product item.  "},{"@id":"traceabilityEvents:name","@type":["rdf:Property","owl:DatatypeProperty"],"rdfs:label":"name","schema:rangeIncludes":{"@id":"xsd:string"},"schema:domainIncludes":[{"@id":"traceabilityEvents:Item"},{"@id":"traceabilityEvents:Party"}],"owl:equivalentProperty":{"@id":"unece:name"},"rdfs:comment":"The entity name of the identified party - usually the business anme from the corresponding natinal registery -eg ACME LTD"},{"@id":"traceabilityEvents:partyID","@type":["rdf:Property","owl:DatatypeProperty"],"rdfs:label":"partyID","schema:rangeIncludes":{"@id":"xsd:string"},"schema:domainIncludes":{"@id":"traceabilityEvents:Party"},"rdfs:comment":"The globally unique identifier of the party. This must be expressed as a URI that is (preferably) resolvable to an entity register such as a national business register - eg https://abr.business.gov.au/ABN/View?abn=41161080146 "},{"@id":"traceabilityEvents:email","@type":["rdf:Property","owl:DatatypeProperty"],"rdfs:label":"email","schema:rangeIncludes":{"@id":"xsd:string"},"schema:domainIncludes":{"@id":"traceabilityEvents:BusinessPartner"},"rdfs:comment":"email address of the verifier person for manual verifications."},{"@id":"traceabilityEvents:domain","@type":["rdf:Property","owl:DatatypeProperty"],"rdfs:label":"domain","schema:rangeIncludes":{"@id":"xsd:string"},"schema:domainIncludes":{"@id":"traceabilityEvents:BusinessPartner"},"rdfs:comment":"DNS domain of the counter party"},{"@id":"traceabilityEvents:role","@type":["rdf:Property","owl:ObjectProperty"],"rdfs:label":"role","schema:rangeIncludes":{"@id":"traceabilityEvents:verificationRole"},"schema:domainIncludes":{"@id":"traceabilityEvents:BusinessPartner"},"rdfs:comment":"Role of the coutner party (business partner or certifier)"}]}