{
  "@context": {
    "rdf": "http://www.w3.org/1999/02/22-rdf-syntax-ns#",
    "rdfs": "http://www.w3.org/2000/01/rdf-schema#",
    "schema": "http://schema.org/",
    "unlcdv": "https://vocabulary.uncefact.org/unlocode-vocab/",
    "xsd": "http://www.w3.org/2001/XMLSchema#"
  },
  "@graph": [
    {
      "@id": "unlcdv:Country",
      "@type": "rdfs:Class",
      "rdfs:comment": "The two-letter alphabetic country codes, adopted in International Standard ISO 3166-1."
    },
    {
      "@id": "unlcdv:Function",
      "@type": "rdfs:Class",
      "rdfs:comment": "1-character function classifier code which identifies the existence of either a facility providing a connection with a specific mode of transport 1 or some other significant function not directly related to any mode of transport at this location"
    },
    {
      "@id": "unlcdv:Subdivision",
      "@type": "rdfs:Class",
      "rdfs:comment": "Code for the administrative division of the country concerned (state, province, department, etc.)."
    },
    {
      "@id": "unlcdv:UNLOCODE",
      "@type": "rdfs:Class",
      "rdfs:comment": "Identifies an administrative or economic area, relevant to international trade and transport, as defined by the competent national authority in each country."
    },
    {
      "@id": "unlcdv:countryCode",
      "@type": "rdf:Property",
      "rdfs:comment": "Related ISO 3166-1 country code.",
      "schema:domainIncludes": [
        {
          "@id": "unlcdv:UNLOCODE"
        },
        {
          "@id": "unlcdv:Subdivision"
        }
      ],
      "schema:rangeIncludes": {
        "@id": "unlcdv:Country"
      }
    },
    {
      "@id": "unlcdv:countrySubdivision",
      "@type": "rdf:Property",
      "rdfs:comment": "Related ISO 3166-2 country subdivision code.",
      "schema:domainIncludes": {
        "@id": "unlcdv:UNLOCODE"
      },
      "schema:rangeIncludes": {
        "@id": "unlcdv:Subdivision"
      }
    },
    {
      "@id": "unlcdv:functions",
      "@type": "rdf:Property",
      "rdfs:comment": "Related function codes.",
      "schema:domainIncludes": {
        "@id": "unlcdv:UNLOCODE"
      },
      "schema:rangeIncludes": {
        "@id": "unlcdv:Function"
      }
    },
    {
      "@id": "unlcdv:subdivisionType",
      "@type": "rdf:Property",
      "rdfs:comment": "The administrative division (state,province, department, etc.).",
      "schema:domainIncludes": {
        "@id": "unlcdv:Subdivision"
      },
      "schema:rangeIncludes": {
        "@id": "xsd:string"
      }
    }
  ]
}
