
{
    "@context": {
        "rdfs": "http://www.w3.org/2000/01/rdf-schema#",
        "unlcdv": "https://vocabulary.uncefact.org/unlocode-vocab/",
        "rdf": "http://www.w3.org/1999/02/22-rdf-syntax-ns#",
        "schema": "http://schema.org/"
    },
    "@graph": [
        {
            "@type": "rdfs:Class",
            "rdfs:comment": "The two-letter alphabetic country codes, adopted in International Standard ISO 3166-1.",
            "@id": "unlcdv:Country"
        },
        {
            "@type": "rdfs:Class",
            "rdfs:comment": "1-character function classifier code which identifies the existence of either a facility providing a connection with a specific mode of transport 1 or some other significant function not directly related to any mode of transport at this location",
            "@id": "unlcdv:Function"
        },
        {
            "@type": "rdfs:Class",
            "rdfs:comment": "Code for the administrative division of the country concerned (state, province, department, etc.).",
            "@id": "unlcdv:Subdivision"
        },
        {
            "@type": "rdfs:Class",
            "rdfs:comment": "Identifies an administrative or economic area, relevant to international trade and transport, as defined by the competent national authority in each country.",
            "@id": "unlcdv:UNLOCODE"
        },
        {
            "@type": "rdf:Property",
            "rdfs:comment": "Related ISO 3166-1 country code.",
            "@id": "unlcdv:countryCode",
            "schema:rangeIncludes": {
                "@id": "unlcdv:Country"
            },
            "schema:domainIncludes": [
                {
                    "@id": "unlcdv:UNLOCODE"
                },
                {
                    "@id": "unlcdv:Subdivision"
                }
            ]
        },
        {
            "@type": "rdf:Property",
            "rdfs:comment": "Related ISO 3166-2 country subdivision code.",
            "@id": "unlcdv:countrySubdivision",
            "schema:rangeIncludes": {
                "@id": "unlcdv:Subdivision"
            },
            "schema:domainIncludes": {
                "@id": "unlcdv:UNLOCODE"
            }
        },
        {
            "@type": "rdf:Property",
            "rdfs:comment": "Related function codes.",
            "@id": "unlcdv:functions",
            "schema:rangeIncludes": {
                "@id": "unlcdv:Function"
            },
            "schema:domainIncludes": {
                "@id": "unlcdv:UNLOCODE"
            }
        },
        {
            "@type": "rdf:Property",
            "schema:rangeIncludes": "xsd:string",
            "rdfs:comment": "The administrative division (state,province, department, etc.).",
            "@id": "unlcdv:subdivisionType",
            "schema:domainIncludes": {
                "@id": "unlcdv:Subdivision"
            }
        }
    ]
}