{
  "@context": {
    "rdf": "http://www.w3.org/1999/02/22-rdf-syntax-ns#",
    "owl": "http://www.w3.org/2002/07/owl#",
    "rdfs": "http://www.w3.org/2000/01/rdf-schema#",
    "untp-core": "https://test.uncefact.org/vocabulary/untp/core/"
  },
  "@graph": [
    {
      "rdfs:label": "conformityTopicCode",
      "@type": "rdfs:Class",
      "@id": "untp-core:conformityTopicCode",
      "rdfs:comment": "A high level category scheme for product and facility conformity declarations (claims or attestations)"
    },
    {
      "@id": "untp-core:conformityTopicCode#environment.energy",
      "@type": "untp-core:conformityTopicCode",
      "untp-core:Name": "environment.energy",
      "rdfs:comment": "claims supporting clean energy transition"
    },
    {
      "@id": "untp-core:conformityTopicCode#environment.emissions",
      "@type": "untp-core:conformityTopicCode",
      "untp-core:Name": "environment.emissions",
      "rdfs:comment": "claims supporting GHG emissions reduction"
    },
    {
      "@id": "untp-core:conformityTopicCode#environment.water",
      "@type": "untp-core:conformityTopicCode",
      "untp-core:Name": "environment.water",
      "rdfs:comment": "claims supporting minimising water usage impact"
    },
    {
      "@id": "untp-core:conformityTopicCode#environment.waste",
      "@type": "untp-core:conformityTopicCode",
      "untp-core:Name": "environment.waste",
      "rdfs:comment": "claims supporting waste processing and reduction"
    },
    {
      "@id": "untp-core:conformityTopicCode#environment.deforestation",
      "@type": "untp-core:conformityTopicCode",
      "untp-core:Name": "environment.deforestation",
      "rdfs:comment": "claims supporting native forest restoration"
    },
    {
      "@id": "untp-core:conformityTopicCode#environment.biodiversity",
      "@type": "untp-core:conformityTopicCode",
      "untp-core:Name": "environment.biodiversity",
      "rdfs:comment": "claims supporting improved biodiversity outcomes"
    },
    {
      "@id": "untp-core:conformityTopicCode#circularity.content",
      "@type": "untp-core:conformityTopicCode",
      "untp-core:Name": "circularity.content",
      "rdfs:comment": "claims supporting the use of recycled content in products"
    },
    {
      "@id": "untp-core:conformityTopicCode#circularity.design",
      "@type": "untp-core:conformityTopicCode",
      "untp-core:Name": "circularity.design",
      "rdfs:comment": "claims supporting product design for circularity outcomes"
    },
    {
      "@id": "untp-core:conformityTopicCode#social.labour",
      "@type": "untp-core:conformityTopicCode",
      "untp-core:Name": "social.labour",
      "rdfs:comment": "claims supporting labour rights including fair wages"
    },
    {
      "@id": "untp-core:conformityTopicCode#social.rights",
      "@type": "untp-core:conformityTopicCode",
      "untp-core:Name": "social.rights",
      "rdfs:comment": "claims supporting human rights and anti-discrimination"
    },
    {
      "@id": "untp-core:conformityTopicCode#social.community",
      "@type": "untp-core:conformityTopicCode",
      "untp-core:Name": "social.community",
      "rdfs:comment": "claims supporting local community development"
    },
    {
      "@id": "untp-core:conformityTopicCode#social.safety",
      "@type": "untp-core:conformityTopicCode",
      "untp-core:Name": "social.safety",
      "rdfs:comment": "claims supporting process and product safety"
    },
    {
      "@id": "untp-core:conformityTopicCode#governance.ethics",
      "@type": "untp-core:conformityTopicCode",
      "untp-core:Name": "governance.ethics",
      "rdfs:comment": "claims supporting ethical conduct and corporate governance"
    },
    {
      "@id": "untp-core:conformityTopicCode#governance.compliance",
      "@type": "untp-core:conformityTopicCode",
      "untp-core:Name": "governance.compliance",
      "rdfs:comment": "claims supporting regulatory compliance including taxation and community protection"
    },
    {
      "@id": "untp-core:conformityTopicCode#governance.transparency",
      "@type": "untp-core:conformityTopicCode",
      "untp-core:Name": "governance.transparency",
      "rdfs:comment": "claims supporting transparency and traceability"
    },
    {
      "rdfs:label": "encryptionMethodCode",
      "@type": "rdfs:Class",
      "@id": "untp-core:encryptionMethodCode",
      "rdfs:comment": ""
    },
    {
      "@id": "untp-core:encryptionMethodCode#none",
      "@type": "untp-core:encryptionMethodCode",
      "untp-core:Name": "none",
      "rdf:value": "",
      "rdfs:comment": "no encryption"
    },
    {
      "@id": "untp-core:encryptionMethodCode#AES",
      "@type": "untp-core:encryptionMethodCode",
      "untp-core:Name": "AES",
      "rdf:value": "",
      "rdfs:comment": "AES standard"
    },
    {
      "rdfs:label": "hashMethodCode",
      "@type": "rdfs:Class",
      "@id": "untp-core:hashMethodCode",
      "rdfs:comment": ""
    },
    {
      "@id": "untp-core:hashMethodCode#SHA-256",
      "@type": "untp-core:hashMethodCode",
      "untp-core:Name": "SHA-256",
      "rdf:value": "Secure Hash Algorithm 256 bits",
      "rdfs:comment": ""
    },
    {
      "@id": "untp-core:VerifiableCredential",
      "@type": "rdfs:Class",
      "rdfs:label": "VerifiableCredential",
      "schema:source": {
        "@id": "https://test.uncefact.org/vocabulary/untp/core/VerifiableCredential"
      },
      "rdfs:comment": "A verifiable credential is a digital and verifiable version of everyday credentials such as certificates and licenses.  It conforms to the W3C Verifiable Credentials Data Model v2.0 (VCDM)"
    },
    {
      "@id": "untp-core:Identifier",
      "@type": "rdfs:Class",
      "rdfs:label": "Identifier",
      "schema:source": {
        "@id": "https://test.uncefact.org/vocabulary/untp/core/Identifier"
      },
      "rdfs:comment": "An identifier of a party, product, or facility that is defined by an identifier scheme and idenfier value."
    },
    {
      "@id": "untp-core:OrganisationID",
      "@type": "rdfs:Class",
      "rdfs:label": "OrganisationID",
      "schema:source": {
        "@id": "https://test.uncefact.org/vocabulary/untp/core/OrganisationID"
      },
      "rdfs:comment": "The ID and Name of an organisation. Used for lightweight links from other classes."
    },
    {
      "@id": "untp-core:Organisation",
      "@type": "rdfs:Class",
      "rdfs:label": "Organisation",
      "schema:source": {
        "@id": "https://test.uncefact.org/vocabulary/untp/core/Organisation"
      },
      "rdfs:subClassOf": "untp-core:OrganisationID",
      "rdfs:comment": "An organisation.  May be a supply chain actor, a certifier, a government agency."
    },
    {
      "@id": "untp-core:FacilityID",
      "@type": "rdfs:Class",
      "rdfs:label": "FacilityID",
      "schema:source": {
        "@id": "https://test.uncefact.org/vocabulary/untp/core/FacilityID"
      },
      "rdfs:comment": "The ID and Name of a facility. Used for lightweight links from other classes."
    },
    {
      "@id": "untp-core:Facility",
      "@type": "rdfs:Class",
      "rdfs:label": "Facility",
      "schema:source": {
        "@id": "https://test.uncefact.org/vocabulary/untp/core/Facility"
      },
      "rdfs:subClassOf": "untp-core:FacilityID",
      "rdfs:comment": "The physical site (eg farm or factory) where the product or materials was produced."
    },
    {
      "@id": "untp-core:LocationID",
      "@type": "rdfs:Class",
      "rdfs:label": "LocationID",
      "schema:source": {
        "@id": "https://test.uncefact.org/vocabulary/untp/core/LocationID"
      },
      "rdfs:comment": "The ID and Name of a location. Used for lightweight links from other classes."
    },
    {
      "@id": "untp-core:Location",
      "@type": "rdfs:Class",
      "rdfs:label": "Location",
      "schema:source": {
        "@id": "https://test.uncefact.org/vocabulary/untp/core/Location"
      },
      "rdfs:subClassOf": "untp-core:LocationID",
      "rdfs:comment": "Location information including address and geolocation of points, areas, and boundaries"
    },
    {
      "@id": "untp-core:Coordinate",
      "@type": "rdfs:Class",
      "rdfs:label": "Coordinate",
      "schema:source": {
        "@id": "https://test.uncefact.org/vocabulary/untp/core/Coordinate"
      },
      "rdfs:comment": "A map coordinate defined by a lattitude & longditude pair."
    },
    {
      "@id": "untp-core:ProductID",
      "@type": "rdfs:Class",
      "rdfs:label": "ProductID",
      "schema:source": {
        "@id": "https://test.uncefact.org/vocabulary/untp/core/ProductID"
      },
      "rdfs:comment": "The ID and Name of a product. Used for lightweight links from other classes."
    },
    {
      "@id": "untp-core:Product",
      "@type": "rdfs:Class",
      "rdfs:label": "Product",
      "schema:source": {
        "@id": "https://test.uncefact.org/vocabulary/untp/core/Product"
      },
      "rdfs:subClassOf": "untp-core:ProductID",
      "rdfs:comment": "The ProductInformation class encapsulates detailed information regarding a specific product, including its identification details, manufacturer, and other pertinent details."
    },
    {
      "@id": "untp-core:Classification",
      "@type": "rdfs:Class",
      "rdfs:label": "Classification",
      "schema:source": {
        "@id": "https://test.uncefact.org/vocabulary/untp/core/Classification"
      },
      "rdfs:comment": "A classification scheme and code / name representing a category value for a product, entity, or facility."
    },
    {
      "@id": "untp-core:Metric",
      "@type": "rdfs:Class",
      "rdfs:label": "Metric",
      "schema:source": {
        "@id": "https://test.uncefact.org/vocabulary/untp/core/Metric"
      },
      "rdfs:comment": "A specific measure of performance against the criteria that governs the claim.  Expressed as an array of metric (ie unit of emasure) / value (ie the actual numeric value) pairs.  "
    },
    {
      "@id": "untp-core:Dimension",
      "@type": "rdfs:Class",
      "rdfs:label": "Dimension",
      "schema:source": {
        "@id": "https://test.uncefact.org/vocabulary/untp/core/Dimension"
      },
      "rdfs:comment": "Overall (length, width, height) dimensions and weight/volume of an item."
    },
    {
      "@id": "untp-core:Measure",
      "@type": "rdfs:Class",
      "rdfs:label": "Measure",
      "schema:source": {
        "@id": "https://test.uncefact.org/vocabulary/untp/core/Measure"
      },
      "rdfs:comment": "The measure class defines a numeric measured value (eg 10) and a coded unit of measure (eg KG)."
    },
    {
      "@id": "untp-core:BinaryFile",
      "@type": "rdfs:Class",
      "rdfs:label": "BinaryFile",
      "schema:source": {
        "@id": "https://test.uncefact.org/vocabulary/untp/core/BinaryFile"
      },
      "rdfs:comment": "A file representing a data snapshot that is used to infomr the conformity assessment."
    },
    {
      "@id": "untp-core:SecureBinaryFile",
      "@type": "rdfs:Class",
      "rdfs:label": "SecureBinaryFile",
      "schema:source": {
        "@id": "https://test.uncefact.org/vocabulary/untp/core/SecureBinaryFile"
      },
      "rdfs:subClassOf": "untp-core:BinaryFile",
      "rdfs:comment": "A binary file that is hashed ()for tamper evidence) and optionally encrypted (for confidentiality)."
    },
    {
      "@id": "untp-core:Declaration",
      "@type": "rdfs:Class",
      "rdfs:label": "Declaration",
      "schema:source": {
        "@id": "https://test.uncefact.org/vocabulary/untp/core/Declaration"
      },
      "rdfs:comment": "A specific assessment about the product or facility against a specific specification.  Eg the carbon intensity of a given product or batch."
    },
    {
      "@id": "untp-core:StandardID",
      "@type": "rdfs:Class",
      "rdfs:label": "StandardID",
      "schema:source": {
        "@id": "https://test.uncefact.org/vocabulary/untp/core/StandardID"
      },
      "rdfs:comment": "The ID and Name of a conformity standard. Used for lightweight links from other classes."
    },
    {
      "@id": "untp-core:Standard",
      "@type": "rdfs:Class",
      "rdfs:label": "Standard",
      "schema:source": {
        "@id": "https://test.uncefact.org/vocabulary/untp/core/Standard"
      },
      "rdfs:subClassOf": "untp-core:StandardID",
      "rdfs:comment": "A standard (eg ISO 14000) that specifies the criteria for conformance."
    },
    {
      "@id": "untp-core:RegulationID",
      "@type": "rdfs:Class",
      "rdfs:label": "RegulationID",
      "schema:source": {
        "@id": "https://test.uncefact.org/vocabulary/untp/core/RegulationID"
      },
      "rdfs:comment": "The ID and Name of a n act or regulation. Used for lightweight links from other classes."
    },
    {
      "@id": "untp-core:Regulation",
      "@type": "rdfs:Class",
      "rdfs:label": "Regulation",
      "schema:source": {
        "@id": "https://test.uncefact.org/vocabulary/untp/core/Regulation"
      },
      "rdfs:subClassOf": "untp-core:RegulationID",
      "rdfs:comment": "A regulation regulation (eg EU deforestation regulation) that defines the criteria for assessment."
    },
    {
      "@id": "untp-core:Criteria",
      "@type": "rdfs:Class",
      "rdfs:label": "Criteria",
      "schema:source": {
        "@id": "https://test.uncefact.org/vocabulary/untp/core/Criteria"
      },
      "rdfs:comment": "A specific rule or criterion within a standard or regulation. eg a carbon intensity calculation rule within an emissions standard."
    },
    {
      "@id": "untp-core:@context",
      "@type": [
        "rdf:Property",
        "owl:DatatypeProperty"
      ],
      "rdfs:label": "@context",
      "schema:rangeIncludes": {
        "@id": "xsd:string"
      },
      "schema:domainIncludes": {
        "@id": "untp-core:VerifiableCredential"
      },
      "rdfs:comment": "A list of JSON-LD contect URIs that define the seamntic meaning of prperties within the credential. "
    },
    {
      "@id": "untp-core:id",
      "@type": [
        "rdf:Property",
        "owl:DatatypeProperty"
      ],
      "rdfs:label": "id",
      "schema:rangeIncludes": {
        "@id": "xsd:string"
      },
      "schema:domainIncludes": [
        {
          "@id": "untp-core:VerifiableCredential"
        },
        {
          "@id": "untp-core:Identifier"
        },
        {
          "@id": "untp-core:OrganisationID"
        },
        {
          "@id": "untp-core:FacilityID"
        },
        {
          "@id": "untp-core:LocationID"
        },
        {
          "@id": "untp-core:ProductID"
        },
        {
          "@id": "untp-core:Classification"
        },
        {
          "@id": "untp-core:BinaryFile"
        },
        {
          "@id": "untp-core:Declaration"
        },
        {
          "@id": "untp-core:StandardID"
        },
        {
          "@id": "untp-core:RegulationID"
        },
        {
          "@id": "untp-core:Criteria"
        }
      ],
      "rdfs:comment": "A unique identifier (URI) assigned to the product passport. May be a UUID"
    },
    {
      "@id": "untp-core:issuer",
      "@type": [
        "rdf:Property",
        "owl:ObjectProperty"
      ],
      "rdfs:label": "issuer",
      "schema:rangeIncludes": {
        "@id": "untp-core:Organisation"
      },
      "schema:domainIncludes": {
        "@id": "untp-core:VerifiableCredential"
      },
      "rdfs:comment": "The organisation that is the isuer of this VC. Note that the \"id\" property MUST be a W3C DID.  Other identifiers such as tax registration numbers can be listed in the \"otherIdentifiers\" property."
    },
    {
      "@id": "untp-core:validFrom",
      "@type": [
        "rdf:Property",
        "owl:DatatypeProperty"
      ],
      "rdfs:label": "validFrom",
      "schema:rangeIncludes": {
        "@id": "xsd:string"
      },
      "schema:domainIncludes": {
        "@id": "untp-core:VerifiableCredential"
      },
      "rdfs:comment": "The date and time from which the credential is valid."
    },
    {
      "@id": "untp-core:validUntil",
      "@type": [
        "rdf:Property",
        "owl:DatatypeProperty"
      ],
      "rdfs:label": "validUntil",
      "schema:rangeIncludes": {
        "@id": "xsd:string"
      },
      "schema:domainIncludes": {
        "@id": "untp-core:VerifiableCredential"
      },
      "rdfs:comment": "The expiry date (if applicable) of this verifiable credential."
    },
    {
      "@id": "untp-core:idScheme",
      "@type": [
        "rdf:Property",
        "owl:DatatypeProperty"
      ],
      "rdfs:label": "idScheme",
      "schema:rangeIncludes": {
        "@id": "xsd:string"
      },
      "schema:domainIncludes": [
        {
          "@id": "untp-core:Identifier"
        },
        {
          "@id": "untp-core:OrganisationID"
        },
        {
          "@id": "untp-core:FacilityID"
        },
        {
          "@id": "untp-core:LocationID"
        },
        {
          "@id": "untp-core:ProductID"
        }
      ],
      "rdfs:comment": "the identifier scheme as defined by the registrar that manages the identifier registry. Eg abr.busines.gov.au If the identifier scheme is registered with UNTP then this URI can use used to dicsover the resolution method (to get more data) and the verification method (to prove ownership)."
    },
    {
      "@id": "untp-core:idSchemeName",
      "@type": [
        "rdf:Property",
        "owl:DatatypeProperty"
      ],
      "rdfs:label": "idSchemeName",
      "schema:rangeIncludes": {
        "@id": "xsd:string"
      },
      "schema:domainIncludes": [
        {
          "@id": "untp-core:Identifier"
        },
        {
          "@id": "untp-core:OrganisationID"
        },
        {
          "@id": "untp-core:FacilityID"
        },
        {
          "@id": "untp-core:LocationID"
        },
        {
          "@id": "untp-core:ProductID"
        }
      ],
      "rdfs:comment": "The identifier scheme name (eg Australian Business Number or GS1 Global Trade Item Number))"
    },
    {
      "@id": "untp-core:idValue",
      "@type": [
        "rdf:Property",
        "owl:DatatypeProperty"
      ],
      "rdfs:label": "idValue",
      "schema:rangeIncludes": {
        "@id": "xsd:string"
      },
      "schema:domainIncludes": [
        {
          "@id": "untp-core:Identifier"
        },
        {
          "@id": "untp-core:OrganisationID"
        },
        {
          "@id": "untp-core:FacilityID"
        },
        {
          "@id": "untp-core:LocationID"
        },
        {
          "@id": "untp-core:ProductID"
        }
      ],
      "rdfs:comment": "The value of the identifier within the scheme (eg 90664869327)"
    },
    {
      "@id": "untp-core:name",
      "@type": [
        "rdf:Property",
        "owl:DatatypeProperty"
      ],
      "rdfs:label": "name",
      "schema:rangeIncludes": {
        "@id": "xsd:string"
      },
      "schema:domainIncludes": [
        {
          "@id": "untp-core:OrganisationID"
        },
        {
          "@id": "untp-core:FacilityID"
        },
        {
          "@id": "untp-core:LocationID"
        },
        {
          "@id": "untp-core:ProductID"
        },
        {
          "@id": "untp-core:StandardID"
        },
        {
          "@id": "untp-core:RegulationID"
        },
        {
          "@id": "untp-core:Criteria"
        }
      ],
      "rdfs:comment": "The name of the organization or company, represented as a text string.  SHOULD match the registered name in the identifeir scheme. Eg PYX Industries Pty Ltd"
    },
    {
      "@id": "untp-core:registrationCountry",
      "@type": [
        "rdf:Property",
        "owl:ObjectProperty"
      ],
      "rdfs:label": "registrationCountry",
      "schema:rangeIncludes": {
        "@id": "untp-core:countryCode"
      },
      "schema:domainIncludes": {
        "@id": "untp-core:Organisation"
      },
      "rdfs:comment": "the country in which this organisation is registered"
    },
    {
      "@id": "untp-core:organisationWebsite",
      "@type": [
        "rdf:Property",
        "owl:DatatypeProperty"
      ],
      "rdfs:label": "organisationWebsite",
      "schema:rangeIncludes": {
        "@id": "xsd:string"
      },
      "schema:domainIncludes": {
        "@id": "untp-core:Organisation"
      },
      "rdfs:comment": "Website for this organisation"
    },
    {
      "@id": "untp-core:industryCategory",
      "@type": [
        "rdf:Property",
        "owl:ObjectProperty"
      ],
      "rdfs:label": "industryCategory",
      "schema:rangeIncludes": {
        "@id": "untp-core:Classification"
      },
      "schema:domainIncludes": {
        "@id": "untp-core:Organisation"
      },
      "rdfs:comment": "The industry categories for this organisations.  Recommend use of UNCPC as the category scheme."
    },
    {
      "@id": "untp-core:otherIdentifiers",
      "@type": [
        "rdf:Property",
        "owl:ObjectProperty"
      ],
      "rdfs:label": "otherIdentifiers",
      "schema:rangeIncludes": {
        "@id": "untp-core:Identifier"
      },
      "schema:domainIncludes": [
        {
          "@id": "untp-core:Organisation"
        },
        {
          "@id": "untp-core:Facility"
        }
      ],
      "rdfs:comment": "An optional lsit of other registered identifiers for this organisations"
    },
    {
      "@id": "untp-core:facilityName",
      "@type": [
        "rdf:Property",
        "owl:DatatypeProperty"
      ],
      "rdfs:label": "facilityName",
      "schema:rangeIncludes": {
        "@id": "xsd:string"
      },
      "schema:domainIncludes": {
        "@id": "untp-core:Facility"
      },
      "rdfs:comment": "The name of the facility, represented as a text string."
    },
    {
      "@id": "untp-core:countryOfOperation",
      "@type": [
        "rdf:Property",
        "owl:ObjectProperty"
      ],
      "rdfs:label": "countryOfOperation",
      "schema:rangeIncludes": {
        "@id": "untp-core:countryCode"
      },
      "schema:domainIncludes": {
        "@id": "untp-core:Facility"
      },
      "rdfs:comment": "The country in which this facility is operating."
    },
    {
      "@id": "untp-core:processCategory",
      "@type": [
        "rdf:Property",
        "owl:ObjectProperty"
      ],
      "rdfs:label": "processCategory",
      "schema:rangeIncludes": {
        "@id": "untp-core:Classification"
      },
      "schema:domainIncludes": {
        "@id": "untp-core:Facility"
      },
      "rdfs:comment": "The idustrial or production processes performed by this facility.  "
    },
    {
      "@id": "untp-core:operatedBy",
      "@type": [
        "rdf:Property",
        "owl:ObjectProperty"
      ],
      "rdfs:label": "operatedBy",
      "schema:rangeIncludes": {
        "@id": "untp-core:OrganisationID"
      },
      "schema:domainIncludes": {
        "@id": "untp-core:Facility"
      },
      "rdfs:comment": "The Party entity responsible for operating the facility."
    },
    {
      "@id": "untp-core:locationInformation",
      "@type": [
        "rdf:Property",
        "owl:ObjectProperty"
      ],
      "rdfs:label": "locationInformation",
      "schema:rangeIncludes": {
        "@id": "untp-core:Location"
      },
      "schema:domainIncludes": {
        "@id": "untp-core:Facility"
      },
      "rdfs:comment": "Geolocation and address information for this facility"
    },
    {
      "@id": "untp-core:areaReference",
      "@type": [
        "rdf:Property",
        "owl:DatatypeProperty"
      ],
      "rdfs:label": "areaReference",
      "schema:rangeIncludes": {
        "@id": "xsd:string"
      },
      "schema:domainIncludes": {
        "@id": "untp-core:Location"
      },
      "rdfs:comment": "The area of the facility as a URI - typically a plus code (see https://maps.google.com/pluscodes/) "
    },
    {
      "@id": "untp-core:geoLocation",
      "@type": [
        "rdf:Property",
        "owl:ObjectProperty"
      ],
      "rdfs:label": "geoLocation",
      "schema:rangeIncludes": {
        "@id": "untp-core:Coordinate"
      },
      "schema:domainIncludes": {
        "@id": "untp-core:Location"
      },
      "rdfs:comment": "The latitude and logditude coordinates that best represent the specified location "
    },
    {
      "@id": "untp-core:boundary",
      "@type": [
        "rdf:Property",
        "owl:ObjectProperty"
      ],
      "rdfs:label": "boundary",
      "schema:rangeIncludes": {
        "@id": "untp-core:Coordinate"
      },
      "schema:domainIncludes": {
        "@id": "untp-core:Location"
      },
      "rdfs:comment": "The list of coordinates that define a closed area polygon as a location boundary."
    },
    {
      "@id": "untp-core:address",
      "@type": [
        "rdf:Property",
        "owl:DatatypeProperty"
      ],
      "rdfs:label": "address",
      "schema:rangeIncludes": {
        "@id": "xsd:string"
      },
      "schema:domainIncludes": {
        "@id": "untp-core:Location"
      },
      "rdfs:comment": "The textual address of the location."
    },
    {
      "@id": "untp-core:Latitude",
      "@type": [
        "rdf:Property",
        "owl:DatatypeProperty"
      ],
      "rdfs:label": "Latitude",
      "schema:rangeIncludes": {
        "@id": "xsd:decimal"
      },
      "schema:domainIncludes": {
        "@id": "untp-core:Coordinate"
      },
      "rdfs:comment": "The latitude of a map location expressed in decimal degrees (between +90 and -90) where negative values represent latitudes south of the equator."
    },
    {
      "@id": "untp-core:Longditude",
      "@type": [
        "rdf:Property",
        "owl:DatatypeProperty"
      ],
      "rdfs:label": "Longditude",
      "schema:rangeIncludes": {
        "@id": "xsd:decimal"
      },
      "schema:domainIncludes": {
        "@id": "untp-core:Coordinate"
      },
      "rdfs:comment": "The longditude of a map location expressed in decimal degrees (between +180 and -180) where negative values represent longditudes west of the prime meridian."
    },
    {
      "@id": "untp-core:serialNumber",
      "@type": [
        "rdf:Property",
        "owl:DatatypeProperty"
      ],
      "rdfs:label": "serialNumber",
      "schema:rangeIncludes": {
        "@id": "xsd:string"
      },
      "schema:domainIncludes": {
        "@id": "untp-core:Product"
      },
      "rdfs:comment": "An array of identifiers representing a specific serialised item of the product."
    },
    {
      "@id": "untp-core:batchNumber",
      "@type": [
        "rdf:Property",
        "owl:DatatypeProperty"
      ],
      "rdfs:label": "batchNumber",
      "schema:rangeIncludes": {
        "@id": "xsd:string"
      },
      "schema:domainIncludes": {
        "@id": "untp-core:Product"
      },
      "rdfs:comment": "Information regarding the specific production batch of the product."
    },
    {
      "@id": "untp-core:productImage",
      "@type": [
        "rdf:Property",
        "owl:ObjectProperty"
      ],
      "rdfs:label": "productImage",
      "schema:rangeIncludes": {
        "@id": "untp-core:BinaryFile"
      },
      "schema:domainIncludes": {
        "@id": "untp-core:Product"
      },
      "rdfs:comment": "A unique identifier (URI) pointing to an image of the product."
    },
    {
      "@id": "untp-core:description",
      "@type": [
        "rdf:Property",
        "owl:DatatypeProperty"
      ],
      "rdfs:label": "description",
      "schema:rangeIncludes": {
        "@id": "xsd:string"
      },
      "schema:domainIncludes": {
        "@id": "untp-core:Product"
      },
      "rdfs:comment": "A textual description providing details about the product."
    },
    {
      "@id": "untp-core:productCategory",
      "@type": [
        "rdf:Property",
        "owl:ObjectProperty"
      ],
      "rdfs:label": "productCategory",
      "schema:rangeIncludes": {
        "@id": "untp-core:Classification"
      },
      "schema:domainIncludes": {
        "@id": "untp-core:Product"
      },
      "rdfs:comment": "A code representing the product's class, typically using the UN CPC (United Nations Central Product Classification) https://unstats.un.org/unsd/classifications/Econ/cpc"
    },
    {
      "@id": "untp-core:furtherInformation",
      "@type": [
        "rdf:Property",
        "owl:DatatypeProperty"
      ],
      "rdfs:label": "furtherInformation",
      "schema:rangeIncludes": {
        "@id": "xsd:string"
      },
      "schema:domainIncludes": {
        "@id": "untp-core:Product"
      },
      "rdfs:comment": "A URL pointing to further human readable information about the product."
    },
    {
      "@id": "untp-core:producedBy",
      "@type": [
        "rdf:Property",
        "owl:ObjectProperty"
      ],
      "rdfs:label": "producedBy",
      "schema:rangeIncludes": {
        "@id": "untp-core:OrganisationID"
      },
      "schema:domainIncludes": {
        "@id": "untp-core:Product"
      },
      "rdfs:comment": "The Party entity that manufactured the product."
    },
    {
      "@id": "untp-core:dimensions",
      "@type": [
        "rdf:Property",
        "owl:ObjectProperty"
      ],
      "rdfs:label": "dimensions",
      "schema:rangeIncludes": {
        "@id": "untp-core:Dimension"
      },
      "schema:domainIncludes": {
        "@id": "untp-core:Product"
      },
      "rdfs:comment": "The physical dimensions of the product. Not every dimension is relevant to every products.  For example bulk materials may have wieght and volume but not length, with, or height."
    },
    {
      "@id": "untp-core:productionDate",
      "@type": [
        "rdf:Property",
        "owl:DatatypeProperty"
      ],
      "rdfs:label": "productionDate",
      "schema:rangeIncludes": {
        "@id": "xsd:string"
      },
      "schema:domainIncludes": {
        "@id": "untp-core:Product"
      },
      "rdfs:comment": "The ISO 8601 date on which the product batch was manufactured."
    },
    {
      "@id": "untp-core:countryOfProduction",
      "@type": [
        "rdf:Property",
        "owl:ObjectProperty"
      ],
      "rdfs:label": "countryOfProduction",
      "schema:rangeIncludes": {
        "@id": "untp-core:countryCode"
      },
      "schema:domainIncludes": {
        "@id": "untp-core:Product"
      },
      "rdfs:comment": "The country in which this item was produced / manufactured."
    },
    {
      "@id": "untp-core:classificationSchemeID",
      "@type": [
        "rdf:Property",
        "owl:DatatypeProperty"
      ],
      "rdfs:label": "classificationSchemeID",
      "schema:rangeIncludes": {
        "@id": "xsd:string"
      },
      "schema:domainIncludes": {
        "@id": "untp-core:Classification"
      },
      "rdfs:comment": "Classification scheme  - eg https://unstats.un.org/unsd/classifications/Econ/cpc "
    },
    {
      "@id": "untp-core:classificationSchemeName",
      "@type": [
        "rdf:Property",
        "owl:DatatypeProperty"
      ],
      "rdfs:label": "classificationSchemeName",
      "schema:rangeIncludes": {
        "@id": "xsd:string"
      },
      "schema:domainIncludes": {
        "@id": "untp-core:Classification"
      },
      "rdfs:comment": "The name of the classificaiotn schema - eg United Nations Central Product Classification"
    },
    {
      "@id": "untp-core:classifierValue",
      "@type": [
        "rdf:Property",
        "owl:DatatypeProperty"
      ],
      "rdfs:label": "classifierValue",
      "schema:rangeIncludes": {
        "@id": "xsd:string"
      },
      "schema:domainIncludes": {
        "@id": "untp-core:Classification"
      },
      "rdfs:comment": "classifier value within the scheme - eg \"01211\" in UN CPC"
    },
    {
      "@id": "untp-core:classifierName",
      "@type": [
        "rdf:Property",
        "owl:DatatypeProperty"
      ],
      "rdfs:label": "classifierName",
      "schema:rangeIncludes": {
        "@id": "xsd:string"
      },
      "schema:domainIncludes": {
        "@id": "untp-core:Classification"
      },
      "rdfs:comment": "Name of the classifier - eg \"Asparagus\" for code \"01211\" in UNCPC"
    },
    {
      "@id": "untp-core:metricName",
      "@type": [
        "rdf:Property",
        "owl:DatatypeProperty"
      ],
      "rdfs:label": "metricName",
      "schema:rangeIncludes": {
        "@id": "xsd:string"
      },
      "schema:domainIncludes": {
        "@id": "untp-core:Metric"
      },
      "rdfs:comment": "A human readable name for this metric (for example \"Tensile strength\")"
    },
    {
      "@id": "untp-core:metricValue",
      "@type": [
        "rdf:Property",
        "owl:ObjectProperty"
      ],
      "rdfs:label": "metricValue",
      "schema:rangeIncludes": {
        "@id": "untp-core:Measure"
      },
      "schema:domainIncludes": {
        "@id": "untp-core:Metric"
      },
      "rdfs:comment": "A numeric value and unit of measure for this metric. Could be a measured value or a specified threshold."
    },
    {
      "@id": "untp-core:accuracy",
      "@type": [
        "rdf:Property",
        "owl:DatatypeProperty"
      ],
      "rdfs:label": "accuracy",
      "schema:rangeIncludes": {
        "@id": "xsd:decimal"
      },
      "schema:domainIncludes": {
        "@id": "untp-core:Metric"
      },
      "rdfs:comment": "A percentage represented as a numeric between 0 and 1 indicating the rage of accuracy of the claimed value (eg 0.05 means that the actual value is within 5% of the claimed value.)"
    },
    {
      "@id": "untp-core:weight",
      "@type": [
        "rdf:Property",
        "owl:ObjectProperty"
      ],
      "rdfs:label": "weight",
      "schema:rangeIncludes": {
        "@id": "untp-core:Measure"
      },
      "schema:domainIncludes": {
        "@id": "untp-core:Dimension"
      },
      "rdfs:comment": "the weight of the product"
    },
    {
      "@id": "untp-core:length",
      "@type": [
        "rdf:Property",
        "owl:ObjectProperty"
      ],
      "rdfs:label": "length",
      "schema:rangeIncludes": {
        "@id": "untp-core:Measure"
      },
      "schema:domainIncludes": {
        "@id": "untp-core:Dimension"
      },
      "rdfs:comment": "The length of the product or packaging"
    },
    {
      "@id": "untp-core:width",
      "@type": [
        "rdf:Property",
        "owl:ObjectProperty"
      ],
      "rdfs:label": "width",
      "schema:rangeIncludes": {
        "@id": "untp-core:Measure"
      },
      "schema:domainIncludes": {
        "@id": "untp-core:Dimension"
      },
      "rdfs:comment": "The width of the product or packaging"
    },
    {
      "@id": "untp-core:height",
      "@type": [
        "rdf:Property",
        "owl:ObjectProperty"
      ],
      "rdfs:label": "height",
      "schema:rangeIncludes": {
        "@id": "untp-core:Measure"
      },
      "schema:domainIncludes": {
        "@id": "untp-core:Dimension"
      },
      "rdfs:comment": "The height of the product or packaging"
    },
    {
      "@id": "untp-core:volume",
      "@type": [
        "rdf:Property",
        "owl:ObjectProperty"
      ],
      "rdfs:label": "volume",
      "schema:rangeIncludes": {
        "@id": "untp-core:Measure"
      },
      "schema:domainIncludes": {
        "@id": "untp-core:Dimension"
      },
      "rdfs:comment": "The displacement volume of the product."
    },
    {
      "@id": "untp-core:value",
      "@type": [
        "rdf:Property",
        "owl:DatatypeProperty"
      ],
      "rdfs:label": "value",
      "schema:rangeIncludes": {
        "@id": "xsd:decimal"
      },
      "schema:domainIncludes": {
        "@id": "untp-core:Measure"
      },
      "rdfs:comment": "The numeric value of the measure"
    },
    {
      "@id": "untp-core:unit",
      "@type": [
        "rdf:Property",
        "owl:ObjectProperty"
      ],
      "rdfs:label": "unit",
      "schema:rangeIncludes": {
        "@id": "untp-core:unitOfMeasure"
      },
      "schema:domainIncludes": {
        "@id": "untp-core:Measure"
      },
      "rdfs:comment": "Unit of measure drawn from the UNECE rec20 measure code list."
    },
    {
      "@id": "untp-core:fileName",
      "@type": [
        "rdf:Property",
        "owl:DatatypeProperty"
      ],
      "rdfs:label": "fileName",
      "schema:rangeIncludes": {
        "@id": "xsd:string"
      },
      "schema:domainIncludes": {
        "@id": "untp-core:BinaryFile"
      },
      "rdfs:comment": "A name for referenced binary file"
    },
    {
      "@id": "untp-core:fileType",
      "@type": [
        "rdf:Property",
        "owl:ObjectProperty"
      ],
      "rdfs:label": "fileType",
      "schema:rangeIncludes": {
        "@id": "untp-core:mimeType"
      },
      "schema:domainIncludes": {
        "@id": "untp-core:BinaryFile"
      },
      "rdfs:comment": "The type of file, represented as a MIME type."
    },
    {
      "@id": "untp-core:fileHash",
      "@type": [
        "rdf:Property",
        "owl:DatatypeProperty"
      ],
      "rdfs:label": "fileHash",
      "schema:rangeIncludes": {
        "@id": "xsd:string"
      },
      "schema:domainIncludes": {
        "@id": "untp-core:SecureBinaryFile"
      },
      "rdfs:comment": "The MD5 hash of the file."
    },
    {
      "@id": "untp-core:hashMethod",
      "@type": [
        "rdf:Property",
        "owl:ObjectProperty"
      ],
      "rdfs:label": "hashMethod",
      "schema:rangeIncludes": {
        "@id": "untp-core:hashMethodCode"
      },
      "schema:domainIncludes": {
        "@id": "untp-core:SecureBinaryFile"
      },
      "rdfs:comment": "The hashing algorithm used to create the file hash.  SHA-265 is the recommedned standard"
    },
    {
      "@id": "untp-core:encryptionMethod",
      "@type": [
        "rdf:Property",
        "owl:ObjectProperty"
      ],
      "rdfs:label": "encryptionMethod",
      "schema:rangeIncludes": {
        "@id": "untp-core:encryptionMethodCode"
      },
      "schema:domainIncludes": {
        "@id": "untp-core:SecureBinaryFile"
      },
      "rdfs:comment": "The symmetric encryption algorithm used to encrypt this binary file.  AES is the recommended standard"
    },
    {
      "@id": "untp-core:referenceStandard",
      "@type": [
        "rdf:Property",
        "owl:ObjectProperty"
      ],
      "rdfs:label": "referenceStandard",
      "schema:rangeIncludes": {
        "@id": "untp-core:Standard"
      },
      "schema:domainIncludes": {
        "@id": "untp-core:Declaration"
      },
      "rdfs:comment": "The reference to the standard that defines the specification / criteria"
    },
    {
      "@id": "untp-core:referenceRegulation",
      "@type": [
        "rdf:Property",
        "owl:ObjectProperty"
      ],
      "rdfs:label": "referenceRegulation",
      "schema:rangeIncludes": {
        "@id": "untp-core:Regulation"
      },
      "schema:domainIncludes": {
        "@id": "untp-core:Declaration"
      },
      "rdfs:comment": "The reference to the regulation that defines the assessment criteria"
    },
    {
      "@id": "untp-core:assessmentCriterion",
      "@type": [
        "rdf:Property",
        "owl:ObjectProperty"
      ],
      "rdfs:label": "assessmentCriterion",
      "schema:rangeIncludes": {
        "@id": "untp-core:Criteria"
      },
      "schema:domainIncludes": {
        "@id": "untp-core:Declaration"
      },
      "rdfs:comment": "The specification against which the assessment is made."
    },
    {
      "@id": "untp-core:values",
      "@type": [
        "rdf:Property",
        "owl:ObjectProperty"
      ],
      "rdfs:label": "values",
      "schema:rangeIncludes": {
        "@id": "untp-core:Metric"
      },
      "schema:domainIncludes": {
        "@id": "untp-core:Declaration"
      },
      "rdfs:comment": "The list of specific values measured as part of this assessment (eg tensile strength)"
    },
    {
      "@id": "untp-core:compliance",
      "@type": [
        "rdf:Property",
        "owl:DatatypeProperty"
      ],
      "rdfs:label": "compliance",
      "schema:rangeIncludes": {
        "@id": "xsd:boolean"
      },
      "schema:domainIncludes": {
        "@id": "untp-core:Declaration"
      },
      "rdfs:comment": "An indicator of whether or not the assessment meets the specification."
    },
    {
      "@id": "untp-core:conformityTopic",
      "@type": [
        "rdf:Property",
        "owl:ObjectProperty"
      ],
      "rdfs:label": "conformityTopic",
      "schema:rangeIncludes": {
        "@id": "untp-core:conformityTopicCode"
      },
      "schema:domainIncludes": {
        "@id": "untp-core:Declaration"
      },
      "rdfs:comment": "The conformity topic category for this assessment (eg vocabulary.uncefact.org/sustainability/emissions)"
    },
    {
      "@id": "untp-core:issuingBody",
      "@type": [
        "rdf:Property",
        "owl:ObjectProperty"
      ],
      "rdfs:label": "issuingBody",
      "schema:rangeIncludes": {
        "@id": "untp-core:OrganisationID"
      },
      "schema:domainIncludes": [
        {
          "@id": "untp-core:Standard"
        },
        {
          "@id": "untp-core:Regulation"
        }
      ],
      "rdfs:comment": "The party that issued the standard (ID and Name reference only)"
    },
    {
      "@id": "untp-core:issueDate",
      "@type": [
        "rdf:Property",
        "owl:DatatypeProperty"
      ],
      "rdfs:label": "issueDate",
      "schema:rangeIncludes": {
        "@id": "xsd:string"
      },
      "schema:domainIncludes": {
        "@id": "untp-core:Standard"
      },
      "rdfs:comment": "The date when the standard was issued."
    },
    {
      "@id": "untp-core:effectiveDate",
      "@type": [
        "rdf:Property",
        "owl:DatatypeProperty"
      ],
      "rdfs:label": "effectiveDate",
      "schema:rangeIncludes": {
        "@id": "xsd:string"
      },
      "schema:domainIncludes": {
        "@id": "untp-core:Regulation"
      },
      "rdfs:comment": "the date at which the regulation came into effect."
    },
    {
      "@id": "untp-core:thresholdValues",
      "@type": [
        "rdf:Property",
        "owl:ObjectProperty"
      ],
      "rdfs:label": "thresholdValues",
      "schema:rangeIncludes": {
        "@id": "untp-core:Metric"
      },
      "schema:domainIncludes": {
        "@id": "untp-core:Criteria"
      },
      "rdfs:comment": "A conformity threshold defined by the specification (eg minimum compressive strength) "
    }
  ],
  "jargon": {}
}